@prefix : <http://www.semanticweb.org/georg/ontologies/2022/3/WOOD#> .
@prefix owl: <http://www.w3.org/2002/07/owl#> .
@prefix rdf: <http://www.w3.org/1999/02/22-rdf-syntax-ns#> .
@prefix xml: <http://www.w3.org/XML/1998/namespace> .
@prefix xsd: <http://www.w3.org/2001/XMLSchema#> .
@prefix rdfs: <http://www.w3.org/2000/01/rdf-schema#> .
@base <http://www.semanticweb.org/georg/ontologies/2022/3/WOOD#> .

<http://www.semanticweb.org/georg/ontologies/2022/3/WOOD> rdf:type owl:Ontology ;
                                                           <http://purl.org/dc/terms/created> "13.07.2022"@en ;
                                                           <http://purl.org/dc/terms/creator> "Georg V"@en ;
                                                           <http://purl.org/dc/terms/license> "https://creativecommons.org/licenses/by/2.0/"@en ;
                                                           rdfs:comment "This Ontology helps to define wood damages in the field of construction. Experts in wood damages can use this ontology for writing reports. It is a sub-ontology to the \"Damage Topology Ontology\" and is defined as an \"Classified damage\". It defines damage types, connected causes, repair methods and investigation procedures. All these categories are part of the Report."@en ;
                                                           rdfs:label "Wood damage Ontology"@en .

#################################################################
#    Annotation properties
#################################################################

###  http://purl.org/dc/terms/created
<http://purl.org/dc/terms/created> rdf:type owl:AnnotationProperty .


###  http://purl.org/dc/terms/creator
<http://purl.org/dc/terms/creator> rdf:type owl:AnnotationProperty .


###  http://purl.org/dc/terms/license
<http://purl.org/dc/terms/license> rdf:type owl:AnnotationProperty .


#################################################################
#    Object Properties
#################################################################

###  http://www.semanticweb.org/christian/ontologies/2021/4/untitled-ontology-14#NeedsRepairProcedure
<http://www.semanticweb.org/christian/ontologies/2021/4/untitled-ontology-14#NeedsRepairProcedure> rdf:type owl:ObjectProperty ;
                                                                                                   rdfs:subPropertyOf :DamageObjectProperties ;
                                                                                                   rdfs:label "Needs Repair Procedure"@en .


###  http://www.semanticweb.org/georg/ontologies/2022/3/WOOD#CanCreateDamage
:CanCreateDamage rdf:type owl:ObjectProperty ;
                 rdfs:subPropertyOf :DamageObjectProperties ;
                 rdfs:label "Can Create Damage"@en .


###  http://www.semanticweb.org/georg/ontologies/2022/3/WOOD#ContainsDamage
:ContainsDamage rdf:type owl:ObjectProperty ;
                rdfs:subPropertyOf :GeneralObjectProperties ;
                owl:inverseOf :IsLocatedIn ;
                rdfs:domain :WoodComponent ;
                rdfs:range :WoodDamage ;
                rdfs:label "Contains Damage"@en .


###  http://www.semanticweb.org/georg/ontologies/2022/3/WOOD#Contracts
:Contracts rdf:type owl:ObjectProperty ;
           rdfs:subPropertyOf :PersonObjectProperties ;
           owl:inverseOf :IsContracted ;
           rdfs:domain :Client ;
           rdfs:range :BuildingDamageExpert .


###  http://www.semanticweb.org/georg/ontologies/2022/3/WOOD#DamageObjectProperties
:DamageObjectProperties rdf:type owl:ObjectProperty ;
                        rdfs:label "Damage Object Properties"@en .


###  http://www.semanticweb.org/georg/ontologies/2022/3/WOOD#DimensionalStability
:DimensionalStability rdf:type owl:ObjectProperty ;
                      rdfs:subPropertyOf :WoodObjectProperties .


###  http://www.semanticweb.org/georg/ontologies/2022/3/WOOD#Executes
:Executes rdf:type owl:ObjectProperty ;
          rdfs:subPropertyOf :GeneralObjectProperties ;
          owl:inverseOf :isWorkedOnBy ;
          rdfs:domain :Worker ;
          rdfs:range :Repair ;
          rdfs:label "Executes"@en .


###  http://www.semanticweb.org/georg/ontologies/2022/3/WOOD#FindsProperties
:FindsProperties rdf:type owl:ObjectProperty ;
                 rdfs:subPropertyOf :InvestigationObjectProperties ;
                 rdfs:label "Finds Properties"@en .


###  http://www.semanticweb.org/georg/ontologies/2022/3/WOOD#FittingType
:FittingType rdf:type owl:ObjectProperty ;
             rdfs:subPropertyOf :RepairObjectProperties ;
             rdfs:label "Fitting Type"@en .


###  http://www.semanticweb.org/georg/ontologies/2022/3/WOOD#GeneralObjectProperties
:GeneralObjectProperties rdf:type owl:ObjectProperty ;
                         rdfs:label "General Object Properties"@en .


###  http://www.semanticweb.org/georg/ontologies/2022/3/WOOD#HasDegreeOfDestruction
:HasDegreeOfDestruction rdf:type owl:ObjectProperty ;
                        rdfs:subPropertyOf :InvestigationObjectProperties ;
                        rdfs:label "Has Degree Of Destruction"@en .


###  http://www.semanticweb.org/georg/ontologies/2022/3/WOOD#HasPlace
:HasPlace rdf:type owl:ObjectProperty ;
          rdfs:subPropertyOf :InvestigationObjectProperties ;
          rdfs:label "Has Place"@en .


###  http://www.semanticweb.org/georg/ontologies/2022/3/WOOD#HasSteps
:HasSteps rdf:type owl:ObjectProperty ;
          rdfs:subPropertyOf :PartOfProcess ;
          rdf:type owl:FunctionalProperty ;
          rdfs:domain :ProcedureStatus ;
          rdfs:range :StepsToTheEvidenceConclusion ;
          rdfs:label "Has Steps"@en .


###  http://www.semanticweb.org/georg/ontologies/2022/3/WOOD#HasText
:HasText rdf:type owl:ObjectProperty ;
         rdfs:subPropertyOf :GeneralObjectProperties ;
         owl:inverseOf :WritesAbout ;
         rdfs:domain <https://w3id.org/bot#Building> ;
         rdfs:range :Report ;
         rdfs:label "Has Text"@en .


###  http://www.semanticweb.org/georg/ontologies/2022/3/WOOD#HasTime
:HasTime rdf:type owl:ObjectProperty ;
         rdfs:subPropertyOf :InvestigationObjectProperties ;
         rdfs:label "Has Time"@en .


###  http://www.semanticweb.org/georg/ontologies/2022/3/WOOD#Includes
:Includes rdf:type owl:ObjectProperty ;
          rdfs:subPropertyOf :GeneralObjectProperties ;
          owl:inverseOf :IsPartOf ;
          rdfs:domain :Report ;
          rdfs:range :WoodComponent ;
          rdfs:label "Includes"@en .


###  http://www.semanticweb.org/georg/ontologies/2022/3/WOOD#InfluenceObjectProperties
:InfluenceObjectProperties rdf:type owl:ObjectProperty ;
                           rdfs:label "Influence Object Properties"@en .


###  http://www.semanticweb.org/georg/ontologies/2022/3/WOOD#InsectResistance
:InsectResistance rdf:type owl:ObjectProperty ;
                  rdfs:subPropertyOf :WoodObjectProperties .


###  http://www.semanticweb.org/georg/ontologies/2022/3/WOOD#InvestigationObjectProperties
:InvestigationObjectProperties rdf:type owl:ObjectProperty ;
                               rdfs:label "Investigation Object Properties"@en .


###  http://www.semanticweb.org/georg/ontologies/2022/3/WOOD#IsContracted
:IsContracted rdf:type owl:ObjectProperty ;
              rdfs:subPropertyOf :PersonObjectProperties ;
              rdfs:domain :BuildingDamageExpert ;
              rdfs:range :Client ;
              rdfs:label "Is Contracted"@en .


###  http://www.semanticweb.org/georg/ontologies/2022/3/WOOD#IsLocatedIn
:IsLocatedIn rdf:type owl:ObjectProperty ;
             rdfs:subPropertyOf :GeneralObjectProperties ;
             rdfs:domain :WoodDamage ;
             rdfs:range :WoodComponent ;
             rdfs:label "Is Located In"@en .


###  http://www.semanticweb.org/georg/ontologies/2022/3/WOOD#IsPartOf
:IsPartOf rdf:type owl:ObjectProperty ;
          rdfs:subPropertyOf :GeneralObjectProperties ;
          rdfs:domain :WoodComponent ;
          rdfs:range :Report ;
          rdfs:label "Is Part Of"@en .


###  http://www.semanticweb.org/georg/ontologies/2022/3/WOOD#IsWrittenBy
:IsWrittenBy rdf:type owl:ObjectProperty ;
             rdfs:subPropertyOf :PersonObjectProperties ;
             owl:inverseOf :Writes ;
             rdfs:domain :Report ;
             rdfs:range :BuildingDamageExpert ;
             rdfs:label "Is Written By"@en .


###  http://www.semanticweb.org/georg/ontologies/2022/3/WOOD#PartOfCost
:PartOfCost rdf:type owl:ObjectProperty ;
            rdfs:subPropertyOf :PartOfProcess ;
            rdfs:domain :Costs ;
            rdfs:range <http://www.semanticweb.org/christian/ontologies/2021/4/untitled-ontology-14#CostOfRestoration> ;
            rdfs:label "Part Of Cost"@en .


###  http://www.semanticweb.org/georg/ontologies/2022/3/WOOD#PartOfEvaluation
:PartOfEvaluation rdf:type owl:ObjectProperty ;
                  rdfs:subPropertyOf :PartOfProcess ;
                  rdfs:domain :Evaluation ;
                  rdfs:range :CauseOfDamage ;
                  rdfs:label "Part Of Evaluation"@en .


###  http://www.semanticweb.org/georg/ontologies/2022/3/WOOD#PartOfFindings
:PartOfFindings rdf:type owl:ObjectProperty ;
                rdfs:subPropertyOf :PartOfProcess ;
                rdfs:domain :LocalFindings ;
                rdfs:range :WoodComponent ;
                rdfs:label "Part Of Findings"@en .


###  http://www.semanticweb.org/georg/ontologies/2022/3/WOOD#PartOfProcess
:PartOfProcess rdf:type owl:ObjectProperty ;
               rdfs:subPropertyOf :ReportObjectProperties ;
               rdfs:label "Part Of Process"@en .


###  http://www.semanticweb.org/georg/ontologies/2022/3/WOOD#PartOfRestoration
:PartOfRestoration rdf:type owl:ObjectProperty ;
                   rdfs:subPropertyOf :PartOfProcess ;
                   rdfs:domain :Restoration ;
                   rdfs:range :Repair ;
                   rdfs:label "Part Of Restoration"@en .


###  http://www.semanticweb.org/georg/ontologies/2022/3/WOOD#PartOfSource
:PartOfSource rdf:type owl:ObjectProperty ;
              rdfs:subPropertyOf :PartOfProcess ;
              rdfs:domain :Source ;
              rdfs:range :WoodDamage ;
              rdfs:label "Part Of Source"@en .


###  http://www.semanticweb.org/georg/ontologies/2022/3/WOOD#PartOfUsedMethods
:PartOfUsedMethods rdf:type owl:ObjectProperty ;
                   rdfs:subPropertyOf :PartOfProcess ;
                   rdfs:domain :UsedMethods ;
                   rdfs:range :Investigation ;
                   rdfs:label "Part Of Used Methods"@en .


###  http://www.semanticweb.org/georg/ontologies/2022/3/WOOD#PersonObjectProperties
:PersonObjectProperties rdf:type owl:ObjectProperty ;
                        rdfs:label "Person Object Properties"@en .


###  http://www.semanticweb.org/georg/ontologies/2022/3/WOOD#Removability
:Removability rdf:type owl:ObjectProperty ;
              rdfs:subPropertyOf :RepairObjectProperties ;
              rdfs:label "Removability"@en .


###  http://www.semanticweb.org/georg/ontologies/2022/3/WOOD#RepairObjectProperties
:RepairObjectProperties rdf:type owl:ObjectProperty ;
                        rdfs:label "Repair Object Properties"@en .


###  http://www.semanticweb.org/georg/ontologies/2022/3/WOOD#ReportObjectProperties
:ReportObjectProperties rdf:type owl:ObjectProperty ;
                        rdfs:label "Report Object Properties"@en .


###  http://www.semanticweb.org/georg/ontologies/2022/3/WOOD#RotDecompositionType
:RotDecompositionType rdf:type owl:ObjectProperty ;
                      rdfs:subPropertyOf :InfluenceObjectProperties ;
                      rdfs:label "Rot Decomposition Type"@en .


###  http://www.semanticweb.org/georg/ontologies/2022/3/WOOD#RotResistance
:RotResistance rdf:type owl:ObjectProperty ;
               rdfs:subPropertyOf :WoodObjectProperties .


###  http://www.semanticweb.org/georg/ontologies/2022/3/WOOD#StatusOfSource
:StatusOfSource rdf:type owl:ObjectProperty ;
                rdfs:subPropertyOf :ReportObjectProperties ;
                rdfs:label "Status Of Source"@en .


###  http://www.semanticweb.org/georg/ontologies/2022/3/WOOD#WoodColour
:WoodColour rdf:type owl:ObjectProperty ;
            rdfs:subPropertyOf :RepairObjectProperties ;
            rdfs:label "Wood Colour"@en .


###  http://www.semanticweb.org/georg/ontologies/2022/3/WOOD#WoodGrain
:WoodGrain rdf:type owl:ObjectProperty ;
           rdfs:subPropertyOf :RepairObjectProperties ;
           rdfs:label "Wood Grain"@en .


###  http://www.semanticweb.org/georg/ontologies/2022/3/WOOD#WoodObjectProperties
:WoodObjectProperties rdf:type owl:ObjectProperty ;
                      rdfs:label "Wood Object Properties"@en .


###  http://www.semanticweb.org/georg/ontologies/2022/3/WOOD#Writes
:Writes rdf:type owl:ObjectProperty ;
        rdfs:subPropertyOf :PersonObjectProperties ;
        rdfs:domain :BuildingDamageExpert ;
        rdfs:range :Report ;
        rdfs:label "Writes"@en .


###  http://www.semanticweb.org/georg/ontologies/2022/3/WOOD#WritesAbout
:WritesAbout rdf:type owl:ObjectProperty ;
             rdfs:subPropertyOf :GeneralObjectProperties ;
             rdfs:domain :Report ;
             rdfs:range <https://w3id.org/bot#Building> ;
             rdfs:label "Writes About"@en .


###  http://www.semanticweb.org/georg/ontologies/2022/3/WOOD#isWorkedOnBy
:isWorkedOnBy rdf:type owl:ObjectProperty ;
              rdfs:subPropertyOf :GeneralObjectProperties ;
              rdfs:domain :Repair ;
              rdfs:range :Worker ;
              rdfs:label "is Worked On By"@en .


#################################################################
#    Data properties
#################################################################

###  http://www.semanticweb.org/georg/ontologies/2022/3/WOOD#AdjacentHumidity
:AdjacentHumidity rdf:type owl:DatatypeProperty ;
                  rdfs:subPropertyOf :WoodDataProperties ;
                  rdfs:domain :WoodComponent ;
                  rdfs:range xsd:int ;
                  rdfs:label "Adjacent Humidity"@en .


###  http://www.semanticweb.org/georg/ontologies/2022/3/WOOD#BuildingDataProperties
:BuildingDataProperties rdf:type owl:DatatypeProperty ;
                        rdfs:label "Building Data Properties"@en .


###  http://www.semanticweb.org/georg/ontologies/2022/3/WOOD#BuildingDate
:BuildingDate rdf:type owl:DatatypeProperty ;
              rdfs:subPropertyOf :BuildingDataProperties ;
              rdfs:range xsd:dateTime ;
              rdfs:label "Building Date"@en .


###  http://www.semanticweb.org/georg/ontologies/2022/3/WOOD#BulkDensity
:BulkDensity rdf:type owl:DatatypeProperty ;
             rdfs:subPropertyOf :WoodDataProperties ;
             rdfs:domain :WoodComponent ;
             rdfs:range xsd:int .


###  http://www.semanticweb.org/georg/ontologies/2022/3/WOOD#CauseDataProperties
:CauseDataProperties rdf:type owl:DatatypeProperty ;
                     rdfs:label "Cause Data Properties"@en .


###  http://www.semanticweb.org/georg/ontologies/2022/3/WOOD#CauseRepaired
:CauseRepaired rdf:type owl:DatatypeProperty ;
               rdfs:subPropertyOf :CauseDataProperties ;
               rdfs:domain :CauseOfDamage ;
               rdfs:range xsd:boolean ;
               rdfs:label "Cause Repaired"@en .


###  http://www.semanticweb.org/georg/ontologies/2022/3/WOOD#Condensation
:Condensation rdf:type owl:DatatypeProperty ;
              rdfs:subPropertyOf :WoodDataProperties ;
              rdfs:domain :WoodComponent ;
              rdfs:range xsd:boolean ;
              rdfs:label "Condensation"@en .


###  http://www.semanticweb.org/georg/ontologies/2022/3/WOOD#ConstructionMethod
:ConstructionMethod rdf:type owl:DatatypeProperty ;
                    rdfs:subPropertyOf :BuildingDataProperties ;
                    rdfs:range xsd:string ;
                    rdfs:label "Construction Method"@en .


###  http://www.semanticweb.org/georg/ontologies/2022/3/WOOD#DamageDataProperties
:DamageDataProperties rdf:type owl:DatatypeProperty ;
                      rdfs:label "Damage Data Properties"@en .


###  http://www.semanticweb.org/georg/ontologies/2022/3/WOOD#DamageRepaired
:DamageRepaired rdf:type owl:DatatypeProperty ;
                rdfs:subPropertyOf :DamageDataProperties ;
                rdfs:domain :WoodDamage ;
                rdfs:range xsd:boolean ;
                rdfs:label "Damage Repaired"@en .


###  http://www.semanticweb.org/georg/ontologies/2022/3/WOOD#DateOfInspection
:DateOfInspection rdf:type owl:DatatypeProperty ;
                  rdfs:subPropertyOf :ReportDataProperties ;
                  rdfs:domain :Report ;
                  rdfs:range xsd:dateTime ;
                  rdfs:label "Date Of Inspection"@en .


###  http://www.semanticweb.org/georg/ontologies/2022/3/WOOD#DateOfSurvey
:DateOfSurvey rdf:type owl:DatatypeProperty ;
              rdfs:subPropertyOf :ReportDataProperties ;
              rdfs:domain :Report ;
              rdfs:range xsd:dateTime ;
              rdfs:label "Date Of Survey"@en .


###  http://www.semanticweb.org/georg/ontologies/2022/3/WOOD#DateRenovation
:DateRenovation rdf:type owl:DatatypeProperty ;
                rdfs:subPropertyOf :BuildingDataProperties ;
                rdfs:range xsd:dateTime ;
                rdfs:label "Date Renovation"@en .


###  http://www.semanticweb.org/georg/ontologies/2022/3/WOOD#GroundContact
:GroundContact rdf:type owl:DatatypeProperty ;
               rdfs:subPropertyOf :WoodDataProperties ;
               rdfs:domain :WoodComponent ;
               rdfs:range xsd:boolean ;
               rdfs:label "Ground Contact"@en .


###  http://www.semanticweb.org/georg/ontologies/2022/3/WOOD#HadRenovation
:HadRenovation rdf:type owl:DatatypeProperty ;
               rdfs:subPropertyOf :BuildingDataProperties ;
               rdfs:range xsd:boolean ;
               rdfs:label "Had Renovation"@en .


###  http://www.semanticweb.org/georg/ontologies/2022/3/WOOD#ModulusOfElasticity
:ModulusOfElasticity rdf:type owl:DatatypeProperty ;
                     rdfs:subPropertyOf :WoodDataProperties ;
                     rdfs:domain :WoodComponent ;
                     rdfs:range xsd:int ;
                     rdfs:label "Modulus Of Elasticity"@en .


###  http://www.semanticweb.org/georg/ontologies/2022/3/WOOD#MonumentProtection
:MonumentProtection rdf:type owl:DatatypeProperty ;
                    rdfs:subPropertyOf :BuildingDataProperties ;
                    rdfs:range xsd:boolean ;
                    rdfs:label "Monument Protection"@en .


###  http://www.semanticweb.org/georg/ontologies/2022/3/WOOD#PH-Value
:PH-Value rdf:type owl:DatatypeProperty ;
          rdfs:subPropertyOf :WoodDataProperties ;
          rdfs:domain :WoodComponent ;
          rdfs:range xsd:int ;
          rdfs:label "PH-Value"@en .


###  http://www.semanticweb.org/georg/ontologies/2022/3/WOOD#ReportDataProperties
:ReportDataProperties rdf:type owl:DatatypeProperty ;
                      rdfs:label "Report Data Properties"@en .


###  http://www.semanticweb.org/georg/ontologies/2022/3/WOOD#Solidity
:Solidity rdf:type owl:DatatypeProperty ;
          rdfs:subPropertyOf :WoodDataProperties ;
          rdfs:domain :WoodComponent ;
          rdfs:range xsd:int ;
          rdfs:label "Solidity"@en .


###  http://www.semanticweb.org/georg/ontologies/2022/3/WOOD#Temperature
:Temperature rdf:type owl:DatatypeProperty ;
             rdfs:subPropertyOf :WoodDataProperties ;
             rdfs:domain :WoodComponent ;
             rdfs:range xsd:int ;
             rdfs:label "Temperature"@en .


###  http://www.semanticweb.org/georg/ontologies/2022/3/WOOD#UserRequirements
:UserRequirements rdf:type owl:DatatypeProperty ;
                  rdfs:subPropertyOf :BuildingDataProperties ;
                  rdfs:range xsd:string ;
                  rdfs:label "User Requirements"@en .


###  http://www.semanticweb.org/georg/ontologies/2022/3/WOOD#Utilization
:Utilization rdf:type owl:DatatypeProperty ;
             rdfs:subPropertyOf :BuildingDataProperties ;
             rdfs:range xsd:string ;
             rdfs:label "Utilization"@en .


###  http://www.semanticweb.org/georg/ontologies/2022/3/WOOD#Weather
:Weather rdf:type owl:DatatypeProperty ;
         rdfs:subPropertyOf :WoodDataProperties ;
         rdfs:domain :WoodComponent ;
         rdfs:range xsd:boolean ;
         rdfs:label "Weather"@en .


###  http://www.semanticweb.org/georg/ontologies/2022/3/WOOD#WoodAge
:WoodAge rdf:type owl:DatatypeProperty ;
         rdfs:subPropertyOf :WoodDataProperties ;
         rdfs:domain :WoodComponent ;
         rdfs:range xsd:dateTime .


###  http://www.semanticweb.org/georg/ontologies/2022/3/WOOD#WoodDataProperties
:WoodDataProperties rdf:type owl:DatatypeProperty ;
                    rdfs:label "Wood Data Properties"@en .


###  http://www.semanticweb.org/georg/ontologies/2022/3/WOOD#WoodMoisture
:WoodMoisture rdf:type owl:DatatypeProperty ;
              rdfs:subPropertyOf :WoodDataProperties ;
              rdfs:domain :WoodComponent ;
              rdfs:range xsd:int .


#################################################################
#    Classes
#################################################################

###  http://www.opengis.net/ont/geosparql#Geometry
<http://www.opengis.net/ont/geosparql#Geometry> rdf:type owl:Class ;
                                                rdfs:subClassOf :WoodComponent .


###  http://www.semanticweb.org/christian/ontologies/2021/4/untitled-ontology-14#CostOfRestoration
<http://www.semanticweb.org/christian/ontologies/2021/4/untitled-ontology-14#CostOfRestoration> rdf:type owl:Class ;
                                                                                                rdfs:comment "Added costs of the needed restoration procedures. first the individual cost positions are indicated and as last the total costs are indicated."@en ;
                                                                                                rdfs:label "Cost of restoration"@en .


###  http://www.semanticweb.org/christian/ontologies/2021/4/untitled-ontology-14#Insectclasses
<http://www.semanticweb.org/christian/ontologies/2021/4/untitled-ontology-14#Insectclasses> rdf:type owl:Class ;
                                                                                            rdfs:subClassOf :BiologicalInfluences ;
                                                                                            owl:disjointWith :Rot ;
                                                                                            rdfs:comment "Describes superordinate classes that describe characteristics, behavior, and distribution of insects."@en ;
                                                                                            rdfs:label "Insectclasses"@en .


###  http://www.semanticweb.org/christian/ontologies/2021/4/untitled-ontology-14#Photos
<http://www.semanticweb.org/christian/ontologies/2021/4/untitled-ontology-14#Photos> rdf:type owl:Class ;
                                                                                     rdfs:subClassOf :BuildingDocumentation ,
                                                                                                     [ rdf:type owl:Restriction ;
                                                                                                       owl:onProperty :StatusOfSource ;
                                                                                                       owl:someValuesFrom :SourcesPresentState
                                                                                                     ] .


###  http://www.semanticweb.org/georg/ontologies/2022/3/WOOD#AaRdT
:AaRdT rdf:type owl:Class ;
       rdfs:subClassOf :ExternalResources ,
                       [ rdf:type owl:Restriction ;
                         owl:onProperty :StatusOfSource ;
                         owl:someValuesFrom :SourcesTargetState
                       ] ;
       rdfs:comment "The generally recognized rules of construction represent the accumulation of scientific, technical and craftsmanship experiences recognized in the construction industry, which are universally known and recognized as correct and necessary."@en ;
       rdfs:label "AaRdT"@en .


###  http://www.semanticweb.org/georg/ontologies/2022/3/WOOD#Acids
:Acids rdf:type owl:Class ;
       rdfs:subClassOf :ChemicalInfluences ,
                       [ rdf:type owl:Restriction ;
                         owl:onProperty :CanCreateDamage ;
                         owl:someValuesFrom :BurnMarks
                       ] ,
                       [ rdf:type owl:Restriction ;
                         owl:onProperty :CanCreateDamage ;
                         owl:someValuesFrom :DecompositionAndMaceration
                       ] ;
       rdfs:comment "The wood strength decreases due to the acid penetration and this can lead to the failure of the structure. If the pH value ranges between 2 < pH < 11, wood corrosion is generally low. Softwoods have a much higher corrosion resistance than hardwoods. glulam constructions have a higher chemical resistance than solid wood constructions."@en ;
       rdfs:label "Acids"@en .


###  http://www.semanticweb.org/georg/ontologies/2022/3/WOOD#ActiveCause
:ActiveCause rdf:type owl:Class ;
             rdfs:subClassOf :DamageStatus ;
             owl:disjointWith :InactiveCause ;
             rdfs:comment "The cause of the damage under investigation is still active. The cause must be eliminated to prevent further damage in the future."@en ;
             rdfs:label "Active cause"@en .


###  http://www.semanticweb.org/georg/ontologies/2022/3/WOOD#AirHumidity
:AirHumidity rdf:type owl:Class ;
             owl:equivalentClass [ rdf:type owl:Restriction ;
                                   owl:onProperty :FindsProperties ;
                                   owl:someValuesFrom :AirHumidity
                                 ] ;
             rdfs:subClassOf :SearchedProperties ;
             rdfs:comment "Air Humidity refers to the proportion of water vapor in the gas mixture of the air."@en ;
             rdfs:label "Air humidity"@en .


###  http://www.semanticweb.org/georg/ontologies/2022/3/WOOD#AxeHatchet
:AxeHatchet rdf:type owl:Class ;
            rdfs:subClassOf :Splitting ;
            rdfs:comment "The axe is a tool and generally consists of a piece of steel with a forged steel cutting edge and the handlerdfs:comment"@en ;
            rdfs:label "Axe/ Hatchet"@en .


###  http://www.semanticweb.org/georg/ontologies/2022/3/WOOD#AxeTest
:AxeTest rdf:type owl:Class ;
         rdfs:subClassOf :InvestigationProcedure ,
                         [ rdf:type owl:Restriction ;
                           owl:onProperty :FindsProperties ;
                           owl:someValuesFrom :ConcealedComponents
                         ] ,
                         [ rdf:type owl:Restriction ;
                           owl:onProperty :HasDegreeOfDestruction ;
                           owl:someValuesFrom :DestructiveProcesses
                         ] ,
                         [ rdf:type owl:Restriction ;
                           owl:onProperty :HasPlace ;
                           owl:someValuesFrom :InSitu
                         ] ,
                         [ rdf:type owl:Restriction ;
                           owl:onProperty :HasTime ;
                           owl:someValuesFrom :FastProcesses
                         ] ;
         rdfs:comment "By removing material using a tool such as an axe, the suspect area can be exposed and examined."@en ;
         rdfs:label "Axe test"@en .


###  http://www.semanticweb.org/georg/ontologies/2022/3/WOOD#AzobeAZO
:AzobeAZO rdf:type owl:Class ;
          rdfs:subClassOf :Hardwood ,
                          [ rdf:type owl:Restriction ;
                            owl:onProperty :DimensionalStability ;
                            owl:someValuesFrom :LowDimensionalStability
                          ] ,
                          [ rdf:type owl:Restriction ;
                            owl:onProperty :DimensionalStability ;
                            owl:someValuesFrom :MediumDimensionalStability
                          ] ,
                          [ rdf:type owl:Restriction ;
                            owl:onProperty :InsectResistance ;
                            owl:someValuesFrom :VeryHighInsectResistance
                          ] ,
                          [ rdf:type owl:Restriction ;
                            owl:onProperty :RotResistance ;
                            owl:someValuesFrom :HighRotResistance
                          ] ;
          rdfs:comment """Wood material of azobe trees.

Colour: 
Light reddish brown/ deep reddish brown with light violet tinge

Special properties resistance to insects:
Also very high resistance to termites and Piddocks,
Exceptions are tropical waters."""@en ;
          rdfs:label "Azobe (AZO)"@en .


###  http://www.semanticweb.org/georg/ontologies/2022/3/WOOD#BandSaws
:BandSaws rdf:type owl:Class ;
          rdfs:subClassOf :Sawing ;
          rdfs:comment "A band saw is a machine tool whose tool consists of a band saw blade soldered or welded into a closed ring"@en ;
          rdfs:label "Band saw"@en .


###  http://www.semanticweb.org/georg/ontologies/2022/3/WOOD#BeamLeafling
:BeamLeafling rdf:type owl:Class ;
              rdfs:subClassOf :Leaflet ,
                              [ rdf:type owl:Restriction ;
                                owl:onProperty :RotDecompositionType ;
                                owl:someValuesFrom :BrownRot
                              ] ;
              rdfs:comment """Preferred wood species:
Hardwood and softwood

Optimal living conditions of wood moisture content in M-%:
> 35%

Optimal living conditions of the temperature range in °C:
26°C to 35°C

Additional notes:
Mycelium survives higher temperature and dry rigidity."""@en ;
              rdfs:label "Beam leafling"@en ,
                         "Gloeophyllum trabeum"@la .


###  http://www.semanticweb.org/georg/ontologies/2022/3/WOOD#BeechBU
:BeechBU rdf:type owl:Class ;
         rdfs:subClassOf :Hardwood ,
                         [ rdf:type owl:Restriction ;
                           owl:onProperty :DimensionalStability ;
                           owl:someValuesFrom :LowDimensionalStability
                         ] ,
                         [ rdf:type owl:Restriction ;
                           owl:onProperty :InsectResistance ;
                           owl:someValuesFrom :LowInsectResistance
                         ] ,
                         [ rdf:type owl:Restriction ;
                           owl:onProperty :RotResistance ;
                           owl:someValuesFrom :VeryLowRotResistance
                         ] ;
         rdfs:comment """Wood material of beech trees.

Colour: 
Pale yellowish to reddish grey, often unevenly pitted with patchy reddish brown. Sapwood and heartwood are not distinguished."""@en ;
         rdfs:label "Beech (BU)"@en .


###  http://www.semanticweb.org/georg/ontologies/2022/3/WOOD#BiologicalInfluences
:BiologicalInfluences rdf:type owl:Class ;
                      rdfs:subClassOf :CauseOfDamage ;
                      rdfs:comment "Influences that have a biological origin."@en ;
                      rdfs:label "Biological influences"@en .


###  http://www.semanticweb.org/georg/ontologies/2022/3/WOOD#BiologicalProcesses
:BiologicalProcesses rdf:type owl:Class ;
                     owl:equivalentClass [ rdf:type owl:Restriction ;
                                           owl:onProperty :CanCreateDamage ;
                                           owl:someValuesFrom :BiologicalProcesses
                                         ] ;
                     rdfs:subClassOf :WoodDamage ;
                     rdfs:comment "It is a process in which changes occure, which are triggered by biological ormanisms."@en ;
                     rdfs:label "Biological processes"@en .


###  http://www.semanticweb.org/georg/ontologies/2022/3/WOOD#BlowerDoorTest
:BlowerDoorTest rdf:type owl:Class ;
                rdfs:subClassOf :InvestigationProcedure ,
                                [ rdf:type owl:Restriction ;
                                  owl:onProperty :FindsProperties ;
                                  owl:someValuesFrom :ThermalInsulation
                                ] ,
                                [ rdf:type owl:Restriction ;
                                  owl:onProperty :HasDegreeOfDestruction ;
                                  owl:someValuesFrom :NonDestructiveProcesses
                                ] ,
                                [ rdf:type owl:Restriction ;
                                  owl:onProperty :HasPlace ;
                                  owl:someValuesFrom :InSitu
                                ] ,
                                [ rdf:type owl:Restriction ;
                                  owl:onProperty :HasTime ;
                                  owl:someValuesFrom :SlowProcesses
                                ] ;
                rdfs:comment "The differential pressure measurement method is used to measure the air tightness of a building. This method is used to detect leaks in the building shell."@en ;
                rdfs:label "Blower-door-test"@en .


###  http://www.semanticweb.org/georg/ontologies/2022/3/WOOD#BlueStainFungi
:BlueStainFungi rdf:type owl:Class ;
                rdfs:subClassOf :WoodDiscoloringFungi ;
                owl:disjointWith :Molds ;
                rdfs:comment """Preferred wood species:
Mainly softwood

Further notes:
Blue-green discoloration of sapwood."""@en ;
                rdfs:label "Blue stain fungi"@en .


###  http://www.semanticweb.org/georg/ontologies/2022/3/WOOD#BrownCellarSponge
:BrownCellarSponge rdf:type owl:Class ;
                   rdfs:subClassOf :WetRotFungi ,
                                   [ rdf:type owl:Restriction ;
                                     owl:onProperty :RotDecompositionType ;
                                     owl:someValuesFrom :BrownRot
                                   ] ;
                   rdfs:comment """Preferred wood species:
Softwood and hardwood

Optimal living conditions of wood moisture content in M-%:
45% to 60%

Optimal living conditions of the temperature range in °C:
22°C to 26°C

Further notes:
Mycelium dies in case of dehydration."""@en ;
                   rdfs:label "Brown cellar sponge"@en ,
                              "Coniophora puteana"@la .


###  http://www.semanticweb.org/georg/ontologies/2022/3/WOOD#BrownRot
:BrownRot rdf:type owl:Class ;
          owl:equivalentClass [ rdf:type owl:Restriction ;
                                owl:onProperty :RotDecompositionType ;
                                owl:someValuesFrom :BrownRot
                              ] ;
          rdfs:subClassOf :WoodDestroyingFungi ;
          rdfs:comment "Brown rot, wood structure is destroyed by decomposition of cellulose"@en ;
          rdfs:label "Brown rot"@en .


###  http://www.semanticweb.org/georg/ontologies/2022/3/WOOD#BrushMachining
:BrushMachining rdf:type owl:Class ;
                rdfs:subClassOf :Separate ;
                rdfs:comment "Brush machining is a process of machining the workpiece with a brushing tool, mainly to change the surface structure but also the shape"@en ;
                rdfs:label "Brush machining"@en .


###  http://www.semanticweb.org/georg/ontologies/2022/3/WOOD#BuildingDamageExpert
:BuildingDamageExpert rdf:type owl:Class ;
                      rdfs:subClassOf <http://xmlns.com/foaf/0.1/Person> ;
                      owl:disjointWith :BuildingOwner ,
                                       :Client ;
                      rdfs:comment "Job title for people which have a background working with damages in buildings."@en ;
                      rdfs:label "Expert for damages in buildings"@en .


###  http://www.semanticweb.org/georg/ontologies/2022/3/WOOD#BuildingDocumentation
:BuildingDocumentation rdf:type owl:Class ;
                       rdfs:subClassOf :Sources ;
                       rdfs:comment "Sources that contain information specific to the current construction project."@en ;
                       rdfs:label "Building documentation"@en .


###  http://www.semanticweb.org/georg/ontologies/2022/3/WOOD#BuildingOwner
:BuildingOwner rdf:type owl:Class ;
               rdfs:subClassOf <http://xmlns.com/foaf/0.1/Person> ;
               rdfs:comment "A person who is the owner of a specific building."@en ;
               rdfs:label "Building owner"@en .


###  http://www.semanticweb.org/georg/ontologies/2022/3/WOOD#BuildingTimber
:BuildingTimber rdf:type owl:Class ;
                rdfs:subClassOf :SolidWood ;
                rdfs:comment "Building timber is made by cutting or profiling round timber."@en ;
                rdfs:label "Building timber"@en .


###  http://www.semanticweb.org/georg/ontologies/2022/3/WOOD#BulkDensity
:BulkDensity rdf:type owl:Class ;
             owl:equivalentClass [ rdf:type owl:Restriction ;
                                   owl:onProperty :FindsProperties ;
                                   owl:someValuesFrom :BulkDensity
                                 ] ;
             rdfs:subClassOf :SearchedProperties .


###  http://www.semanticweb.org/georg/ontologies/2022/3/WOOD#BurnMarks
:BurnMarks rdf:type owl:Class ;
           owl:equivalentClass [ rdf:type owl:Restriction ;
                                 owl:onProperty :CanCreateDamage ;
                                 owl:someValuesFrom :BurnMarks
                               ] ;
           rdfs:subClassOf :ChemicalProcesses ;
           rdfs:comment "A combustion is an exothermic reaction in which a combustible fuel is oxidized by oxygen. Burn marks are produced during combustion."@en ;
           rdfs:label "Burn marks"@en .


###  http://www.semanticweb.org/georg/ontologies/2022/3/WOOD#Burning
:Burning rdf:type owl:Class ;
         rdfs:subClassOf :ServiceStresses ,
                         [ rdf:type owl:Restriction ;
                           owl:onProperty :CanCreateDamage ;
                           owl:someValuesFrom :BurnMarks
                         ] ,
                         [ rdf:type owl:Restriction ;
                           owl:onProperty :CanCreateDamage ;
                           owl:someValuesFrom :Cracks
                         ] ,
                         [ rdf:type owl:Restriction ;
                           owl:onProperty :CanCreateDamage ;
                           owl:someValuesFrom :Fractures
                         ] ,
                         [ rdf:type owl:Restriction ;
                           owl:onProperty :CanCreateDamage ;
                           owl:someValuesFrom :Holes
                         ] ;
         rdfs:comment "Fire damage to structural components, which reduces the load-bearing of the cross-sections of the structure."@en ;
         rdfs:label "Burning"@en .


###  http://www.semanticweb.org/georg/ontologies/2022/3/WOOD#ButterflySpore
:ButterflySpore rdf:type owl:Class ;
                rdfs:subClassOf :WetRotFungi ,
                                [ rdf:type owl:Restriction ;
                                  owl:onProperty :RotDecompositionType ;
                                  owl:someValuesFrom :WhiteRot
                                ] ;
                rdfs:comment """Preferred wood species:
Hardwood and hardly any softwood

Optimal living conditions of wood moisture content in M-%:
> 35%

Optimal living conditions of the temperature range in °C:
23°C to 26°C

Additional notes:
Mycelium dies when dried out."""@en ;
                rdfs:label "Butterfly spore"@en ,
                           "Coriolus versicolor"@la .


###  http://www.semanticweb.org/georg/ontologies/2022/3/WOOD#Calculations
:Calculations rdf:type owl:Class ;
              rdfs:subClassOf :BuildingDocumentation ,
                              [ rdf:type owl:Restriction ;
                                owl:onProperty :StatusOfSource ;
                                owl:someValuesFrom :SourcesPresentState
                              ] ;
              rdfs:comment "Calculations that represent information about the building. This can be information on structural analysis, thermal insulation, noise protection and other topics."@en ;
              rdfs:label "Calculations"@en .


###  http://www.semanticweb.org/georg/ontologies/2022/3/WOOD#Carve
:Carve rdf:type owl:Class ;
       rdfs:subClassOf :Separate ;
       rdfs:comment "Carving is a manufacturing process in which chips are separated by hitting the tool. The chisel is applied at a steep angle to the workpiece surface"@en ;
       rdfs:label "Carve"@en .


###  http://www.semanticweb.org/georg/ontologies/2022/3/WOOD#CauseOfDamage
:CauseOfDamage rdf:type owl:Class ;
               rdfs:comment "Describes the cause of the damage. Any damage can only come from a specific cause. Thus, every damage is linked to the cause."@en ;
               rdfs:label "Cause of damage"@en .


###  http://www.semanticweb.org/georg/ontologies/2022/3/WOOD#CementFiberBoards
:CementFiberBoards rdf:type owl:Class ;
                   rdfs:subClassOf :WoodBasedMaterials ;
                   rdfs:comment "Cement fiber boards consist of Portland cement, silicate aggregates and cellulose fibers."@en ;
                   rdfs:label "Cement fiber boards"@en .


###  http://www.semanticweb.org/georg/ontologies/2022/3/WOOD#Chainsaws
:Chainsaws rdf:type owl:Class ;
           rdfs:subClassOf :Sawing ;
           rdfs:comment "The chainsaw uses a cutting chain, which is driven by a small motor"@en ;
           rdfs:label "Chainsaw"@en .


###  http://www.semanticweb.org/georg/ontologies/2022/3/WOOD#ChemicalInfluences
:ChemicalInfluences rdf:type owl:Class ;
                    rdfs:subClassOf :CauseOfDamage ;
                    rdfs:comment "Influences that have a Chemical origin."@en ;
                    rdfs:label "Chemical influences"@en .


###  http://www.semanticweb.org/georg/ontologies/2022/3/WOOD#ChemicalProcesses
:ChemicalProcesses rdf:type owl:Class ;
                   owl:equivalentClass [ rdf:type owl:Restriction ;
                                         owl:onProperty :CanCreateDamage ;
                                         owl:someValuesFrom :ChemicalProcesses
                                       ] ;
                   rdfs:subClassOf :WoodDamage ;
                   rdfs:comment "It is a process where chemical reactions change the component."@en ;
                   rdfs:label "Chemical processes"@en .


###  http://www.semanticweb.org/georg/ontologies/2022/3/WOOD#ChemicalReaction
:ChemicalReaction rdf:type owl:Class ;
                  owl:equivalentClass [ rdf:type owl:Restriction ;
                                        owl:onProperty :FindsProperties ;
                                        owl:someValuesFrom :ChemicalReaction
                                      ] ;
                  rdfs:subClassOf :SearchedProperties ;
                  rdfs:comment "A chemical reaction is a process in which one or usually multiple chemical compounds are converted into others and energy is released or absorbed."@en ;
                  rdfs:label "Chemical reaction"@en .


###  http://www.semanticweb.org/georg/ontologies/2022/3/WOOD#Chipboard
:Chipboard rdf:type owl:Class ;
           rdfs:subClassOf :WoodBasedMaterials ;
           rdfs:comment "Flat pressed boards are made by pressing small wood chips with adhesives or mineral binders. The chips are preferably parallel to the surface of the board and are usually produced in several layers. In both directions of the panel plane there are almost equivalent tensile, compressive and flexural strengths achieved."@en ;
           rdfs:label "Chipboard"@en .


###  http://www.semanticweb.org/georg/ontologies/2022/3/WOOD#Chisel
:Chisel rdf:type owl:Class ;
        rdfs:subClassOf :Carve ;
        rdfs:comment "The chisel is a tool made of steel, which has a hardened wedge-shaped cutting edge. Chisels are used with a hammer to divide objects or to cut off parts from them"@en ;
        rdfs:label "Chisel"@en .


###  http://www.semanticweb.org/georg/ontologies/2022/3/WOOD#Chromatography
:Chromatography rdf:type owl:Class ;
                rdfs:subClassOf :InvestigationProcedure ,
                                [ rdf:type owl:Restriction ;
                                  owl:onProperty :FindsProperties ;
                                  owl:someValuesFrom :RotContamination
                                ] ,
                                [ rdf:type owl:Restriction ;
                                  owl:onProperty :HasDegreeOfDestruction ;
                                  owl:someValuesFrom :LowDestructiveProcesses
                                ] ,
                                [ rdf:type owl:Restriction ;
                                  owl:onProperty :HasPlace ;
                                  owl:someValuesFrom :InSitu
                                ] ,
                                [ rdf:type owl:Restriction ;
                                  owl:onProperty :HasPlace ;
                                  owl:someValuesFrom :Laboratory
                                ] ,
                                [ rdf:type owl:Restriction ;
                                  owl:onProperty :HasTime ;
                                  owl:someValuesFrom :SlowProcesses
                                ] ;
                rdfs:comment "In chromatography, a mixture of substances is separated into its individual components. This can provide an indication about the fungal infestation."@en ;
                rdfs:label "Chromatography"@en .


###  http://www.semanticweb.org/georg/ontologies/2022/3/WOOD#CircularSaws
:CircularSaws rdf:type owl:Class ;
              rdfs:subClassOf :Sawing ;
              rdfs:comment "A circular saw is a machine tool for cutting workpieces. It uses a round cutting disc, which is rotated in its axis"@en ;
              rdfs:label "Circular saw"@en .


###  http://www.semanticweb.org/georg/ontologies/2022/3/WOOD#Clamps
:Clamps rdf:type owl:Class ;
        rdfs:subClassOf :JoinTools ,
                        [ rdf:type owl:Restriction ;
                          owl:onProperty :FittingType ;
                          owl:someValuesFrom :ForceFit
                        ] ,
                        [ rdf:type owl:Restriction ;
                          owl:onProperty :Removability ;
                          owl:someValuesFrom :Solvable
                        ] ;
        rdfs:comment "Clamping devices are all devices for firmly fixing a workpiece or tool during the machining process"@en ;
        rdfs:label "Clamps"@en .


###  http://www.semanticweb.org/georg/ontologies/2022/3/WOOD#Classification
:Classification rdf:type owl:Class ;
                rdfs:subClassOf :WoodComponent ;
                rdfs:comment "Assignment of service classes according to DIN EN 335 for wooden components."@en ;
                rdfs:label "Classification"@en .


###  http://www.semanticweb.org/georg/ontologies/2022/3/WOOD#Client
:Client rdf:type owl:Class ;
        rdfs:subClassOf <http://xmlns.com/foaf/0.1/Person> ;
        rdfs:comment "A person who conducts a transaction with a counterparty."@en ;
        rdfs:label "Client"@en .


###  http://www.semanticweb.org/georg/ontologies/2022/3/WOOD#Coat
:Coat rdf:type owl:Class ;
      rdfs:subClassOf :Repair ;
      rdfs:comment "Fabricate by applying a strong adhesive layer of shapeless fabric to a workpiece"@en ;
      rdfs:label "Coat"@en .


###  http://www.semanticweb.org/georg/ontologies/2022/3/WOOD#CoatTools
:CoatTools rdf:type owl:Class ;
           rdfs:subClassOf :Coat ;
           rdfs:comment "List of tools often used when coating components."@en ;
           rdfs:label "Coat tools"@en .


###  http://www.semanticweb.org/georg/ontologies/2022/3/WOOD#ColourConcealed
:ColourConcealed rdf:type owl:Class ;
                 owl:equivalentClass [ rdf:type owl:Restriction ;
                                       owl:onProperty :WoodColour ;
                                       owl:someValuesFrom :ColourConcealed
                                     ] ;
                 rdfs:subClassOf :ComponentColour ;
                 owl:disjointWith :ColourEmphasized ;
                 rdfs:comment "The color of the component is covered and no longer visible to the viewer."@en ;
                 rdfs:label "Colour concealed"@en .


###  http://www.semanticweb.org/georg/ontologies/2022/3/WOOD#ColourEmphasized
:ColourEmphasized rdf:type owl:Class ;
                  owl:equivalentClass [ rdf:type owl:Restriction ;
                                        owl:onProperty :WoodColour ;
                                        owl:someValuesFrom :ColourEmphasized
                                      ] ;
                  rdfs:subClassOf :ComponentColour ;
                  rdfs:comment "The colour of the component is still visible, but has changed accordingly to the used coating procedure."@en ;
                  rdfs:label "Colour emphasized"@en .


###  http://www.semanticweb.org/georg/ontologies/2022/3/WOOD#ComponentColour
:ComponentColour rdf:type owl:Class ;
                 rdfs:subClassOf :Coat ;
                 rdfs:comment "The color of the component after application of the selected coating."@en ;
                 rdfs:label "Component colour"@en .


###  http://www.semanticweb.org/georg/ontologies/2022/3/WOOD#ComponentGrain
:ComponentGrain rdf:type owl:Class ;
                rdfs:subClassOf :Coat ;
                rdfs:comment "Component grain describes a wavy pattern on the surface of the wood that is observed after the use of surface treatment."@en ;
                rdfs:label "Component grain"@en .


###  http://www.semanticweb.org/georg/ontologies/2022/3/WOOD#ConcealedComponents
:ConcealedComponents rdf:type owl:Class ;
                     owl:equivalentClass [ rdf:type owl:Restriction ;
                                           owl:onProperty :FindsProperties ;
                                           owl:someValuesFrom :ConcealedComponents
                                         ] ;
                     rdfs:subClassOf :SearchedProperties ;
                     rdfs:comment "Concealed components are components that are not directly visible to the viewer."@en ;
                     rdfs:label "Concealed components"@en .


###  http://www.semanticweb.org/georg/ontologies/2022/3/WOOD#ConnectionType
:ConnectionType rdf:type owl:Class ;
                rdfs:subClassOf :Join ;
                rdfs:comment "There are different options available for connecting at least two or more components. The connection should prevent the bodies from separating under applied forces."@en ;
                rdfs:label "Connection type"@en .


###  http://www.semanticweb.org/georg/ontologies/2022/3/WOOD#ConstructionVeneerPlywood
:ConstructionVeneerPlywood rdf:type owl:Class ;
                           rdfs:subClassOf :WoodBasedMaterials ;
                           rdfs:comment "Construction veneer plywood is created by arranging dried veneers and gluing them together."@en ;
                           rdfs:label "Construction veneer plywood"@en .


###  http://www.semanticweb.org/georg/ontologies/2022/3/WOOD#ConstructionWood
:ConstructionWood rdf:type owl:Class ;
                  rdfs:subClassOf :WoodComponent ;
                  rdfs:comment "Construction products made out of wood"@en ;
                  rdfs:label "Construction wood"@en .


###  http://www.semanticweb.org/georg/ontologies/2022/3/WOOD#Contracts
:Contracts rdf:type owl:Class ;
           rdfs:subClassOf :BuildingDocumentation ,
                           [ rdf:type owl:Restriction ;
                             owl:onProperty :StatusOfSource ;
                             owl:someValuesFrom :SourcesTargetState
                           ] .


###  http://www.semanticweb.org/georg/ontologies/2022/3/WOOD#Corrosion
:Corrosion rdf:type owl:Class ;
           owl:equivalentClass [ rdf:type owl:Restriction ;
                                 owl:onProperty :CanCreateDamage ;
                                 owl:someValuesFrom :Corrosion
                               ] ;
           rdfs:subClassOf :ChemicalProcesses ;
           rdfs:comment "Wood is corrosion resistend but fasteners, made of components that can rust, can lead to damages."@en ;
           rdfs:label "Corrosion"@en .


###  http://www.semanticweb.org/georg/ontologies/2022/3/WOOD#CorrosionOfSteelFasteners
:CorrosionOfSteelFasteners rdf:type owl:Class ;
                           rdfs:subClassOf :ChemicalInfluences ,
                                           [ rdf:type owl:Restriction ;
                                             owl:onProperty :CanCreateDamage ;
                                             owl:someValuesFrom :Corrosion
                                           ] ;
                           rdfs:comment "Steel fasteners embedded in the wood are largely protected against corrosion by the corrosion-resistant wood. However, non-embedded pieces of fasteners can corrode quickly if left untreated."@en ;
                           rdfs:label "Corrosion of steel fasteners"@en .


###  http://www.semanticweb.org/georg/ontologies/2022/3/WOOD#Costs
:Costs rdf:type owl:Class ;
       rdfs:subClassOf :StepsToTheEvidenceConclusion ;
       rdfs:comment "The cost of restoration can also be provided if a restoratoin procedure has been chosen. There are several ways to specify the cost of refurbishment in the report. Some possibilities are, for example: As an estimated costs, precise determination of costs by calculation, use of contractor quotations, determination on the basis of the manufacturer's costs, remaining reduced value, increase in value."@en ;
       rdfs:label "Cost"@en .


###  http://www.semanticweb.org/georg/ontologies/2022/3/WOOD#Cracks
:Cracks rdf:type owl:Class ;
        owl:equivalentClass [ rdf:type owl:Restriction ;
                              owl:onProperty :CanCreateDamage ;
                              owl:someValuesFrom :Cracks
                            ] ;
        rdfs:subClassOf :MechanicalProcesses ;
        rdfs:comment "Separation gap created by the tearing of a material object."@en ;
        rdfs:label "Cracks"@en .


###  http://www.semanticweb.org/georg/ontologies/2022/3/WOOD#CrossBeams
:CrossBeams rdf:type owl:Class ;
            rdfs:subClassOf :SolidWood ;
            rdfs:comment "Cross beams consist of four quarter timber segments of softwood which are glued together. These segments are fibre-parallel to each other. The outside of the round timber segments is turned inwards so that the inside of the rectangular cross-section creates a tube."@en ;
            rdfs:label "Cross beams"@en .


###  http://www.semanticweb.org/georg/ontologies/2022/3/WOOD#DNAAnalysis
:DNAAnalysis rdf:type owl:Class ;
             rdfs:subClassOf :InvestigationProcedure ,
                             [ rdf:type owl:Restriction ;
                               owl:onProperty :FindsProperties ;
                               owl:someValuesFrom :RotContamination
                             ] ,
                             [ rdf:type owl:Restriction ;
                               owl:onProperty :HasDegreeOfDestruction ;
                               owl:someValuesFrom :LowDestructiveProcesses
                             ] ,
                             [ rdf:type owl:Restriction ;
                               owl:onProperty :HasPlace ;
                               owl:someValuesFrom :Laboratory
                             ] ,
                             [ rdf:type owl:Restriction ;
                               owl:onProperty :HasTime ;
                               owl:someValuesFrom :SlowProcesses
                             ] ;
             rdfs:comment "It is possible to detect structural wood fungi via DNA which is still present in the infested wood. This method is always useful when the type of fungus cannot be clearly determined from the appearance on site."@en ;
             rdfs:label "DNA analysis"@en .


###  http://www.semanticweb.org/georg/ontologies/2022/3/WOOD#DamagePattern
:DamagePattern rdf:type owl:Class ;
               rdfs:subClassOf :OpticalInspection ,
                               [ rdf:type owl:Restriction ;
                                 owl:onProperty :FindsProperties ;
                                 owl:someValuesFrom :InsectContamination
                               ] ;
               owl:disjointWith :Discoloration ;
               rdfs:comment "The recognition of patterns or structures of the component or the destructive elements."@en ;
               rdfs:label "Damage Pattern"@en .


###  http://www.semanticweb.org/georg/ontologies/2022/3/WOOD#DamageStatus
:DamageStatus rdf:type owl:Class ;
              rdfs:subClassOf :Report ;
              rdfs:comment "Damages can have different states. Each state can change the implication the damage has on the building."@en ;
              rdfs:label "Damage Status"@en .


###  http://www.semanticweb.org/georg/ontologies/2022/3/WOOD#DecompositionAndMaceration
:DecompositionAndMaceration rdf:type owl:Class ;
                            owl:equivalentClass [ rdf:type owl:Restriction ;
                                                  owl:onProperty :CanCreateDamage ;
                                                  owl:someValuesFrom :DecompositionAndMaceration
                                                ] ;
                            rdfs:subClassOf :ChemicalProcesses ;
                            rdfs:comment "Intensive treatment of the wood with wood preservatives and fire proofing agents using potassium, ammonium salts or phosphate compounds causes a defibering of the outer wood structure. The structure becomes woolly, which is called maceration."@en ;
                            rdfs:label "Decomposition/ Maceration"@en .


###  http://www.semanticweb.org/georg/ontologies/2022/3/WOOD#Deflection
:Deflection rdf:type owl:Class ;
            owl:equivalentClass [ rdf:type owl:Restriction ;
                                  owl:onProperty :CanCreateDamage ;
                                  owl:someValuesFrom :Deflection
                                ] ;
            rdfs:subClassOf :MechanicalProcesses ;
            rdfs:comment "Deflection is the deformation of an elongated component that is overloaded and thus permanently deformed."@en ;
            rdfs:label "Deflection"@en .


###  http://www.semanticweb.org/georg/ontologies/2022/3/WOOD#DegreeOfDestruction
:DegreeOfDestruction rdf:type owl:Class ;
                     rdfs:subClassOf :Investigation ;
                     rdfs:comment "Level of destruction caused by the used investigation procedure."@en ;
                     rdfs:label "Degree of destruction"@en .


###  http://www.semanticweb.org/georg/ontologies/2022/3/WOOD#Delocalization
:Delocalization rdf:type owl:Class ;
                owl:equivalentClass [ rdf:type owl:Restriction ;
                                      owl:onProperty :CanCreateDamage ;
                                      owl:someValuesFrom :Delocalization
                                    ] ;
                rdfs:subClassOf :MechanicalProcesses ;
                rdfs:comment "The part was dislocated from its original position. It must be re-installed."@en ;
                rdfs:label "Delocalization"@en .


###  http://www.semanticweb.org/georg/ontologies/2022/3/WOOD#Dendrochronology
:Dendrochronology rdf:type owl:Class ;
                  rdfs:subClassOf :InvestigationProcedure ,
                                  [ rdf:type owl:Restriction ;
                                    owl:onProperty :FindsProperties ;
                                    owl:someValuesFrom :WoodAge
                                  ] ,
                                  [ rdf:type owl:Restriction ;
                                    owl:onProperty :FindsProperties ;
                                    owl:someValuesFrom :WoodSpecies
                                  ] ,
                                  [ rdf:type owl:Restriction ;
                                    owl:onProperty :HasDegreeOfDestruction ;
                                    owl:someValuesFrom :DestructiveProcesses
                                  ] ,
                                  [ rdf:type owl:Restriction ;
                                    owl:onProperty :HasPlace ;
                                    owl:someValuesFrom :Laboratory
                                  ] ,
                                  [ rdf:type owl:Restriction ;
                                    owl:onProperty :HasTime ;
                                    owl:someValuesFrom :SlowProcesses
                                  ] ;
                  rdfs:comment "This requires a sample of the component to be analyzed. The age of the tree can be determined from the annual rings of the used wood. The examinations can only be carried out by experts."@en ;
                  rdfs:label "Dendrochronology"@en .


###  http://www.semanticweb.org/georg/ontologies/2022/3/WOOD#DestructiveProcesses
:DestructiveProcesses rdf:type owl:Class ;
                      owl:equivalentClass [ rdf:type owl:Restriction ;
                                            owl:onProperty :HasDegreeOfDestruction ;
                                            owl:someValuesFrom :DestructiveProcesses
                                          ] ;
                      rdfs:subClassOf :DegreeOfDestruction ;
                      rdfs:comment "The examination object will be partially or fully destroyed."@en ;
                      rdfs:label "Destructive processes"@en .


###  http://www.semanticweb.org/georg/ontologies/2022/3/WOOD#DimensionalStability
:DimensionalStability rdf:type owl:Class ;
                      rdfs:subClassOf :WoodTypes .


###  http://www.semanticweb.org/georg/ontologies/2022/3/WOOD#Discoloration
:Discoloration rdf:type owl:Class ;
               rdfs:subClassOf :OpticalInspection ,
                               [ rdf:type owl:Restriction ;
                                 owl:onProperty :FindsProperties ;
                                 owl:someValuesFrom :ChemicalReaction
                               ] ;
               rdfs:label "Discoloration"@en ,
                          "The change of color in the component."@en .


###  http://www.semanticweb.org/georg/ontologies/2022/3/WOOD#DouglasFirDGA
:DouglasFirDGA rdf:type owl:Class ;
               rdfs:subClassOf :Softwood ,
                               [ rdf:type owl:Restriction ;
                                 owl:onProperty :DimensionalStability ;
                                 owl:someValuesFrom :HighDimensionalStability
                               ] ,
                               [ rdf:type owl:Restriction ;
                                 owl:onProperty :InsectResistance ;
                                 owl:someValuesFrom :MediumInsectResistance
                               ] ,
                               [ rdf:type owl:Restriction ;
                                 owl:onProperty :RotResistance ;
                                 owl:someValuesFrom :MediumRotResistance
                               ] ;
               rdfs:comment """Wood material of Douglas fir trees.

Colour: 
Yellowish white / reddish brown, darkens with time, late wood dark

Special properties resistance to fungi:
sapwood sensitive to blue stain"""@en ;
               rdfs:label "Douglas fir (DGA)"@en .


###  http://www.semanticweb.org/georg/ontologies/2022/3/WOOD#Drawings
:Drawings rdf:type owl:Class ;
          rdfs:subClassOf :BuildingDocumentation ,
                          [ rdf:type owl:Restriction ;
                            owl:onProperty :StatusOfSource ;
                            owl:someValuesFrom :SourcesPresentState
                          ] ;
          rdfs:comment "A drawing is a visually represented subject."@en ;
          rdfs:label "Drawings"@en .


###  http://www.semanticweb.org/georg/ontologies/2022/3/WOOD#DrillCoreTest
:DrillCoreTest rdf:type owl:Class ;
               rdfs:subClassOf :InvestigationProcedure ,
                               [ rdf:type owl:Restriction ;
                                 owl:onProperty :FindsProperties ;
                                 owl:someValuesFrom :BulkDensity
                               ] ,
                               [ rdf:type owl:Restriction ;
                                 owl:onProperty :FindsProperties ;
                                 owl:someValuesFrom :MaterialSolidity
                               ] ,
                               [ rdf:type owl:Restriction ;
                                 owl:onProperty :FindsProperties ;
                                 owl:someValuesFrom :WoodAge
                               ] ,
                               [ rdf:type owl:Restriction ;
                                 owl:onProperty :FindsProperties ;
                                 owl:someValuesFrom :WoodMoisture
                               ] ,
                               [ rdf:type owl:Restriction ;
                                 owl:onProperty :FindsProperties ;
                                 owl:someValuesFrom :WoodSpecies
                               ] ,
                               [ rdf:type owl:Restriction ;
                                 owl:onProperty :HasDegreeOfDestruction ;
                                 owl:someValuesFrom :DestructiveProcesses
                               ] ,
                               [ rdf:type owl:Restriction ;
                                 owl:onProperty :HasPlace ;
                                 owl:someValuesFrom :Laboratory
                               ] ,
                               [ rdf:type owl:Restriction ;
                                 owl:onProperty :HasTime ;
                                 owl:someValuesFrom :SlowProcesses
                               ] ;
               rdfs:comment "In the drilling core process, cylindrical samples are taken with the help of a mill, which have a diameter starting from 4mm to 50mm. The applications of the cores taken from wood are manifold. The boreholes can be closed again with suitable new wood plugs after core removal."@en ;
               rdfs:label "Drill core test"@en .


###  http://www.semanticweb.org/georg/ontologies/2022/3/WOOD#Drilling
:Drilling rdf:type owl:Class ;
          rdfs:subClassOf :Separate ;
          rdfs:comment "Drilling is the technical term for a hole created by using rotating tools"@en ;
          rdfs:label "Drilling"@en .


###  http://www.semanticweb.org/georg/ontologies/2022/3/WOOD#DrillingMachines
:DrillingMachines rdf:type owl:Class ;
                  rdfs:subClassOf :Drilling ;
                  rdfs:comment "Drilling machine is electric device for drilling holes"@en ;
                  rdfs:label "Drilling machine"@en .


###  http://www.semanticweb.org/georg/ontologies/2022/3/WOOD#DrillingResistanceMeasurement
:DrillingResistanceMeasurement rdf:type owl:Class ;
                               rdfs:subClassOf :InvestigationProcedure ,
                                               [ rdf:type owl:Restriction ;
                                                 owl:onProperty :FindsProperties ;
                                                 owl:someValuesFrom :BulkDensity
                                               ] ,
                                               [ rdf:type owl:Restriction ;
                                                 owl:onProperty :FindsProperties ;
                                                 owl:someValuesFrom :ConcealedComponents
                                               ] ,
                                               [ rdf:type owl:Restriction ;
                                                 owl:onProperty :FindsProperties ;
                                                 owl:someValuesFrom :InsectContamination
                                               ] ,
                                               [ rdf:type owl:Restriction ;
                                                 owl:onProperty :FindsProperties ;
                                                 owl:someValuesFrom :MaterialSolidity
                                               ] ,
                                               [ rdf:type owl:Restriction ;
                                                 owl:onProperty :FindsProperties ;
                                                 owl:someValuesFrom :RotContamination
                                               ] ,
                                               [ rdf:type owl:Restriction ;
                                                 owl:onProperty :HasDegreeOfDestruction ;
                                                 owl:someValuesFrom :LowDestructiveProcesses
                                               ] ,
                                               [ rdf:type owl:Restriction ;
                                                 owl:onProperty :HasPlace ;
                                                 owl:someValuesFrom :InSitu
                                               ] ,
                                               [ rdf:type owl:Restriction ;
                                                 owl:onProperty :HasTime ;
                                                 owl:someValuesFrom :SlowProcesses
                                               ] ;
                               rdfs:comment "For the drilling resistance measurement, a drilling needle with 1.5mm diameter is drilled into the wood. The density of the wood is registered and recorded."@en ;
                               rdfs:label "Drilling resistance measurement"@en .


###  http://www.semanticweb.org/georg/ontologies/2022/3/WOOD#DrillingTest
:DrillingTest rdf:type owl:Class ;
              rdfs:subClassOf :InvestigationProcedure ,
                              [ rdf:type owl:Restriction ;
                                owl:onProperty :FindsProperties ;
                                owl:someValuesFrom :BulkDensity
                              ] ,
                              [ rdf:type owl:Restriction ;
                                owl:onProperty :FindsProperties ;
                                owl:someValuesFrom :ChemicalReaction
                              ] ,
                              [ rdf:type owl:Restriction ;
                                owl:onProperty :FindsProperties ;
                                owl:someValuesFrom :ConcealedComponents
                              ] ,
                              [ rdf:type owl:Restriction ;
                                owl:onProperty :FindsProperties ;
                                owl:someValuesFrom :InsectContamination
                              ] ,
                              [ rdf:type owl:Restriction ;
                                owl:onProperty :FindsProperties ;
                                owl:someValuesFrom :RotContamination
                              ] ,
                              [ rdf:type owl:Restriction ;
                                owl:onProperty :FindsProperties ;
                                owl:someValuesFrom :WoodAge
                              ] ,
                              [ rdf:type owl:Restriction ;
                                owl:onProperty :FindsProperties ;
                                owl:someValuesFrom :WoodMoisture
                              ] ,
                              [ rdf:type owl:Restriction ;
                                owl:onProperty :FindsProperties ;
                                owl:someValuesFrom :WoodSpecies
                              ] ,
                              [ rdf:type owl:Restriction ;
                                owl:onProperty :HasDegreeOfDestruction ;
                                owl:someValuesFrom :LowDestructiveProcesses
                              ] ,
                              [ rdf:type owl:Restriction ;
                                owl:onProperty :HasPlace ;
                                owl:someValuesFrom :InSitu
                              ] ,
                              [ rdf:type owl:Restriction ;
                                owl:onProperty :HasTime ;
                                owl:someValuesFrom :SlowProcesses
                              ] ;
              rdfs:comment "If suspicious spots are discovered, they can be drilled into in order to draw to draw conclusions from the drill dust."@en ;
              rdfs:label "Drilling test"@en .


###  http://www.semanticweb.org/georg/ontologies/2022/3/WOOD#DryRot
:DryRot rdf:type owl:Class ;
        rdfs:subClassOf :WoodDestroyingFungi ,
                        [ rdf:type owl:Restriction ;
                          owl:onProperty :RotDecompositionType ;
                          owl:someValuesFrom :BrownRot
                        ] ;
        rdfs:comment """Preferred wood species:
Mainly softwood, also hardwood

Optimal living conditions of wood moisture content in M-%:
20% to 40%

Optimal living conditions of the temperature range in °C:
18°C to 22°C

Further notes:
Dry rot requires only a certain degree of wood moisture at the beginning of its growth. It is the only structural wood fungus capable of attacking dry wood, which it moisturizes itself by transporting water via strand mycelium."""@en ;
        rdfs:label "Dry rot"@en ,
                   "Serpula lacrimans"@la .


###  http://www.semanticweb.org/georg/ontologies/2022/3/WOOD#DuoTrioBeams
:DuoTrioBeams rdf:type owl:Class ;
              rdfs:subClassOf :SolidWood ;
              rdfs:comment "Duo beams and trio beams consist of two or three flat-sided and fibre-parallel planks which are glued to each other."@en ;
              rdfs:label "Duo/ Trio-beams"@en .


###  http://www.semanticweb.org/georg/ontologies/2022/3/WOOD#DynamicOverstress
:DynamicOverstress rdf:type owl:Class ;
                   rdfs:subClassOf :mechanicalInfluences ;
                   rdfs:comment "A dynamic stress applies forces and moments to a structure that change in direction, position, and magnitude."@en ;
                   rdfs:label "Dynamic overstress"@en .


###  http://www.semanticweb.org/georg/ontologies/2022/3/WOOD#EModulus
:EModulus rdf:type owl:Class ;
          owl:equivalentClass [ rdf:type owl:Restriction ;
                                owl:onProperty :FindsProperties ;
                                owl:someValuesFrom :EModulus
                              ] ;
          rdfs:subClassOf :SearchedProperties ;
          rdfs:comment "The modulus of elasticity, also called E-modulus, is a parameter that describes the relationship between stress and extension during the deformation of a solid body."@en ;
          rdfs:label "E-modulus"@en .


###  http://www.semanticweb.org/georg/ontologies/2022/3/WOOD#ElectricalResistance
:ElectricalResistance rdf:type owl:Class ;
                      rdfs:subClassOf :InvestigationProcedure ,
                                      [ rdf:type owl:Restriction ;
                                        owl:onProperty :FindsProperties ;
                                        owl:someValuesFrom :WoodMoisture
                                      ] ,
                                      [ rdf:type owl:Restriction ;
                                        owl:onProperty :HasDegreeOfDestruction ;
                                        owl:someValuesFrom :NonDestructiveProcesses
                                      ] ,
                                      [ rdf:type owl:Restriction ;
                                        owl:onProperty :HasPlace ;
                                        owl:someValuesFrom :InSitu
                                      ] ,
                                      [ rdf:type owl:Restriction ;
                                        owl:onProperty :HasTime ;
                                        owl:someValuesFrom :SlowProcesses
                                      ] ;
                      rdfs:comment "Two electrodes are driven into the wood and the electric current is measured, which flows through the wood depending on the moisture content of the wood. With these methods, however, only the moisture of the direct surface is measured; no statement can be made about the internal moisture concentration."@en ;
                      rdfs:label "Electrical resistance"@en .


###  http://www.semanticweb.org/georg/ontologies/2022/3/WOOD#Endoscopy
:Endoscopy rdf:type owl:Class ;
           rdfs:subClassOf :InvestigationProcedure ,
                           [ rdf:type owl:Restriction ;
                             owl:onProperty :FindsProperties ;
                             owl:someValuesFrom :ConcealedComponents
                           ] ,
                           [ rdf:type owl:Restriction ;
                             owl:onProperty :FindsProperties ;
                             owl:someValuesFrom :InsectContamination
                           ] ,
                           [ rdf:type owl:Restriction ;
                             owl:onProperty :HasDegreeOfDestruction ;
                             owl:someValuesFrom :LowDestructiveProcesses
                           ] ,
                           [ rdf:type owl:Restriction ;
                             owl:onProperty :HasPlace ;
                             owl:someValuesFrom :InSitu
                           ] ,
                           [ rdf:type owl:Restriction ;
                             owl:onProperty :HasTime ;
                             owl:someValuesFrom :SlowProcesses
                           ] ;
           rdfs:comment "For concealed components, the endoscope is used. Holes with a maximum diameter of 5 to 20mm are drilled and the endoscope is inserted. This enables an optical inspection even of components that are not visible."@en ;
           rdfs:label "Endoscopy"@en .


###  http://www.semanticweb.org/georg/ontologies/2022/3/WOOD#Evaluation
:Evaluation rdf:type owl:Class ;
            rdfs:subClassOf :StepsToTheEvidenceConclusion ;
            rdfs:comment "The evaluations of the results are to be presented in a comprehensible conclusion from the findings and causes."@en ;
            rdfs:label "Evaluation"@en .


###  http://www.semanticweb.org/georg/ontologies/2022/3/WOOD#ExcessiveLoadsFromConstructionOrUsage
:ExcessiveLoadsFromConstructionOrUsage rdf:type owl:Class ;
                                       rdfs:subClassOf :StaticOverstress ;
                                       rdfs:comment "Failure of the structure due to excessive loads can occur in certain cases: Through unplanned useage of the construction or through a new load redistribution due to the failure of individual components."@en ;
                                       rdfs:label "Excessive loads from construction or usage"@en .


###  http://www.semanticweb.org/georg/ontologies/2022/3/WOOD#ExplosionAndSonicBoom
:ExplosionAndSonicBoom rdf:type owl:Class ;
                       rdfs:subClassOf :DynamicOverstress ,
                                       [ rdf:type owl:Restriction ;
                                         owl:onProperty :CanCreateDamage ;
                                         owl:someValuesFrom :BurnMarks
                                       ] ,
                                       [ rdf:type owl:Restriction ;
                                         owl:onProperty :CanCreateDamage ;
                                         owl:someValuesFrom :Cracks
                                       ] ,
                                       [ rdf:type owl:Restriction ;
                                         owl:onProperty :CanCreateDamage ;
                                         owl:someValuesFrom :Delocalization
                                       ] ,
                                       [ rdf:type owl:Restriction ;
                                         owl:onProperty :CanCreateDamage ;
                                         owl:someValuesFrom :Fractures
                                       ] ,
                                       [ rdf:type owl:Restriction ;
                                         owl:onProperty :CanCreateDamage ;
                                         owl:someValuesFrom :Holes
                                       ] ,
                                       [ rdf:type owl:Restriction ;
                                         owl:onProperty :CanCreateDamage ;
                                         owl:someValuesFrom :MissingPart
                                       ] ;
                       rdfs:comment "Explosions on components, which can overstress, burn and destroy these components. Furthermore, the vibration can cause cracks, deformations and fastener failures."@en ;
                       rdfs:label "Explosion/ Sonic boom"@en .


###  http://www.semanticweb.org/georg/ontologies/2022/3/WOOD#ExternalResources
:ExternalResources rdf:type owl:Class ;
                   rdfs:subClassOf :Sources ;
                   rdfs:comment "Sources that contain general knowledge about construction projects."@en ;
                   rdfs:label "External resources"@en .


###  http://www.semanticweb.org/georg/ontologies/2022/3/WOOD#FastProcesses
:FastProcesses rdf:type owl:Class ;
               owl:equivalentClass [ rdf:type owl:Restriction ;
                                     owl:onProperty :HasTime ;
                                     owl:someValuesFrom :FastProcesses
                                   ] ;
               rdfs:subClassOf :TestDuration ;
               rdfs:comment "Processes that need no further preparation and use tools that are common during a first inspection."@en ;
               rdfs:label "Fast processes"@en .


###  http://www.semanticweb.org/georg/ontologies/2022/3/WOOD#FenceLeaflet
:FenceLeaflet rdf:type owl:Class ;
              rdfs:subClassOf :Leaflet ,
                              [ rdf:type owl:Restriction ;
                                owl:onProperty :RotDecompositionType ;
                                owl:someValuesFrom :BrownRot
                              ] ;
              rdfs:comment """Preferred wood species:
Hardwood

Optimal living conditions of wood moisture content in M-%:
40% to 60%

Optimal living conditions of the temperature range in °C:
26°C to 36°C

Additional notes:
Mycelium survives higher temperature and dry rigidity."""@en ;
              rdfs:label "Fence leaflet"@en ,
                         "Gloeophyllum sepiarium"@la .


###  http://www.semanticweb.org/georg/ontologies/2022/3/WOOD#Files
:Files rdf:type owl:Class ;
       rdfs:subClassOf :Separate ;
       rdfs:comment "Filing is an process of removing material with repeated rectilinear or circular cutting motion. The tool has teeth with low height, which are tightly packed together"@en ;
       rdfs:label "Files"@en .


###  http://www.semanticweb.org/georg/ontologies/2022/3/WOOD#FinishedProcedure
:FinishedProcedure rdf:type owl:Class ;
                   rdfs:subClassOf :ProcedureStatus ;
                   owl:disjointWith :InWorkingProcedure ;
                   rdfs:comment "Investigation procedure is finished and all necessary information has been inserted."@en ;
                   rdfs:label "Finished procedure"@en .


###  http://www.semanticweb.org/georg/ontologies/2022/3/WOOD#FirLeafBlossom
:FirLeafBlossom rdf:type owl:Class ;
                rdfs:subClassOf :Leaflet ,
                                [ rdf:type owl:Restriction ;
                                  owl:onProperty :RotDecompositionType ;
                                  owl:someValuesFrom :BrownRot
                                ] ;
                rdfs:comment """Preferred wood species:
Hardwood

Optimal living conditions of wood moisture content in M-%:
35% to 40%

Optimal living conditions of the temperature range in °C:
26°C to 35°C

Additional notes:
Mycelium survives higher temperature and dry rigidity."""@en ;
                rdfs:label "FIr leaf blossom"@en ,
                           "Gloeophyllum abietinum"@la .


###  http://www.semanticweb.org/georg/ontologies/2022/3/WOOD#FirTA
:FirTA rdf:type owl:Class ;
       rdfs:subClassOf :Softwood ,
                       [ rdf:type owl:Restriction ;
                         owl:onProperty :DimensionalStability ;
                         owl:someValuesFrom :HighDimensionalStability
                       ] ,
                       [ rdf:type owl:Restriction ;
                         owl:onProperty :InsectResistance ;
                         owl:someValuesFrom :LowInsectResistance
                       ] ,
                       [ rdf:type owl:Restriction ;
                         owl:onProperty :RotResistance ;
                         owl:someValuesFrom :LowRotResistance
                       ] ;
       rdfs:comment """Wood material of fir trees.

Colour:
Early wood almost white, late wood pale reddish, sapwood and heartwood is not distinguished.

Special properties resistance to fungi:
Sensitive to blue stain."""@en ;
       rdfs:label "Fir (TA)"@en .


###  http://www.semanticweb.org/georg/ontologies/2022/3/WOOD#FireproofingPaint
:FireproofingPaint rdf:type owl:Class ;
                   rdfs:subClassOf :PropertiesChange ;
                   rdfs:comment "When exposed to fire, the fire protection coating foams up and protects against oxygen ingress"@en ;
                   rdfs:label "Fireproofing paint"@en .


###  http://www.semanticweb.org/georg/ontologies/2022/3/WOOD#FlatPressedBoard
:FlatPressedBoard rdf:type owl:Class ;
                  rdfs:subClassOf :WoodBasedMaterials ;
                  rdfs:comment "The production of OSB is made by gluing together larger chips . The chips are approx. 0.6 mm thick, 75 mm to 130 mm long and approx. 35 mm wide.They lie in the surface layer predominantly in the direction of the longitudinal side of the board and in the middle layer transverse to it. OSB has depending on the direction of the chips different strength properties."@en ;
                  rdfs:label "Oriented Strand Board (OSB)"@en .


###  http://www.semanticweb.org/georg/ontologies/2022/3/WOOD#FoldingRule
:FoldingRule rdf:type owl:Class ;
             rdfs:subClassOf :GeometricMeasurements ,
                             [ rdf:type owl:Restriction ;
                               owl:onProperty :HasDegreeOfDestruction ;
                               owl:someValuesFrom :NonDestructiveProcesses
                             ] ,
                             [ rdf:type owl:Restriction ;
                               owl:onProperty :HasTime ;
                               owl:someValuesFrom :FastProcesses
                             ] ;
             rdfs:comment "A folding rule is a haptic measuring instrument used to measure short distances."@en ;
             rdfs:label "Folding rule"@en .


###  http://www.semanticweb.org/georg/ontologies/2022/3/WOOD#ForceFit
:ForceFit rdf:type owl:Class ;
          owl:equivalentClass [ rdf:type owl:Restriction ;
                                owl:onProperty :FittingType ;
                                owl:someValuesFrom :ForceFit
                              ] ;
          rdfs:subClassOf :ConnectionType ;
          rdfs:comment "In this connection, movement is prevented by static friction. The components are pressed against each other, the resulting static friction opposes that of the direction of movement."@en ;
          rdfs:label "Force fit"@en .


###  http://www.semanticweb.org/georg/ontologies/2022/3/WOOD#FormFitting
:FormFitting rdf:type owl:Class ;
             owl:equivalentClass [ rdf:type owl:Restriction ;
                                   owl:onProperty :FittingType ;
                                   owl:someValuesFrom :FormFitting
                                 ] ;
             rdfs:subClassOf :ConnectionType ;
             rdfs:comment "The form-fit connection works because one of the components involved is in the way, which prevents it from coming loose. The connection is achieved either by the interlocking of at least two workpieces or by the insertion of a further part, a connecting element."@en ;
             rdfs:label "Form fitting"@en .


###  http://www.semanticweb.org/georg/ontologies/2022/3/WOOD#Fractures
:Fractures rdf:type owl:Class ;
           owl:equivalentClass [ rdf:type owl:Restriction ;
                                 owl:onProperty :CanCreateDamage ;
                                 owl:someValuesFrom :Fractures
                               ] ;
           rdfs:subClassOf :MechanicalProcesses ;
           rdfs:comment "The cracking or breaking of a hard object."@en ;
           rdfs:label "Fractures"@en .


###  http://www.semanticweb.org/georg/ontologies/2022/3/WOOD#FrameSaws
:FrameSaws rdf:type owl:Class ;
           rdfs:subClassOf :Sawing ;
           rdfs:comment "Frame saws are used in a sawmill and are driven by a flywheel"@en ;
           rdfs:label "Frame saw"@en .


###  http://www.semanticweb.org/georg/ontologies/2022/3/WOOD#Fumigant
:Fumigant rdf:type owl:Class ;
          rdfs:subClassOf :PropertiesChange ;
          rdfs:comment "Fumigation is a method of pest control or elimination of harmful microorganisms by completely filling a space with gaseous pesticides"@en ;
          rdfs:label "Fumigant"@en .


###  http://www.semanticweb.org/georg/ontologies/2022/3/WOOD#GK1
:GK1 rdf:type owl:Class ;
     rdfs:subClassOf :Classification ;
     rdfs:comment "The wood or wood product is indoors and not exposed to weathering and not exposed to humidification."@en ;
     rdfs:label "GK 1"@en .


###  http://www.semanticweb.org/georg/ontologies/2022/3/WOOD#GK2
:GK2 rdf:type owl:Class ;
     rdfs:subClassOf :Classification ;
     rdfs:comment "The wood or wood product is under the roof and not exposed to the weather, but there may be occasional but not continuous humidification. Condensation of water on the surface of the wood and the wood products may occur."@en ;
     rdfs:label "GK 2"@en .


###  http://www.semanticweb.org/georg/ontologies/2022/3/WOOD#GK4
:GK4 rdf:type owl:Class ;
     rdfs:subClassOf :Classification ;
     rdfs:comment "The wood or wood product has direct earth contact or direct contact with fresh water."@en ;
     rdfs:label "GK 4"@en .


###  http://www.semanticweb.org/georg/ontologies/2022/3/WOOD#GK5
:GK5 rdf:type owl:Class ;
     rdfs:subClassOf :Classification ;
     rdfs:comment "The wood or wood product is permanently or regularly immersed in salt water."@en ;
     rdfs:label "Gk 5"@en .


###  http://www.semanticweb.org/georg/ontologies/2022/3/WOOD#GeometricChange
:GeometricChange rdf:type owl:Class ;
                 owl:equivalentClass [ rdf:type owl:Restriction ;
                                       owl:onProperty :FindsProperties ;
                                       owl:someValuesFrom :GeometricChange
                                     ] ;
                 rdfs:subClassOf :SearchedProperties ;
                 rdfs:comment "Geometric deformation of a body is the change of its shape due to the action of an external force."@en ;
                 rdfs:label "Geometric change"@en .


###  http://www.semanticweb.org/georg/ontologies/2022/3/WOOD#GeometricMeasurements
:GeometricMeasurements rdf:type owl:Class ;
                       rdfs:subClassOf :InvestigationProcedure ,
                                       [ rdf:type owl:Restriction ;
                                         owl:onProperty :FindsProperties ;
                                         owl:someValuesFrom :GeometricChange
                                       ] ,
                                       [ rdf:type owl:Restriction ;
                                         owl:onProperty :HasPlace ;
                                         owl:someValuesFrom :InSitu
                                       ] ;
                       rdfs:comment "Geometric examination for deformation or other deviation."@en ;
                       rdfs:label "Geometric measurements"@en .


###  http://www.semanticweb.org/georg/ontologies/2022/3/WOOD#Gk3.1
:Gk3.1 rdf:type owl:Class ;
       rdfs:subClassOf :Classification ;
       rdfs:comment "The wood or wood product is above ground and exposed to the weather. The water will not settle."@en ;
       rdfs:label "GK 3.1"@en .


###  http://www.semanticweb.org/georg/ontologies/2022/3/WOOD#Gk3.2
:Gk3.2 rdf:type owl:Class ;
       rdfs:subClassOf :Classification ;
       rdfs:comment "The wood or wood product is above ground and exposed to the weather. The water may settle."@en ;
       rdfs:label "GK 3.2"@en .


###  http://www.semanticweb.org/georg/ontologies/2022/3/WOOD#Glaze
:Glaze rdf:type owl:Class ;
       rdfs:subClassOf :CoatTools ,
                       [ rdf:type owl:Restriction ;
                         owl:onProperty :WoodColour ;
                         owl:someValuesFrom :ColourConcealed
                       ] ,
                       [ rdf:type owl:Restriction ;
                         owl:onProperty :WoodGrain ;
                         owl:someValuesFrom :GrainConcealed
                       ] ;
       rdfs:comment "Glazing is a liquid or powder coating material that is applied thinly to objects and built up by chemical or physical processes to form a continuous, solid layer. The wood grain is concealed"@en ;
       rdfs:label "Glaze"@en .


###  http://www.semanticweb.org/georg/ontologies/2022/3/WOOD#Glue
:Glue rdf:type owl:Class ;
      rdfs:subClassOf :JoinTools ,
                      [ rdf:type owl:Restriction ;
                        owl:onProperty :FittingType ;
                        owl:someValuesFrom :MeltLocking
                      ] ,
                      [ rdf:type owl:Restriction ;
                        owl:onProperty :Removability ;
                        owl:someValuesFrom :Unsolvable
                      ] ;
      rdfs:comment "Wood glue is an adhesive used to tightly bond pieces of wood together. Different substances can be used as glue"@en ;
      rdfs:label "Glue"@en .


###  http://www.semanticweb.org/georg/ontologies/2022/3/WOOD#GluedLaminatedTimber
:GluedLaminatedTimber rdf:type owl:Class ;
                      rdfs:subClassOf :SolidWood ;
                      rdfs:comment "Glued laminated timber (Glulam) is a hardened and tempered solid wood, in which the strength-reducing influence of the growth-related defects is cancelled out, up to a to a certain extent. It consists of at least three boards glued together."@en ;
                      rdfs:label "Glued laminated timber"@en .


###  http://www.semanticweb.org/georg/ontologies/2022/3/WOOD#GrainConcealed
:GrainConcealed rdf:type owl:Class ;
                owl:equivalentClass [ rdf:type owl:Restriction ;
                                      owl:onProperty :WoodGrain ;
                                      owl:someValuesFrom :GrainConcealed
                                    ] ;
                rdfs:subClassOf :ComponentGrain ;
                owl:disjointWith :GrainEmphasized ;
                rdfs:comment "The grain of the component  is covered and no longer visible to the viewer."@en ;
                rdfs:label "Grain concealed"@en .


###  http://www.semanticweb.org/georg/ontologies/2022/3/WOOD#GrainEmphasized
:GrainEmphasized rdf:type owl:Class ;
                 owl:equivalentClass [ rdf:type owl:Restriction ;
                                       owl:onProperty :WoodGrain ;
                                       owl:someValuesFrom :GrainEmphasized
                                     ] ;
                 rdfs:subClassOf :ComponentGrain ;
                 rdfs:comment "The grain of the component is still visible, but has changed accordingly to the used coating procedure."@en ;
                 rdfs:label "Grain emphasized"@en .


###  http://www.semanticweb.org/georg/ontologies/2022/3/WOOD#GrainRemainsVisible
:GrainRemainsVisible rdf:type owl:Class ;
                     owl:equivalentClass [ rdf:type owl:Restriction ;
                                           owl:onProperty :WoodGrain ;
                                           owl:someValuesFrom :GrainRemainsVisible
                                         ] ;
                     rdfs:subClassOf :ComponentGrain ;
                     rdfs:comment "The colour of the component is still visible and unchainged."@en ;
                     rdfs:label "Grain remains visible"@en .


###  http://www.semanticweb.org/georg/ontologies/2022/3/WOOD#GravimetricMethod
:GravimetricMethod rdf:type owl:Class ;
                   rdfs:subClassOf :InvestigationProcedure ,
                                   [ rdf:type owl:Restriction ;
                                     owl:onProperty :FindsProperties ;
                                     owl:someValuesFrom :WoodMoisture
                                   ] ,
                                   [ rdf:type owl:Restriction ;
                                     owl:onProperty :HasDegreeOfDestruction ;
                                     owl:someValuesFrom :LowDestructiveProcesses
                                   ] ,
                                   [ rdf:type owl:Restriction ;
                                     owl:onProperty :HasPlace ;
                                     owl:someValuesFrom :Laboratory
                                   ] ,
                                   [ rdf:type owl:Restriction ;
                                     owl:onProperty :HasTime ;
                                     owl:someValuesFrom :SlowProcesses
                                   ] ;
                   rdfs:comment "A building material sample is weighed in the laboratory, dried in a oven and then weighed again.  The difference gives the moisture content. The moisture determination is very accurate."@en ;
                   rdfs:label "Gravimetric method"@en .


###  http://www.semanticweb.org/georg/ontologies/2022/3/WOOD#Grinding
:Grinding rdf:type owl:Class ;
          rdfs:subClassOf :Separate ;
          rdfs:comment "Grinding is a chip removing manufacturing process. The edges of the microscopically small mineral crystals in the grinding tool act as cutting edges"@en ;
          rdfs:label "Grinding"@en .


###  http://www.semanticweb.org/georg/ontologies/2022/3/WOOD#GrindingMachines
:GrindingMachines rdf:type owl:Class ;
                  rdfs:subClassOf :Grinding ;
                  rdfs:comment "Grinders are tools for smoothing surfaces or removing coatings from surfaces"@en ;
                  rdfs:label "Grinding machine"@en .


###  http://www.semanticweb.org/georg/ontologies/2022/3/WOOD#GypsumFiberboards
:GypsumFiberboards rdf:type owl:Class ;
                   rdfs:subClassOf :WoodBasedMaterials ;
                   rdfs:comment "Gypsum fiberboards are made from gypsum and paper fibers. The paper fibers serve as reinforcement. A homogeneous mixture of both raw materials and water is pressed into slabs under high pressure, dried and cut to the respective formats."@en ;
                   rdfs:label "Gypsum fiberboards"@en .


###  http://www.semanticweb.org/georg/ontologies/2022/3/WOOD#Handsaw
:Handsaw rdf:type owl:Class ;
         rdfs:subClassOf :Sawing ;
         rdfs:comment "The saw is a tool for cutting wood by chip removal"@en ;
         rdfs:label "Handsaw"@en .


###  http://www.semanticweb.org/georg/ontologies/2022/3/WOOD#Hardwood
:Hardwood rdf:type owl:Class ;
          rdfs:subClassOf :WoodTypes ;
          owl:disjointWith :Softwood ;
          rdfs:comment "Hardwood refers to the wood of trees that have proper leaves."@en ;
          rdfs:label "Hardwood"@en .


###  http://www.semanticweb.org/georg/ontologies/2022/3/WOOD#Heartwood
:Heartwood rdf:type owl:Class ;
           rdfs:subClassOf :Structure ;
           owl:disjointWith :Sapwood ;
           rdfs:comment "Heartwood is refering to the physiologically no longer active, often dark, inner zone in the cross-section of the trunk. It is formed by secondary metabolic processes of the dying parenchyma in the inner sapwood." ;
           rdfs:label "Heartwood"@en .


###  http://www.semanticweb.org/georg/ontologies/2022/3/WOOD#HighDimensionalStability
:HighDimensionalStability rdf:type owl:Class ;
                          owl:equivalentClass [ rdf:type owl:Restriction ;
                                                owl:onProperty :DimensionalStability ;
                                                owl:someValuesFrom :HighDimensionalStability
                                              ] ;
                          rdfs:subClassOf :DimensionalStability ;
                          rdfs:comment "The dimensional stability of these wood types are on the upper spectrum. These wood types have a high dimemsional stabilit and will mostly mainain its original dimension when put under pressure."@en ;
                          rdfs:label "High dimensional stability"@en .


###  http://www.semanticweb.org/georg/ontologies/2022/3/WOOD#HighInsectResistance
:HighInsectResistance rdf:type owl:Class ;
                      owl:equivalentClass [ rdf:type owl:Restriction ;
                                            owl:onProperty :InsectResistance ;
                                            owl:someValuesFrom :HighInsectResistance
                                          ] ;
                      rdfs:subClassOf :InsectResistance ;
                      rdfs:comment "The insect resistance of these wood types are on the upper spectrum. These wood types have a high insect resistance and insects will mostly not be able to harm these materials."@en ;
                      rdfs:label "High insect resistance"@en .


###  http://www.semanticweb.org/georg/ontologies/2022/3/WOOD#HighRotResistance
:HighRotResistance rdf:type owl:Class ;
                   owl:equivalentClass [ rdf:type owl:Restriction ;
                                         owl:onProperty :RotResistance ;
                                         owl:someValuesFrom :HighRotResistance
                                       ] ;
                   rdfs:subClassOf :RotResistance ;
                   rdfs:comment "The rot resistance of these wood types are on the upper spectrum. These wood types have a high rot resistance and rot will mostly not be able to harm these materials."@en ;
                   rdfs:label "High rot resistance"@en .


###  http://www.semanticweb.org/georg/ontologies/2022/3/WOOD#Holes
:Holes rdf:type owl:Class ;
       owl:equivalentClass [ rdf:type owl:Restriction ;
                             owl:onProperty :CanCreateDamage ;
                             owl:someValuesFrom :Holes
                           ] ;
       rdfs:subClassOf :MechanicalProcesses ;
       rdfs:comment "Due to damage a place where the substance is no longer present."@en ;
       rdfs:label "Holes"@en .


###  http://www.semanticweb.org/georg/ontologies/2022/3/WOOD#HumanRemoval
:HumanRemoval rdf:type owl:Class ;
              rdfs:subClassOf :ServiceStresses ,
                              [ rdf:type owl:Restriction ;
                                owl:onProperty :CanCreateDamage ;
                                owl:someValuesFrom :Delocalization
                              ] ,
                              [ rdf:type owl:Restriction ;
                                owl:onProperty :CanCreateDamage ;
                                owl:someValuesFrom :MissingPart
                              ] ;
              rdfs:comment "Unprofessional intervention in the structural system can lead to a change in the load transfer and thus to components being overstressed."@en ;
              rdfs:label "Human removal"@en .


###  http://www.semanticweb.org/georg/ontologies/2022/3/WOOD#Impact
:Impact rdf:type owl:Class ;
        rdfs:subClassOf :ServiceStresses ,
                        [ rdf:type owl:Restriction ;
                          owl:onProperty :CanCreateDamage ;
                          owl:someValuesFrom :Cracks
                        ] ,
                        [ rdf:type owl:Restriction ;
                          owl:onProperty :CanCreateDamage ;
                          owl:someValuesFrom :Delocalization
                        ] ,
                        [ rdf:type owl:Restriction ;
                          owl:onProperty :CanCreateDamage ;
                          owl:someValuesFrom :Fractures
                        ] ,
                        [ rdf:type owl:Restriction ;
                          owl:onProperty :CanCreateDamage ;
                          owl:someValuesFrom :Holes
                        ] ;
        rdfs:comment "Impact on components, which can overstress and destroy these components. Furthermore, the vibration can cause cracks, deformations and fastener failures."@en ;
        rdfs:label "Impact"@en .


###  http://www.semanticweb.org/georg/ontologies/2022/3/WOOD#InSitu
:InSitu rdf:type owl:Class ;
        owl:equivalentClass [ rdf:type owl:Restriction ;
                              owl:onProperty :HasPlace ;
                              owl:someValuesFrom :InSitu
                            ] ;
        rdfs:subClassOf :ProcedureLocation ;
        rdfs:comment "Research method conducted and evaluated at the construction site."@en ;
        rdfs:label "In situ"@en .


###  http://www.semanticweb.org/georg/ontologies/2022/3/WOOD#InWorkingProcedure
:InWorkingProcedure rdf:type owl:Class ;
                    rdfs:subClassOf :ProcedureStatus ;
                    rdfs:comment "Investigation procedure is still in progress and there is still information that is not given in the report that is necesssary."@en ;
                    rdfs:label "In working procedure"@en .


###  http://www.semanticweb.org/georg/ontologies/2022/3/WOOD#InactiveCause
:InactiveCause rdf:type owl:Class ;
               rdfs:subClassOf :DamageStatus ;
               rdfs:label "Inactive cause"@en .


###  http://www.semanticweb.org/georg/ontologies/2022/3/WOOD#IndicatorPaper
:IndicatorPaper rdf:type owl:Class ;
                rdfs:subClassOf :InvestigationProcedure ,
                                [ rdf:type owl:Restriction ;
                                  owl:onProperty :FindsProperties ;
                                  owl:someValuesFrom :ChemicalReaction
                                ] ,
                                [ rdf:type owl:Restriction ;
                                  owl:onProperty :FindsProperties ;
                                  owl:someValuesFrom :PHValue
                                ] ,
                                [ rdf:type owl:Restriction ;
                                  owl:onProperty :FindsProperties ;
                                  owl:someValuesFrom :RotContamination
                                ] ,
                                [ rdf:type owl:Restriction ;
                                  owl:onProperty :HasDegreeOfDestruction ;
                                  owl:someValuesFrom :NonDestructiveProcesses
                                ] ,
                                [ rdf:type owl:Restriction ;
                                  owl:onProperty :HasPlace ;
                                  owl:someValuesFrom :InSitu
                                ] ,
                                [ rdf:type owl:Restriction ;
                                  owl:onProperty :HasTime ;
                                  owl:someValuesFrom :SlowProcesses
                                ] ;
                rdfs:comment "Detection of brown rot fungi by measuring the concentration of oxalic acid. During the decomposition of wood substance by brown rot, oxalic acid is produced, reducing the pH of the wood from pH = 5 to pH = 3. In the field, a simple color reaction test provides evidence of active fungal attack. The blue color of the indicator turns to green, yellow, when infestation is present. For chemical analysis in the laboratory, only small amounts of a sample of approx. 2 to 5 g are required."@en ;
                rdfs:label "Indicator paper"@en .


###  http://www.semanticweb.org/georg/ontologies/2022/3/WOOD#InsectContamination
:InsectContamination rdf:type owl:Class ;
                     owl:equivalentClass [ rdf:type owl:Restriction ;
                                           owl:onProperty :FindsProperties ;
                                           owl:someValuesFrom :InsectContamination
                                         ] ;
                     rdfs:subClassOf :SearchedProperties ;
                     rdfs:comment "Insect contermination is the condition of infestation of the component caused by insects."@en ;
                     rdfs:label "Insect contamination"@en .


###  http://www.semanticweb.org/georg/ontologies/2022/3/WOOD#InsectInfestation
:InsectInfestation rdf:type owl:Class ;
                   owl:equivalentClass [ rdf:type owl:Restriction ;
                                         owl:onProperty :CanCreateDamage ;
                                         owl:someValuesFrom :InsectInfestation
                                       ] ;
                   rdfs:subClassOf :BiologicalProcesses ;
                   rdfs:comment "An infestation of the wood substance by insects."@en ;
                   rdfs:label "Insect infestation"@en .


###  http://www.semanticweb.org/georg/ontologies/2022/3/WOOD#InsectResistance
:InsectResistance rdf:type owl:Class ;
                  rdfs:subClassOf :WoodTypes .


###  http://www.semanticweb.org/georg/ontologies/2022/3/WOOD#InsufficientBeamDimensions
:InsufficientBeamDimensions rdf:type owl:Class ;
                            rdfs:subClassOf :StaticOverstress ;
                            rdfs:comment "Insufficent beam dimensions and therefore a structural failure can occure when for example the loads where determined inaccurate."@en ;
                            rdfs:label "Insufficent beam dimensions"@en .


###  http://www.semanticweb.org/georg/ontologies/2022/3/WOOD#Investigation
:Investigation rdf:type owl:Class ;
               rdfs:comment "List of investigation procedures. Can be used to find the cause of wood damages."@en ;
               rdfs:label "Investigation"@en .


###  http://www.semanticweb.org/georg/ontologies/2022/3/WOOD#InvestigationProcedure
:InvestigationProcedure rdf:type owl:Class ;
                        rdfs:subClassOf :Investigation ;
                        rdfs:comment "List of investigation processes."@en ;
                        rdfs:label "Investigation procedure"@en .


###  http://www.semanticweb.org/georg/ontologies/2022/3/WOOD#Join
:Join rdf:type owl:Class ;
      rdfs:subClassOf :Repair ;
      rdfs:comment "Permanently joining or otherwise bringing together two or more workpieces. Thereby the cohesion is created locally and increased as a whole"@en ;
      rdfs:label "Join"@en .


###  http://www.semanticweb.org/georg/ontologies/2022/3/WOOD#JoinTools
:JoinTools rdf:type owl:Class ;
           rdfs:subClassOf :Join ;
           rdfs:comment "List of tools often used in joining work."@en ;
           rdfs:label "Join tools"@en .


###  http://www.semanticweb.org/georg/ontologies/2022/3/WOOD#Laboratory
:Laboratory rdf:type owl:Class ;
            owl:equivalentClass [ rdf:type owl:Restriction ;
                                  owl:onProperty :HasPlace ;
                                  owl:someValuesFrom :Laboratory
                                ] ;
            rdfs:subClassOf :ProcedureLocation ;
            rdfs:comment "Research method conducted and evaluated in part at the laboratory."@en ;
            rdfs:label "Laboratory"@en .


###  http://www.semanticweb.org/georg/ontologies/2022/3/WOOD#Laminate
:Laminate rdf:type owl:Class ;
          rdfs:subClassOf :CoatTools ,
                          [ rdf:type owl:Restriction ;
                            owl:onProperty :WoodColour ;
                            owl:someValuesFrom :ColourConcealed
                          ] ,
                          [ rdf:type owl:Restriction ;
                            owl:onProperty :WoodGrain ;
                            owl:someValuesFrom :GrainConcealed
                          ] ;
          rdfs:comment "Wood is coated with additional solid material"@en ;
          rdfs:label "Laminate"@en .


###  http://www.semanticweb.org/georg/ontologies/2022/3/WOOD#LaminatedVeneerLumber
:LaminatedVeneerLumber rdf:type owl:Class ;
                       rdfs:subClassOf :WoodBasedMaterials ;
                       rdfs:comment "Laminated veneer lumber is created by gluing together approximately 3 mm thick, dried veneers from from softwood. There are different veneer arrangements which are distinguished."@en ;
                       rdfs:label "Laminated veneer lumber"@en .


###  http://www.semanticweb.org/georg/ontologies/2022/3/WOOD#LarchEuropeanLA
:LarchEuropeanLA rdf:type owl:Class ;
                 rdfs:subClassOf :Softwood ,
                                 [ rdf:type owl:Restriction ;
                                   owl:onProperty :DimensionalStability ;
                                   owl:someValuesFrom :HighDimensionalStability
                                 ] ,
                                 [ rdf:type owl:Restriction ;
                                   owl:onProperty :InsectResistance ;
                                   owl:someValuesFrom :HighInsectResistance
                                 ] ,
                                 [ rdf:type owl:Restriction ;
                                   owl:onProperty :InsectResistance ;
                                   owl:someValuesFrom :MediumInsectResistance
                                 ] ,
                                 [ rdf:type owl:Restriction ;
                                   owl:onProperty :RotResistance ;
                                   owl:someValuesFrom :LowRotResistance
                                 ] ,
                                 [ rdf:type owl:Restriction ;
                                   owl:onProperty :RotResistance ;
                                   owl:someValuesFrom :MediumRotResistance
                                 ] ;
                 rdfs:comment """Wood material of Douglas larch european trees.

Colour:
Yellowish/ reddish brown, darkens with time, late wood deep brown."""@en ;
                 rdfs:label "Larch european (LA)"@en .


###  http://www.semanticweb.org/georg/ontologies/2022/3/WOOD#LaserMeasuringDevice
:LaserMeasuringDevice rdf:type owl:Class ;
                      rdfs:subClassOf :GeometricMeasurements ,
                                      [ rdf:type owl:Restriction ;
                                        owl:onProperty :HasDegreeOfDestruction ;
                                        owl:someValuesFrom :NonDestructiveProcesses
                                      ] ,
                                      [ rdf:type owl:Restriction ;
                                        owl:onProperty :HasTime ;
                                        owl:someValuesFrom :FastProcesses
                                      ] ;
                      rdfs:comment "Laser gauges are used to measure lengths by emitting a laser that emits a distance by impacting to the nearest object."@en ;
                      rdfs:label "Laser measuring device"@en .


###  http://www.semanticweb.org/georg/ontologies/2022/3/WOOD#Lathe
:Lathe rdf:type owl:Class ;
       rdfs:subClassOf :Turning ;
       rdfs:comment "The lathe is a machine tool used for the manufacturing process of turning. Rotationally symmetrical workpieces are produced with a lathe"@en ;
       rdfs:label "Lathe"@en .


###  http://www.semanticweb.org/georg/ontologies/2022/3/WOOD#Leaflet
:Leaflet rdf:type owl:Class ;
         rdfs:subClassOf :WetRotFungi ;
         rdfs:comment "leaflets are fungi that generally do not form visible surface mycelium"@en ;
         rdfs:label "Leaflet"@en .


###  http://www.semanticweb.org/georg/ontologies/2022/3/WOOD#LoadTest
:LoadTest rdf:type owl:Class ;
          rdfs:subClassOf :InvestigationProcedure ,
                          [ rdf:type owl:Restriction ;
                            owl:onProperty :FindsProperties ;
                            owl:someValuesFrom :EModulus
                          ] ,
                          [ rdf:type owl:Restriction ;
                            owl:onProperty :FindsProperties ;
                            owl:someValuesFrom :MaterialSolidity
                          ] ,
                          [ rdf:type owl:Restriction ;
                            owl:onProperty :HasDegreeOfDestruction ;
                            owl:someValuesFrom :DestructiveProcesses
                          ] ,
                          [ rdf:type owl:Restriction ;
                            owl:onProperty :HasDegreeOfDestruction ;
                            owl:someValuesFrom :NonDestructiveProcesses
                          ] ,
                          [ rdf:type owl:Restriction ;
                            owl:onProperty :HasPlace ;
                            owl:someValuesFrom :InSitu
                          ] ,
                          [ rdf:type owl:Restriction ;
                            owl:onProperty :HasTime ;
                            owl:someValuesFrom :SlowProcesses
                          ] ;
          rdfs:comment "The proof of sufficient load-bearing capacity of structures can be determined by load-bearing tests on site. The load-deformation behavior during the test provides conclusions about the remaining load-bearing capacity of the components."@en ;
          rdfs:label "Load test"@en .


###  http://www.semanticweb.org/georg/ontologies/2022/3/WOOD#LocalFindings
:LocalFindings rdf:type owl:Class ;
               rdfs:subClassOf :StepsToTheEvidenceConclusion ;
               rdfs:comment "Local findings include details of taken photos, sketches, entries in documents, examination and measurement results."@en ;
               rdfs:label "Local findings"@en .


###  http://www.semanticweb.org/georg/ontologies/2022/3/WOOD#LowDestructiveProcesses
:LowDestructiveProcesses rdf:type owl:Class ;
                         owl:equivalentClass [ rdf:type owl:Restriction ;
                                               owl:onProperty :HasDegreeOfDestruction ;
                                               owl:someValuesFrom :LowDestructiveProcesses
                                             ] ;
                         rdfs:subClassOf :DegreeOfDestruction ;
                         rdfs:comment "The examination object will suffer minor damages."@en ;
                         rdfs:label "Low-destructive processes"@en .


###  http://www.semanticweb.org/georg/ontologies/2022/3/WOOD#LowDimensionalStability
:LowDimensionalStability rdf:type owl:Class ;
                         owl:equivalentClass [ rdf:type owl:Restriction ;
                                               owl:onProperty :DimensionalStability ;
                                               owl:someValuesFrom :LowDimensionalStability
                                             ] ;
                         rdfs:subClassOf :DimensionalStability ;
                         rdfs:comment "The dimensional stability of these wood types are low in comparison to other wood types. They will not mainain its original dimension when put under pressure."@en ;
                         rdfs:label "Low dimensional stability"@en .


###  http://www.semanticweb.org/georg/ontologies/2022/3/WOOD#LowInsectResistance
:LowInsectResistance rdf:type owl:Class ;
                     owl:equivalentClass [ rdf:type owl:Restriction ;
                                           owl:onProperty :InsectResistance ;
                                           owl:someValuesFrom :LowInsectResistance
                                         ] ;
                     rdfs:subClassOf :InsectResistance ;
                     rdfs:comment "The insect resistance of these wood types are low in comparison to other wood types."@en ;
                     rdfs:label "Low insect resistance"@en .


###  http://www.semanticweb.org/georg/ontologies/2022/3/WOOD#LowRotResistance
:LowRotResistance rdf:type owl:Class ;
                  owl:equivalentClass [ rdf:type owl:Restriction ;
                                        owl:onProperty :RotResistance ;
                                        owl:someValuesFrom :LowRotResistance
                                      ] ;
                  rdfs:subClassOf :RotResistance ;
                  rdfs:comment "The rot resistance of these wood types are low in comparison to other wood types."@en ;
                  rdfs:label "Low rot resistance"@en .


###  http://www.semanticweb.org/georg/ontologies/2022/3/WOOD#MapleAH
:MapleAH rdf:type owl:Class ;
         rdfs:subClassOf :Hardwood ,
                         [ rdf:type owl:Restriction ;
                           owl:onProperty :DimensionalStability ;
                           owl:someValuesFrom :HighDimensionalStability
                         ] ,
                         [ rdf:type owl:Restriction ;
                           owl:onProperty :DimensionalStability ;
                           owl:someValuesFrom :MediumDimensionalStability
                         ] ,
                         [ rdf:type owl:Restriction ;
                           owl:onProperty :InsectResistance ;
                           owl:someValuesFrom :VeryLowInsectResistance
                         ] ,
                         [ rdf:type owl:Restriction ;
                           owl:onProperty :RotResistance ;
                           owl:someValuesFrom :VeryLowRotResistance
                         ] ;
         rdfs:comment """Wood material of Maple trees.

Colour: 
Yellowish white, slightly yellowing, silky glossy. Sapwood and heartwood are not distinguished.

Special properties resistance to rot:
Very low resistance to blue stain fungi.

Special properties resistance to insects:
Very low resistance to anobium."""@en ;
         rdfs:label "Maple (AH)"@en .


###  http://www.semanticweb.org/georg/ontologies/2022/3/WOOD#MaterialSolidity
:MaterialSolidity rdf:type owl:Class ;
                  owl:equivalentClass [ rdf:type owl:Restriction ;
                                        owl:onProperty :FindsProperties ;
                                        owl:someValuesFrom :MaterialSolidity
                                      ] ;
                  rdfs:subClassOf :SearchedProperties ;
                  rdfs:comment "Material solidity is the ability of a material to withstand mechanical stress before failure occurs. This is specified as mechanical stress."@en ;
                  rdfs:label "Material solidity"@en .


###  http://www.semanticweb.org/georg/ontologies/2022/3/WOOD#Measurements
:Measurements rdf:type owl:Class ;
              rdfs:subClassOf :BuildingDocumentation ,
                              [ rdf:type owl:Restriction ;
                                owl:onProperty :StatusOfSource ;
                                owl:someValuesFrom :SourcesPresentState
                              ] ;
              rdfs:comment "A measurement is the process by which a value of a physical quantity is determined as a multiple of a unit."@en ;
              rdfs:label "Measurements"@en .


###  http://www.semanticweb.org/georg/ontologies/2022/3/WOOD#MeasuringMagnifier
:MeasuringMagnifier rdf:type owl:Class ;
                    rdfs:subClassOf :OpticalInspection ,
                                    [ rdf:type owl:Restriction ;
                                      owl:onProperty :FindsProperties ;
                                      owl:someValuesFrom :ChemicalReaction
                                    ] ,
                                    [ rdf:type owl:Restriction ;
                                      owl:onProperty :FindsProperties ;
                                      owl:someValuesFrom :InsectContamination
                                    ] ,
                                    [ rdf:type owl:Restriction ;
                                      owl:onProperty :FindsProperties ;
                                      owl:someValuesFrom :WoodAge
                                    ] ,
                                    [ rdf:type owl:Restriction ;
                                      owl:onProperty :FindsProperties ;
                                      owl:someValuesFrom :WoodSpecies
                                    ] ;
                    rdfs:comment "A magnifying glass is a magnifying device used to see small details more closely."@en ;
                    rdfs:label "Measuring magnifier"@en .


###  http://www.semanticweb.org/georg/ontologies/2022/3/WOOD#MeasuringTape
:MeasuringTape rdf:type owl:Class ;
               rdfs:subClassOf :GeometricMeasurements ,
                               [ rdf:type owl:Restriction ;
                                 owl:onProperty :HasDegreeOfDestruction ;
                                 owl:someValuesFrom :NonDestructiveProcesses
                               ] ,
                               [ rdf:type owl:Restriction ;
                                 owl:onProperty :HasTime ;
                                 owl:someValuesFrom :FastProcesses
                               ] ;
               rdfs:comment "A tape measure is a haptic measuring instrument used to measure short distances."@en ;
               rdfs:label "Measuring tape"@en .


###  http://www.semanticweb.org/georg/ontologies/2022/3/WOOD#MechanicalProcesses
:MechanicalProcesses rdf:type owl:Class ;
                     owl:equivalentClass [ rdf:type owl:Restriction ;
                                           owl:onProperty :CanCreateDamage ;
                                           owl:someValuesFrom :MechanicalProcesses
                                         ] ;
                     rdfs:subClassOf :WoodDamage ;
                     rdfs:comment "It is an process where menchnical influences change the component."@en ;
                     rdfs:label "Mechanical processes"@en .


###  http://www.semanticweb.org/georg/ontologies/2022/3/WOOD#MediumDimensionalStability
:MediumDimensionalStability rdf:type owl:Class ;
                            owl:equivalentClass [ rdf:type owl:Restriction ;
                                                  owl:onProperty :DimensionalStability ;
                                                  owl:someValuesFrom :MediumDimensionalStability
                                                ] ;
                            rdfs:subClassOf :DimensionalStability ;
                            rdfs:comment "The dimensional stability of these wood types are mediocre. When put under pressure these woods will show some movement."@en ;
                            rdfs:label "Medium dimensional stability"@en .


###  http://www.semanticweb.org/georg/ontologies/2022/3/WOOD#MediumInsectResistance
:MediumInsectResistance rdf:type owl:Class ;
                        owl:equivalentClass [ rdf:type owl:Restriction ;
                                              owl:onProperty :InsectResistance ;
                                              owl:someValuesFrom :MediumInsectResistance
                                            ] ;
                        rdfs:subClassOf :InsectResistance ;
                        rdfs:comment "The insect resistance of these wood types are mediocre. Insect will be able to harm these materials."@en ;
                        rdfs:label "Medium insect resistance"@en .


###  http://www.semanticweb.org/georg/ontologies/2022/3/WOOD#MediumRotResistance
:MediumRotResistance rdf:type owl:Class ;
                     owl:equivalentClass [ rdf:type owl:Restriction ;
                                           owl:onProperty :RotResistance ;
                                           owl:someValuesFrom :MediumRotResistance
                                         ] ;
                     rdfs:subClassOf :RotResistance ;
                     rdfs:comment "The rot resistance of these wood types are mediocre. rot will be able to harm these materials."@en ;
                     rdfs:label "Medium rot resistance"@en .


###  http://www.semanticweb.org/georg/ontologies/2022/3/WOOD#MeltLocking
:MeltLocking rdf:type owl:Class ;
             owl:equivalentClass [ rdf:type owl:Restriction ;
                                   owl:onProperty :FittingType ;
                                   owl:someValuesFrom :MeltLocking
                                 ] ;
             rdfs:subClassOf :ConnectionType ;
             rdfs:comment "In a melt locking bond, the components are connected to each other by atomic or molecular bonds. This is also the reason that this type of joint can only be broken by destroying the bonded components."@en ;
             rdfs:label "Melt locking"@en .


###  http://www.semanticweb.org/georg/ontologies/2022/3/WOOD#MerantiDarkRedMER
:MerantiDarkRedMER rdf:type owl:Class ;
                   rdfs:subClassOf :Hardwood ,
                                   [ rdf:type owl:Restriction ;
                                     owl:onProperty :DimensionalStability ;
                                     owl:someValuesFrom :HighDimensionalStability
                                   ] ,
                                   [ rdf:type owl:Restriction ;
                                     owl:onProperty :InsectResistance ;
                                     owl:someValuesFrom :HighInsectResistance
                                   ] ,
                                   [ rdf:type owl:Restriction ;
                                     owl:onProperty :InsectResistance ;
                                     owl:someValuesFrom :MediumInsectResistance
                                   ] ,
                                   [ rdf:type owl:Restriction ;
                                     owl:onProperty :RotResistance ;
                                     owl:someValuesFrom :HighRotResistance
                                   ] ,
                                   [ rdf:type owl:Restriction ;
                                     owl:onProperty :RotResistance ;
                                     owl:someValuesFrom :MediumRotResistance
                                   ] ;
                   rdfs:comment """Wood material of meranti dark red trees.

Colour: 
Yellowish grey to pinkish grey/ reddish brown."""@en ;
                   rdfs:label "Meranti dark red (MER)"@en .


###  http://www.semanticweb.org/georg/ontologies/2022/3/WOOD#MerbauMEB
:MerbauMEB rdf:type owl:Class ;
           rdfs:subClassOf :Hardwood ,
                           [ rdf:type owl:Restriction ;
                             owl:onProperty :DimensionalStability ;
                             owl:someValuesFrom :VeryHighDimensionalStability
                           ] ,
                           [ rdf:type owl:Restriction ;
                             owl:onProperty :InsectResistance ;
                             owl:someValuesFrom :HighInsectResistance
                           ] ,
                           [ rdf:type owl:Restriction ;
                             owl:onProperty :InsectResistance ;
                             owl:someValuesFrom :VeryHighInsectResistance
                           ] ,
                           [ rdf:type owl:Restriction ;
                             owl:onProperty :RotResistance ;
                             owl:someValuesFrom :VeryHighRotResistance
                           ] ;
           rdfs:comment """Wood material of merbau trees.

Colour: 
Yellowish white/ light brown to reddish brown. Darkens after time."""@en ;
           rdfs:label "Merbau (MEB)"@en .


###  http://www.semanticweb.org/georg/ontologies/2022/3/WOOD#MetalComponents
:MetalComponents rdf:type owl:Class ;
                 owl:equivalentClass [ rdf:type owl:Restriction ;
                                       owl:onProperty :FindsProperties ;
                                       owl:someValuesFrom :MetalComponents
                                     ] ;
                 rdfs:subClassOf :SearchedProperties ;
                 rdfs:comment "Metal components that are inside or on the surface of the component."@en ;
                 rdfs:label "Metal components"@en .


###  http://www.semanticweb.org/georg/ontologies/2022/3/WOOD#MetalDetector
:MetalDetector rdf:type owl:Class ;
               rdfs:subClassOf :InvestigationProcedure ,
                               [ rdf:type owl:Restriction ;
                                 owl:onProperty :FindsProperties ;
                                 owl:someValuesFrom :MetalComponents
                               ] ,
                               [ rdf:type owl:Restriction ;
                                 owl:onProperty :HasDegreeOfDestruction ;
                                 owl:someValuesFrom :NonDestructiveProcesses
                               ] ,
                               [ rdf:type owl:Restriction ;
                                 owl:onProperty :HasPlace ;
                                 owl:someValuesFrom :InSitu
                               ] ,
                               [ rdf:type owl:Restriction ;
                                 owl:onProperty :HasTime ;
                                 owl:someValuesFrom :SlowProcesses
                               ] ;
               rdfs:comment "Hidden joints and metallic debris can be found with this. Also wires and power cables."@en ;
               rdfs:label "Metal detector"@en .


###  http://www.semanticweb.org/georg/ontologies/2022/3/WOOD#Microscopy
:Microscopy rdf:type owl:Class ;
            rdfs:subClassOf :InvestigationProcedure ,
                            [ rdf:type owl:Restriction ;
                              owl:onProperty :FindsProperties ;
                              owl:someValuesFrom :ChemicalReaction
                            ] ,
                            [ rdf:type owl:Restriction ;
                              owl:onProperty :FindsProperties ;
                              owl:someValuesFrom :InsectContamination
                            ] ,
                            [ rdf:type owl:Restriction ;
                              owl:onProperty :FindsProperties ;
                              owl:someValuesFrom :WoodAge
                            ] ,
                            [ rdf:type owl:Restriction ;
                              owl:onProperty :FindsProperties ;
                              owl:someValuesFrom :WoodSpecies
                            ] ,
                            [ rdf:type owl:Restriction ;
                              owl:onProperty :HasDegreeOfDestruction ;
                              owl:someValuesFrom :LowDestructiveProcesses
                            ] ,
                            [ rdf:type owl:Restriction ;
                              owl:onProperty :HasPlace ;
                              owl:someValuesFrom :InSitu
                            ] ,
                            [ rdf:type owl:Restriction ;
                              owl:onProperty :HasTime ;
                              owl:someValuesFrom :SlowProcesses
                            ] ;
            rdfs:comment "Further damage can be found during microscopic examination. This procedure is well suited in combination with a drill core removal."@en ;
            rdfs:label "Microscopy"@en .


###  http://www.semanticweb.org/georg/ontologies/2022/3/WOOD#Milling
:Milling rdf:type owl:Class ;
         rdfs:subClassOf :Separate ;
         rdfs:comment "In milling, the material is removed as the milling tool rotates around its own axis at high speed while either the tool traces the contour to be produced or the workpiece is moved accordingly"@en ;
         rdfs:label "Milling"@en .


###  http://www.semanticweb.org/georg/ontologies/2022/3/WOOD#MissingPart
:MissingPart rdf:type owl:Class ;
             owl:equivalentClass [ rdf:type owl:Restriction ;
                                   owl:onProperty :CanCreateDamage ;
                                   owl:someValuesFrom :MissingPart
                                 ] ;
             rdfs:subClassOf :MechanicalProcesses ;
             rdfs:comment "A missing part or a gap of the material. The Possible cause is no longer evident."@en ;
             rdfs:label "Missing part"@en .


###  http://www.semanticweb.org/georg/ontologies/2022/3/WOOD#MoisturePenetration
:MoisturePenetration rdf:type owl:Class ;
                     rdfs:subClassOf :CauseOfDamage ,
                                     [ rdf:type owl:Restriction ;
                                       owl:onProperty :CanCreateDamage ;
                                       owl:someValuesFrom :InsectInfestation
                                     ] ,
                                     [ rdf:type owl:Restriction ;
                                       owl:onProperty :CanCreateDamage ;
                                       owl:someValuesFrom :RotInfestation
                                     ] ,
                                     [ rdf:type owl:Restriction ;
                                       owl:onProperty :CanCreateDamage ;
                                       owl:someValuesFrom :WashoutStresses
                                     ] ;
                     rdfs:comment "Moisture penetration happens, when water enters the component."@en ;
                     rdfs:label "Moisture penetration"@en .


###  http://www.semanticweb.org/georg/ontologies/2022/3/WOOD#Molds
:Molds rdf:type owl:Class ;
       rdfs:subClassOf :WoodDiscoloringFungi ;
       rdfs:comment """Preferred wood species:
Softwood and hardwood

Further notes:
Surface growth on the wood."""@en ;
       rdfs:label "Molds"@en .


###  http://www.semanticweb.org/georg/ontologies/2022/3/WOOD#MusselCrempling
:MusselCrempling rdf:type owl:Class ;
                 rdfs:subClassOf :WetRotFungi ,
                                 [ rdf:type owl:Restriction ;
                                   owl:onProperty :RotDecompositionType ;
                                   owl:someValuesFrom :BrownRot
                                 ] ;
                 rdfs:comment """Preferred wood species:
Softwood and rarely Hardwood

Optimal living conditions of wood moisture content in M-%:
50% to 70%

Optimal living conditions of the temperature range in °C:
23°C to 26°C

Additional notes:
Mycelium dies when dried out."""@en ;
                 rdfs:label "Mussel crempling"@en ,
                            "Paxillus panuoides"@la .


###  http://www.semanticweb.org/georg/ontologies/2022/3/WOOD#Nailing
:Nailing rdf:type owl:Class ;
         rdfs:subClassOf :JoinTools ,
                         [ rdf:type owl:Restriction ;
                           owl:onProperty :FittingType ;
                           owl:someValuesFrom :ForceFit
                         ] ,
                         [ rdf:type owl:Restriction ;
                           owl:onProperty :Removability ;
                           owl:someValuesFrom :Unsolvable
                         ] ;
         rdfs:comment "A nail is a metal pin that contains a head"@en ;
         rdfs:label "Nailling"@en .


###  http://www.semanticweb.org/georg/ontologies/2022/3/WOOD#NonDestructiveProcesses
:NonDestructiveProcesses rdf:type owl:Class ;
                         owl:equivalentClass [ rdf:type owl:Restriction ;
                                               owl:onProperty :HasDegreeOfDestruction ;
                                               owl:someValuesFrom :NonDestructiveProcesses
                                             ] ;
                         rdfs:subClassOf :DegreeOfDestruction ;
                         rdfs:comment "The examination object will not be harmed."@en ;
                         rdfs:label "Non-destructive processes"@en .


###  http://www.semanticweb.org/georg/ontologies/2022/3/WOOD#Norm
:Norm rdf:type owl:Class ;
      rdfs:subClassOf :ExternalResources ,
                      [ rdf:type owl:Restriction ;
                        owl:onProperty :StatusOfSource ;
                        owl:someValuesFrom :SourcesTargetState
                      ] ;
      rdfs:comment "Norming refers to the formulation, issuance, and application of rules, guidelines, or characteristics by a recognized organization and its standards bodies."@en ;
      rdfs:label "Norm"@en .


###  http://www.semanticweb.org/georg/ontologies/2022/3/WOOD#OakEI
:OakEI rdf:type owl:Class ;
       rdfs:subClassOf :Hardwood ,
                       [ rdf:type owl:Restriction ;
                         owl:onProperty :DimensionalStability ;
                         owl:someValuesFrom :MediumDimensionalStability
                       ] ,
                       [ rdf:type owl:Restriction ;
                         owl:onProperty :InsectResistance ;
                         owl:someValuesFrom :HighInsectResistance
                       ] ,
                       [ rdf:type owl:Restriction ;
                         owl:onProperty :RotResistance ;
                         owl:someValuesFrom :HighRotResistance
                       ] ;
       rdfs:comment """Wood material of oak trees.

Colour: 
Grey/ greyish yellow. Darkens to light/ dark brown."""@en ;
       rdfs:label "Oak (EI)"@en .


###  http://www.semanticweb.org/georg/ontologies/2022/3/WOOD#OakWhorling
:OakWhorling rdf:type owl:Class ;
             rdfs:subClassOf :WetRotFungi ,
                             [ rdf:type owl:Restriction ;
                               owl:onProperty :RotDecompositionType ;
                               owl:someValuesFrom :BrownRot
                             ] ;
             rdfs:comment """Preferred wood species:
Oak wood

Optimal living conditions of wood moisture content in M-%:
>50%"""@en ;
             rdfs:label "Daedalia quercina"@la ,
                        "Oak whorling"@en .


###  http://www.semanticweb.org/georg/ontologies/2022/3/WOOD#Oil
:Oil rdf:type owl:Class ;
     rdfs:subClassOf :CoatTools ,
                     [ rdf:type owl:Restriction ;
                       owl:onProperty :WoodColour ;
                       owl:someValuesFrom :ColourEmphasized
                     ] ,
                     [ rdf:type owl:Restriction ;
                       owl:onProperty :WoodGrain ;
                       owl:someValuesFrom :GrainEmphasized
                     ] ;
     rdfs:comment "Oiling is the treatment of the surface with Oil. The wood grain and color is emphasized"@en ;
     rdfs:label "Oil"@en .


###  http://www.semanticweb.org/georg/ontologies/2022/3/WOOD#OpticalInspection
:OpticalInspection rdf:type owl:Class ;
                   rdfs:subClassOf :InvestigationProcedure ,
                                   [ rdf:type owl:Restriction ;
                                     owl:onProperty :FindsProperties ;
                                     owl:someValuesFrom :ChemicalReaction
                                   ] ,
                                   [ rdf:type owl:Restriction ;
                                     owl:onProperty :FindsProperties ;
                                     owl:someValuesFrom :GeometricChange
                                   ] ,
                                   [ rdf:type owl:Restriction ;
                                     owl:onProperty :FindsProperties ;
                                     owl:someValuesFrom :InsectContamination
                                   ] ,
                                   [ rdf:type owl:Restriction ;
                                     owl:onProperty :FindsProperties ;
                                     owl:someValuesFrom :MetalComponents
                                   ] ,
                                   [ rdf:type owl:Restriction ;
                                     owl:onProperty :FindsProperties ;
                                     owl:someValuesFrom :RotContamination
                                   ] ,
                                   [ rdf:type owl:Restriction ;
                                     owl:onProperty :FindsProperties ;
                                     owl:someValuesFrom :WoodAge
                                   ] ,
                                   [ rdf:type owl:Restriction ;
                                     owl:onProperty :FindsProperties ;
                                     owl:someValuesFrom :WoodSpecies
                                   ] ,
                                   [ rdf:type owl:Restriction ;
                                     owl:onProperty :HasDegreeOfDestruction ;
                                     owl:someValuesFrom :NonDestructiveProcesses
                                   ] ,
                                   [ rdf:type owl:Restriction ;
                                     owl:onProperty :HasPlace ;
                                     owl:someValuesFrom :InSitu
                                   ] ,
                                   [ rdf:type owl:Restriction ;
                                     owl:onProperty :HasTime ;
                                     owl:someValuesFrom :FastProcesses
                                   ] ;
                   rdfs:comment "Visual examinations provide the fastest results for damages that are visible to the naked eye. The type and extent of the damage can be determined and even initial conclusions for causes can be drawn."@en ;
                   rdfs:label "Optical inspection"@en .


###  http://www.semanticweb.org/georg/ontologies/2022/3/WOOD#PHMeter
:PHMeter rdf:type owl:Class ;
         rdfs:subClassOf :InvestigationProcedure ,
                         [ rdf:type owl:Restriction ;
                           owl:onProperty :FindsProperties ;
                           owl:someValuesFrom :ChemicalReaction
                         ] ,
                         [ rdf:type owl:Restriction ;
                           owl:onProperty :FindsProperties ;
                           owl:someValuesFrom :PHValue
                         ] ,
                         [ rdf:type owl:Restriction ;
                           owl:onProperty :FindsProperties ;
                           owl:someValuesFrom :RotContamination
                         ] ,
                         [ rdf:type owl:Restriction ;
                           owl:onProperty :HasDegreeOfDestruction ;
                           owl:someValuesFrom :NonDestructiveProcesses
                         ] ,
                         [ rdf:type owl:Restriction ;
                           owl:onProperty :HasPlace ;
                           owl:someValuesFrom :InSitu
                         ] ,
                         [ rdf:type owl:Restriction ;
                           owl:onProperty :HasTime ;
                           owl:someValuesFrom :SlowProcesses
                         ] ;
         rdfs:comment "Detection of brown rot fungi by measuring the concentration of oxalic acid. During the decomposition of wood substance by brown rot, oxalic acid is produced, reducing the pH of the wood from pH = 5 to pH = 3. In the field, a simple color reaction test provides evidence of active fungal attack. The blue color of the indicator turns to green, yellow, when infestation is present. For chemical analysis in the laboratory, only small amounts of a sample of approx. 2 to 5 g are required."@en ;
         rdfs:label "PH meter"@en .


###  http://www.semanticweb.org/georg/ontologies/2022/3/WOOD#PHValue
:PHValue rdf:type owl:Class ;
         owl:equivalentClass [ rdf:type owl:Restriction ;
                               owl:onProperty :FindsProperties ;
                               owl:someValuesFrom :PHValue
                             ] ;
         rdfs:subClassOf :SearchedProperties ;
         rdfs:comment "The PH value is a measure of the acidic or basic character of an aqueous solution."@en ;
         rdfs:label "PH value"@en .


###  http://www.semanticweb.org/georg/ontologies/2022/3/WOOD#PenetrationResistanceTest
:PenetrationResistanceTest rdf:type owl:Class ;
                           rdfs:subClassOf :InvestigationProcedure ,
                                           [ rdf:type owl:Restriction ;
                                             owl:onProperty :FindsProperties ;
                                             owl:someValuesFrom :BulkDensity
                                           ] ,
                                           [ rdf:type owl:Restriction ;
                                             owl:onProperty :FindsProperties ;
                                             owl:someValuesFrom :ConcealedComponents
                                           ] ,
                                           [ rdf:type owl:Restriction ;
                                             owl:onProperty :FindsProperties ;
                                             owl:someValuesFrom :InsectContamination
                                           ] ,
                                           [ rdf:type owl:Restriction ;
                                             owl:onProperty :FindsProperties ;
                                             owl:someValuesFrom :RotContamination
                                           ] ,
                                           [ rdf:type owl:Restriction ;
                                             owl:onProperty :HasDegreeOfDestruction ;
                                             owl:someValuesFrom :LowDestructiveProcesses
                                           ] ,
                                           [ rdf:type owl:Restriction ;
                                             owl:onProperty :HasPlace ;
                                             owl:someValuesFrom :InSitu
                                           ] ,
                                           [ rdf:type owl:Restriction ;
                                             owl:onProperty :HasTime ;
                                             owl:someValuesFrom :FastProcesses
                                           ] ;
                           rdfs:comment "In the penetration resistance test, a pointed tool, such as a chisel, is used to pierce the material. The resistance during penetration gives information about the condition of the material."@en ;
                           rdfs:label "Penetration resistance test"@en .


###  http://www.semanticweb.org/georg/ontologies/2022/3/WOOD#Photogrammetry
:Photogrammetry rdf:type owl:Class ;
                rdfs:subClassOf :GeometricMeasurements ,
                                [ rdf:type owl:Restriction ;
                                  owl:onProperty :HasDegreeOfDestruction ;
                                  owl:someValuesFrom :LowDestructiveProcesses
                                ] ,
                                [ rdf:type owl:Restriction ;
                                  owl:onProperty :HasTime ;
                                  owl:someValuesFrom :SlowProcesses
                                ] ;
                rdfs:comment "Photogrammetry is a measuring method or evaluation procedure to indirectly determine the position and shape of an object from photographs by image measurement."@en ;
                rdfs:label "Photogrammetry"@en .


###  http://www.semanticweb.org/georg/ontologies/2022/3/WOOD#Pictures
:Pictures rdf:type owl:Class ;
          rdfs:subClassOf :OpticalInspection ,
                          [ rdf:type owl:Restriction ;
                            owl:onProperty :FindsProperties ;
                            owl:someValuesFrom :ChemicalReaction
                          ] ,
                          [ rdf:type owl:Restriction ;
                            owl:onProperty :FindsProperties ;
                            owl:someValuesFrom :InsectContamination
                          ] ,
                          [ rdf:type owl:Restriction ;
                            owl:onProperty :FindsProperties ;
                            owl:someValuesFrom :WoodAge
                          ] ,
                          [ rdf:type owl:Restriction ;
                            owl:onProperty :FindsProperties ;
                            owl:someValuesFrom :WoodSpecies
                          ] ,
                          [ rdf:type owl:Restriction ;
                            owl:onProperty :StatusOfSource ;
                            owl:someValuesFrom :SourcesPresentState
                          ] ;
          rdfs:comment "Photography refers to a genre of fine art in which optical processes are used to project a light image onto a light-sensitive medium and store it permanently."@en ;
          rdfs:label "Pictures"@en .


###  http://www.semanticweb.org/georg/ontologies/2022/3/WOOD#PineKI
:PineKI rdf:type owl:Class ;
        rdfs:subClassOf :Softwood ,
                        [ rdf:type owl:Restriction ;
                          owl:onProperty :DimensionalStability ;
                          owl:someValuesFrom :HighDimensionalStability
                        ] ,
                        [ rdf:type owl:Restriction ;
                          owl:onProperty :DimensionalStability ;
                          owl:someValuesFrom :MediumDimensionalStability
                        ] ,
                        [ rdf:type owl:Restriction ;
                          owl:onProperty :InsectResistance ;
                          owl:someValuesFrom :LowInsectResistance
                        ] ,
                        [ rdf:type owl:Restriction ;
                          owl:onProperty :RotResistance ;
                          owl:someValuesFrom :LowRotResistance
                        ] ,
                        [ rdf:type owl:Restriction ;
                          owl:onProperty :RotResistance ;
                          owl:someValuesFrom :MediumRotResistance
                        ] ;
        rdfs:comment """Wood material of pine trees.

Colour:
Light yellowish white/ reddish white, browning after time, late wood darker.


Special properties resistance to fungi:
Sapwood very sensitive to blue stain."""@en ;
        rdfs:label "Pine (KI)"@en .


###  http://www.semanticweb.org/georg/ontologies/2022/3/WOOD#PinePIP
:PinePIP rdf:type owl:Class ;
         rdfs:subClassOf :Softwood ,
                         [ rdf:type owl:Restriction ;
                           owl:onProperty :DimensionalStability ;
                           owl:someValuesFrom :HighDimensionalStability
                         ] ,
                         [ rdf:type owl:Restriction ;
                           owl:onProperty :DimensionalStability ;
                           owl:someValuesFrom :MediumDimensionalStability
                         ] ,
                         [ rdf:type owl:Restriction ;
                           owl:onProperty :InsectResistance ;
                           owl:someValuesFrom :LowInsectResistance
                         ] ,
                         [ rdf:type owl:Restriction ;
                           owl:onProperty :InsectResistance ;
                           owl:someValuesFrom :MediumInsectResistance
                         ] ,
                         [ rdf:type owl:Restriction ;
                           owl:onProperty :RotResistance ;
                           owl:someValuesFrom :LowRotResistance
                         ] ,
                         [ rdf:type owl:Restriction ;
                           owl:onProperty :RotResistance ;
                           owl:someValuesFrom :MediumRotResistance
                         ] ;
         rdfs:comment """Wood material of pine trees.

Colour:
Yellowish/ reddish yellow to reddish brown/ late wood is dark.

Special properties resistance to fungi:
Different vulnerabilities for heartwood and sapwood. Sapwood has a low sensitivity, heartwood has a medium sensitivity."""@en ;
         rdfs:label "Pine (PIP)"@en .


###  http://www.semanticweb.org/georg/ontologies/2022/3/WOOD#Plane
:Plane rdf:type owl:Class ;
       rdfs:subClassOf :Separate ;
       rdfs:comment "Plane is a method of machining wood. The surface of the wood is machined by removing chips from the material. The aim is to level and smooth the surface."@en ;
       rdfs:label "Plane"@en .


###  http://www.semanticweb.org/georg/ontologies/2022/3/WOOD#Planer
:Planer rdf:type owl:Class ;
        rdfs:subClassOf :Plane ;
        rdfs:comment "The planer is a tool where the surface of the wood is machined by removing chips from the material with the plane iron"@en ;
        rdfs:label "Planer"@en .


###  http://www.semanticweb.org/georg/ontologies/2022/3/WOOD#ProcedureLocation
:ProcedureLocation rdf:type owl:Class ;
                   rdfs:subClassOf :Investigation ;
                   rdfs:comment "Location where the examination method is evaluated. If the research method is only partially evaluated on site, only the additional site is listed."@en ;
                   rdfs:label "Procedure location"@en .


###  http://www.semanticweb.org/georg/ontologies/2022/3/WOOD#ProcedureStatus
:ProcedureStatus rdf:type owl:Class ;
                 rdfs:subClassOf :Report ;
                 rdfs:comment "Status of each investigation procedure of each individual damge, that has to be conducted."@en ;
                 rdfs:label "Procedure status"@en .


###  http://www.semanticweb.org/georg/ontologies/2022/3/WOOD#ProfileBoards
:ProfileBoards rdf:type owl:Class ;
               rdfs:subClassOf :SolidWood ;
               rdfs:comment "Planed and profiled lumber is sawn from round timber and then planed and milled."@en ;
               rdfs:label "Profile boards"@en .


###  http://www.semanticweb.org/georg/ontologies/2022/3/WOOD#PropertiesChange
:PropertiesChange rdf:type owl:Class ;
                  rdfs:subClassOf :Repair ;
                  rdfs:comment "Manufacturing by changing the properties of the material from which a workpiece is made"@en ;
                  rdfs:label "Properties change"@en .


###  http://www.semanticweb.org/georg/ontologies/2022/3/WOOD#Protocols
:Protocols rdf:type owl:Class ;
           rdfs:subClassOf :BuildingDocumentation ,
                           [ rdf:type owl:Restriction ;
                             owl:onProperty :StatusOfSource ;
                             owl:someValuesFrom :SourcesPresentState
                           ] ;
           rdfs:comment "A record is a verbatim transcript, or a transcript limited to the essential points, of a meeting, negotiation, or conversation."@en ;
           rdfs:label "Protocols"@en .


###  http://www.semanticweb.org/georg/ontologies/2022/3/WOOD#RadiocarbonMethod
:RadiocarbonMethod rdf:type owl:Class ;
                   rdfs:subClassOf :InvestigationProcedure ,
                                   [ rdf:type owl:Restriction ;
                                     owl:onProperty :FindsProperties ;
                                     owl:someValuesFrom :WoodAge
                                   ] ,
                                   [ rdf:type owl:Restriction ;
                                     owl:onProperty :HasDegreeOfDestruction ;
                                     owl:someValuesFrom :LowDestructiveProcesses
                                   ] ,
                                   [ rdf:type owl:Restriction ;
                                     owl:onProperty :HasPlace ;
                                     owl:someValuesFrom :Laboratory
                                   ] ,
                                   [ rdf:type owl:Restriction ;
                                     owl:onProperty :HasTime ;
                                     owl:someValuesFrom :SlowProcesses
                                   ] ;
                   rdfs:comment "Radioactive age determination, means the determination of the age of objects based on the radionuclides they contain."@en ;
                   rdfs:label "Radiocarbon method"@en .


###  http://www.semanticweb.org/georg/ontologies/2022/3/WOOD#RaspFile
:RaspFile rdf:type owl:Class ;
          rdfs:subClassOf :Files ;
          rdfs:comment "Files have a handle and a file blade"@en ;
          rdfs:label "Rasp/ File"@en .


###  http://www.semanticweb.org/georg/ontologies/2022/3/WOOD#Reagents
:Reagents rdf:type owl:Class ;
          rdfs:subClassOf :InvestigationProcedure ,
                          [ rdf:type owl:Restriction ;
                            owl:onProperty :FindsProperties ;
                            owl:someValuesFrom :Salinity
                          ] ,
                          [ rdf:type owl:Restriction ;
                            owl:onProperty :HasDegreeOfDestruction ;
                            owl:someValuesFrom :LowDestructiveProcesses
                          ] ,
                          [ rdf:type owl:Restriction ;
                            owl:onProperty :HasPlace ;
                            owl:someValuesFrom :Laboratory
                          ] ,
                          [ rdf:type owl:Restriction ;
                            owl:onProperty :HasTime ;
                            owl:someValuesFrom :SlowProcesses
                          ] ;
          rdfs:comment "Detection reagents are used to detect the increased content of salts and other substances."@en ;
          rdfs:label "Reagents"@en .


###  http://www.semanticweb.org/georg/ontologies/2022/3/WOOD#Records
:Records rdf:type owl:Class ;
         rdfs:subClassOf :BuildingDocumentation ,
                         [ rdf:type owl:Restriction ;
                           owl:onProperty :StatusOfSource ;
                           owl:someValuesFrom :SourcesPresentState
                         ] ;
         rdfs:comment "A record is a thing that is evidence of the past, especially a report that is recorded in writing or other permanent form."@en ;
         rdfs:label "Records"@en .


###  http://www.semanticweb.org/georg/ontologies/2022/3/WOOD#ReductionInLoadCapacityDueToWear
:ReductionInLoadCapacityDueToWear rdf:type owl:Class ;
                                  rdfs:subClassOf :ServiceStresses ,
                                                  [ rdf:type owl:Restriction ;
                                                    owl:onProperty :CanCreateDamage ;
                                                    owl:someValuesFrom :Cracks
                                                  ] ,
                                                  [ rdf:type owl:Restriction ;
                                                    owl:onProperty :CanCreateDamage ;
                                                    owl:someValuesFrom :Deflection
                                                  ] ,
                                                  [ rdf:type owl:Restriction ;
                                                    owl:onProperty :CanCreateDamage ;
                                                    owl:someValuesFrom :Delocalization
                                                  ] ,
                                                  [ rdf:type owl:Restriction ;
                                                    owl:onProperty :CanCreateDamage ;
                                                    owl:someValuesFrom :Fractures
                                                  ] ,
                                                  [ rdf:type owl:Restriction ;
                                                    owl:onProperty :CanCreateDamage ;
                                                    owl:someValuesFrom :Holes
                                                  ] ;
                                  rdfs:comment "Reduction in load capacitiy due to wear of the component. This can happen if the component has been used incorrectly or if the maximum age of the component has been exceeded."@en ;
                                  rdfs:label "Reduction in load capacitiy due to wear"@en .


###  http://www.semanticweb.org/georg/ontologies/2022/3/WOOD#Regulations
:Regulations rdf:type owl:Class ;
             rdfs:subClassOf :ExternalResources ,
                             [ rdf:type owl:Restriction ;
                               owl:onProperty :StatusOfSource ;
                               owl:someValuesFrom :SourcesTargetState
                             ] ;
             rdfs:comment "Building regulations come from the laws of the country in which the building project is located. The building codes are regulations that dictate the building process."@en ;
             rdfs:label "Regulations"@en .


###  http://www.semanticweb.org/georg/ontologies/2022/3/WOOD#Removal
:Removal rdf:type owl:Class ;
         rdfs:subClassOf :Join ;
         rdfs:comment "It is about the removal of the previously attached connecting medium."@en ;
         rdfs:label "Removal"@en .


###  http://www.semanticweb.org/georg/ontologies/2022/3/WOOD#Repair
:Repair rdf:type owl:Class ;
        rdfs:comment "List of repair procedures for wood damages."@en ;
        rdfs:label "Repair"@en .


###  http://www.semanticweb.org/georg/ontologies/2022/3/WOOD#Report
:Report rdf:type owl:Class ;
        rdfs:comment "An report is a document that is commissioned by an expert for a court or by a private person, it is to be prepared objectively and impartially. It is presented in a way that is understandable for a layperson and fully comprehensible for an expert. An report is a reasoned presentation of empirical principles and the derivation of conclusions for the actual assessment of an occurrence."@en ;
        rdfs:label "Report"@en .


###  http://www.semanticweb.org/georg/ontologies/2022/3/WOOD#Restoration
:Restoration rdf:type owl:Class ;
             rdfs:subClassOf :StepsToTheEvidenceConclusion ;
             rdfs:comment "Restoration options can also be provided. These can be named and described, but it is important to ensure that the report remains concise and the costs remain economical."@en ;
             rdfs:label "Restoration"@en .


###  http://www.semanticweb.org/georg/ontologies/2022/3/WOOD#RobiniaROB
:RobiniaROB rdf:type owl:Class ;
            rdfs:subClassOf :Hardwood ,
                            [ rdf:type owl:Restriction ;
                              owl:onProperty :DimensionalStability ;
                              owl:someValuesFrom :MediumDimensionalStability
                            ] ,
                            [ rdf:type owl:Restriction ;
                              owl:onProperty :InsectResistance ;
                              owl:someValuesFrom :HighInsectResistance
                            ] ,
                            [ rdf:type owl:Restriction ;
                              owl:onProperty :RotResistance ;
                              owl:someValuesFrom :VeryHighRotResistance
                            ] ;
            rdfs:comment """Wood material of Robinia trees.

Colour: 
Light yellow to greenish yellow to olive green. Later shiny golden brown."""@en ;
            rdfs:label "Robinia (ROB)"@en .


###  http://www.semanticweb.org/georg/ontologies/2022/3/WOOD#Rot
:Rot rdf:type owl:Class ;
     rdfs:subClassOf :BiologicalInfluences ,
                     [ rdf:type owl:Restriction ;
                       owl:onProperty :CanCreateDamage ;
                       owl:someValuesFrom :RotInfestation
                     ] ;
     rdfs:comment "List of fungi that occur in the building. The cause of any fungal growth in wood is moisture. The fungi germinate from spores which need moisture to grow. These spores are contained in the air or lie on the wood. With suitable humidity and environmental conditions, growth begins."@en ;
     rdfs:label "Rot"@en .


###  http://www.semanticweb.org/georg/ontologies/2022/3/WOOD#RotContamination
:RotContamination rdf:type owl:Class ;
                  owl:equivalentClass [ rdf:type owl:Restriction ;
                                        owl:onProperty :FindsProperties ;
                                        owl:someValuesFrom :RotContamination
                                      ] ;
                  rdfs:subClassOf :SearchedProperties ;
                  rdfs:comment "Rot contermination is the condition of infestation of the component caused by Rot."@en ;
                  rdfs:label "Rot contamination"@en .


###  http://www.semanticweb.org/georg/ontologies/2022/3/WOOD#RotInfestation
:RotInfestation rdf:type owl:Class ;
                owl:equivalentClass [ rdf:type owl:Restriction ;
                                      owl:onProperty :CanCreateDamage ;
                                      owl:someValuesFrom :RotInfestation
                                    ] ;
                rdfs:subClassOf :BiologicalProcesses ;
                rdfs:comment "An infestation of the wood substance by rot."@en ;
                rdfs:label "Rot infestation"@en .


###  http://www.semanticweb.org/georg/ontologies/2022/3/WOOD#RotResistance
:RotResistance rdf:type owl:Class ;
               rdfs:subClassOf :WoodTypes .


###  http://www.semanticweb.org/georg/ontologies/2022/3/WOOD#Roundwood
:Roundwood rdf:type owl:Class ;
           rdfs:subClassOf :SolidWood ;
           rdfs:comment "Roundwood consists of logs or log sections."@en ;
           rdfs:label "Roundwood"@en .


###  http://www.semanticweb.org/georg/ontologies/2022/3/WOOD#Salinity
:Salinity rdf:type owl:Class ;
          owl:equivalentClass [ rdf:type owl:Restriction ;
                                owl:onProperty :FindsProperties ;
                                owl:someValuesFrom :Salinity
                              ] ;
          rdfs:subClassOf :SearchedProperties ;
          rdfs:comment "Salinity refers to the salt content of a component."@en ;
          rdfs:label "Salinity"@en .


###  http://www.semanticweb.org/georg/ontologies/2022/3/WOOD#Salts
:Salts rdf:type owl:Class ;
       rdfs:subClassOf :ChemicalInfluences ,
                       [ rdf:type owl:Restriction ;
                         owl:onProperty :CanCreateDamage ;
                         owl:someValuesFrom :DecompositionAndMaceration
                       ] ;
       rdfs:comment "In case of overdosage of salt-containing wood preservatives on wooden components, maceration is likely to occur. The salt can also be washed out of clay bricks or lime mortar."@en ;
       rdfs:label "Salts"@en .


###  http://www.semanticweb.org/georg/ontologies/2022/3/WOOD#Sandpaper
:Sandpaper rdf:type owl:Class ;
           rdfs:subClassOf :Grinding ;
           rdfs:comment "Sandpaper is used to smooth rough surfaces or to break edges. It is also suitable for larger material removal"@en ;
           rdfs:label "Sandpaper"@en .


###  http://www.semanticweb.org/georg/ontologies/2022/3/WOOD#Sapwood
:Sapwood rdf:type owl:Class ;
         rdfs:subClassOf :Structure ;
         rdfs:comment "Sapwood is the physiologically active wood below the cambium in the trunk of a tree. Its capillaries conduct water and nutrient salts into the tree crown and store sugar and starch in the parenchyma." ;
         rdfs:label "Sapwood"@en .


###  http://www.semanticweb.org/georg/ontologies/2022/3/WOOD#Sawing
:Sawing rdf:type owl:Class ;
        rdfs:subClassOf :Separate ;
        rdfs:comment "Sawing is a cutting manufacturing process for slitting and separating workpieces"@en ;
        rdfs:label "Sawing"@en .


###  http://www.semanticweb.org/georg/ontologies/2022/3/WOOD#ScalySawfly
:ScalySawfly rdf:type owl:Class ;
             rdfs:subClassOf :Leaflet ,
                             [ rdf:type owl:Restriction ;
                               owl:onProperty :RotDecompositionType ;
                               owl:someValuesFrom :BrownRot
                             ] ;
             rdfs:comment """Preferred wood species:
Hardwood

Optimal living conditions of wood moisture content in M-%:
30% to 40%

Optimal living conditions of the temperature range in °C:
26°C to 35°C

Additional notes:
Mycelium dies after prolonged dehydration."""@en ;
             rdfs:label "Lentinus lepideus"@la ,
                        "Scaly sawfly"@en .


###  http://www.semanticweb.org/georg/ontologies/2022/3/WOOD#Scraper
:Scraper rdf:type owl:Class ;
         rdfs:subClassOf :Scraping ;
         rdfs:comment "A scraper is a tool provided with at least one cutting edge for scraping"@en ;
         rdfs:label "Scraper"@en .


###  http://www.semanticweb.org/georg/ontologies/2022/3/WOOD#Scraping
:Scraping rdf:type owl:Class ;
          rdfs:subClassOf :Separate ;
          rdfs:comment "Scraping involves running a sharp blade over the wood. The chip angle is negative to the cutting edge"@en ;
          rdfs:label "Scraping"@en .


###  http://www.semanticweb.org/georg/ontologies/2022/3/WOOD#Screws
:Screws rdf:type owl:Class ;
        rdfs:subClassOf :JoinTools ,
                        [ rdf:type owl:Restriction ;
                          owl:onProperty :FittingType ;
                          owl:someValuesFrom :ForceFit
                        ] ,
                        [ rdf:type owl:Restriction ;
                          owl:onProperty :Removability ;
                          owl:someValuesFrom :Solvable
                        ] ;
        rdfs:comment "A screw is a connecting element that has a thread"@en ;
        rdfs:label "Screws"@en .


###  http://www.semanticweb.org/georg/ontologies/2022/3/WOOD#SearchedProperties
:SearchedProperties rdf:type owl:Class ;
                    rdfs:subClassOf :Investigation ;
                    rdfs:comment "Propteries of damages and wooden components, that can be found using a investigation procedure. Analyzing and comparing these properties the investigator can find causes of damages."@en ;
                    rdfs:label "Searched properties"@en .


###  http://www.semanticweb.org/georg/ontologies/2022/3/WOOD#Separate
:Separate rdf:type owl:Class ;
          rdfs:subClassOf :Repair ;
          rdfs:comment "To fabricate by undoing the cohesion of bodies, reducing the cohesion in part or in whole"@en ;
          rdfs:label "Separate"@en .


###  http://www.semanticweb.org/georg/ontologies/2022/3/WOOD#ServiceStresses
:ServiceStresses rdf:type owl:Class ;
                 rdfs:subClassOf :mechanicalInfluences ;
                 rdfs:comment "The service stress refers to a variable or moving load on a structural component. These can come, for example, from people, vehicles or snow."@en ;
                 rdfs:label "Service stresses"@en .


###  http://www.semanticweb.org/georg/ontologies/2022/3/WOOD#Shocks
:Shocks rdf:type owl:Class ;
        rdfs:subClassOf :DynamicOverstress ,
                        [ rdf:type owl:Restriction ;
                          owl:onProperty :CanCreateDamage ;
                          owl:someValuesFrom :Cracks
                        ] ,
                        [ rdf:type owl:Restriction ;
                          owl:onProperty :CanCreateDamage ;
                          owl:someValuesFrom :Delocalization
                        ] ,
                        [ rdf:type owl:Restriction ;
                          owl:onProperty :CanCreateDamage ;
                          owl:someValuesFrom :Fractures
                        ] ;
        rdfs:comment "Shocks can occur due to construction work or even traffic."@en ;
        rdfs:label "Shocks"@en .


###  http://www.semanticweb.org/georg/ontologies/2022/3/WOOD#SlowProcesses
:SlowProcesses rdf:type owl:Class ;
               owl:equivalentClass [ rdf:type owl:Restriction ;
                                     owl:onProperty :HasTime ;
                                     owl:someValuesFrom :SlowProcesses
                                   ] ;
               rdfs:subClassOf :TestDuration ;
               rdfs:comment "Processes that need some time of preperation or use tools that are not likely to be brought to the first inspection. These procedures are mostly conducted during a second inspection visit."@en ;
               rdfs:label "Slow processes"@en .


###  http://www.semanticweb.org/georg/ontologies/2022/3/WOOD#Softwood
:Softwood rdf:type owl:Class ;
          rdfs:subClassOf :WoodTypes ;
          rdfs:comment "Softwood is the name given to all types of wood whose timber comes from needle trees. They owe their name to the fact that their leaves look like small needles."@en ;
          rdfs:label "Softwood"@en .


###  http://www.semanticweb.org/georg/ontologies/2022/3/WOOD#SolidStructuralTimber
:SolidStructuralTimber rdf:type owl:Class ;
                       rdfs:subClassOf :SolidWood ;
                       rdfs:comment "Is made out of higher quality building timber products with regard to dimensional accuracy, dimensional stability, reduced cracking and surface quality."@en ;
                       rdfs:label "Solid structural timber"@en .


###  http://www.semanticweb.org/georg/ontologies/2022/3/WOOD#SolidWood
:SolidWood rdf:type owl:Class ;
           rdfs:subClassOf :ConstructionWood ;
           owl:disjointWith :WoodBasedMaterials ;
           rdfs:comment "Wood products for the construction site, that consist of a single solid wood, or a number of solid wood parts that are glued together."@en ;
           rdfs:label "Solid wood"@en .


###  http://www.semanticweb.org/georg/ontologies/2022/3/WOOD#Solvable
:Solvable rdf:type owl:Class ;
          owl:equivalentClass [ rdf:type owl:Restriction ;
                                owl:onProperty :Removability ;
                                owl:someValuesFrom :Solvable
                              ] ;
          rdfs:subClassOf :Removal ;
          owl:disjointWith :Unsolvable ;
          rdfs:comment "The connecting medium can be detached after use without leaving any permanent traces."@en ;
          rdfs:label "Solvable"@en .


###  http://www.semanticweb.org/georg/ontologies/2022/3/WOOD#SoundTest
:SoundTest rdf:type owl:Class ;
           rdfs:subClassOf :InvestigationProcedure ,
                           [ rdf:type owl:Restriction ;
                             owl:onProperty :FindsProperties ;
                             owl:someValuesFrom :ConcealedComponents
                           ] ,
                           [ rdf:type owl:Restriction ;
                             owl:onProperty :FindsProperties ;
                             owl:someValuesFrom :WoodMoisture
                           ] ,
                           [ rdf:type owl:Restriction ;
                             owl:onProperty :HasDegreeOfDestruction ;
                             owl:someValuesFrom :NonDestructiveProcesses
                           ] ,
                           [ rdf:type owl:Restriction ;
                             owl:onProperty :HasPlace ;
                             owl:someValuesFrom :InSitu
                           ] ,
                           [ rdf:type owl:Restriction ;
                             owl:onProperty :HasTime ;
                             owl:someValuesFrom :FastProcesses
                           ] ;
           rdfs:comment "By tapping the suspect area, conclusions can be drawn about the condition of the material or cavities."@en ;
           rdfs:label "Sound test"@en .


###  http://www.semanticweb.org/georg/ontologies/2022/3/WOOD#Source
:Source rdf:type owl:Class ;
        rdfs:subClassOf :StepsToTheEvidenceConclusion ;
        rdfs:comment "The causes of the defect are to be presented in a comprehensible description based on the findings"@en ;
        rdfs:label "Source"@en .


###  http://www.semanticweb.org/georg/ontologies/2022/3/WOOD#Sources
:Sources rdf:type owl:Class ;
         rdfs:subClassOf :Report ;
         rdfs:comment "List of sources that have information regarding the building. These sources can show the current state, an older state or the required state. They are often used to compare these different states to point out a deficiency."@en ;
         rdfs:label "Sources"@en .


###  http://www.semanticweb.org/georg/ontologies/2022/3/WOOD#SourcesPresentState
:SourcesPresentState rdf:type owl:Class ;
                     owl:equivalentClass [ rdf:type owl:Restriction ;
                                           owl:onProperty :StatusOfSource ;
                                           owl:someValuesFrom :SourcesPresentState
                                         ] ;
                     rdfs:subClassOf :Sources ;
                     rdfs:comment "Building status at the moment."@en ;
                     rdfs:label "Sources present state"@en .


###  http://www.semanticweb.org/georg/ontologies/2022/3/WOOD#SourcesTargetState
:SourcesTargetState rdf:type owl:Class ;
                    owl:equivalentClass [ rdf:type owl:Restriction ;
                                          owl:onProperty :StatusOfSource ;
                                          owl:someValuesFrom :SourcesTargetState
                                        ] ;
                    rdfs:subClassOf :Sources ;
                    rdfs:comment "Building status that should be achieved."@en ;
                    rdfs:label "Sources target state"@en .


###  http://www.semanticweb.org/georg/ontologies/2022/3/WOOD#Splitting
:Splitting rdf:type owl:Class ;
           rdfs:subClassOf :Separate ;
           rdfs:comment "Splitting is a manufacturing process for dividing a workpiece by using a wedge-shaped tool"@en ;
           rdfs:label "Splitting"@en .


###  http://www.semanticweb.org/georg/ontologies/2022/3/WOOD#SpruceFI
:SpruceFI rdf:type owl:Class ;
          rdfs:subClassOf :Softwood ,
                          [ rdf:type owl:Restriction ;
                            owl:onProperty :DimensionalStability ;
                            owl:someValuesFrom :HighDimensionalStability
                          ] ,
                          [ rdf:type owl:Restriction ;
                            owl:onProperty :InsectResistance ;
                            owl:someValuesFrom :LowInsectResistance
                          ] ,
                          [ rdf:type owl:Restriction ;
                            owl:onProperty :RotResistance ;
                            owl:someValuesFrom :LowRotResistance
                          ] ;
          rdfs:comment """Wood material of spruce trees.

Colour:
Early wood yellowish white, late wood reddish yellow, sapwood and heartwood is not distinguished.

Special properties resistance to fungi:
Sensitive to blue stain."""@en ;
          rdfs:label "Spruce (FI)"@en .


###  http://www.semanticweb.org/georg/ontologies/2022/3/WOOD#Stain
:Stain rdf:type owl:Class ;
       rdfs:subClassOf :CoatTools ,
                       [ rdf:type owl:Restriction ;
                         owl:onProperty :WoodColour ;
                         owl:someValuesFrom :ColourEmphasized
                       ] ,
                       [ rdf:type owl:Restriction ;
                         owl:onProperty :WoodGrain ;
                         owl:someValuesFrom :GrainRemainsVisible
                       ] ;
       rdfs:comment "Staining is the treatment of the surface with a chemical solution known as stain. The wood grain remains visible"@en ;
       rdfs:label "Stain"@en .


###  http://www.semanticweb.org/georg/ontologies/2022/3/WOOD#StaticOverstress
:StaticOverstress rdf:type owl:Class ;
                  rdfs:subClassOf :mechanicalInfluences ,
                                  [ rdf:type owl:Restriction ;
                                    owl:onProperty :CanCreateDamage ;
                                    owl:someValuesFrom :Cracks
                                  ] ,
                                  [ rdf:type owl:Restriction ;
                                    owl:onProperty :CanCreateDamage ;
                                    owl:someValuesFrom :Deflection
                                  ] ,
                                  [ rdf:type owl:Restriction ;
                                    owl:onProperty :CanCreateDamage ;
                                    owl:someValuesFrom :Delocalization
                                  ] ,
                                  [ rdf:type owl:Restriction ;
                                    owl:onProperty :CanCreateDamage ;
                                    owl:someValuesFrom :Fractures
                                  ] ,
                                  [ rdf:type owl:Restriction ;
                                    owl:onProperty :CanCreateDamage ;
                                    owl:someValuesFrom :Holes
                                  ] ;
                  rdfs:comment "A static stress applies forces and moments on a structure that are constant and uniform and produces only a single response."@en ;
                  rdfs:label "Static overstresses"@en .


###  http://www.semanticweb.org/georg/ontologies/2022/3/WOOD#SteelBrush
:SteelBrush rdf:type owl:Class ;
            rdfs:subClassOf :BrushMachining ;
            rdfs:comment "A brush consists of a base body and a brush trim. It belongs to the method of machining without a geometrically defined cutting edge"@en ;
            rdfs:label "Steel brush"@en .


###  http://www.semanticweb.org/georg/ontologies/2022/3/WOOD#StepsToTheEvidenceConclusion
:StepsToTheEvidenceConclusion rdf:type owl:Class ;
                              rdfs:subClassOf :Report ;
                              rdfs:comment "Paragraphs that are necessray for describing the found evidence in an report."@en ;
                              rdfs:label "Steps to the evidence conclusion"@en .


###  http://www.semanticweb.org/georg/ontologies/2022/3/WOOD#Stethoscope
:Stethoscope rdf:type owl:Class ;
             rdfs:subClassOf :InvestigationProcedure ,
                             [ rdf:type owl:Restriction ;
                               owl:onProperty :FindsProperties ;
                               owl:someValuesFrom :InsectContamination
                             ] ,
                             [ rdf:type owl:Restriction ;
                               owl:onProperty :HasDegreeOfDestruction ;
                               owl:someValuesFrom :NonDestructiveProcesses
                             ] ,
                             [ rdf:type owl:Restriction ;
                               owl:onProperty :HasPlace ;
                               owl:someValuesFrom :InSitu
                             ] ,
                             [ rdf:type owl:Restriction ;
                               owl:onProperty :HasTime ;
                               owl:someValuesFrom :SlowProcesses
                             ] ;
             rdfs:comment "The stethoscope can be used to detect sewing noises from active insect infestations."@en ;
             rdfs:label "Stethoscope"@en .


###  http://www.semanticweb.org/georg/ontologies/2022/3/WOOD#Structure
:Structure rdf:type owl:Class ;
           rdfs:subClassOf :WoodComponent ;
           rdfs:comment "wood structure is differentiated by different properties." ;
           rdfs:label "Structure"@en .


###  http://www.semanticweb.org/georg/ontologies/2022/3/WOOD#SurfacePlaners
:SurfacePlaners rdf:type owl:Class ;
                rdfs:subClassOf :Plane ;
                rdfs:comment "The jointer is a tool for smoothing and planing wood or wood materials"@en ;
                rdfs:label "Surface planer"@en .


###  http://www.semanticweb.org/georg/ontologies/2022/3/WOOD#TeakTEK
:TeakTEK rdf:type owl:Class ;
         rdfs:subClassOf :Hardwood ,
                         [ rdf:type owl:Restriction ;
                           owl:onProperty :DimensionalStability ;
                           owl:someValuesFrom :VeryHighDimensionalStability
                         ] ,
                         [ rdf:type owl:Restriction ;
                           owl:onProperty :InsectResistance ;
                           owl:someValuesFrom :VeryHighInsectResistance
                         ] ,
                         [ rdf:type owl:Restriction ;
                           owl:onProperty :RotResistance ;
                           owl:someValuesFrom :VeryHighRotResistance
                         ] ;
         rdfs:comment """Wood material of teak trees.

Colour:
Grey/ golden yellow, later medium/ to dark brown. Often narrow black veins. Shiny surface.

Special properties resistance to insects:
Termite-proof."""@en ;
         rdfs:label "Teak (TEK)"@en .


###  http://www.semanticweb.org/georg/ontologies/2022/3/WOOD#TechnicalLiterature
:TechnicalLiterature rdf:type owl:Class ;
                     rdfs:subClassOf :ExternalResources ,
                                     [ rdf:type owl:Restriction ;
                                       owl:onProperty :StatusOfSource ;
                                       owl:someValuesFrom :SourcesTargetState
                                     ] ;
                     rdfs:comment "Technical literature is a subset of literature. It is for a specialized audience thats mostly focused on professional application or acquiring new scientific knowledge."@en ;
                     rdfs:label "Technical literature"@en .


###  http://www.semanticweb.org/georg/ontologies/2022/3/WOOD#TechnicalPlans
:TechnicalPlans rdf:type owl:Class ;
                rdfs:subClassOf :BuildingDocumentation ,
                                [ rdf:type owl:Restriction ;
                                  owl:onProperty :StatusOfSource ;
                                  owl:someValuesFrom :SourcesPresentState
                                ] ;
                rdfs:comment "A technical drawing is a graphic document used to represent in graphic and sometimes also in written form information about components."@en ;
                rdfs:label "Technical plans"@en .


###  http://www.semanticweb.org/georg/ontologies/2022/3/WOOD#Tenon
:Tenon rdf:type owl:Class ;
       rdfs:subClassOf :JoinTools ,
                       [ rdf:type owl:Restriction ;
                         owl:onProperty :FittingType ;
                         owl:someValuesFrom :FormFitting
                       ] ,
                       [ rdf:type owl:Restriction ;
                         owl:onProperty :Removability ;
                         owl:someValuesFrom :Solvable
                       ] ;
       rdfs:comment "A mortise joint is a wood joint in carpentry. It consists of a tenon and the mortise"@en ;
       rdfs:label "Tenon"@en .


###  http://www.semanticweb.org/georg/ontologies/2022/3/WOOD#TestDuration
:TestDuration rdf:type owl:Class ;
              rdfs:subClassOf :Investigation ;
              rdfs:comment "TIme a test procedure can take to be conducted. This time is estimated and sorted into categories of procedures length. It is sorted into procedures that can be done on the spot during the first inspection of the buildung and procedures that need some form of preparation and are better done on a second inspection."@en ;
              rdfs:label "Test duration"@en .


###  http://www.semanticweb.org/georg/ontologies/2022/3/WOOD#Theodolite
:Theodolite rdf:type owl:Class ;
            rdfs:subClassOf :GeometricMeasurements ,
                            [ rdf:type owl:Restriction ;
                              owl:onProperty :HasDegreeOfDestruction ;
                              owl:someValuesFrom :NonDestructiveProcesses
                            ] ,
                            [ rdf:type owl:Restriction ;
                              owl:onProperty :HasTime ;
                              owl:someValuesFrom :SlowProcesses
                            ] ;
            rdfs:comment "A theodolite is an angle measuring instrument used to measure horizontal directions and zenith or vertical angles."@en ;
            rdfs:label "Theodolite"@en .


###  http://www.semanticweb.org/georg/ontologies/2022/3/WOOD#ThermalInsulation
:ThermalInsulation rdf:type owl:Class ;
                   owl:equivalentClass [ rdf:type owl:Restriction ;
                                         owl:onProperty :FindsProperties ;
                                         owl:someValuesFrom :ThermalInsulation
                                       ] ;
                   rdfs:subClassOf :SearchedProperties ;
                   rdfs:comment "Thermal insulation is the reduction of heat transfer between objects in thermal contact or in the area of radiation influence to each other."@en ;
                   rdfs:label "Thermal insulation"@en .


###  http://www.semanticweb.org/georg/ontologies/2022/3/WOOD#Thermography
:Thermography rdf:type owl:Class ;
              rdfs:subClassOf :InvestigationProcedure ,
                              [ rdf:type owl:Restriction ;
                                owl:onProperty :FindsProperties ;
                                owl:someValuesFrom :ThermalInsulation
                              ] ,
                              [ rdf:type owl:Restriction ;
                                owl:onProperty :HasDegreeOfDestruction ;
                                owl:someValuesFrom :NonDestructiveProcesses
                              ] ,
                              [ rdf:type owl:Restriction ;
                                owl:onProperty :HasPlace ;
                                owl:someValuesFrom :InSitu
                              ] ,
                              [ rdf:type owl:Restriction ;
                                owl:onProperty :HasTime ;
                                owl:someValuesFrom :SlowProcesses
                              ] ;
              rdfs:comment "Thermography can be used to record the thermal radiation of an object. This allows conclusions to be drawn about thermal bridges and causes of moisture."@en ;
              rdfs:label "Thermography"@en .


###  http://www.semanticweb.org/georg/ontologies/2022/3/WOOD#ThicknessPlaners
:ThicknessPlaners rdf:type owl:Class ;
                  rdfs:subClassOf :Plane ;
                  rdfs:comment "A thickness planer planes a workpiece to a desired thickness"@en ;
                  rdfs:label "Thickness planer"@en .


###  http://www.semanticweb.org/georg/ontologies/2022/3/WOOD#ThreeandFiveLayerBoards
:ThreeandFiveLayerBoards rdf:type owl:Class ;
                         rdfs:subClassOf :WoodBasedMaterials ;
                         rdfs:comment "The boards consist of three or five layers of boards, which are crossed at right angles, laid on top of each other and glued together. The strength properties have a very wide range. They can be controlled by the quality of the wood used and the thickness ratios of the individual layers."@en ;
                         rdfs:label "Three-/ Five-layer boards"@en .


###  http://www.semanticweb.org/georg/ontologies/2022/3/WOOD#TooHighIceSnowWaterLoads
:TooHighIceSnowWaterLoads rdf:type owl:Class ;
                          rdfs:subClassOf :StaticOverstress ;
                          rdfs:comment "Overstresses on the component that result from not calculated snow or water loads."@en ;
                          rdfs:label "Too high snow and water loads"@en .


###  http://www.semanticweb.org/georg/ontologies/2022/3/WOOD#TooHighLoadsFromDeposition
:TooHighLoadsFromDeposition rdf:type owl:Class ;
                            rdfs:subClassOf :StaticOverstress ;
                            rdfs:comment "Overstresses on the component that result from created deposition. This could occure for example in an salt deposit."@en ;
                            rdfs:label "Too high loads from deposition"@en .


###  http://www.semanticweb.org/georg/ontologies/2022/3/WOOD#Turning
:Turning rdf:type owl:Class ;
         rdfs:subClassOf :Separate ;
         rdfs:comment "Turning is a manufacturing process in which the workpiece is rotated. It is a machining technique"@en ;
         rdfs:label "Turning"@en .


###  http://www.semanticweb.org/georg/ontologies/2022/3/WOOD#UltrasonicEchoMethod
:UltrasonicEchoMethod rdf:type owl:Class ;
                      rdfs:subClassOf :InvestigationProcedure ,
                                      [ rdf:type owl:Restriction ;
                                        owl:onProperty :FindsProperties ;
                                        owl:someValuesFrom :ConcealedComponents
                                      ] ,
                                      [ rdf:type owl:Restriction ;
                                        owl:onProperty :FindsProperties ;
                                        owl:someValuesFrom :EModulus
                                      ] ,
                                      [ rdf:type owl:Restriction ;
                                        owl:onProperty :FindsProperties ;
                                        owl:someValuesFrom :MaterialSolidity
                                      ] ,
                                      [ rdf:type owl:Restriction ;
                                        owl:onProperty :HasDegreeOfDestruction ;
                                        owl:someValuesFrom :NonDestructiveProcesses
                                      ] ,
                                      [ rdf:type owl:Restriction ;
                                        owl:onProperty :HasPlace ;
                                        owl:someValuesFrom :InSitu
                                      ] ,
                                      [ rdf:type owl:Restriction ;
                                        owl:onProperty :HasTime ;
                                        owl:someValuesFrom :SlowProcesses
                                      ] ;
                      rdfs:comment "An ultrasonic pulse is emitted and the speed is determined. To calculate the E-modulus, the bulk density is also required."@en ;
                      rdfs:label "Ultrasonic echo method"@en .


###  http://www.semanticweb.org/georg/ontologies/2022/3/WOOD#Unsolvable
:Unsolvable rdf:type owl:Class ;
            owl:equivalentClass [ rdf:type owl:Restriction ;
                                  owl:onProperty :Removability ;
                                  owl:someValuesFrom :Unsolvable
                                ] ;
            rdfs:subClassOf :Removal ;
            rdfs:comment "The connecting medium can not be detached after use without leaving any permanent traces."@en ;
            rdfs:label "Unsolvable"@en .


###  http://www.semanticweb.org/georg/ontologies/2022/3/WOOD#UsedMethods
:UsedMethods rdf:type owl:Class ;
             rdfs:subClassOf :StepsToTheEvidenceConclusion ;
             rdfs:comment "The equipment used is stated and the execution is described. The site visits are summarized."@en ;
             rdfs:label "Used methods (Pre-note)"@en .


###  http://www.semanticweb.org/georg/ontologies/2022/3/WOOD#VeryHighDimensionalStability
:VeryHighDimensionalStability rdf:type owl:Class ;
                              owl:equivalentClass [ rdf:type owl:Restriction ;
                                                    owl:onProperty :DimensionalStability ;
                                                    owl:someValuesFrom :VeryHighDimensionalStability
                                                  ] ;
                              rdfs:subClassOf :DimensionalStability ;
                              rdfs:comment "The dimensional stability of these wood types are the highest among wood types. These wood types have a very high dimemsional stabilit and will mainain its original dimension when put under pressure."@en ;
                              rdfs:label "Very high dimensional stability"@en .


###  http://www.semanticweb.org/georg/ontologies/2022/3/WOOD#VeryHighInsectResistance
:VeryHighInsectResistance rdf:type owl:Class ;
                          owl:equivalentClass [ rdf:type owl:Restriction ;
                                                owl:onProperty :InsectResistance ;
                                                owl:someValuesFrom :VeryHighInsectResistance
                                              ] ;
                          rdfs:subClassOf :InsectResistance ;
                          rdfs:comment "The insect resistance of these wood types are the highest among wood types. These wood types have a very high insect resistance and insects will not be able to harm these materials."@en ;
                          rdfs:label "Very high insect resistance"@en .


###  http://www.semanticweb.org/georg/ontologies/2022/3/WOOD#VeryHighRotResistance
:VeryHighRotResistance rdf:type owl:Class ;
                       owl:equivalentClass [ rdf:type owl:Restriction ;
                                             owl:onProperty :RotResistance ;
                                             owl:someValuesFrom :VeryHighRotResistance
                                           ] ;
                       rdfs:subClassOf :RotResistance ;
                       rdfs:comment "The rot resistance of these wood types are the highest among wood types. These wood types have a very high rot resistance and rot will not be able to harm these materials."@en ;
                       rdfs:label "Very high rot resistance"@en .


###  http://www.semanticweb.org/georg/ontologies/2022/3/WOOD#VeryLowDimensionalStability
:VeryLowDimensionalStability rdf:type owl:Class ;
                             owl:equivalentClass [ rdf:type owl:Restriction ;
                                                   owl:onProperty :DimensionalStability ;
                                                   owl:someValuesFrom :VeryLowDimensionalStability
                                                 ] ;
                             rdfs:subClassOf :DimensionalStability ;
                             rdfs:comment "The dimensional stability of these wood types are the lowest in comparison to other wood types. When put under pressure these wood types will have drastic movement."@en ;
                             rdfs:label "Very low dimensional stability"@en .


###  http://www.semanticweb.org/georg/ontologies/2022/3/WOOD#VeryLowInsectResistance
:VeryLowInsectResistance rdf:type owl:Class ;
                         owl:equivalentClass [ rdf:type owl:Restriction ;
                                               owl:onProperty :InsectResistance ;
                                               owl:someValuesFrom :VeryLowInsectResistance
                                             ] ;
                         rdfs:subClassOf :InsectResistance ;
                         rdfs:comment "The insect resistance of these wood types are the lowest in comparison to other wood types. These materials will not be able to hinder a insect contamination."@en ;
                         rdfs:label "Very low insect resistance"@en .


###  http://www.semanticweb.org/georg/ontologies/2022/3/WOOD#VeryLowRotResistance
:VeryLowRotResistance rdf:type owl:Class ;
                      owl:equivalentClass [ rdf:type owl:Restriction ;
                                            owl:onProperty :RotResistance ;
                                            owl:someValuesFrom :VeryLowRotResistance
                                          ] ;
                      rdfs:subClassOf :RotResistance ;
                      rdfs:comment "The rot resistance of these wood types are the lowest in comparison to other wood types. These materials will not be able to hinder a rot contamination."@en ;
                      rdfs:label "Very low rot resistance"@en .


###  http://www.semanticweb.org/georg/ontologies/2022/3/WOOD#VibrationsAndOscillations
:VibrationsAndOscillations rdf:type owl:Class ;
                           rdfs:subClassOf :DynamicOverstress ,
                                           [ rdf:type owl:Restriction ;
                                             owl:onProperty :CanCreateDamage ;
                                             owl:someValuesFrom :Cracks
                                           ] ,
                                           [ rdf:type owl:Restriction ;
                                             owl:onProperty :CanCreateDamage ;
                                             owl:someValuesFrom :Delocalization
                                           ] ;
                           rdfs:comment "Vibrations from usage or natural disasters can cause cracks, delocalizations and fastener failures."@en ;
                           rdfs:label "Vibrations/ Oscillations"@en .


###  http://www.semanticweb.org/georg/ontologies/2022/3/WOOD#WashoutStresses
:WashoutStresses rdf:type owl:Class ;
                 owl:equivalentClass [ rdf:type owl:Restriction ;
                                       owl:onProperty :CanCreateDamage ;
                                       owl:someValuesFrom :WashoutStresses
                                     ] ;
                 rdfs:subClassOf :ChemicalProcesses ;
                 rdfs:comment "In the case of wooden components with direct rainfall, the wood's natural adhesive, lignin, is gradually washed out of the pores. This weakens the wood and it is more susceptible to damage from UV radiation and insects that can penetrate into the interior of the wood."@en ;
                 rdfs:label "Washout stresses"@en .


###  http://www.semanticweb.org/georg/ontologies/2022/3/WOOD#Wax
:Wax rdf:type owl:Class ;
     rdfs:subClassOf :CoatTools ,
                     [ rdf:type owl:Restriction ;
                       owl:onProperty :WoodColour ;
                       owl:someValuesFrom :ColourEmphasized
                     ] ,
                     [ rdf:type owl:Restriction ;
                       owl:onProperty :WoodGrain ;
                       owl:someValuesFrom :GrainEmphasized
                     ] ;
     rdfs:comment "Waxing is the treatment of the surface with wax. The wood grain and color is emphasized"@en ;
     rdfs:label "Wax"@en .


###  http://www.semanticweb.org/georg/ontologies/2022/3/WOOD#WesternHemlockHEM
:WesternHemlockHEM rdf:type owl:Class ;
                   rdfs:subClassOf :Softwood ,
                                   [ rdf:type owl:Restriction ;
                                     owl:onProperty :DimensionalStability ;
                                     owl:someValuesFrom :HighDimensionalStability
                                   ] ,
                                   [ rdf:type owl:Restriction ;
                                     owl:onProperty :InsectResistance ;
                                     owl:someValuesFrom :LowInsectResistance
                                   ] ,
                                   [ rdf:type owl:Restriction ;
                                     owl:onProperty :RotResistance ;
                                     owl:someValuesFrom :LowRotResistance
                                   ] ,
                                   [ rdf:type owl:Restriction ;
                                     owl:onProperty :RotResistance ;
                                     owl:someValuesFrom :MediumRotResistance
                                   ] ;
                   rdfs:comment """Wood material of western hemlock trees.

Colour:
Early wood light brownish grey, occasionally lighter stripes, late wood somewhat darkens with time, sapwood and heartwood is not distinguished."""@en ;
                   rdfs:label "Western hemlock (HEM)"@en .


###  http://www.semanticweb.org/georg/ontologies/2022/3/WOOD#WesternRedcedarRCW
:WesternRedcedarRCW rdf:type owl:Class ;
                    rdfs:subClassOf :Softwood ,
                                    [ rdf:type owl:Restriction ;
                                      owl:onProperty :DimensionalStability ;
                                      owl:someValuesFrom :VeryHighDimensionalStability
                                    ] ,
                                    [ rdf:type owl:Restriction ;
                                      owl:onProperty :InsectResistance ;
                                      owl:someValuesFrom :VeryHighInsectResistance
                                    ] ,
                                    [ rdf:type owl:Restriction ;
                                      owl:onProperty :RotResistance ;
                                      owl:someValuesFrom :VeryHighRotResistance
                                    ] ;
                    rdfs:comment """Wood material of western redcedar trees.

Colour:
White/ reddish brown, darkens with time, late wood darker"""@en ;
                    rdfs:label "Western redcedar (RCW)"@en .


###  http://www.semanticweb.org/georg/ontologies/2022/3/WOOD#WetRotFungi
:WetRotFungi rdf:type owl:Class ;
             rdfs:subClassOf :WoodDestroyingFungi ;
             rdfs:comment "Wet rot fungi require a relatively high level of wood moisture to grow. If the wood moisture is lacking, growth will temporarily cease."@en ;
             rdfs:label "Wet rot fungi"@en .


###  http://www.semanticweb.org/georg/ontologies/2022/3/WOOD#WhitePoreSponge
:WhitePoreSponge rdf:type owl:Class ;
                 rdfs:subClassOf :WetRotFungi ,
                                 [ rdf:type owl:Restriction ;
                                   owl:onProperty :RotDecompositionType ;
                                   owl:someValuesFrom :BrownRot
                                 ] ;
                 rdfs:comment """Preferred wood species:
Softwood and hardwood

Optimal living conditions of wood moisture content in M-%:
35% to 50%

Optimal living conditions of the temperature range in °C:
25°C to 31°C

Additional notes:
Long dry rigidity possible."""@en ;
                 rdfs:label "Poria vaillantii"@la ,
                            "White pore sponge"@en .


###  http://www.semanticweb.org/georg/ontologies/2022/3/WOOD#WhiteRot
:WhiteRot rdf:type owl:Class ;
          owl:equivalentClass [ rdf:type owl:Restriction ;
                                owl:onProperty :RotDecompositionType ;
                                owl:someValuesFrom :WhiteRot
                              ] ;
          rdfs:subClassOf :WoodDestroyingFungi ;
          rdfs:comment "White rot, wood structure is destroyed by degradation of the lignin"@en ;
          rdfs:label "White rot"@en .


###  http://www.semanticweb.org/georg/ontologies/2022/3/WOOD#WindLoads
:WindLoads rdf:type owl:Class ;
           rdfs:subClassOf :DynamicOverstress ,
                           [ rdf:type owl:Restriction ;
                             owl:onProperty :CanCreateDamage ;
                             owl:someValuesFrom :Cracks
                           ] ,
                           [ rdf:type owl:Restriction ;
                             owl:onProperty :CanCreateDamage ;
                             owl:someValuesFrom :Deflection
                           ] ,
                           [ rdf:type owl:Restriction ;
                             owl:onProperty :CanCreateDamage ;
                             owl:someValuesFrom :Delocalization
                           ] ,
                           [ rdf:type owl:Restriction ;
                             owl:onProperty :CanCreateDamage ;
                             owl:someValuesFrom :Fractures
                           ] ,
                           [ rdf:type owl:Restriction ;
                             owl:onProperty :CanCreateDamage ;
                             owl:someValuesFrom :Holes
                           ] ;
           rdfs:comment "Extreme wind conditions that were not planned for and lead to failure of the component."@en ;
           rdfs:label "Wind loads"@en .


###  http://www.semanticweb.org/georg/ontologies/2022/3/WOOD#WoodAge
:WoodAge rdf:type owl:Class ;
         owl:equivalentClass [ rdf:type owl:Restriction ;
                               owl:onProperty :FindsProperties ;
                               owl:someValuesFrom :WoodAge
                             ] ;
         rdfs:subClassOf :SearchedProperties .


###  http://www.semanticweb.org/georg/ontologies/2022/3/WOOD#WoodBasedMaterials
:WoodBasedMaterials rdf:type owl:Class ;
                    rdfs:subClassOf :ConstructionWood ;
                    rdfs:comment "Wood based materials are pressed from shredded wood or sticks. To create wood based materials the splint can be used, but also waste products of wood production is often used. The industry offers a large number of wood-based materials that are optimised for their specific use in constructions."@en ;
                    rdfs:label "Wood based materials"@en .


###  http://www.semanticweb.org/georg/ontologies/2022/3/WOOD#WoodComponent
:WoodComponent rdf:type owl:Class ;
               rdfs:comment "List of essential properties of wooden components."@en ;
               rdfs:label "Wood component"@en .


###  http://www.semanticweb.org/georg/ontologies/2022/3/WOOD#WoodDamage
:WoodDamage rdf:type owl:Class ;
            rdfs:subClassOf <https://w3id.org/dot#ClassifiedDamage> ;
            rdfs:comment "Damages in wooden components."@en ;
            rdfs:label "Wood damages"@en .


###  http://www.semanticweb.org/georg/ontologies/2022/3/WOOD#WoodDestroyingFungi
:WoodDestroyingFungi rdf:type owl:Class ;
                     rdfs:subClassOf :Rot ;
                     owl:disjointWith :WoodDiscoloringFungi ;
                     rdfs:comment "The wood-destroying fungi present in the buildings break down cell walls and cause rot in this way. Brown rot is particularly dangerous; with increasing wood destruction, the wood becomes longitudinally and transversely cracked and gradually takes on a brown color. The remaining substance decays to a powder."@en ;
                     rdfs:label "Wood destroying fungi"@en .


###  http://www.semanticweb.org/georg/ontologies/2022/3/WOOD#WoodDiscoloringFungi
:WoodDiscoloringFungi rdf:type owl:Class ;
                      rdfs:subClassOf :Rot ;
                      rdfs:comment "Wood staining fungi do not affect the strength of the wood, but stain the wood and can endanger the health of the occupants. The stain may result in a reduction in the value of timber or timber products."@en ;
                      rdfs:label "Wood discoloring fungi"@en .


###  http://www.semanticweb.org/georg/ontologies/2022/3/WOOD#WoodFiberBoards
:WoodFiberBoards rdf:type owl:Class ;
                 rdfs:subClassOf :WoodBasedMaterials ;
                 rdfs:comment "Wood fiberboards are produced using the dry process with binders or in the wet process without binders by strong pressing. The bonding is based on the felting of the fibers and their own bonding ability."@en ;
                 rdfs:label "Wood fiber boards"@en .


###  http://www.semanticweb.org/georg/ontologies/2022/3/WOOD#WoodFiberInsulationBoards
:WoodFiberInsulationBoards rdf:type owl:Class ;
                           rdfs:subClassOf :WoodBasedMaterials ;
                           rdfs:comment "Wood fiber insulation boards are made in a wet process from wood fibers. They have a higher insulation factor than regular wood fiber boards. The bond is based on the felting of the fibers as well as their own bonding ability. The gross density is max. 400 kg/m."@en ;
                           rdfs:label "Wood fiber insulation boards"@en .


###  http://www.semanticweb.org/georg/ontologies/2022/3/WOOD#WoodMoisture
:WoodMoisture rdf:type owl:Class ;
              owl:equivalentClass [ rdf:type owl:Restriction ;
                                    owl:onProperty :FindsProperties ;
                                    owl:someValuesFrom :WoodMoisture
                                  ] ;
              rdfs:subClassOf :SearchedProperties .


###  http://www.semanticweb.org/georg/ontologies/2022/3/WOOD#WoodPreservative
:WoodPreservative rdf:type owl:Class ;
                  rdfs:subClassOf :PropertiesChange ;
                  rdfs:comment "Wood preservatives are intended to prevent infestation of wood or wood-based materials by wood-destroying organisms or to combat such infestation"@en ;
                  rdfs:label "Wood preservative"@en .


###  http://www.semanticweb.org/georg/ontologies/2022/3/WOOD#WoodSpecies
:WoodSpecies rdf:type owl:Class ;
             owl:equivalentClass [ rdf:type owl:Restriction ;
                                   owl:onProperty :FindsProperties ;
                                   owl:someValuesFrom :WoodSpecies
                                 ] ;
             rdfs:subClassOf :SearchedProperties ;
             rdfs:comment "Wood species is subcategories of wood that have Characteristic Distinctions."@en ;
             rdfs:label "Wood species"@en .


###  http://www.semanticweb.org/georg/ontologies/2022/3/WOOD#WoodTypes
:WoodTypes rdf:type owl:Class ;
           rdfs:subClassOf :WoodComponent ;
           rdfs:comment "Wood species used as a building material. Abbreviation according to DIN 4076"@en ;
           rdfs:label "Wood types"@en .


###  http://www.semanticweb.org/georg/ontologies/2022/3/WOOD#WoodWoolLightweightPanels
:WoodWoolLightweightPanels rdf:type owl:Class ;
                           rdfs:subClassOf :WoodBasedMaterials ;
                           rdfs:comment "Wood wool lightweight boards are made from wood wool and mineral binders such as cement."@en ;
                           rdfs:label "Wood wool lightweight panels"@en .


###  http://www.semanticweb.org/georg/ontologies/2022/3/WOOD#Worker
:Worker rdf:type owl:Class ;
        rdfs:subClassOf <http://xmlns.com/foaf/0.1/Person> ;
        rdfs:comment "A worker is a person who has a salaried employment."@en ;
        rdfs:label "Worker"@en .


###  http://www.semanticweb.org/georg/ontologies/2022/3/WOOD#XRays
:XRays rdf:type owl:Class ;
       rdfs:subClassOf :InvestigationProcedure ,
                       [ rdf:type owl:Restriction ;
                         owl:onProperty :FindsProperties ;
                         owl:someValuesFrom :ConcealedComponents
                       ] ,
                       [ rdf:type owl:Restriction ;
                         owl:onProperty :FindsProperties ;
                         owl:someValuesFrom :MaterialSolidity
                       ] ,
                       [ rdf:type owl:Restriction ;
                         owl:onProperty :FindsProperties ;
                         owl:someValuesFrom :MetalComponents
                       ] ,
                       [ rdf:type owl:Restriction ;
                         owl:onProperty :HasDegreeOfDestruction ;
                         owl:someValuesFrom :NonDestructiveProcesses
                       ] ,
                       [ rdf:type owl:Restriction ;
                         owl:onProperty :HasPlace ;
                         owl:someValuesFrom :InSitu
                       ] ,
                       [ rdf:type owl:Restriction ;
                         owl:onProperty :HasTime ;
                         owl:someValuesFrom :SlowProcesses
                       ] ;
       rdfs:comment "The X-ray method can be used to obtain images of the internal wood structure and joints. An in-situ application is possible with appropriate equipment."@en ;
       rdfs:label "X-rays"@en .


###  http://www.semanticweb.org/georg/ontologies/2022/3/WOOD#hygrometer
:hygrometer rdf:type owl:Class ;
            rdfs:subClassOf :InvestigationProcedure ,
                            [ rdf:type owl:Restriction ;
                              owl:onProperty :FindsProperties ;
                              owl:someValuesFrom :AirHumidity
                            ] ,
                            [ rdf:type owl:Restriction ;
                              owl:onProperty :HasDegreeOfDestruction ;
                              owl:someValuesFrom :NonDestructiveProcesses
                            ] ,
                            [ rdf:type owl:Restriction ;
                              owl:onProperty :HasPlace ;
                              owl:someValuesFrom :InSitu
                            ] ,
                            [ rdf:type owl:Restriction ;
                              owl:onProperty :HasTime ;
                              owl:someValuesFrom :SlowProcesses
                            ] ;
            rdfs:comment "A hygrometer is a measuring instrument for determining the relative humidity of the air."@en ;
            rdfs:label "Hygrometer"@en .


###  http://www.semanticweb.org/georg/ontologies/2022/3/WOOD#insectIdentification
:insectIdentification rdf:type owl:Class ;
                      rdfs:subClassOf :InvestigationProcedure ,
                                      [ rdf:type owl:Restriction ;
                                        owl:onProperty :FindsProperties ;
                                        owl:someValuesFrom :InsectContamination
                                      ] ,
                                      [ rdf:type owl:Restriction ;
                                        owl:onProperty :HasDegreeOfDestruction ;
                                        owl:someValuesFrom :LowDestructiveProcesses
                                      ] ,
                                      [ rdf:type owl:Restriction ;
                                        owl:onProperty :HasPlace ;
                                        owl:someValuesFrom :InSitu
                                      ] ,
                                      [ rdf:type owl:Restriction ;
                                        owl:onProperty :HasPlace ;
                                        owl:someValuesFrom :Laboratory
                                      ] ,
                                      [ rdf:type owl:Restriction ;
                                        owl:onProperty :HasTime ;
                                        owl:someValuesFrom :SlowProcesses
                                      ] ;
                      rdfs:comment "The identification of the type of insect contamination can be done by examining the insects found. This is only possible in case of an active infestation."@en ;
                      rdfs:label "Insect identification"@en .


###  http://www.semanticweb.org/georg/ontologies/2022/3/WOOD#mechanicalInfluences
:mechanicalInfluences rdf:type owl:Class ;
                      rdfs:subClassOf :CauseOfDamage ;
                      rdfs:comment "Influences with a mechanical force."@en ;
                      rdfs:label "Mechanical influences"@en .


###  http://www.semanticweb.org/georg/ontologies/2022/3/WOOD#millingMachine
:millingMachine rdf:type owl:Class ;
                rdfs:subClassOf :Milling ;
                rdfs:comment "A milling machine removes material from a workpiece by cutting it into the desired shape using rotating cutting tools"@en ;
                rdfs:label "Milling machine"@en .


###  http://www.semanticweb.org/georg/ontologies/2022/3/WOOD#3DLaserScanning
<http://www.semanticweb.org/georg/ontologies/2022/3/WOOD#3DLaserScanning> rdf:type owl:Class ;
                                                                          rdfs:subClassOf :GeometricMeasurements ,
                                                                                          [ rdf:type owl:Restriction ;
                                                                                            owl:onProperty :HasDegreeOfDestruction ;
                                                                                            owl:someValuesFrom :NonDestructiveProcesses
                                                                                          ] ,
                                                                                          [ rdf:type owl:Restriction ;
                                                                                            owl:onProperty :HasTime ;
                                                                                            owl:someValuesFrom :SlowProcesses
                                                                                          ] ;
                                                                          rdfs:comment "Laser scanning refers to the line or grid-like sweeping of a body with a laser beam in order to measure it or to generate  an 3D image."@en ;
                                                                          rdfs:label "3D laser scanning"@en .


###  http://xmlns.com/foaf/0.1/Person
<http://xmlns.com/foaf/0.1/Person> rdf:type owl:Class .


###  https://w3id.org/bot#Building
<https://w3id.org/bot#Building> rdf:type owl:Class ;
                                rdfs:subClassOf :Report .


###  https://w3id.org/dot#ClassifiedDamage
<https://w3id.org/dot#ClassifiedDamage> rdf:type owl:Class ;
                                        rdfs:isDefinedBy <https://w3id.org/dot#> ;
                                        rdfs:label "Classified Damage"@en .


#################################################################
#    Individuals
#################################################################

###  http://www.semanticweb.org/christian/ontologies/2021/4/untitled-ontology-14#BuildingOwner1
<http://www.semanticweb.org/christian/ontologies/2021/4/untitled-ontology-14#BuildingOwner1> rdf:type owl:NamedIndividual ,
                                                                                                      :BuildingOwner .


###  http://www.semanticweb.org/georg/ontologies/2022/3/WOOD#Building001
:Building001 rdf:type owl:NamedIndividual ;
             :HasText :Report001 ;
             :BuildingDate "2022-01-01T00:00:00"^^xsd:dateTime ;
             :ConstructionMethod "Timbered house" ;
             :HadRenovation "false"^^xsd:boolean ;
             :MonumentProtection "false"^^xsd:boolean ;
             :Utilization "Residential Building" .


###  http://www.semanticweb.org/georg/ontologies/2022/3/WOOD#Cause001
:Cause001 rdf:type owl:NamedIndividual ,
                   :CauseOfDamage ;
          :CauseRepaired "false"^^xsd:boolean .


###  http://www.semanticweb.org/georg/ontologies/2022/3/WOOD#Client001
:Client001 rdf:type owl:NamedIndividual ,
                    :Client ;
           :Contracts :Expert001 .


###  http://www.semanticweb.org/georg/ontologies/2022/3/WOOD#Company001
:Company001 rdf:type owl:NamedIndividual .


###  http://www.semanticweb.org/georg/ontologies/2022/3/WOOD#Damage001
:Damage001 rdf:type owl:NamedIndividual ,
                    :WoodDamage ;
           :DamageRepaired "false"^^xsd:boolean .


###  http://www.semanticweb.org/georg/ontologies/2022/3/WOOD#Damage002
:Damage002 rdf:type owl:NamedIndividual ,
                    :Rot ;
           :IsLocatedIn :WoodComponent001 .


###  http://www.semanticweb.org/georg/ontologies/2022/3/WOOD#Expert001
:Expert001 rdf:type owl:NamedIndividual ,
                    :BuildingDamageExpert .


###  http://www.semanticweb.org/georg/ontologies/2022/3/WOOD#Procedure1
:Procedure1 rdf:type owl:NamedIndividual ,
                     :StepsToTheEvidenceConclusion .


###  http://www.semanticweb.org/georg/ontologies/2022/3/WOOD#Procedures001
:Procedures001 rdf:type owl:NamedIndividual ,
                        :Investigation .


###  http://www.semanticweb.org/georg/ontologies/2022/3/WOOD#Repair001
:Repair001 rdf:type owl:NamedIndividual ,
                    :Chainsaws .


###  http://www.semanticweb.org/georg/ontologies/2022/3/WOOD#Report001
:Report001 rdf:type owl:NamedIndividual ,
                    :Report ;
           :Includes :WoodComponent001 ;
           :DateOfInspection "2022-01-01T00:00:00"^^xsd:dateTime ;
           :DateOfSurvey "2022-01-01T00:00:00"^^xsd:dateTime .


###  http://www.semanticweb.org/georg/ontologies/2022/3/WOOD#WoodComponent001
:WoodComponent001 rdf:type owl:NamedIndividual ,
                           :WoodComponent ;
                  :ContainsDamage :Cause001 ,
                                  :Damage002 ;
                  :AdjacentHumidity "70"^^xsd:int ;
                  :Condensation "false"^^xsd:boolean ;
                  :GroundContact "false"^^xsd:boolean ;
                  :Temperature "20"^^xsd:int ;
                  :Weather "false"^^xsd:boolean ;
                  :WoodMoisture "18"^^xsd:int .


###  http://www.semanticweb.org/georg/ontologies/2022/3/WOOD#Worker001
:Worker001 rdf:type owl:NamedIndividual ,
                    :Worker .


#################################################################
#    Annotations
#################################################################

:BulkDensity rdfs:comment "Bulk density is the density of a porous solid, based on the volume including the pore spaces."@en ;
             rdfs:label "Bulk Density"@en ,
                        "Bulk density"@en .


:Contracts rdfs:comment "A contract is a legal agreement between two or more partners."@en ;
           rdfs:label "Contracts"@en .


:DimensionalStability rdfs:comment "Dimensional stability is the ability of a material to maintain its original dimensions when subjected to varying degrees of temperature, moisture, pressure, or other stress."@en ;
                      rdfs:label "Dimensional Stability"@en .


:InsectResistance rdfs:comment "Incest resistance is the ability of a material to naturally hinder insects to destroy its substance."@en ;
                  rdfs:label "Insect Resistance"@en ,
                             "Insect resistance"@en .


:RotResistance rdfs:comment "Rot resistance is the ability of a material to stop rot contamination."@en ;
               rdfs:label "Rot Resistance"@en ,
                          "Rot resistance"@en .


:WoodAge rdfs:comment "Age of the wood determined by appropriate examination procedures."@en ;
         rdfs:label "Wood Age"@en ,
                    "Wood age"@en .


:WoodMoisture rdfs:comment "Wood moisture indicates the degree of presence of water in or on a wooden component."@en ;
              rdfs:label "Wood Moisture"@en ,
                         "Wood moisture"@en .


#################################################################
#    General axioms
#################################################################

[ rdf:type owl:AllDisjointClasses ;
  owl:members ( :AaRdT
                :Norm
                :Regulations
                :TechnicalLiterature
              )
] .


[ rdf:type owl:AllDisjointClasses ;
  owl:members ( :AzobeAZO
                :BeechBU
                :MapleAH
                :MerantiDarkRedMER
                :MerbauMEB
                :OakEI
                :RobiniaROB
                :TeakTEK
              )
] .


[ rdf:type owl:AllDisjointClasses ;
  owl:members ( :BandSaws
                :Chainsaws
                :CircularSaws
                :FrameSaws
                :Handsaw
              )
] .


[ rdf:type owl:AllDisjointClasses ;
  owl:members ( :BeamLeafling
                :FenceLeaflet
                :FirLeafBlossom
                :ScalySawfly
              )
] .


[ rdf:type owl:AllDisjointClasses ;
  owl:members ( :BiologicalInfluences
                :ChemicalInfluences
                :MoisturePenetration
                :mechanicalInfluences
              )
] .


[ rdf:type owl:AllDisjointClasses ;
  owl:members ( :BrownCellarSponge
                :ButterflySpore
                :Leaflet
                :MusselCrempling
                :OakWhorling
                :WhitePoreSponge
              )
] .


[ rdf:type owl:AllDisjointClasses ;
  owl:members ( :BuildingOwner
                :Client
                :Worker
              )
] .


[ rdf:type owl:AllDisjointClasses ;
  owl:members ( :BuildingTimber
                :CrossBeams
                :DuoTrioBeams
                :GluedLaminatedTimber
                :ProfileBoards
                :Roundwood
                :SolidStructuralTimber
              )
] .


[ rdf:type owl:AllDisjointClasses ;
  owl:members ( :CementFiberBoards
                :Chipboard
                :ConstructionVeneerPlywood
                :FlatPressedBoard
                :GypsumFiberboards
                :LaminatedVeneerLumber
                :ThreeandFiveLayerBoards
                :WoodFiberBoards
                :WoodFiberInsulationBoards
                :WoodWoolLightweightPanels
              )
] .


[ rdf:type owl:AllDisjointClasses ;
  owl:members ( :Clamps
                :Glue
                :Nailing
                :Screws
                :Tenon
              )
] .


[ rdf:type owl:AllDisjointClasses ;
  owl:members ( :Coat
                :Join
                :PropertiesChange
                :Separate
              )
] .


[ rdf:type owl:AllDisjointClasses ;
  owl:members ( :Costs
                :Evaluation
                :LocalFindings
                :Restoration
                :Source
                :UsedMethods
              )
] .


[ rdf:type owl:AllDisjointClasses ;
  owl:members ( :DouglasFirDGA
                :FirTA
                :LarchEuropeanLA
                :PineKI
                :PinePIP
                :SpruceFI
                :WesternHemlockHEM
                :WesternRedcedarRCW
              )
] .


[ rdf:type owl:AllDisjointClasses ;
  owl:members ( :DynamicOverstress
                :ServiceStresses
                :StaticOverstress
              )
] .


[ rdf:type owl:AllDisjointClasses ;
  owl:members ( :ExcessiveLoadsFromConstructionOrUsage
                :InsufficientBeamDimensions
                :TooHighIceSnowWaterLoads
                :TooHighLoadsFromDeposition
              )
] .


[ rdf:type owl:AllDisjointClasses ;
  owl:members ( :ExplosionAndSonicBoom
                :Shocks
                :VibrationsAndOscillations
                :WindLoads
              )
] .


[ rdf:type owl:AllDisjointClasses ;
  owl:members ( :FireproofingPaint
                :Fumigant
                :WoodPreservative
              )
] .


[ rdf:type owl:AllDisjointClasses ;
  owl:members ( :FoldingRule
                :LaserMeasuringDevice
                :MeasuringTape
                :Photogrammetry
                :Theodolite
                <http://www.semanticweb.org/georg/ontologies/2022/3/WOOD#3DLaserScanning>
              )
] .


[ rdf:type owl:AllDisjointClasses ;
  owl:members ( :ForceFit
                :FormFitting
                :MeltLocking
              )
] .


[ rdf:type owl:AllDisjointClasses ;
  owl:members ( :GK1
                :GK2
                :GK4
                :GK5
                :Gk3.1
                :Gk3.2
              )
] .


[ rdf:type owl:AllDisjointClasses ;
  owl:members ( :Glaze
                :Laminate
                :Oil
                :Stain
                :Wax
              )
] .


[ rdf:type owl:AllDisjointClasses ;
  owl:members ( :GrainConcealed
                :GrainEmphasized
                :GrainRemainsVisible
              )
] .


###  Generated by the OWL API (version 5.1.18) https://github.com/owlcs/owlapi/
