@prefix : <http://www.semanticweb.org/wood#> .
@prefix owl: <http://www.w3.org/2002/07/owl#> .
@prefix rdf: <http://www.w3.org/1999/02/22-rdf-syntax-ns#> .
@prefix xml: <http://www.w3.org/XML/1998/namespace> .
@prefix xsd: <http://www.w3.org/2001/XMLSchema#> .
@prefix rdfs: <http://www.w3.org/2000/01/rdf-schema#> .
@base <http://www.semanticweb.org/wood#> .

<http://www.semanticweb.org/wood> rdf:type owl:Ontology ;
                                   <http://purl.org/dc/terms/created> "19.08.2022"@en ;
                                   <http://purl.org/dc/terms/creator> "Georg Vinkeloe"@en ;
                                   <http://purl.org/dc/terms/description> "The \"Wood Damage Ontology\" helps to define and document wood damages in construction. Wood damage experts can use this ontology for writing reports. It focuses on wood components and can be used in all areas of structural damage where wood has been installed. It is an extension of the Damage Topology Ontology (dot) and falls under the category of classified damage. It defines damage types, associated causes, repair methods and investigation procedures. All these categories are part of the report. In the ontology, these categories are defined and have connections to each other."@en ;
                                   <http://purl.org/dc/terms/license> "https://creativecommons.org/licenses/by/2.0/"@en ;
                                   <http://purl.org/dc/terms/title> "Wood Damage Ontology"@en ;
                                   <http://purl.org/vocab/vann/preferredNamespacePrefix> "wood"@en ;
                                   <http://purl.org/vocab/vann/preferredNamespaceUri> "http://www.semanticweb.org/wood"@en .

#################################################################
#    Annotation properties
#################################################################

###  http://purl.org/dc/terms/created
<http://purl.org/dc/terms/created> rdf:type owl:AnnotationProperty .


###  http://purl.org/dc/terms/creator
<http://purl.org/dc/terms/creator> rdf:type owl:AnnotationProperty .


###  http://purl.org/dc/terms/description
<http://purl.org/dc/terms/description> rdf:type owl:AnnotationProperty .


###  http://purl.org/dc/terms/license
<http://purl.org/dc/terms/license> rdf:type owl:AnnotationProperty .


###  http://purl.org/dc/terms/title
<http://purl.org/dc/terms/title> rdf:type owl:AnnotationProperty .


###  http://purl.org/vocab/vann/preferredNamespacePrefix
<http://purl.org/vocab/vann/preferredNamespacePrefix> rdf:type owl:AnnotationProperty .


###  http://purl.org/vocab/vann/preferredNamespaceUri
<http://purl.org/vocab/vann/preferredNamespaceUri> rdf:type owl:AnnotationProperty .


###  http://swrl.stanford.edu/ontologies/3.3/swrla.owl#isRuleEnabled
<http://swrl.stanford.edu/ontologies/3.3/swrla.owl#isRuleEnabled> rdf:type owl:AnnotationProperty .


#################################################################
#    Object Properties
#################################################################

###  http://www.semanticweb.org/wood#ChangesProperties
:ChangesProperties rdf:type owl:ObjectProperty ;
                   rdfs:subPropertyOf owl:topObjectProperty ;
                   rdf:type owl:AsymmetricProperty ,
                            owl:IrreflexiveProperty ;
                   rdfs:domain :CauseOfDamage ;
                   rdfs:range :SearchedProperties ;
                   rdfs:label "Changes Properties"@en .


###  http://www.semanticweb.org/wood#ContainsDamage
:ContainsDamage rdf:type owl:ObjectProperty ;
                rdfs:subPropertyOf owl:topObjectProperty ;
                rdf:type owl:AsymmetricProperty ,
                         owl:IrreflexiveProperty ;
                rdfs:domain :WoodComponent ;
                rdfs:range :WoodDamage ;
                rdfs:label "Contains Damage"@en .


###  http://www.semanticweb.org/wood#Contracts
:Contracts rdf:type owl:ObjectProperty ;
           rdfs:subPropertyOf owl:topObjectProperty ;
           owl:inverseOf :IsContracted ;
           rdf:type owl:AsymmetricProperty ,
                    owl:IrreflexiveProperty ;
           rdfs:domain :Client ;
           rdfs:range :BuildingDamageExpert .


###  http://www.semanticweb.org/wood#CreatedByCause
:CreatedByCause rdf:type owl:ObjectProperty ;
                rdfs:subPropertyOf owl:topObjectProperty ;
                rdf:type owl:AsymmetricProperty ,
                         owl:IrreflexiveProperty ;
                rdfs:domain :WoodDamage ;
                rdfs:range :CauseOfDamage ;
                rdfs:label "Created By Cause"@en .


###  http://www.semanticweb.org/wood#Executes
:Executes rdf:type owl:ObjectProperty ;
          rdfs:subPropertyOf owl:topObjectProperty ;
          owl:inverseOf :IsWorkedOnBy ;
          rdf:type owl:AsymmetricProperty ,
                   owl:IrreflexiveProperty ;
          rdfs:domain :Worker ;
          rdfs:range :RepairProcedure ;
          rdfs:label "Executes"@en .


###  http://www.semanticweb.org/wood#GivesInstruction
:GivesInstruction rdf:type owl:ObjectProperty ;
                  rdfs:subPropertyOf owl:topObjectProperty ;
                  owl:inverseOf :ReceivesInstructions ;
                  rdf:type owl:AsymmetricProperty ,
                           owl:IrreflexiveProperty ;
                  rdfs:domain :BuildingDamageExpert ;
                  rdfs:range :Worker ;
                  rdfs:label "Gives Instruction"@en .


###  http://www.semanticweb.org/wood#IsContracted
:IsContracted rdf:type owl:ObjectProperty ;
              rdfs:subPropertyOf owl:topObjectProperty ;
              rdf:type owl:AsymmetricProperty ,
                       owl:IrreflexiveProperty ;
              rdfs:domain :BuildingDamageExpert ;
              rdfs:range :Client ;
              rdfs:label "Is Contracted"@en .


###  http://www.semanticweb.org/wood#IsWorkedOnBy
:IsWorkedOnBy rdf:type owl:ObjectProperty ;
              rdfs:subPropertyOf owl:topObjectProperty ;
              rdf:type owl:AsymmetricProperty ,
                       owl:IrreflexiveProperty ;
              rdfs:domain :RepairProcedure ;
              rdfs:range :Worker ;
              rdfs:label "Is Worked On By"@en .


###  http://www.semanticweb.org/wood#IsWrittenBy
:IsWrittenBy rdf:type owl:ObjectProperty ;
             rdfs:subPropertyOf owl:topObjectProperty ;
             owl:inverseOf :Writes ;
             rdf:type owl:AsymmetricProperty ,
                      owl:IrreflexiveProperty ;
             rdfs:domain :Report ;
             rdfs:range :BuildingDamageExpert ;
             rdfs:label "Is Written By"@en .


###  http://www.semanticweb.org/wood#NeedsInvestigationProcedure
:NeedsInvestigationProcedure rdf:type owl:ObjectProperty ;
                             rdfs:subPropertyOf owl:topObjectProperty ;
                             rdf:type owl:IrreflexiveProperty ;
                             rdfs:domain :InvestigationProcedure ;
                             rdfs:range :SearchedProperties ;
                             rdfs:label "Needs Investigation Procedure"@en .


###  http://www.semanticweb.org/wood#NeedsRepairMethod
:NeedsRepairMethod rdf:type owl:ObjectProperty ;
                   rdfs:subPropertyOf owl:topObjectProperty ;
                   rdf:type owl:AsymmetricProperty ,
                            owl:IrreflexiveProperty ;
                   rdfs:domain :WoodDamage ;
                   rdfs:range :RepairProcedure ;
                   rdfs:label "Needs Repair Method"@en .


###  http://www.semanticweb.org/wood#PartOfCause
:PartOfCause rdf:type owl:ObjectProperty ;
             rdfs:subPropertyOf owl:topObjectProperty ;
             rdf:type owl:InverseFunctionalProperty ,
                      owl:AsymmetricProperty ,
                      owl:IrreflexiveProperty ;
             rdfs:domain :Cause ;
             rdfs:range :WoodDamage ;
             rdfs:label "Part Of Cause"@en .


###  http://www.semanticweb.org/wood#PartOfCost
:PartOfCost rdf:type owl:ObjectProperty ;
            rdfs:subPropertyOf owl:topObjectProperty ;
            rdf:type owl:InverseFunctionalProperty ,
                     owl:AsymmetricProperty ,
                     owl:IrreflexiveProperty ;
            rdfs:domain :Costs ;
            rdfs:range :CostOfRestoration ;
            rdfs:label "Part Of Cost"@en .


###  http://www.semanticweb.org/wood#PartOfEvaluation
:PartOfEvaluation rdf:type owl:ObjectProperty ;
                  rdfs:subPropertyOf owl:topObjectProperty ;
                  rdf:type owl:InverseFunctionalProperty ,
                           owl:AsymmetricProperty ,
                           owl:IrreflexiveProperty ;
                  rdfs:domain :Evaluation ;
                  rdfs:range :CauseOfDamage ;
                  rdfs:label "Part Of Evaluation"@en .


###  http://www.semanticweb.org/wood#PartOfFindings
:PartOfFindings rdf:type owl:ObjectProperty ;
                rdfs:subPropertyOf owl:topObjectProperty ;
                rdf:type owl:InverseFunctionalProperty ,
                         owl:AsymmetricProperty ,
                         owl:IrreflexiveProperty ;
                rdfs:domain :LocalFindings ;
                rdfs:range :WoodComponent ;
                rdfs:label "Part Of Findings"@en .


###  http://www.semanticweb.org/wood#PartOfRestoration
:PartOfRestoration rdf:type owl:ObjectProperty ;
                   rdfs:subPropertyOf owl:topObjectProperty ;
                   rdf:type owl:InverseFunctionalProperty ,
                            owl:AsymmetricProperty ,
                            owl:IrreflexiveProperty ;
                   rdfs:domain :Restoration ;
                   rdfs:range :RepairProcedure ;
                   rdfs:label "Part Of Restoration"@en .


###  http://www.semanticweb.org/wood#PartOfUsedMethods
:PartOfUsedMethods rdf:type owl:ObjectProperty ;
                   rdfs:subPropertyOf owl:topObjectProperty ;
                   rdf:type owl:InverseFunctionalProperty ,
                            owl:AsymmetricProperty ,
                            owl:IrreflexiveProperty ;
                   rdfs:domain :UsedMethods ;
                   rdfs:range :Investigation ;
                   rdfs:label "Part Of Used Methods"@en .


###  http://www.semanticweb.org/wood#ReceivesInstructions
:ReceivesInstructions rdf:type owl:ObjectProperty ;
                      rdfs:subPropertyOf owl:topObjectProperty ;
                      rdf:type owl:AsymmetricProperty ,
                               owl:IrreflexiveProperty ;
                      rdfs:domain :Worker ;
                      rdfs:range :BuildingDamageExpert ;
                      rdfs:label "Receives Instructions"@en .


###  http://www.semanticweb.org/wood#Writes
:Writes rdf:type owl:ObjectProperty ;
        rdfs:subPropertyOf owl:topObjectProperty ;
        rdf:type owl:AsymmetricProperty ,
                 owl:IrreflexiveProperty ;
        rdfs:domain :BuildingDamageExpert ;
        rdfs:range :Report ;
        rdfs:label "Writes"@en .


###  http://www.w3.org/2002/07/owl#differentFrom
owl:differentFrom rdf:type owl:ObjectProperty .


###  http://www.w3.org/2002/07/owl#sameAs
owl:sameAs rdf:type owl:ObjectProperty .


#################################################################
#    Data properties
#################################################################

###  http://www.semanticweb.org/wood#BuildingDate
:BuildingDate rdf:type owl:DatatypeProperty ;
              rdfs:subPropertyOf owl:topDataProperty ;
              rdfs:domain <https://w3id.org/bot#Building> ;
              rdfs:range xsd:dateTime ;
              rdfs:label "Building Date"@en .


###  http://www.semanticweb.org/wood#ChangedAirHumidity
:ChangedAirHumidity rdf:type owl:DatatypeProperty ;
                    rdfs:subPropertyOf owl:topDataProperty ;
                    rdfs:domain :SearchedProperties ;
                    rdfs:range xsd:integer ;
                    rdfs:label "Changed Air Humidity"@en .


###  http://www.semanticweb.org/wood#ChangedBulkDensity
:ChangedBulkDensity rdf:type owl:DatatypeProperty ;
                    rdfs:subPropertyOf owl:topDataProperty ;
                    rdfs:domain :SearchedProperties ;
                    rdfs:range xsd:integer ;
                    rdfs:label "Changed Bulk Density"@en .


###  http://www.semanticweb.org/wood#ChangedEmodulus
:ChangedEmodulus rdf:type owl:DatatypeProperty ;
                 rdfs:subPropertyOf owl:topDataProperty ;
                 rdfs:domain :SearchedProperties ;
                 rdfs:range xsd:integer ;
                 rdfs:label "Changed E-modulus"@en .


###  http://www.semanticweb.org/wood#ChangedMaterialSolidity
:ChangedMaterialSolidity rdf:type owl:DatatypeProperty ;
                         rdfs:subPropertyOf owl:topDataProperty ;
                         rdfs:domain :SearchedProperties ;
                         rdfs:range xsd:integer ;
                         rdfs:label "Changed Material Solidity"@en .


###  http://www.semanticweb.org/wood#ChangedPHValue
:ChangedPHValue rdf:type owl:DatatypeProperty ;
                rdfs:subPropertyOf owl:topDataProperty ;
                rdfs:domain :SearchedProperties ;
                rdfs:range xsd:integer ;
                rdfs:label "Changed PH Value"@en .


###  http://www.semanticweb.org/wood#ChangedSalinity
:ChangedSalinity rdf:type owl:DatatypeProperty ;
                 rdfs:subPropertyOf owl:topDataProperty ;
                 rdfs:domain :SearchedProperties ;
                 rdfs:range xsd:integer ;
                 rdfs:label "Changed Salinity"@en .


###  http://www.semanticweb.org/wood#ChangedThermalInsulation
:ChangedThermalInsulation rdf:type owl:DatatypeProperty ;
                          rdfs:subPropertyOf owl:topDataProperty ;
                          rdfs:domain :SearchedProperties ;
                          rdfs:range xsd:integer ;
                          rdfs:label "Changed Thermal Insulation"@en .


###  http://www.semanticweb.org/wood#ChangedWoodMoisture
:ChangedWoodMoisture rdf:type owl:DatatypeProperty ;
                     rdfs:subPropertyOf owl:topDataProperty ;
                     rdfs:domain :SearchedProperties ;
                     rdfs:range xsd:integer ;
                     rdfs:label "Changed Wood Moisture"@en .


###  http://www.semanticweb.org/wood#ChemicalReaction
:ChemicalReaction rdf:type owl:DatatypeProperty ;
                  rdfs:subPropertyOf owl:topDataProperty ;
                  rdfs:domain :SearchedProperties ;
                  rdfs:range xsd:boolean .


###  http://www.semanticweb.org/wood#ConcealedComponents
:ConcealedComponents rdf:type owl:DatatypeProperty ;
                     rdfs:subPropertyOf owl:topDataProperty ;
                     rdfs:domain :SearchedProperties ;
                     rdfs:range xsd:boolean .


###  http://www.semanticweb.org/wood#ConstructionMethod
:ConstructionMethod rdf:type owl:DatatypeProperty ;
                    rdfs:subPropertyOf owl:topDataProperty ;
                    rdfs:domain <https://w3id.org/bot#Building> ;
                    rdfs:range xsd:string ;
                    rdfs:label "Construction Method"@en .


###  http://www.semanticweb.org/wood#DateOfInspection
:DateOfInspection rdf:type owl:DatatypeProperty ;
                  rdfs:subPropertyOf owl:topDataProperty ;
                  rdfs:domain :Report ;
                  rdfs:range xsd:dateTime ;
                  rdfs:label "Date Of Inspection"@en .


###  http://www.semanticweb.org/wood#DateOfSurvey
:DateOfSurvey rdf:type owl:DatatypeProperty ;
              rdfs:subPropertyOf owl:topDataProperty ;
              rdfs:domain :Report ;
              rdfs:range xsd:dateTime ;
              rdfs:label "Date Of Survey"@en .


###  http://www.semanticweb.org/wood#DateRenovation
:DateRenovation rdf:type owl:DatatypeProperty ;
                rdfs:subPropertyOf owl:topDataProperty ;
                rdfs:domain <https://w3id.org/bot#Building> ;
                rdfs:range xsd:dateTime ;
                rdfs:label "Date Renovation"@en .


###  http://www.semanticweb.org/wood#GeometricChange
:GeometricChange rdf:type owl:DatatypeProperty ;
                 rdfs:subPropertyOf owl:topDataProperty ;
                 rdfs:domain :SearchedProperties ;
                 rdfs:range xsd:boolean .


###  http://www.semanticweb.org/wood#HadRenovation
:HadRenovation rdf:type owl:DatatypeProperty ;
               rdfs:subPropertyOf owl:topDataProperty ;
               rdfs:domain <https://w3id.org/bot#Building> ;
               rdfs:range xsd:boolean ;
               rdfs:label "Had Renovation"@en .


###  http://www.semanticweb.org/wood#InsectContamination
:InsectContamination rdf:type owl:DatatypeProperty ;
                     rdfs:subPropertyOf owl:topDataProperty ;
                     rdfs:domain :SearchedProperties ;
                     rdfs:range xsd:boolean .


###  http://www.semanticweb.org/wood#MetalComponents
:MetalComponents rdf:type owl:DatatypeProperty ;
                 rdfs:subPropertyOf owl:topDataProperty ;
                 rdfs:domain :SearchedProperties ;
                 rdfs:range xsd:boolean .


###  http://www.semanticweb.org/wood#MonumentProtection
:MonumentProtection rdf:type owl:DatatypeProperty ;
                    rdfs:subPropertyOf owl:topDataProperty ;
                    rdfs:domain <https://w3id.org/bot#Building> ;
                    rdfs:range xsd:boolean ;
                    rdfs:label "Monument Protection"@en .


###  http://www.semanticweb.org/wood#NormalAirHumidity
:NormalAirHumidity rdf:type owl:DatatypeProperty ;
                   rdfs:subPropertyOf owl:topDataProperty ;
                   rdfs:domain :SearchedProperties ;
                   rdfs:range xsd:integer ;
                   rdfs:label "Normal Air Humidity"@en .


###  http://www.semanticweb.org/wood#NormalBulkDensity
:NormalBulkDensity rdf:type owl:DatatypeProperty ;
                   rdfs:subPropertyOf owl:topDataProperty ;
                   rdfs:domain :SearchedProperties ;
                   rdfs:range xsd:integer ;
                   rdfs:label "Normal Bulk Density"@en .


###  http://www.semanticweb.org/wood#NormalEmodulus
:NormalEmodulus rdf:type owl:DatatypeProperty ;
                rdfs:subPropertyOf owl:topDataProperty ;
                rdfs:domain :SearchedProperties ;
                rdfs:range xsd:integer ;
                rdfs:label "Normal E-modulus"@en .


###  http://www.semanticweb.org/wood#NormalMaterialSolidity
:NormalMaterialSolidity rdf:type owl:DatatypeProperty ;
                        rdfs:subPropertyOf owl:topDataProperty ;
                        rdfs:domain :SearchedProperties ;
                        rdfs:range xsd:integer ;
                        rdfs:label "Normal Material Solidity"@en .


###  http://www.semanticweb.org/wood#NormalPHValue
:NormalPHValue rdf:type owl:DatatypeProperty ;
               rdfs:subPropertyOf owl:topDataProperty ;
               rdfs:domain :SearchedProperties ;
               rdfs:range xsd:integer ;
               rdfs:label "Normal PH Value"@en .


###  http://www.semanticweb.org/wood#NormalSalinity
:NormalSalinity rdf:type owl:DatatypeProperty ;
                rdfs:subPropertyOf owl:topDataProperty ;
                rdfs:domain :SearchedProperties ;
                rdfs:range xsd:integer ;
                rdfs:label "Normal Salinity"@en .


###  http://www.semanticweb.org/wood#NormalThermalInsulation
:NormalThermalInsulation rdf:type owl:DatatypeProperty ;
                         rdfs:subPropertyOf owl:topDataProperty ;
                         rdfs:domain :SearchedProperties ;
                         rdfs:range xsd:integer ;
                         rdfs:label "Normal Thermal Insulation"@en .


###  http://www.semanticweb.org/wood#NormalWoodMoisture
:NormalWoodMoisture rdf:type owl:DatatypeProperty ;
                    rdfs:subPropertyOf owl:topDataProperty ;
                    rdfs:domain :SearchedProperties ;
                    rdfs:range xsd:integer ;
                    rdfs:label "Normal Wood Moisture"@en .


###  http://www.semanticweb.org/wood#ProjectName
:ProjectName rdf:type owl:DatatypeProperty ;
             rdfs:subPropertyOf owl:topDataProperty ;
             rdfs:domain :Report ;
             rdfs:range xsd:string ;
             rdfs:label "Project Name"@en .


###  http://www.semanticweb.org/wood#RotContamination
:RotContamination rdf:type owl:DatatypeProperty ;
                  rdfs:subPropertyOf owl:topDataProperty ;
                  rdfs:domain :SearchedProperties ;
                  rdfs:range xsd:boolean .


###  http://www.semanticweb.org/wood#Utilization
:Utilization rdf:type owl:DatatypeProperty ;
             rdfs:subPropertyOf owl:topDataProperty ;
             rdfs:domain <https://w3id.org/bot#Building> ;
             rdfs:range xsd:string ;
             rdfs:label "Utilization"@en .


###  http://www.semanticweb.org/wood#WoodAge
:WoodAge rdf:type owl:DatatypeProperty ;
         rdfs:subPropertyOf owl:topDataProperty ;
         rdfs:domain :WoodComponent ;
         rdfs:range xsd:dateTime .


#################################################################
#    Classes
#################################################################

###  http://www.opengis.net/ont/geosparql#Geometry
<http://www.opengis.net/ont/geosparql#Geometry> rdf:type owl:Class ;
                                                rdfs:subClassOf :WoodComponent .


###  http://www.semanticweb.org/wood#BiologicalInfluences
:BiologicalInfluences rdf:type owl:Class ;
                      rdfs:subClassOf :CauseOfDamage ;
                      rdfs:comment "Influences that have a biological origin."@en ;
                      rdfs:label "Biological influences"@en .


###  http://www.semanticweb.org/wood#BiologicalProcesses
:BiologicalProcesses rdf:type owl:Class ;
                     rdfs:subClassOf :WoodDamage ;
                     rdfs:comment "It is a process in which changes occur, which are triggered by biological organisms."@en ;
                     rdfs:label "Biological processes"@en .


###  http://www.semanticweb.org/wood#BrownRot
:BrownRot rdf:type owl:Class ;
          rdfs:subClassOf :WoodDestroyingFungi ;
          rdfs:comment "Brown rot: Wood structure is destroyed by decomposition of cellulose"@en ;
          rdfs:label "Brown rot"@en .


###  http://www.semanticweb.org/wood#BrushMachining
:BrushMachining rdf:type owl:Class ;
                rdfs:subClassOf :Separate ;
                rdfs:comment "Brush machining is a process of machining the workpiece with a brushing tool, to change the surface structure but also the shape."@en ;
                rdfs:label "Brush machining"@en .


###  http://www.semanticweb.org/wood#BuildingDamageExpert
:BuildingDamageExpert rdf:type owl:Class ;
                      rdfs:subClassOf <http://xmlns.com/foaf/0.1/Person> ;
                      owl:disjointWith :BuildingOwner ,
                                       :Client ;
                      rdfs:comment "Job title for people which have a background working with damages in buildings."@en ;
                      rdfs:label "Building damage expert"@en .


###  http://www.semanticweb.org/wood#BuildingDocumentation
:BuildingDocumentation rdf:type owl:Class ;
                       rdfs:subClassOf :Sources ;
                       rdfs:comment "Sources that contain information specific to the current construction project."@en ;
                       rdfs:label "Building documentation"@en .


###  http://www.semanticweb.org/wood#BuildingOwner
:BuildingOwner rdf:type owl:Class ;
               rdfs:subClassOf <http://xmlns.com/foaf/0.1/Person> ;
               rdfs:comment "A person who is the owner of a specific building."@en ;
               rdfs:label "Building owner"@en .


###  http://www.semanticweb.org/wood#Carving
:Carving rdf:type owl:Class ;
         rdfs:subClassOf :Separate ;
         rdfs:comment "Carving is a manufacturing process in which chips are separated by hitting the tool. The chisel is applied at a steep angle to the workpiece surface."@en ;
         rdfs:label "Carving"@en .


###  http://www.semanticweb.org/wood#Cause
:Cause rdf:type owl:Class ;
       rdfs:subClassOf :StepsToTheEvidenceConclusion ;
       rdfs:comment "The causes of the defect are to be presented in a comprehensible description based on the findings."@en ;
       rdfs:label "Cause"@en .


###  http://www.semanticweb.org/wood#CauseActive
:CauseActive rdf:type owl:Class ;
             rdfs:subClassOf :CauseStatus ;
             owl:disjointWith :CauseInactive ;
             rdfs:comment "Cause still has current effects on the component."@en ;
             rdfs:label "Cause Active"@en .


###  http://www.semanticweb.org/wood#CauseInactive
:CauseInactive rdf:type owl:Class ;
               rdfs:subClassOf :CauseStatus ;
               rdfs:comment "Cause has no current effect on the component."@en ;
               rdfs:label "Cause Inactive"@en .


###  http://www.semanticweb.org/wood#CauseOfDamage
:CauseOfDamage rdf:type owl:Class ;
               rdfs:comment "Describes the cause of the damage. Any damage can only come from a specific cause. Thus, every damage is linked to the cause."@en ;
               rdfs:label "Cause of damage"@en .


###  http://www.semanticweb.org/wood#CauseStatus
:CauseStatus rdf:type owl:Class ;
             rdfs:subClassOf :WoodComponent ;
             rdfs:comment "Indicates whether a cause still has current effects on the component."@en ;
             rdfs:label "Cause Status"@en .


###  http://www.semanticweb.org/wood#ChemicalInfluences
:ChemicalInfluences rdf:type owl:Class ;
                    rdfs:subClassOf :CauseOfDamage ;
                    rdfs:comment "Influences that have a chemical origin."@en ;
                    rdfs:label "Chemical influences"@en .


###  http://www.semanticweb.org/wood#ChemicalProcesses
:ChemicalProcesses rdf:type owl:Class ;
                   rdfs:subClassOf :WoodDamage ;
                   rdfs:comment "It is a process where chemical reactions change the component."@en ;
                   rdfs:label "Chemical processes"@en .


###  http://www.semanticweb.org/wood#Classification
:Classification rdf:type owl:Class ;
                rdfs:subClassOf :WoodComponent ;
                rdfs:comment "Assignment of service classes according to DIN EN 335 for wooden components."@en ;
                rdfs:label "Classification"@en .


###  http://www.semanticweb.org/wood#Client
:Client rdf:type owl:Class ;
        rdfs:subClassOf <http://xmlns.com/foaf/0.1/Person> .


###  http://www.semanticweb.org/wood#Coat
:Coat rdf:type owl:Class ;
      rdfs:subClassOf :RepairProcedure ;
      rdfs:comment "Fabricate by applying a strong adhesive layer of shapeless fabric to a workpiece."@en ;
      rdfs:label "Coat"@en .


###  http://www.semanticweb.org/wood#ColourConcealed
:ColourConcealed rdf:type owl:Class ;
                 rdfs:subClassOf :ComponentColour ;
                 owl:disjointWith :ColourEmphasized ;
                 rdfs:comment "The color of the component is covered and no longer visible to the viewer."@en ;
                 rdfs:label "Colour concealed"@en .


###  http://www.semanticweb.org/wood#ColourEmphasized
:ColourEmphasized rdf:type owl:Class ;
                  rdfs:subClassOf :ComponentColour ;
                  rdfs:comment "The colour of the component is still visible but has changed accordingly to the used coating procedure."@en ;
                  rdfs:label "Colour emphasized"@en .


###  http://www.semanticweb.org/wood#ComponentColour
:ComponentColour rdf:type owl:Class ;
                 rdfs:subClassOf :Coat ;
                 rdfs:comment "The color of the component after application of the selected coating."@en ;
                 rdfs:label "Component colour"@en .


###  http://www.semanticweb.org/wood#ComponentGrain
:ComponentGrain rdf:type owl:Class ;
                rdfs:subClassOf :Coat ;
                rdfs:comment "Component grain describes a wavy pattern on the surface of the wood that is observed after the use of surface treatment."@en ;
                rdfs:label "Component grain"@en .


###  http://www.semanticweb.org/wood#ConnectionType
:ConnectionType rdf:type owl:Class ;
                rdfs:subClassOf :Join ;
                rdfs:comment "There are different options available for connecting at least two or more components. The connection should prevent the bodies from separating under applied forces."@en ;
                rdfs:label "Connection type"@en .


###  http://www.semanticweb.org/wood#ConstructionWood
:ConstructionWood rdf:type owl:Class ;
                  rdfs:subClassOf :WoodComponent ;
                  rdfs:comment "Construction products made from wood."@en ;
                  rdfs:label "Construction wood"@en .


###  http://www.semanticweb.org/wood#CostOfRestoration
:CostOfRestoration rdf:type owl:Class ;
                   rdfs:comment "Added costs of the needed restoration procedures. First, the individual cost positions are indicated and last the total costs are indicated."@en ;
                   rdfs:label "Cost of restoration"@en .


###  http://www.semanticweb.org/wood#Costs
:Costs rdf:type owl:Class ;
       rdfs:subClassOf :StepsToTheEvidenceConclusion ;
       rdfs:comment "The cost of restoration can also be provided if a restoration procedure has been chosen. There are several ways to specify the cost of refurbishment in the report. Some possibilities are, for example: As an estimated costs, precise determination of costs by calculation, use of contractor quotations, determination based on the manufacturer's costs, remaining reduced value, increase in value."@en ;
       rdfs:label "Cost"@en .


###  http://www.semanticweb.org/wood#DegreeOfDestruction
:DegreeOfDestruction rdf:type owl:Class ;
                     rdfs:subClassOf :Investigation ;
                     rdfs:comment "Level of destruction caused by the used investigation procedure."@en ;
                     rdfs:label "Degree of destruction"@en .


###  http://www.semanticweb.org/wood#DestructiveProcesses
:DestructiveProcesses rdf:type owl:Class ;
                      rdfs:subClassOf :DegreeOfDestruction ;
                      rdfs:comment "The examination object will be partially or fully destroyed."@en ;
                      rdfs:label "Destructive processes"@en .


###  http://www.semanticweb.org/wood#DimensionalStability
:DimensionalStability rdf:type owl:Class ;
                      rdfs:subClassOf :WoodTypes ;
                      rdfs:comment "Dimensional stability is the ability of a material to maintain its original dimensions when subjected to varying degrees of temperature, moisture, pressure, or other stress."@en ;
                      rdfs:label "Dimensional Stability"@en .


###  http://www.semanticweb.org/wood#Drilling
:Drilling rdf:type owl:Class ;
          rdfs:subClassOf :Separate ;
          rdfs:comment "Drilling is the technical term for a hole created by using rotating tools."@en ;
          rdfs:label "Drilling"@en .


###  http://www.semanticweb.org/wood#DynamicOverstress
:DynamicOverstress rdf:type owl:Class ;
                   rdfs:subClassOf :mechanicalInfluences ;
                   rdfs:comment "A dynamic stress applies forces and torques to a structure and can change in direction, position and magnitude."@en ;
                   rdfs:label "Dynamic overstress"@en .


###  http://www.semanticweb.org/wood#Evaluation
:Evaluation rdf:type owl:Class ;
            rdfs:subClassOf :StepsToTheEvidenceConclusion ;
            rdfs:comment "The evaluations of the results are to be presented in a comprehensible conclusion from the findings and causes."@en ;
            rdfs:label "Evaluation"@en .


###  http://www.semanticweb.org/wood#ExternalResources
:ExternalResources rdf:type owl:Class ;
                   rdfs:subClassOf :Sources ;
                   rdfs:comment "Sources that contain general knowledge about construction projects."@en ;
                   rdfs:label "External resources"@en .


###  http://www.semanticweb.org/wood#FastProcesses
:FastProcesses rdf:type owl:Class ;
               rdfs:subClassOf :TestDuration ;
               owl:disjointWith :SlowProcesses ;
               rdfs:comment "Processes that need no further preparation and use tools that are common during a first inspection."@en ;
               rdfs:label "Fast processes"@en .


###  http://www.semanticweb.org/wood#Filing
:Filing rdf:type owl:Class ;
        rdfs:subClassOf :Separate ;
        rdfs:comment "Filing is a process of removing material with repeated rectilinear or circular cutting motion. The tool has teeth with low height, which are tightly packed together."@en ;
        rdfs:label "Filing"@en .


###  http://www.semanticweb.org/wood#ForceFit
:ForceFit rdf:type owl:Class ;
          rdfs:subClassOf :ConnectionType ;
          rdfs:comment "In this connection, movement is prevented by static friction. The components are pressed against each other, the resulting static friction opposes that of the direction of movement."@en ;
          rdfs:label "Force fit"@en .


###  http://www.semanticweb.org/wood#FormFitting
:FormFitting rdf:type owl:Class ;
             rdfs:subClassOf :ConnectionType ;
             rdfs:comment "The form-fit connection works because one of the components involved is in the way, which prevents it from coming loose. The connection is achieved either by the interlocking of at least two workpieces or by the insertion of a further part, a connecting element."@en ;
             rdfs:label "Form fitting"@en .


###  http://www.semanticweb.org/wood#GK1
:GK1 rdf:type owl:Class ;
     rdfs:subClassOf :Classification ;
     rdfs:comment "The wood or wood product is indoors and not exposed to weathering and not exposed to humidification."@en ;
     rdfs:label "GK 1"@en .


###  http://www.semanticweb.org/wood#GK2
:GK2 rdf:type owl:Class ;
     rdfs:subClassOf :Classification ;
     rdfs:comment "The wood or wood product is under the roof and not exposed to the weather, but there may be occasional but not continuous humidification. Condensation of water on the surface of the wood and the wood products may occur."@en ;
     rdfs:label "GK 2"@en .


###  http://www.semanticweb.org/wood#GK4
:GK4 rdf:type owl:Class ;
     rdfs:subClassOf :Classification ;
     rdfs:comment "The wood or wood product has direct earth contact or direct contact with fresh water."@en ;
     rdfs:label "GK 4"@en .


###  http://www.semanticweb.org/wood#GK5
:GK5 rdf:type owl:Class ;
     rdfs:subClassOf :Classification ;
     rdfs:comment "The wood or wood product is permanently or regularly immersed in salt water."@en ;
     rdfs:label "Gk 5"@en .


###  http://www.semanticweb.org/wood#Gk3point1
:Gk3point1 rdf:type owl:Class ;
           rdfs:subClassOf :Classification ;
           rdfs:comment "The wood or wood product is above ground and exposed to the weather. The water will not settle."@en ;
           rdfs:label "GK 3.1"@en .


###  http://www.semanticweb.org/wood#Gk3point2
:Gk3point2 rdf:type owl:Class ;
           rdfs:subClassOf :Classification ;
           rdfs:comment "The wood or wood product is above ground and exposed to the weather. The water may settle."@en ;
           rdfs:label "GK 3.2"@en .


###  http://www.semanticweb.org/wood#GrainConcealed
:GrainConcealed rdf:type owl:Class ;
                rdfs:subClassOf :ComponentGrain ;
                rdfs:comment "The grain of the component  is covered and no longer visible to the viewer."@en ;
                rdfs:label "Grain concealed"@en .


###  http://www.semanticweb.org/wood#GrainEmphasized
:GrainEmphasized rdf:type owl:Class ;
                 rdfs:subClassOf :ComponentGrain ;
                 rdfs:comment "The grain of the component is still visible but has changed accordingly to the used coating procedure."@en ;
                 rdfs:label "Grain emphasized"@en .


###  http://www.semanticweb.org/wood#GrainRemainsVisible
:GrainRemainsVisible rdf:type owl:Class ;
                     rdfs:subClassOf :ComponentGrain ;
                     rdfs:comment "The colour of the component is still visible and unchanged."@en ;
                     rdfs:label "Grain remains visible"@en .


###  http://www.semanticweb.org/wood#Grinding
:Grinding rdf:type owl:Class ;
          rdfs:subClassOf :Separate ;
          rdfs:comment "Grinding is a chip removing manufacturing process. The edges of the microscopically small mineral crystals in the grinding tool function as cutting edges."@en ;
          rdfs:label "Grinding"@en .


###  http://www.semanticweb.org/wood#Hardwood
:Hardwood rdf:type owl:Class ;
          rdfs:subClassOf :WoodTypes ;
          owl:disjointWith :Softwood ;
          rdfs:comment "Hardwood refers to the wood of trees that have proper leaves."@en ;
          rdfs:label "Hardwood"@en .


###  http://www.semanticweb.org/wood#HighDimensionalStability
:HighDimensionalStability rdf:type owl:Class ;
                          rdfs:subClassOf :DimensionalStability ;
                          rdfs:comment "The dimensional stability of these wood types is on the upper spectrum. These wood types have a high dimensional stability and will mostly maintain its original dimension when put under pressure."@en ;
                          rdfs:label "High dimensional stability"@en .


###  http://www.semanticweb.org/wood#HighInsectResistance
:HighInsectResistance rdf:type owl:Class ;
                      rdfs:subClassOf :InsectResistance ;
                      rdfs:comment "The insect resistance of these wood types is on the upper spectrum. These wood types have a high insect resistance and insects will mostly not be able to harm these materials."@en ;
                      rdfs:label "High insect resistance"@en .


###  http://www.semanticweb.org/wood#HighRotResistance
:HighRotResistance rdf:type owl:Class ;
                   rdfs:subClassOf :RotResistance ;
                   rdfs:comment "The rot resistance of these wood types is on the upper spectrum. These wood types have a high rot resistance and rot will mostly not be able to harm these materials."@en ;
                   rdfs:label "High rot resistance"@en .


###  http://www.semanticweb.org/wood#InSitu
:InSitu rdf:type owl:Class ;
        rdfs:subClassOf :ProcedureLocation ;
        owl:disjointWith :Laboratory ;
        rdfs:comment "Research method conducted and evaluated at the construction site."@en ;
        rdfs:label "In situ"@en .


###  http://www.semanticweb.org/wood#InsectResistance
:InsectResistance rdf:type owl:Class ;
                  rdfs:subClassOf :WoodTypes ;
                  rdfs:comment "Incest resistance is the ability of a material to naturally hinder insects to destroy its substance."@en ;
                  rdfs:label "Insect Resistance"@en .


###  http://www.semanticweb.org/wood#Investigation
:Investigation rdf:type owl:Class ;
               rdfs:comment "List of investigation procedures. Can be used to find the cause of wood damages."@en ;
               rdfs:label "Investigation"@en .


###  http://www.semanticweb.org/wood#InvestigationProcedure
:InvestigationProcedure rdf:type owl:Class ;
                        rdfs:subClassOf :Investigation ;
                        rdfs:comment "List of investigation processes."@en ;
                        rdfs:label "Investigation procedure"@en .


###  http://www.semanticweb.org/wood#Join
:Join rdf:type owl:Class ;
      rdfs:subClassOf :RepairProcedure ;
      rdfs:comment "Permanently joining or otherwise bringing together two or more workpieces. Thereby the cohesion is created locally and increased as a whole."@en ;
      rdfs:label "Join"@en .


###  http://www.semanticweb.org/wood#Laboratory
:Laboratory rdf:type owl:Class ;
            rdfs:subClassOf :ProcedureLocation ;
            rdfs:comment "Research method conducted and evaluated in part at the laboratory."@en ;
            rdfs:label "Laboratory"@en .


###  http://www.semanticweb.org/wood#Leaflet
:Leaflet rdf:type owl:Class ;
         rdfs:subClassOf :WetRotFungi ;
         rdfs:comment "Leaflets are fungi that generally do not form visible surface mycelium."@en ;
         rdfs:label "Leaflet"@en .


###  http://www.semanticweb.org/wood#LocalFindings
:LocalFindings rdf:type owl:Class ;
               rdfs:subClassOf :StepsToTheEvidenceConclusion ;
               rdfs:comment "Local findings include details of taken photos, sketches, entries in documents, examination, and measurement results."@en ;
               rdfs:label "Local findings"@en .


###  http://www.semanticweb.org/wood#LowDestructiveProcesses
:LowDestructiveProcesses rdf:type owl:Class ;
                         rdfs:subClassOf :DegreeOfDestruction ;
                         rdfs:comment "The examination object will suffer minor damages."@en ;
                         rdfs:label "Low-destructive processes"@en .


###  http://www.semanticweb.org/wood#LowDimensionalStability
:LowDimensionalStability rdf:type owl:Class ;
                         rdfs:subClassOf :DimensionalStability ;
                         rdfs:comment "The dimensional stability of these wood types is low in comparison to other wood types. They will not maintain its original dimension when put under pressure."@en ;
                         rdfs:label "Low dimensional stability"@en .


###  http://www.semanticweb.org/wood#LowInsectResistance
:LowInsectResistance rdf:type owl:Class ;
                     rdfs:subClassOf :InsectResistance ;
                     rdfs:comment "The insect resistance of these wood types is low in comparison to other wood types."@en ;
                     rdfs:label "Low insect resistance"@en .


###  http://www.semanticweb.org/wood#LowRotResistance
:LowRotResistance rdf:type owl:Class ;
                  rdfs:subClassOf :RotResistance ;
                  rdfs:comment "The rot resistance of these wood types is low in comparison to other wood types."@en ;
                  rdfs:label "Low rot resistance"@en .


###  http://www.semanticweb.org/wood#MechanicalProcesses
:MechanicalProcesses rdf:type owl:Class ;
                     rdfs:subClassOf :WoodDamage ;
                     rdfs:comment "It is a process where menchnical influences change the component."@en ;
                     rdfs:label "Mechanical processes"@en .


###  http://www.semanticweb.org/wood#MediumDimensionalStability
:MediumDimensionalStability rdf:type owl:Class ;
                            rdfs:subClassOf :DimensionalStability ;
                            rdfs:comment "The dimensional stability of these wood types is mediocre. When put under pressure these woods will show some movement."@en ;
                            rdfs:label "Medium dimensional stability"@en .


###  http://www.semanticweb.org/wood#MediumInsectResistance
:MediumInsectResistance rdf:type owl:Class ;
                        rdfs:subClassOf :InsectResistance ;
                        rdfs:comment "The insect resistance of these wood types is mediocre. Insect will be able to harm these materials."@en ;
                        rdfs:label "Medium insect resistance"@en .


###  http://www.semanticweb.org/wood#MediumRotResistance
:MediumRotResistance rdf:type owl:Class ;
                     rdfs:subClassOf :RotResistance ;
                     rdfs:comment "The rot resistance of these wood types is mediocre. Rot will be able to harm these materials."@en ;
                     rdfs:label "Medium rot resistance"@en .


###  http://www.semanticweb.org/wood#MeltLocking
:MeltLocking rdf:type owl:Class ;
             rdfs:subClassOf :ConnectionType ;
             rdfs:comment "In a melt locking bond, the components are connected to each other by atomic or molecular bonds. This is also the reason that this type of joint can only be broken by destroying the bonded components."@en ;
             rdfs:label "Melt locking"@en .


###  http://www.semanticweb.org/wood#Milling
:Milling rdf:type owl:Class ;
         rdfs:subClassOf :Separate ;
         rdfs:comment "In milling, the material is removed as the milling tool rotates around its own axis at high speed while either the tool traces the contour to be produced or the workpiece is moved accordingly."@en ;
         rdfs:label "Milling"@en .


###  http://www.semanticweb.org/wood#NonDestructiveProcesses
:NonDestructiveProcesses rdf:type owl:Class ;
                         rdfs:subClassOf :DegreeOfDestruction ;
                         rdfs:comment "The examination object will not be harmed."@en ;
                         rdfs:label "Non-destructive processes"@en .


###  http://www.semanticweb.org/wood#Planing
:Planing rdf:type owl:Class ;
         rdfs:subClassOf :Separate ;
         rdfs:comment "Planing is a method of machining wood. The surface of the wood is machined by removing chips from the material. The aim is to level and smooth the surface."@en ;
         rdfs:label "Planing"@en .


###  http://www.semanticweb.org/wood#ProcedureLocation
:ProcedureLocation rdf:type owl:Class ;
                   rdfs:subClassOf :Investigation ;
                   rdfs:comment "Location where the examination method is evaluated. If the research method is only partially evaluated on site, only the additional site is listed."@en ;
                   rdfs:label "Procedure location"@en .


###  http://www.semanticweb.org/wood#PropertiesChange
:PropertiesChange rdf:type owl:Class ;
                  rdfs:subClassOf :RepairProcedure ;
                  rdfs:comment "Manufacturing by changing the properties of the material from which a workpiece is made."@en ;
                  rdfs:label "Properties change"@en .


###  http://www.semanticweb.org/wood#Removal
:Removal rdf:type owl:Class ;
         rdfs:subClassOf :Join ;
         rdfs:comment "It is about the removal of the previously attached connecting medium."@en ;
         rdfs:label "Removal"@en .


###  http://www.semanticweb.org/wood#RepairProcedure
:RepairProcedure rdf:type owl:Class ;
                 rdfs:comment "List of repair procedures for wood damages."@en ;
                 rdfs:label "Repair procedure"@en .


###  http://www.semanticweb.org/wood#Report
:Report rdf:type owl:Class .


###  http://www.semanticweb.org/wood#Restoration
:Restoration rdf:type owl:Class ;
             rdfs:subClassOf :StepsToTheEvidenceConclusion ;
             rdfs:comment "Restoration options can also be provided. These can be named and described, but it is important to ensure that the report remains concise, and the costs remain economical."@en ;
             rdfs:label "Restoration"@en .


###  http://www.semanticweb.org/wood#Rot
:Rot rdf:type owl:Class ;
     rdfs:subClassOf :BiologicalInfluences ;
     rdfs:comment "List of fungi that occur in the building. The cause of any fungal growth in wood is moisture. The fungi germinate from spores which need moisture to grow. These spores are contained in the air or lie on the wood. With suitable humidity and environmental conditions, growth begins."@en ;
     rdfs:label "Rot"@en .


###  http://www.semanticweb.org/wood#RotResistance
:RotResistance rdf:type owl:Class ;
               rdfs:subClassOf :WoodTypes ;
               rdfs:comment "Rot resistance is the ability of a material to stop rot contamination."@en ;
               rdfs:label "Rot Resistance"@en .


###  http://www.semanticweb.org/wood#Sawing
:Sawing rdf:type owl:Class ;
        rdfs:subClassOf :Separate ;
        rdfs:comment "Sawing is a cutting manufacturing process for slitting and separating workpieces."@en ;
        rdfs:label "Sawing"@en .


###  http://www.semanticweb.org/wood#Scraping
:Scraping rdf:type owl:Class ;
          rdfs:subClassOf :Separate ;
          rdfs:comment "Scraping involves running a sharp blade over the wood. The chip angle is negative to the cutting edge."@en ;
          rdfs:label "Scraping"@en .


###  http://www.semanticweb.org/wood#SearchedProperties
:SearchedProperties rdf:type owl:Class ;
                    rdfs:subClassOf :Investigation ;
                    rdfs:comment "Properties of damages and wooden components, which can be found using an investigation procedure. Analyzing and comparing these properties the investigator can find causes of damages."@en ;
                    rdfs:label "Searched properties"@en .


###  http://www.semanticweb.org/wood#Separate
:Separate rdf:type owl:Class ;
          rdfs:subClassOf :RepairProcedure ;
          rdfs:comment "To fabricate by undoing the cohesion of bodies, reducing the cohesion in part or in whole."@en ;
          rdfs:label "Separate"@en .


###  http://www.semanticweb.org/wood#ServiceStresses
:ServiceStresses rdf:type owl:Class ;
                 rdfs:subClassOf :mechanicalInfluences ;
                 rdfs:comment "The service stress refers to a variable or moving load on a structural component. These can come, for example, from people, vehicles, or snow."@en ;
                 rdfs:label "Service stresses"@en .


###  http://www.semanticweb.org/wood#SlowProcesses
:SlowProcesses rdf:type owl:Class ;
               rdfs:subClassOf :TestDuration ;
               rdfs:comment "Processes that need some time of preparation or use tools that are not likely to be brought to the first inspection. These procedures are mostly conducted during a second inspection visit."@en ;
               rdfs:label "Slow processes"@en .


###  http://www.semanticweb.org/wood#Softwood
:Softwood rdf:type owl:Class ;
          rdfs:subClassOf :WoodTypes ;
          rdfs:comment "Softwood is the name given to all types of wood whose timber comes from needle trees."@en ;
          rdfs:label "Softwood"@en .


###  http://www.semanticweb.org/wood#SolidWood
:SolidWood rdf:type owl:Class ;
           rdfs:subClassOf :ConstructionWood ;
           owl:disjointWith :WoodBasedMaterials ;
           rdfs:comment "Wood products for the construction site, which consist of a single solid wood, or a number of solid wood parts that are glued together."@en ;
           rdfs:label "Solid wood"@en .


###  http://www.semanticweb.org/wood#Solvable
:Solvable rdf:type owl:Class ;
          rdfs:subClassOf :Removal ;
          owl:disjointWith :Unsolvable ;
          rdfs:comment "The connecting medium can be detached after use without leaving any permanent traces."@en ;
          rdfs:label "Solvable"@en .


###  http://www.semanticweb.org/wood#Sources
:Sources rdf:type owl:Class ;
         rdfs:subClassOf :Report ;
         rdfs:comment "List of sources that have information regarding the building. These sources can show the current state, an older state, or the required state. They are often used to compare these different states to point out a deficiency."@en ;
         rdfs:label "Sources"@en .


###  http://www.semanticweb.org/wood#SourcesPresentState
:SourcesPresentState rdf:type owl:Class ;
                     rdfs:subClassOf :Sources ;
                     rdfs:comment "Current building status."@en ;
                     rdfs:label "Sources present state"@en .


###  http://www.semanticweb.org/wood#SourcesTargetState
:SourcesTargetState rdf:type owl:Class ;
                    rdfs:subClassOf :Sources ;
                    rdfs:comment "Building status that should be achieved."@en ;
                    rdfs:label "Sources target state"@en .


###  http://www.semanticweb.org/wood#Splitting
:Splitting rdf:type owl:Class ;
           rdfs:subClassOf :Separate ;
           rdfs:comment "Splitting is a manufacturing process for dividing a workpiece by using a wedge-shaped tool."@en ;
           rdfs:label "Splitting"@en .


###  http://www.semanticweb.org/wood#StaticOverstress
:StaticOverstress rdf:type owl:Class ;
                  rdfs:subClassOf :mechanicalInfluences ;
                  rdfs:comment "A static stress applies forces and moments on a structure that are constant and uniform; it produces only a single response."@en ;
                  rdfs:label "Static overstresses"@en .


###  http://www.semanticweb.org/wood#StepsToTheEvidenceConclusion
:StepsToTheEvidenceConclusion rdf:type owl:Class ;
                              rdfs:subClassOf :Report ;
                              rdfs:comment "Paragraphs that are necessary for describing the found evidence in a report."@en ;
                              rdfs:label "Steps to the evidence conclusion"@en .


###  http://www.semanticweb.org/wood#TestDuration
:TestDuration rdf:type owl:Class ;
              rdfs:subClassOf :Investigation ;
              rdfs:comment "Time a test procedure can take to be conducted. This time is estimated and sorted into categories of procedures length. It is sorted into procedures that can be done on the spot during the first inspection of the building and procedures that need some form of preparation and are better done on a second inspection."@en ;
              rdfs:label "Test duration"@en .


###  http://www.semanticweb.org/wood#Turning
:Turning rdf:type owl:Class ;
         rdfs:subClassOf :Separate ;
         rdfs:comment "Turning is a manufacturing process in which the workpiece is rotated. It is a machining technique."@en ;
         rdfs:label "Turning"@en .


###  http://www.semanticweb.org/wood#Unsolvable
:Unsolvable rdf:type owl:Class ;
            rdfs:subClassOf :Removal ;
            rdfs:comment "The connecting medium cannot be detached after use without leaving any permanent traces."@en ;
            rdfs:label "Unsolvable"@en .


###  http://www.semanticweb.org/wood#UsedMethods
:UsedMethods rdf:type owl:Class ;
             rdfs:subClassOf :StepsToTheEvidenceConclusion ;
             rdfs:comment "The equipment used is stated and the execution is described. The site visits are summarized."@en ;
             rdfs:label "Used methods (Pre-note)"@en .


###  http://www.semanticweb.org/wood#VeryHighDimensionalStability
:VeryHighDimensionalStability rdf:type owl:Class ;
                              rdfs:subClassOf :DimensionalStability ;
                              rdfs:comment "The dimensional stability of these wood types is the highest among wood types. These wood types have a very high dimensional stability and will maintain its original dimension when put under pressure."@en ;
                              rdfs:label "Very high dimensional stability"@en .


###  http://www.semanticweb.org/wood#VeryHighInsectResistance
:VeryHighInsectResistance rdf:type owl:Class ;
                          rdfs:subClassOf :InsectResistance ;
                          rdfs:comment "The insect resistance of these wood types is the highest among wood types. These wood types have a very high insect resistance and insects will not be able to harm these materials."@en ;
                          rdfs:label "Very high insect resistance"@en .


###  http://www.semanticweb.org/wood#VeryHighRotResistance
:VeryHighRotResistance rdf:type owl:Class ;
                       rdfs:subClassOf :RotResistance ;
                       rdfs:comment "The rot resistance of these wood types is the highest among wood types. These wood types have a very high rot resistance and rot will not be able to harm these materials."@en ;
                       rdfs:label "Very high rot resistance"@en .


###  http://www.semanticweb.org/wood#VeryLowDimensionalStability
:VeryLowDimensionalStability rdf:type owl:Class ;
                             rdfs:subClassOf :DimensionalStability ;
                             rdfs:comment "The dimensional stability of these wood types is the lowest in comparison to other wood types. When put under pressure these wood types will have drastic movement."@en ;
                             rdfs:label "Very low dimensional stability"@en .


###  http://www.semanticweb.org/wood#VeryLowInsectResistance
:VeryLowInsectResistance rdf:type owl:Class ;
                         rdfs:subClassOf :InsectResistance ;
                         rdfs:comment "The insect resistance of these wood types is the lowest in comparison to other wood types. These materials will not be able to hinder an insect contamination."@en ;
                         rdfs:label "Very low insect resistance"@en .


###  http://www.semanticweb.org/wood#VeryLowRotResistance
:VeryLowRotResistance rdf:type owl:Class ;
                      rdfs:subClassOf :RotResistance ;
                      rdfs:comment "The rot resistance of these wood types is the lowest in comparison to other wood types. These materials will not be able to hinder a rot contamination."@en ;
                      rdfs:label "Very low rot resistance"@en .


###  http://www.semanticweb.org/wood#WetRotFungi
:WetRotFungi rdf:type owl:Class ;
             rdfs:subClassOf :WoodDestroyingFungi ;
             rdfs:comment "Wet rot fungi requires a high level of wood moisture to grow. If the wood moisture is lacking, growth will temporarily cease."@en ;
             rdfs:label "Wet rot fungi"@en .


###  http://www.semanticweb.org/wood#WhiteRot
:WhiteRot rdf:type owl:Class ;
          rdfs:subClassOf :WoodDestroyingFungi ;
          rdfs:comment "White rot: Wood structure is destroyed by degradation of the lignin."@en ;
          rdfs:label "White rot"@en .


###  http://www.semanticweb.org/wood#WoodBasedMaterials
:WoodBasedMaterials rdf:type owl:Class ;
                    rdfs:subClassOf :ConstructionWood ;
                    rdfs:comment "Wood-based materials are pressed from shredded wood or sticks. To create wood-based materials the splint can be used, but also waste products of wood production is often used. The industry offers a large number of wood-based materials that are optimized for their specific use in constructions."@en ;
                    rdfs:label "Wood based materials"@en .


###  http://www.semanticweb.org/wood#WoodComponent
:WoodComponent rdf:type owl:Class .


###  http://www.semanticweb.org/wood#WoodDamage
:WoodDamage rdf:type owl:Class ;
            rdfs:subClassOf <https://w3id.org/dot#ClassifiedDamage> ;
            rdfs:comment "Damages in wooden components."@en ;
            rdfs:label "Wood damages"@en .


###  http://www.semanticweb.org/wood#WoodDestroyingFungi
:WoodDestroyingFungi rdf:type owl:Class ;
                     rdfs:subClassOf :Rot ;
                     rdfs:comment "The wood-destroying fungi that are present in the buildings decompose the cell walls and cause rot in this way. Brown rot is particularly dangerous; with increasing wood destruction, the wood becomes longitudinally and transversely cracked and gradually takes on a brown color. The remaining substance decays to a powder."@en ;
                     rdfs:label "Wood destroying fungi"@en .


###  http://www.semanticweb.org/wood#WoodDiscoloringFungi
:WoodDiscoloringFungi rdf:type owl:Class ;
                      rdfs:subClassOf :Rot ;
                      rdfs:comment "Wood staining fungi do not affect the strength of the wood but stain the wood and can endanger the health of the occupants. The stain may result in a reduction in the value of timber or timber products."@en ;
                      rdfs:label "Wood discoloring fungi"@en .


###  http://www.semanticweb.org/wood#WoodTypes
:WoodTypes rdf:type owl:Class ;
           rdfs:subClassOf :WoodComponent ;
           rdfs:comment "Wood species used as a building material. Abbreviation according to DIN 4076."@en ;
           rdfs:label "Wood types"@en .


###  http://www.semanticweb.org/wood#Worker
:Worker rdf:type owl:Class ;
        rdfs:subClassOf <http://xmlns.com/foaf/0.1/Person> ;
        rdfs:comment "A worker is a person who has a salaried employment."@en ;
        rdfs:label "Worker"@en .


###  http://www.semanticweb.org/wood#mechanicalInfluences
:mechanicalInfluences rdf:type owl:Class ;
                      rdfs:subClassOf :CauseOfDamage ;
                      rdfs:comment "Influences caused by a mechanical force."@en ;
                      rdfs:label "Mechanical influences"@en .


###  http://www.semanticweb.org/wooddestroying_insects#WoodDestroyingInsects
<http://www.semanticweb.org/wooddestroying_insects#WoodDestroyingInsects> rdf:type owl:Class ;
                                                                          rdfs:subClassOf :BiologicalInfluences .


###  http://xmlns.com/foaf/0.1/Person
<http://xmlns.com/foaf/0.1/Person> rdf:type owl:Class .


###  https://w3id.org/bot#Building
<https://w3id.org/bot#Building> rdf:type owl:Class ;
                                rdfs:subClassOf :Report .


###  https://w3id.org/dot#ClassifiedDamage
<https://w3id.org/dot#ClassifiedDamage> rdf:type owl:Class ;
                                        rdfs:isDefinedBy <https://w3id.org/dot#> ;
                                        rdfs:label "Classified Damage"@en .


#################################################################
#    Individuals
#################################################################

###  http://www.semanticweb.org/wood#AaRdT
:AaRdT rdf:type owl:NamedIndividual ,
                :ExternalResources ,
                :Sources ,
                :SourcesTargetState ;
       rdfs:comment "The generally recognized rules of construction represent the accumulation of scientific, technical and artisanship experiences recognized in the construction industry, which are universally known and recognized as correct and necessary."@en ;
       rdfs:label "AaRdT"@en .


###  http://www.semanticweb.org/wood#Acids
:Acids rdf:type owl:NamedIndividual ,
                :CauseOfDamage ,
                :ChemicalInfluences ;
       :ChangesProperties :ChemicalReaction ,
                          :EModulus ,
                          :MaterialSolidity ,
                          :PHValue ;
       rdfs:comment "The wood strength decreases due to the acid penetration, and this can lead to the failure of the structure. If the pH value ranges between 2 < pH < 11, wood corrosion is generally low. Softwoods have a much higher corrosion resistance than hardwoods. Glulam constructions have a higher chemical resistance than solid wood constructions."@en ;
       rdfs:label "Acids"@en .


###  http://www.semanticweb.org/wood#AirHumidity
:AirHumidity rdf:type owl:NamedIndividual ,
                      :SearchedProperties ;
             :NeedsInvestigationProcedure :Hygrometer ;
             rdfs:comment "Air humidity refers to the proportion of water vapor in the gas mixture of the air."@en ;
             rdfs:label "Air Humidity"@en .


###  http://www.semanticweb.org/wood#Axe
:Axe rdf:type owl:NamedIndividual ,
              :RepairProcedure ,
              :Separate ,
              :Splitting ;
     rdfs:comment "The axe is a tool and consists of a piece of steel with a forged steel cutting edge and the handle."@en ;
     rdfs:label "Axe"@en .


###  http://www.semanticweb.org/wood#AxeTest
:AxeTest rdf:type owl:NamedIndividual ,
                  :DestructiveProcesses ,
                  :FastProcesses ,
                  :InSitu ,
                  :InvestigationProcedure ;
         rdfs:comment "By removing material using a tool such as an axe, the suspect area can be exposed and examined."@en ;
         rdfs:label "Axe Test"@en .


###  http://www.semanticweb.org/wood#AzobeAZO
:AzobeAZO rdf:type owl:NamedIndividual ,
                   :Hardwood ,
                   :HighRotResistance ,
                   :LowDimensionalStability ,
                   :MediumDimensionalStability ,
                   :VeryHighInsectResistance ,
                   :WoodTypes ;
          rdfs:comment """Wood material of azobe trees.

Colour: 
Light reddish brown/ deep reddish brown with light violet tinge.

Special properties resistance to insects:
Also, very high resistance to termites and Piddocks. Exceptions are tropical waters."""@en ;
          rdfs:label "Azobe (AZO)"@en .


###  http://www.semanticweb.org/wood#BandSaw
:BandSaw rdf:type owl:NamedIndividual ,
                  :RepairProcedure ,
                  :Sawing ,
                  :Separate ;
         rdfs:comment "A bandsaw is a machine tool whose tool consists of a band saw blade soldered or welded into a closed ring."@en ;
         rdfs:label "Bandsaw"@en .


###  http://www.semanticweb.org/wood#BeamLeafling
:BeamLeafling rdf:type owl:NamedIndividual ,
                       :BiologicalInfluences ,
                       :BrownRot ,
                       :CauseOfDamage ,
                       :Leaflet ,
                       :Rot ;
              :ChangesProperties :MaterialSolidity ,
                                 :PHValue ,
                                 :RotContamination ,
                                 :WoodMoisture ;
              rdfs:comment """Preferred wood species:
Hardwood and softwood

Optimal living conditions of wood moisture content in M-%:
> 35%

Optimal living conditions of the temperature range in °C:
26°C to 35°C

Additional notes:
Mycelium survives higher temperature and dry rigidity."""@en ;
              rdfs:label "Beam Leafling"@en ,
                         "Gloeophyllum trabeum"@la .


###  http://www.semanticweb.org/wood#BeechBU
:BeechBU rdf:type owl:NamedIndividual ,
                  :Hardwood ,
                  :LowDimensionalStability ,
                  :LowInsectResistance ,
                  :VeryLowRotResistance ,
                  :WoodTypes ;
         rdfs:comment """Wood material of beech trees.

Colour: 
Pale yellowish to reddish grey, often unevenly pitted with patchy reddish brown. Sapwood and heartwood are not distinguished."""@en ;
         rdfs:label "Beech (BU)"@en .


###  http://www.semanticweb.org/wood#BlowerDoorTest
:BlowerDoorTest rdf:type owl:NamedIndividual ,
                         :InSitu ,
                         :InvestigationProcedure ,
                         :NonDestructiveProcesses ,
                         :SlowProcesses ;
                rdfs:comment "The differential pressure measurement method is used to measure the air tightness of a building. This method is used to detect leaks in the building shell."@en ;
                rdfs:label "Blower Door Test"@en .


###  http://www.semanticweb.org/wood#BlueStainFungi
:BlueStainFungi rdf:type owl:NamedIndividual ,
                         :BiologicalInfluences ,
                         :CauseOfDamage ,
                         :Rot ,
                         :WoodDiscoloringFungi ;
                :ChangesProperties :PHValue ,
                                   :RotContamination ,
                                   :WoodMoisture ;
                rdfs:comment """Preferred wood species:
Mainly softwood.

Further notes:
Blue-green discoloration of sapwood."""@en ;
                rdfs:label "Blue Stain Fungi"@en .


###  http://www.semanticweb.org/wood#BrownCellarSponge
:BrownCellarSponge rdf:type owl:NamedIndividual ,
                            :BiologicalInfluences ,
                            :BrownRot ,
                            :CauseOfDamage ,
                            :Rot ,
                            :WetRotFungi ;
                   :ChangesProperties :MaterialSolidity ,
                                      :PHValue ,
                                      :RotContamination ,
                                      :WoodMoisture ;
                   rdfs:comment """Preferred wood species:
Softwood and hardwood.

Optimal living conditions of wood moisture content in M-%:
45% to 60%

Optimal living conditions of the temperature range in °C:
22°C to 26°C

Further notes:
Mycelium dies in case of dehydration."""@en ;
                   rdfs:label "Brown Cellar Sponge"@en ,
                              "Coniophora puteana"@la .


###  http://www.semanticweb.org/wood#Building
:Building rdf:type owl:NamedIndividual ,
                   <https://w3id.org/bot#Building> .


###  http://www.semanticweb.org/wood#BuildingTimber
:BuildingTimber rdf:type owl:NamedIndividual ,
                         :ConstructionWood ,
                         :SolidWood ;
                rdfs:comment "Building timber is made by cutting or profiling round timber."@en ;
                rdfs:label "Building Timber"@en .


###  http://www.semanticweb.org/wood#BulkDensity
:BulkDensity rdf:type owl:NamedIndividual ,
                      :SearchedProperties ;
             :NeedsInvestigationProcedure :DrillCoreTest ,
                                          :DrillingResistanceMeasurement ,
                                          :DrillingTest ,
                                          :PenetrationResistanceTest ;
             rdfs:comment "Bulk density is the density of a porous solid, based on the volume including the pore spaces."@en ;
             rdfs:label "Bulk Density"@en .


###  http://www.semanticweb.org/wood#BurnMarks
:BurnMarks rdf:type owl:NamedIndividual ,
                    :ChemicalProcesses ,
                    :GK1 ,
                    :GK2 ,
                    :GK4 ,
                    :GK5 ,
                    :Gk3point1 ,
                    :Gk3point2 ,
                    :WoodDamage ;
           :CreatedByCause :Acids ,
                           :Burning ,
                           :Explosions ;
           :NeedsRepairMethod :Axe ,
                              :BandSaw ,
                              :Chainsaw ,
                              :Chisel ,
                              :CircularSaw ,
                              :File ,
                              :FireproofingPaint ,
                              :FrameSaw ,
                              :Glaze ,
                              :GrindingMachine ,
                              :Handsaw ,
                              :Laminate ,
                              :Planer ,
                              :Sandpaper ,
                              :Scraper ,
                              :SteelBrush ,
                              :ThicknessPlaner ;
           rdfs:comment "A combustion is an exothermic reaction in which a combustible fuel is oxidized. Burn marks are produced during combustion."@en ;
           rdfs:label "Burn Marks"@en .


###  http://www.semanticweb.org/wood#Burning
:Burning rdf:type owl:NamedIndividual ,
                  :CauseOfDamage ,
                  :ServiceStresses ,
                  :mechanicalInfluences ;
         :ChangesProperties :EModulus ,
                            :MaterialSolidity ;
         rdfs:comment "Fire damage to structural components, which reduces the load bearing of the cross-sections of the structure."@en ;
         rdfs:label "Burning"@en .


###  http://www.semanticweb.org/wood#ButterflySpore
:ButterflySpore rdf:type owl:NamedIndividual ,
                         :BiologicalInfluences ,
                         :BrownRot ,
                         :CauseOfDamage ,
                         :Rot ,
                         :WetRotFungi ;
                :ChangesProperties :MaterialSolidity ,
                                   :PHValue ,
                                   :RotContamination ,
                                   :WoodMoisture ;
                rdfs:comment """Preferred wood species:
Hardwood and hardly any softwood.

Optimal living conditions of wood moisture content in M-%:
> 35%

Optimal living conditions of the temperature range in °C:
23°C to 26°C

Additional notes:
Mycelium dies when dried out."""@en ;
                rdfs:label "Butterfly Spore"@en ,
                           "Coriolus versicolor"@la .


###  http://www.semanticweb.org/wood#Calculations
:Calculations rdf:type owl:NamedIndividual ,
                       :BuildingDocumentation ,
                       :Sources ,
                       :SourcesPresentState ;
              rdfs:comment "Calculations that represent information about the building. This can be information on structural analysis, thermal insulation, noise protection and other topics."@en ;
              rdfs:label "Calculations"@en .


###  http://www.semanticweb.org/wood#CementFiberBoards
:CementFiberBoards rdf:type owl:NamedIndividual ,
                            :ConstructionWood ,
                            :WoodBasedMaterials ;
                   rdfs:comment "Cement fiber boards consist of Portland cement, silicate aggregates and cellulose fibers."@en ;
                   rdfs:label "Cement Fiber Boards"@en .


###  http://www.semanticweb.org/wood#Chainsaw
:Chainsaw rdf:type owl:NamedIndividual ,
                   :RepairProcedure ,
                   :Sawing ,
                   :Separate ;
          rdfs:comment "The chainsaw uses a cutting chain, which is driven by a small motor."@en ;
          rdfs:label "Chainsaw"@en .


###  http://www.semanticweb.org/wood#ChangeOfColour
:ChangeOfColour rdf:type owl:NamedIndividual ,
                         :FastProcesses ,
                         :InSitu ,
                         :InvestigationProcedure ,
                         :NonDestructiveProcesses ;
                rdfs:comment "The colour in the component changes."@en ;
                rdfs:label "Change Of Colour"@en .


###  http://www.semanticweb.org/wood#ChemicalReaction
:ChemicalReaction rdf:type owl:NamedIndividual ,
                           :SearchedProperties ;
                  :NeedsInvestigationProcedure :ChangeOfColour ,
                                               :DamagePattern ,
                                               :DrillingTest ,
                                               :IndicatorPaper ,
                                               :MeasuringMagnifier ,
                                               :Microscopy ,
                                               :PHMeter ,
                                               :Pictures .


###  http://www.semanticweb.org/wood#Chipboards
:Chipboards rdf:type owl:NamedIndividual ,
                     :ConstructionWood ,
                     :WoodBasedMaterials ;
            rdfs:comment "Flat pressed boards are made by pressing small wood chips with adhesives or mineral binders. The chips are preferably parallel to the surface of the board and are usually produced in several layers. In both directions of the panel plane there are almost equivalent tensile, compressive, and flexural strengths achieved."@en ;
            rdfs:label "Chipboards"@en .


###  http://www.semanticweb.org/wood#Chisel
:Chisel rdf:type owl:NamedIndividual ,
                 :Carving ,
                 :RepairProcedure ,
                 :Separate ;
        rdfs:comment "The chisel is a tool made of steel, which has a hardened wedge-shaped cutting edge. Chisels are used with a hammer to divide objects or to cut off parts from them."@en ;
        rdfs:label "Chisel"@en .


###  http://www.semanticweb.org/wood#Chromatography
:Chromatography rdf:type owl:NamedIndividual ,
                         :InSitu ,
                         :InvestigationProcedure ,
                         :LowDestructiveProcesses ,
                         :SlowProcesses ;
                rdfs:comment "In chromatography, a mixture of substances is separated into its individual components. This can provide an indication about the fungal infestation."@en ;
                rdfs:label "Chromatography"@en .


###  http://www.semanticweb.org/wood#CircularSaw
:CircularSaw rdf:type owl:NamedIndividual ,
                      :RepairProcedure ,
                      :Sawing ,
                      :Separate ;
             rdfs:comment "A circular saw is a machine tool for cutting workpieces. It uses a round cutting disc, which is rotated in its axis."@en ;
             rdfs:label "Circular Saw"@en .


###  http://www.semanticweb.org/wood#Clamps
:Clamps rdf:type owl:NamedIndividual ,
                 :ForceFit ,
                 :Join ,
                 :RepairProcedure ,
                 :Solvable ;
        rdfs:comment "Clamping devices are all devices for firmly fixing a workpiece or tool during the machining process."@en ;
        rdfs:label "Clamps"@en .


###  http://www.semanticweb.org/wood#Client
:Client rdf:type owl:NamedIndividual ,
                 :Client .


###  http://www.semanticweb.org/wood#ConcealedComponents
:ConcealedComponents rdf:type owl:NamedIndividual ,
                              :SearchedProperties ;
                     :NeedsInvestigationProcedure :AxeTest ,
                                                  :DrillingResistanceMeasurement ,
                                                  :DrillingTest ,
                                                  :Endoscopy ,
                                                  :PenetrationResistanceTest ,
                                                  :SoundTest ,
                                                  :UltrasonicEchoMethod ,
                                                  :XRays .


###  http://www.semanticweb.org/wood#ConstructionVeneerPlywood
:ConstructionVeneerPlywood rdf:type owl:NamedIndividual ,
                                    :ConstructionWood ,
                                    :WoodBasedMaterials ;
                           rdfs:comment "Construction veneer plywood is created by arranging dried veneers and gluing them together."@en ;
                           rdfs:label "Construction Veneer Plywood"@en .


###  http://www.semanticweb.org/wood#Contracts
:Contracts rdf:type owl:NamedIndividual ,
                    :BuildingDocumentation ,
                    :Sources ,
                    :SourcesTargetState .


###  http://www.semanticweb.org/wood#Corrosion
:Corrosion rdf:type owl:NamedIndividual ,
                    :ChemicalProcesses ,
                    :GK2 ,
                    :GK4 ,
                    :GK5 ,
                    :Gk3point1 ,
                    :Gk3point2 ,
                    :WoodDamage ;
           :CreatedByCause :CorrosionOfSteelFasteners ;
           :NeedsRepairMethod :Axe ,
                              :BandSaw ,
                              :Chainsaw ,
                              :Chisel ,
                              :CircularSaw ,
                              :DrillingMachine ,
                              :File ,
                              :FrameSaw ,
                              :GrindingMachine ,
                              :Handsaw ,
                              :Sandpaper ,
                              :Scraper ,
                              :SteelBrush ;
           rdfs:comment "Wood is corrosion resistant but fasteners, made of components that can rust, can lead to damages."@en ;
           rdfs:label "Corrosion"@en .


###  http://www.semanticweb.org/wood#CorrosionOfSteelFasteners
:CorrosionOfSteelFasteners rdf:type owl:NamedIndividual ,
                                    :CauseOfDamage ,
                                    :ChemicalInfluences ;
                           :ChangesProperties :ChemicalReaction ,
                                              :MetalComponents ;
                           rdfs:comment "Steel fasteners embedded in the wood are largely protected against corrosion by the corrosion-resistant wood. However, non-embedded pieces of fasteners can corrode quickly if left untreated."@en ;
                           rdfs:label "Corrosion Of Steel Fasteners"@en .


###  http://www.semanticweb.org/wood#Cracks
:Cracks rdf:type owl:NamedIndividual ,
                 :GK1 ,
                 :GK2 ,
                 :GK4 ,
                 :GK5 ,
                 :Gk3point1 ,
                 :Gk3point2 ,
                 :MechanicalProcesses ,
                 :WoodDamage ;
        :CreatedByCause :Burning ,
                        :ExcessiveLoadsFromConstruction ,
                        :Explosions ,
                        :Impact ,
                        :InsufficientBeamDimensions ,
                        :ReductionInLoadCapacityDueToWear ,
                        :Shocks ,
                        :TooHighLoadsFromDeposition ,
                        :TooHighSnowLoads ,
                        :Vibrations ,
                        :WindLoads ;
        :NeedsRepairMethod :Clamps ,
                           :Glue ,
                           :Nailing ,
                           :Screws ,
                           :Tenon ;
        rdfs:comment "Separation gap created by the tearing of a material object."@en ;
        rdfs:label "Cracks"@en .


###  http://www.semanticweb.org/wood#CrossBeams
:CrossBeams rdf:type owl:NamedIndividual ,
                     :ConstructionWood ,
                     :SolidWood ;
            rdfs:comment "Cross beams consist of four quarter timber segments of softwood which are glued together. These segments are fiber-parallel to each other. The outside of the round timber segments is turned inwards so that the inside of the rectangular cross-section creates a tube."@en ;
            rdfs:label "Cross Beams"@en .


###  http://www.semanticweb.org/wood#DNAAnalysis
:DNAAnalysis rdf:type owl:NamedIndividual ,
                      :InvestigationProcedure ,
                      :Laboratory ,
                      :LowDestructiveProcesses ,
                      :SlowProcesses ;
             rdfs:comment "It is possible to detect structural wood fungi via DNA which is still present in the infested wood. This method is always useful when the type of fungus cannot be clearly determined from the appearance on site."@en ;
             rdfs:label "DNA Analysis"@en .


###  http://www.semanticweb.org/wood#DamagePattern
:DamagePattern rdf:type owl:NamedIndividual ,
                        :FastProcesses ,
                        :InSitu ,
                        :InvestigationProcedure ,
                        :NonDestructiveProcesses ;
               rdfs:comment "The recognition of patterns or structures of the component or the destructive elements."@en ;
               rdfs:label "Damage Pattern"@en .


###  http://www.semanticweb.org/wood#Deflection
:Deflection rdf:type owl:NamedIndividual ,
                     :GK1 ,
                     :GK2 ,
                     :GK4 ,
                     :GK5 ,
                     :Gk3point1 ,
                     :Gk3point2 ,
                     :MechanicalProcesses ,
                     :WoodDamage ;
            :CreatedByCause :ExcessiveLoadsFromConstruction ,
                            :InsufficientBeamDimensions ,
                            :ReductionInLoadCapacityDueToWear ,
                            :TooHighLoadsFromDeposition ,
                            :TooHighSnowLoads ,
                            :WindLoads ;
            :NeedsRepairMethod :Axe ,
                               :BandSaw ,
                               :Chainsaw ,
                               :CircularSaw ,
                               :Clamps ,
                               :FrameSaw ,
                               :Glue ,
                               :Handsaw ,
                               :Nailing ,
                               :Screws ,
                               :Tenon ;
            rdfs:comment "Deflection is the deformation of an elongated component that is overloaded and thus permanently deformed."@en ;
            rdfs:label "Deflection"@en .


###  http://www.semanticweb.org/wood#Delocalization
:Delocalization rdf:type owl:NamedIndividual ,
                         :GK1 ,
                         :GK2 ,
                         :GK4 ,
                         :GK5 ,
                         :Gk3point1 ,
                         :Gk3point2 ,
                         :MechanicalProcesses ,
                         :WoodDamage ;
                :CreatedByCause :ExcessiveLoadsFromConstruction ,
                                :Explosions ,
                                :HumanRemoval ,
                                :Impact ,
                                :InsufficientBeamDimensions ,
                                :ReductionInLoadCapacityDueToWear ,
                                :Shocks ,
                                :TooHighLoadsFromDeposition ,
                                :TooHighSnowLoads ,
                                :Vibrations ,
                                :WindLoads ;
                :NeedsRepairMethod :Clamps ,
                                   :Glue ,
                                   :Nailing ,
                                   :Screws ,
                                   :Tenon ;
                rdfs:comment "The part was dislocated from its original position. It must be re-installed."@en ;
                rdfs:label "Delocalization"@en .


###  http://www.semanticweb.org/wood#Dendrochronology
:Dendrochronology rdf:type owl:NamedIndividual ,
                           :DestructiveProcesses ,
                           :InvestigationProcedure ,
                           :Laboratory ,
                           :SlowProcesses ;
                  rdfs:comment "This requires a sample of the component to be analyzed. The age of the tree can be determined from the annual rings of the used wood. Experts can only conduct the examinations."@en ;
                  rdfs:label "Dendrochronology"@en .


###  http://www.semanticweb.org/wood#DouglasFirDGA
:DouglasFirDGA rdf:type owl:NamedIndividual ,
                        :HighDimensionalStability ,
                        :MediumInsectResistance ,
                        :MediumRotResistance ,
                        :Softwood ,
                        :WoodTypes ;
               rdfs:comment """Wood material of Douglas fir trees.

Colour: 
Yellowish white / reddish brown, darkens with time, late wood dark.

Special properties resistance to fungi:
Sapwood sensitive to blue stain."""@en ;
               rdfs:label "Douglas Fir (DGA)"@en .


###  http://www.semanticweb.org/wood#Drawings
:Drawings rdf:type owl:NamedIndividual ,
                   :BuildingDocumentation ,
                   :Sources ,
                   :SourcesPresentState ;
          rdfs:comment "A drawing is a visually represented subject."@en ;
          rdfs:label "Drawings"@en .


###  http://www.semanticweb.org/wood#DrillCoreTest
:DrillCoreTest rdf:type owl:NamedIndividual ,
                        :DestructiveProcesses ,
                        :InvestigationProcedure ,
                        :Laboratory ,
                        :SlowProcesses ;
               rdfs:comment "In the drilling core process, cylindrical samples are taken with the help of a mill, which have a diameter starting from 4mm to 50mm. The applications of the cores taken from wood are manifold. The boreholes can be closed again with suitable new wood plugs after core removal."@en ;
               rdfs:label "Drill Core Test"@en .


###  http://www.semanticweb.org/wood#DrillingMachine
:DrillingMachine rdf:type owl:NamedIndividual ,
                          :Drilling ,
                          :RepairProcedure ,
                          :Separate ;
                 rdfs:comment "Drilling machine is electric device for drilling holes."@en ;
                 rdfs:label "Drilling Machine"@en .


###  http://www.semanticweb.org/wood#DrillingResistanceMeasurement
:DrillingResistanceMeasurement rdf:type owl:NamedIndividual ,
                                        :InSitu ,
                                        :InvestigationProcedure ,
                                        :LowDestructiveProcesses ,
                                        :SlowProcesses ;
                               rdfs:comment "For the drilling resistance measurement, a drilling needle with 1.5mm diameter is drilled into the wood. The density of the wood is registered and recorded."@en ;
                               rdfs:label "Drilling Resistance Measurement"@en .


###  http://www.semanticweb.org/wood#DrillingTest
:DrillingTest rdf:type owl:NamedIndividual ,
                       :InSitu ,
                       :InvestigationProcedure ,
                       :LowDestructiveProcesses ,
                       :SlowProcesses ;
              rdfs:comment "If suspicious spots are discovered, they can be drilled into to draw to draw conclusions from the drill dust."@en ;
              rdfs:label "Drilling Test"@en .


###  http://www.semanticweb.org/wood#DryRot
:DryRot rdf:type owl:NamedIndividual ,
                 :BiologicalInfluences ,
                 :BrownRot ,
                 :CauseOfDamage ,
                 :Rot ,
                 :WoodDestroyingFungi ;
        :ChangesProperties :MaterialSolidity ,
                           :PHValue ,
                           :RotContamination ,
                           :WoodMoisture ;
        rdfs:comment """Preferred wood species:
Mainly softwood, also hardwood.

Optimal living conditions of wood moisture content in M-%:
20% to 40%

Optimal living conditions of the temperature range in °C:
18°C to 22°C

Further notes:
Dry rot requires only a certain degree of wood moisture at the beginning of its growth. It is the only structural wood fungus capable of attacking dry wood, which it moisturizes itself by transporting water via strand mycelium."""@en ;
        rdfs:label "Dry Rot"@en ,
                   "Serpula lacrimans"@la .


###  http://www.semanticweb.org/wood#DuoTrioBeams
:DuoTrioBeams rdf:type owl:NamedIndividual ,
                       :ConstructionWood ,
                       :SolidWood ;
              rdfs:comment "Duo beams and trio beams consist of two or three flat-sided and fiber-parallel planks which are glued to each other."@en ;
              rdfs:label "Duo/Trio-Beams"@en .


###  http://www.semanticweb.org/wood#EModulus
:EModulus rdf:type owl:NamedIndividual ,
                   :SearchedProperties ;
          :NeedsInvestigationProcedure :LoadTest ,
                                       :UltrasonicEchoMethod ;
          rdfs:comment "The modulus of elasticity, also called E-modulus, is a parameter that describes the relationship between stress and extension during the deformation of a solid body."@en ;
          rdfs:label "E-Modulus"@en .


###  http://www.semanticweb.org/wood#ElectricalResistance
:ElectricalResistance rdf:type owl:NamedIndividual ,
                               :InSitu ,
                               :InvestigationProcedure ,
                               :NonDestructiveProcesses ,
                               :SlowProcesses ;
                      rdfs:comment "Two electrodes are driven into the wood and the electric current is measured, which flows through the wood depending on the moisture content of the wood. With these methods, however, only the moisture of the direct surface is measured; no statement can be made about the internal moisture concentration."@en ;
                      rdfs:label "Electrical Resistance"@en .


###  http://www.semanticweb.org/wood#Endoscopy
:Endoscopy rdf:type owl:NamedIndividual ,
                    :InSitu ,
                    :InvestigationProcedure ,
                    :LowDestructiveProcesses ,
                    :SlowProcesses ;
           rdfs:comment "For concealed components, the endoscope is used. Holes with a maximum diameter of 5 to 20mm are drilled and the endoscope is inserted. This enables an optical inspection even of components that are not visible."@en ;
           rdfs:label "Endoscopy"@en .


###  http://www.semanticweb.org/wood#ExcessiveLoadsFromConstruction
:ExcessiveLoadsFromConstruction rdf:type owl:NamedIndividual ,
                                         :CauseOfDamage ,
                                         :StaticOverstress ,
                                         :mechanicalInfluences ;
                                :ChangesProperties :GeometricChange ;
                                rdfs:comment "Failure of the structure due to excessive loads can occur in certain cases: Through unplanned usage of the construction or through a new load redistribution due to the failure of individual components."@en ;
                                rdfs:label "Excessive Loads From Construction"@en .


###  http://www.semanticweb.org/wood#Expert
:Expert rdf:type owl:NamedIndividual ,
                 :BuildingDamageExpert ;
        rdfs:label "Expert"@en .


###  http://www.semanticweb.org/wood#Explosions
:Explosions rdf:type owl:NamedIndividual ,
                     :CauseOfDamage ,
                     :DynamicOverstress ,
                     :mechanicalInfluences ;
            :ChangesProperties :GeometricChange ,
                               :MaterialSolidity ;
            rdfs:comment "Explosions on components, which can overstress, burn, and destroy these components. Furthermore, the vibration can cause cracks, deformations, and fastener failures."@en ;
            rdfs:label "Explosions"@en .


###  http://www.semanticweb.org/wood#FenceLeaflet
:FenceLeaflet rdf:type owl:NamedIndividual ,
                       :BiologicalInfluences ,
                       :BrownRot ,
                       :CauseOfDamage ,
                       :Leaflet ,
                       :Rot ;
              :ChangesProperties :MaterialSolidity ,
                                 :PHValue ,
                                 :RotContamination ,
                                 :WoodMoisture ;
              rdfs:comment """Preferred wood species:
Hardwood.

Optimal living conditions of wood moisture content in M-%:
40% to 60%

Optimal living conditions of the temperature range in °C:
26°C to 36°C

Additional notes:
Mycelium survives higher temperature and dry rigidity."""@en ;
              rdfs:label "Fence Leaflet"@en ,
                         "Gloeophyllum sepiarium"@la .


###  http://www.semanticweb.org/wood#File
:File rdf:type owl:NamedIndividual ,
               :Filing ,
               :RepairProcedure ,
               :Separate ;
      rdfs:comment "Files have a handle and a file blade."@en ;
      rdfs:label "File"@en .


###  http://www.semanticweb.org/wood#FirLeafBlossom
:FirLeafBlossom rdf:type owl:NamedIndividual ,
                         :BiologicalInfluences ,
                         :BrownRot ,
                         :CauseOfDamage ,
                         :Leaflet ,
                         :Rot ;
                :ChangesProperties :MaterialSolidity ,
                                   :PHValue ,
                                   :RotContamination ,
                                   :WoodMoisture ;
                rdfs:comment """Preferred wood species:
Hardwood.

Optimal living conditions of wood moisture content in M-%:
35% to 40%

Optimal living conditions of the temperature range in °C:
26°C to 35°C

Additional notes:
Mycelium survives higher temperature and dry rigidity."""@en ;
                rdfs:label "Fir Leaf Blossom"@en ,
                           "Gloeophyllum abietinum"@la .


###  http://www.semanticweb.org/wood#FirTA
:FirTA rdf:type owl:NamedIndividual ,
                :HighDimensionalStability ,
                :LowInsectResistance ,
                :LowRotResistance ,
                :Softwood ,
                :WoodTypes ;
       rdfs:comment """Wood material of fir trees.

Colour:
Early wood almost white, late wood pale reddish, sapwood and heartwood are not distinguished.

Special properties resistance to fungi:
Sensitive to blue stain."""@en ;
       rdfs:label "Fir (TA)"@en .


###  http://www.semanticweb.org/wood#FireproofingPaint
:FireproofingPaint rdf:type owl:NamedIndividual ,
                            :PropertiesChange ,
                            :RepairProcedure ;
                   rdfs:comment "When exposed to fire, the fire protection coating foams up and protects against oxygen ingress."@en ;
                   rdfs:label "Fireproofing Paint"@en .


###  http://www.semanticweb.org/wood#FoldingRule
:FoldingRule rdf:type owl:NamedIndividual ,
                      :FastProcesses ,
                      :InSitu ,
                      :InvestigationProcedure ,
                      :NonDestructiveProcesses ;
             rdfs:comment "A folding rule is a haptic measuring instrument used to measure short distances."@en ;
             rdfs:label "Folding Rule"@en .


###  http://www.semanticweb.org/wood#Fractures
:Fractures rdf:type owl:NamedIndividual ,
                    :GK1 ,
                    :GK2 ,
                    :GK4 ,
                    :GK5 ,
                    :Gk3point1 ,
                    :Gk3point2 ,
                    :MechanicalProcesses ,
                    :WoodDamage ;
           :CreatedByCause :Burning ,
                           :ExcessiveLoadsFromConstruction ,
                           :Explosions ,
                           :Impact ,
                           :InsufficientBeamDimensions ,
                           :ReductionInLoadCapacityDueToWear ,
                           :Shocks ,
                           :TooHighLoadsFromDeposition ,
                           :TooHighSnowLoads ,
                           :WindLoads ;
           :NeedsRepairMethod :Clamps ,
                              :Glue ,
                              :Nailing ,
                              :Screws ,
                              :Tenon ;
           rdfs:comment "The cracking or breaking of a hard object."@en ;
           rdfs:label "Fractures"@en .


###  http://www.semanticweb.org/wood#FrameSaw
:FrameSaw rdf:type owl:NamedIndividual ,
                   :RepairProcedure ,
                   :Sawing ,
                   :Separate ;
          rdfs:comment "Frame saws are used in a sawmill and are driven by a flywheel."@en ;
          rdfs:label "Frame Saw"@en .


###  http://www.semanticweb.org/wood#Fumigant
:Fumigant rdf:type owl:NamedIndividual ,
                   :PropertiesChange ,
                   :RepairProcedure ;
          rdfs:comment "Fumigation is a method of pest control or elimination of harmful microorganisms by completely filling a space with gaseous pesticides."@en ;
          rdfs:label "Fumigant"@en .


###  http://www.semanticweb.org/wood#GeometricChange
:GeometricChange rdf:type owl:NamedIndividual ,
                          :SearchedProperties ;
                 :NeedsInvestigationProcedure :ChangeOfColour ,
                                              :DamagePattern ,
                                              :FoldingRule ,
                                              :LaserMeasuringDevice ,
                                              :MeasuringMagnifier ,
                                              :MeasuringTape ,
                                              :Photogrammetry ,
                                              :Pictures ,
                                              :Theodolite ,
                                              <http://www.semanticweb.org/wood#3DLaserScanning> .


###  http://www.semanticweb.org/wood#Glaze
:Glaze rdf:type owl:NamedIndividual ,
                :Coat ,
                :ColourConcealed ,
                :GrainConcealed ,
                :RepairProcedure ;
       rdfs:comment "Glazing is a liquid or powder coating material that is applied thinly to objects and built up by chemical or physical processes to form a continuous, solid layer. The wood grain is concealed."@en ;
       rdfs:label "Glaze"@en .


###  http://www.semanticweb.org/wood#Glue
:Glue rdf:type owl:NamedIndividual ,
               :Join ,
               :MeltLocking ,
               :RepairProcedure ,
               :Unsolvable ;
      rdfs:comment "Wood glue is an adhesive used to tightly bond pieces of wood together. Different substances can be used as glue."@en ;
      rdfs:label "Glue"@en .


###  http://www.semanticweb.org/wood#GluedLaminatedTimber
:GluedLaminatedTimber rdf:type owl:NamedIndividual ,
                               :ConstructionWood ,
                               :SolidWood ;
                      rdfs:comment "Glued laminated timber (Glulam) is a hardened and tempered solid wood, in which the strength-reducing influence of the growth-related defects is cancelled out, up to a to a certain extent. It consists of at least three boards glued together."@en ;
                      rdfs:label "Glued Laminated Timber"@en .


###  http://www.semanticweb.org/wood#GravimetricMethod
:GravimetricMethod rdf:type owl:NamedIndividual ,
                            :InvestigationProcedure ,
                            :Laboratory ,
                            :LowDestructiveProcesses ,
                            :SlowProcesses ;
                   rdfs:comment "A building material sample is weighed in the laboratory, dried in an oven, and then weighed again. The difference gives the moisture content. The moisture determination is very accurate."@en ;
                   rdfs:label "Gravimetric Method"@en .


###  http://www.semanticweb.org/wood#GrindingMachine
:GrindingMachine rdf:type owl:NamedIndividual ,
                          :Grinding ,
                          :RepairProcedure ,
                          :Separate ;
                 rdfs:comment "Grinders are tools for smoothing surfaces or removing coatings from surfaces."@en ;
                 rdfs:label "Grinding Machine"@en .


###  http://www.semanticweb.org/wood#GypsumFiberboards
:GypsumFiberboards rdf:type owl:NamedIndividual ,
                            :ConstructionWood ,
                            :WoodBasedMaterials ;
                   rdfs:comment "Gypsum fiberboards are made from gypsum and paper fibers. The paper fibers serve as reinforcement. A homogeneous mixture of both raw materials and water is pressed into slabs under high pressure, dried and cut to the respective formats."@en ;
                   rdfs:label "Gypsum Fiberboards"@en .


###  http://www.semanticweb.org/wood#Handsaw
:Handsaw rdf:type owl:NamedIndividual ,
                  :RepairProcedure ,
                  :Sawing ,
                  :Separate ;
         rdfs:comment "The saw is a tool for cutting wood by chip removal."@en ;
         rdfs:label "Handsaw"@en .


###  http://www.semanticweb.org/wood#Holes
:Holes rdf:type owl:NamedIndividual ,
                :GK1 ,
                :GK2 ,
                :GK4 ,
                :GK5 ,
                :Gk3point1 ,
                :Gk3point2 ,
                :MechanicalProcesses ,
                :WoodDamage ;
       :CreatedByCause :Burning ,
                       :ExcessiveLoadsFromConstruction ,
                       :Explosions ,
                       :HumanRemoval ,
                       :Impact ,
                       :InsufficientBeamDimensions ,
                       :ReductionInLoadCapacityDueToWear ,
                       :Shocks ,
                       :TooHighLoadsFromDeposition ,
                       :TooHighSnowLoads ,
                       :WindLoads ;
       :NeedsRepairMethod :Axe ,
                          :BandSaw ,
                          :Chainsaw ,
                          :CircularSaw ,
                          :FrameSaw ,
                          :Handsaw ;
       rdfs:comment "Due to damage, there is a place where the material is no longer present."@en ;
       rdfs:label "Holes"@en .


###  http://www.semanticweb.org/wood#HumanRemoval
:HumanRemoval rdf:type owl:NamedIndividual ,
                       :CauseOfDamage ,
                       :ServiceStresses ,
                       :mechanicalInfluences ;
              :ChangesProperties :GeometricChange ,
                                 :ThermalInsulation ;
              rdfs:comment "Unprofessional intervention in the structural system can lead to a change in the load transfer and thus to components being overstressed."@en ;
              rdfs:label "Human Removal"@en .


###  http://www.semanticweb.org/wood#Hygrometer
:Hygrometer rdf:type owl:NamedIndividual ,
                     :InSitu ,
                     :InvestigationProcedure ,
                     :NonDestructiveProcesses ,
                     :SlowProcesses ;
            rdfs:comment "A hygrometer is a measuring instrument for determining the relative humidity of the air."@en ;
            rdfs:label "Hygrometer"@en .


###  http://www.semanticweb.org/wood#Impact
:Impact rdf:type owl:NamedIndividual ,
                 :CauseOfDamage ,
                 :ServiceStresses ,
                 :mechanicalInfluences ;
        :ChangesProperties :GeometricChange ;
        rdfs:comment "Impact on components, which can overstress and destroy these components. Furthermore, vibrations can cause cracks, deformations, and fastener failures."@en ;
        rdfs:label "Impact"@en .


###  http://www.semanticweb.org/wood#IndicatorPaper
:IndicatorPaper rdf:type owl:NamedIndividual ,
                         :InSitu ,
                         :InvestigationProcedure ,
                         :NonDestructiveProcesses ,
                         :SlowProcesses ;
                rdfs:comment "Detection of brown rot fungi by measuring the concentration of oxalic acid. During the decomposition of wood substance by brown rot, oxalic acid is produced, reducing the pH of the wood from pH = 5 to pH = 3. In the field, a simple color reaction test provides evidence of active fungal attack. The blue colour of the indicator turns to green or yellow, when infestation is present. For chemical analysis in the laboratory, only small amounts of a sample of approx. 2 to 5 g are required."@en ;
                rdfs:label "Indicator Paper"@en .


###  http://www.semanticweb.org/wood#InsectContamination
:InsectContamination rdf:type owl:NamedIndividual ,
                              :SearchedProperties ;
                     :NeedsInvestigationProcedure :ChangeOfColour ,
                                                  :DamagePattern ,
                                                  :DrillingResistanceMeasurement ,
                                                  :DrillingTest ,
                                                  :Endoscopy ,
                                                  :InsectIdentification ,
                                                  :MeasuringMagnifier ,
                                                  :Microscopy ,
                                                  :PenetrationResistanceTest ,
                                                  :Pictures ,
                                                  :Stethoscope .


###  http://www.semanticweb.org/wood#InsectIdentification
:InsectIdentification rdf:type owl:NamedIndividual ,
                               :InSitu ,
                               :InvestigationProcedure ,
                               :LowDestructiveProcesses ,
                               :SlowProcesses ;
                      rdfs:comment "The identification of the type of insect contamination can be done by examining the insects found. This is only possible in case of an active infestation."@en ;
                      rdfs:label "Insect Identification"@en .


###  http://www.semanticweb.org/wood#InsectInfestation
:InsectInfestation rdf:type owl:NamedIndividual ,
                            :BiologicalProcesses ,
                            :GK1 ,
                            :GK2 ,
                            :GK4 ,
                            :GK5 ,
                            :Gk3point1 ,
                            :Gk3point2 ,
                            :WoodDamage ;
                   :CreatedByCause :InsectInfluences ,
                                   :MoisturePenetration ;
                   :NeedsRepairMethod :Axe ,
                                      :BandSaw ,
                                      :Chainsaw ,
                                      :CircularSaw ,
                                      :FrameSaw ,
                                      :Fumigant ,
                                      :Handsaw ,
                                      :WoodPreservatives ;
                   rdfs:comment "An infestation of the wood substance by insects."@en ;
                   rdfs:label "Insect Infestation"@en .


###  http://www.semanticweb.org/wood#InsectInfluences
:InsectInfluences rdf:type owl:NamedIndividual ,
                           :BiologicalInfluences ,
                           :CauseOfDamage ,
                           <http://www.semanticweb.org/wooddestroying_insects#WoodDestroyingInsects> ;
                  :ChangesProperties :InsectContamination ,
                                     :MaterialSolidity ;
                  rdfs:comment "Describes superordinate classes that describe characteristics, behavior, and distribution of insects."@en ;
                  rdfs:label "Insect Influences"@en .


###  http://www.semanticweb.org/wood#InsufficientBeamDimensions
:InsufficientBeamDimensions rdf:type owl:NamedIndividual ,
                                     :CauseOfDamage ,
                                     :StaticOverstress ,
                                     :mechanicalInfluences ;
                            :ChangesProperties :GeometricChange ;
                            rdfs:comment "Insufficient beam dimensions and therefore a structural failure can occur when for example the loads were determined inaccurate."@en ;
                            rdfs:label "Insufficient Beam Dimensions"@en .


###  http://www.semanticweb.org/wood#Laminate
:Laminate rdf:type owl:NamedIndividual ,
                   :Coat ,
                   :ColourConcealed ,
                   :GrainConcealed ,
                   :RepairProcedure ;
          rdfs:comment "Wood is coated with additional solid material."@en ;
          rdfs:label "Laminate"@en .


###  http://www.semanticweb.org/wood#LaminatedVeneerLumber
:LaminatedVeneerLumber rdf:type owl:NamedIndividual ,
                                :ConstructionWood ,
                                :WoodBasedMaterials ;
                       rdfs:comment "Laminated veneer lumber is created by gluing together approximately 3 mm thick, dried veneers from softwood. There are different veneer arrangements which are distinguished."@en ;
                       rdfs:label "Laminated Veneer Lumber"@en .


###  http://www.semanticweb.org/wood#LarchEuropeanLA
:LarchEuropeanLA rdf:type owl:NamedIndividual ,
                          :HighDimensionalStability ,
                          :HighInsectResistance ,
                          :LowRotResistance ,
                          :MediumInsectResistance ,
                          :MediumRotResistance ,
                          :Softwood ,
                          :WoodTypes ;
                 rdfs:comment """Wood material of Douglas larch European trees.

Colour:
Yellowish/ reddish brown, darkens with time, late wood deep brown."""@en ;
                 rdfs:label "Larch European (LA)"@en .


###  http://www.semanticweb.org/wood#LaserMeasuringDevice
:LaserMeasuringDevice rdf:type owl:NamedIndividual ,
                               :FastProcesses ,
                               :InSitu ,
                               :InvestigationProcedure ,
                               :NonDestructiveProcesses ;
                      rdfs:comment "Laser gauges are used to measure lengths by emitting a laser that measures a distance when it collides with the nearest object."@en ;
                      rdfs:label "Laser Measuring Device"@en .


###  http://www.semanticweb.org/wood#Lathe
:Lathe rdf:type owl:NamedIndividual ,
                :RepairProcedure ,
                :Separate ,
                :Turning ;
       rdfs:comment "The lathe is a machine tool used for the manufacturing process of turning. Rotationally symmetrical workpieces are produced with a lathe."@en ;
       rdfs:label "Lathe"@en .


###  http://www.semanticweb.org/wood#LoadTest
:LoadTest rdf:type owl:NamedIndividual ,
                   :InSitu ,
                   :InvestigationProcedure ,
                   :NonDestructiveProcesses ,
                   :SlowProcesses ;
          rdfs:comment "The proof of sufficient load-bearing capacity of structures can be determined by load-bearing tests on site. The load-deformation behavior during the test provides conclusions about the remaining load-bearing capacity of the components."@en ;
          rdfs:label "Load Test"@en .


###  http://www.semanticweb.org/wood#Maceration
:Maceration rdf:type owl:NamedIndividual ,
                     :ChemicalProcesses ,
                     :GK1 ,
                     :GK2 ,
                     :GK4 ,
                     :GK5 ,
                     :Gk3point1 ,
                     :Gk3point2 ,
                     :WoodDamage ;
            :CreatedByCause :Acids ,
                            :Salts ;
            :NeedsRepairMethod :Axe ,
                               :BandSaw ,
                               :Chainsaw ,
                               :Chisel ,
                               :CircularSaw ,
                               :DrillingMachine ,
                               :FrameSaw ,
                               :Handsaw ,
                               :WoodPreservatives ;
            rdfs:comment "Intensive treatment of the wood with wood preservatives and fire proofing agents using potassium, ammonium salts or phosphate compounds causes a defibering of the outer wood structure. The structure becomes woolly, which is called maceration."@en ;
            rdfs:label "Maceration"@en .


###  http://www.semanticweb.org/wood#MapleAH
:MapleAH rdf:type owl:NamedIndividual ,
                  :Hardwood ,
                  :HighDimensionalStability ,
                  :MediumDimensionalStability ,
                  :VeryLowInsectResistance ,
                  :VeryLowRotResistance ,
                  :WoodTypes ;
         rdfs:comment """Wood material of Maple trees.

Colour: 
Yellowish white, slightly yellowing, silky glossy. Sapwood and heartwood are not distinguished.

Special properties resistance to rot:
Very low resistance to blue stain fungi.

Special properties resistance to insects:
Very low resistance to anobium."""@en ;
         rdfs:label "Maple (AH)"@en .


###  http://www.semanticweb.org/wood#MaterialSolidity
:MaterialSolidity rdf:type owl:NamedIndividual ,
                           :SearchedProperties ;
                  :NeedsInvestigationProcedure :DrillCoreTest ,
                                               :DrillingResistanceMeasurement ,
                                               :LoadTest ,
                                               :UltrasonicEchoMethod ,
                                               :XRays ;
                  rdfs:comment "Material solidity is the ability of a material to withstand mechanical stress before failure occurs. This is specified as mechanical stress."@en ;
                  rdfs:label "Material Solidity"@en .


###  http://www.semanticweb.org/wood#Measurements
:Measurements rdf:type owl:NamedIndividual ,
                       :BuildingDocumentation ,
                       :Sources ,
                       :SourcesPresentState ;
              rdfs:comment "A measurement is the process by which a value of a physical quantity is determined as a multiple of a unit."@en ;
              rdfs:label "Measurements"@en .


###  http://www.semanticweb.org/wood#MeasuringMagnifier
:MeasuringMagnifier rdf:type owl:NamedIndividual ,
                             :FastProcesses ,
                             :InSitu ,
                             :InvestigationProcedure ,
                             :NonDestructiveProcesses ;
                    rdfs:comment "A magnifying glass is a magnifying device used to see small details more closely."@en ;
                    rdfs:label "Measuring Magnifier"@en .


###  http://www.semanticweb.org/wood#MeasuringTape
:MeasuringTape rdf:type owl:NamedIndividual ,
                        :FastProcesses ,
                        :InSitu ,
                        :InvestigationProcedure ,
                        :NonDestructiveProcesses ;
               rdfs:comment "A tape measure is a haptic measuring instrument used to measure short distances."@en ;
               rdfs:label "Measuring Tape"@en .


###  http://www.semanticweb.org/wood#MeratiDarkRedMER
:MeratiDarkRedMER rdf:type owl:NamedIndividual ,
                           :Hardwood ,
                           :HighDimensionalStability ,
                           :HighInsectResistance ,
                           :HighRotResistance ,
                           :MediumInsectResistance ,
                           :MediumRotResistance ,
                           :WoodTypes ;
                  rdfs:comment """Wood material of meranti dark red trees.

Colour: 
Yellowish grey to pinkish grey/ reddish brown."""@en ;
                  rdfs:label "Merati Dark Red (MER)"@en .


###  http://www.semanticweb.org/wood#MerbauMEB
:MerbauMEB rdf:type owl:NamedIndividual ,
                    :Hardwood ,
                    :HighInsectResistance ,
                    :VeryHighDimensionalStability ,
                    :VeryHighInsectResistance ,
                    :VeryHighRotResistance ,
                    :WoodTypes ;
           rdfs:comment """Wood material of merbau trees.

Colour: 
Yellowish white/ light brown to reddish brown. Darkens after time."""@en ;
           rdfs:label "Merbau (MEB)"@en .


###  http://www.semanticweb.org/wood#MetalComponents
:MetalComponents rdf:type owl:NamedIndividual ,
                          :SearchedProperties ;
                 :NeedsInvestigationProcedure :ChangeOfColour ,
                                              :DamagePattern ,
                                              :MeasuringMagnifier ,
                                              :MetalDetector ,
                                              :Pictures ,
                                              :XRays .


###  http://www.semanticweb.org/wood#MetalDetector
:MetalDetector rdf:type owl:NamedIndividual ,
                        :InSitu ,
                        :InvestigationProcedure ,
                        :NonDestructiveProcesses ,
                        :SlowProcesses ;
               rdfs:comment "Hidden joints and metallic debris can be found with a metal detector. Also wires and power cables."@en ;
               rdfs:label "Metal Detector"@en .


###  http://www.semanticweb.org/wood#Microscopy
:Microscopy rdf:type owl:NamedIndividual ,
                     :InSitu ,
                     :InvestigationProcedure ,
                     :LowDestructiveProcesses ,
                     :SlowProcesses ;
            rdfs:comment "Further damage can be found during microscopic examination. This procedure is well suited in combination with a drill core removal."@en ;
            rdfs:label "Microscopy"@en .


###  http://www.semanticweb.org/wood#MillingMachine
:MillingMachine rdf:type owl:NamedIndividual ,
                         :Milling ,
                         :RepairProcedure ,
                         :Separate ;
                rdfs:comment "A milling machine removes material from a workpiece by cutting it into the desired shape using rotating cutting tools."@en ;
                rdfs:label "Milling Machine"@en .


###  http://www.semanticweb.org/wood#MissingPart
:MissingPart rdf:type owl:NamedIndividual ,
                      :GK1 ,
                      :GK2 ,
                      :GK4 ,
                      :GK5 ,
                      :Gk3point1 ,
                      :Gk3point2 ,
                      :MechanicalProcesses ,
                      :WoodDamage ;
             :CreatedByCause :Burning ,
                             :Explosions ,
                             :HumanRemoval ;
             :NeedsRepairMethod :Clamps ,
                                :Glue ,
                                :Nailing ,
                                :Screws ,
                                :Tenon ;
             rdfs:comment "A missing part or a gap of the material. The Possible cause is no longer evident."@en ;
             rdfs:label "Missing Part"@en .


###  http://www.semanticweb.org/wood#MoisturePenetration
:MoisturePenetration rdf:type owl:NamedIndividual ,
                              :CauseOfDamage ;
                     :ChangesProperties :AirHumidity ,
                                        :BulkDensity ,
                                        :EModulus ,
                                        :ThermalInsulation ,
                                        :WoodMoisture ;
                     rdfs:comment "Moisture penetration happens when water enters the component."@en ;
                     rdfs:label "Moisture Penetration"@en .


###  http://www.semanticweb.org/wood#Molds
:Molds rdf:type owl:NamedIndividual ,
                :BiologicalInfluences ,
                :CauseOfDamage ,
                :Rot ,
                :WoodDiscoloringFungi ;
       :ChangesProperties :PHValue ,
                          :RotContamination ,
                          :WoodMoisture ;
       rdfs:comment """Preferred wood species:
Softwood and hardwood.

Further notes:
Surface growth on the wood."""@en ;
       rdfs:label "Molds"@en .


###  http://www.semanticweb.org/wood#MusselCrempling
:MusselCrempling rdf:type owl:NamedIndividual ,
                          :BiologicalInfluences ,
                          :BrownRot ,
                          :CauseOfDamage ,
                          :Rot ,
                          :WetRotFungi ;
                 :ChangesProperties :MaterialSolidity ,
                                    :PHValue ,
                                    :RotContamination ,
                                    :WoodMoisture ;
                 rdfs:comment """Preferred wood species:
Softwood and rarely Hardwood.

Optimal living conditions of wood moisture content in M-%:
50% to 70%

Optimal living conditions of the temperature range in °C:
23°C to 26°C

Additional notes:
Mycelium dies when dried out."""@en ;
                 rdfs:label "Mussel Crempling"@en ,
                            "Paxillus panuoides"@la .


###  http://www.semanticweb.org/wood#Nailing
:Nailing rdf:type owl:NamedIndividual ,
                  :ForceFit ,
                  :Join ,
                  :RepairProcedure ,
                  :Unsolvable ;
         rdfs:comment "A nail is a pin that contains a head."@en ;
         rdfs:label "Nailing"@en .


###  http://www.semanticweb.org/wood#Norms
:Norms rdf:type owl:NamedIndividual ,
                :ExternalResources ,
                :Sources ,
                :SourcesTargetState ;
       rdfs:comment "Norming refers to the formulation, issuance, and application of rules, guidelines, or characteristics by a recognized organization and its standardization bodies."@en ;
       rdfs:label "Norms"@en .


###  http://www.semanticweb.org/wood#OakEI
:OakEI rdf:type owl:NamedIndividual ,
                :Hardwood ,
                :HighInsectResistance ,
                :HighRotResistance ,
                :MediumDimensionalStability ,
                :WoodTypes ;
       rdfs:comment """Wood material of oak trees.

Colour: 
Grey/ greyish yellow. Darkens to light/ dark brown."""@en ;
       rdfs:label "Oak (EI)"@en .


###  http://www.semanticweb.org/wood#OakWhorling
:OakWhorling rdf:type owl:NamedIndividual ,
                      :BiologicalInfluences ,
                      :BrownRot ,
                      :CauseOfDamage ,
                      :Rot ,
                      :WetRotFungi ;
             :ChangesProperties :MaterialSolidity ,
                                :PHValue ,
                                :RotContamination ,
                                :WoodMoisture ;
             rdfs:comment """Preferred wood species:
Oak wood.

Optimal living conditions of wood moisture content in M-%:
>50%"""@en ;
             rdfs:label "Daedalia quercina"@la ,
                        "Oak Whorling"@en .


###  http://www.semanticweb.org/wood#Oil
:Oil rdf:type owl:NamedIndividual ,
              :Coat ,
              :ColourEmphasized ,
              :GrainEmphasized ,
              :RepairProcedure ;
     rdfs:comment "Oiling is the treatment of the surface with Oil. The wood grain and color are emphasized."@en ;
     rdfs:label "Oil"@en .


###  http://www.semanticweb.org/wood#OrientedStrandBoardOSB
:OrientedStrandBoardOSB rdf:type owl:NamedIndividual ,
                                 :ConstructionWood ,
                                 :WoodBasedMaterials ;
                        rdfs:comment "The production of OSB is made by gluing together larger chips. The chips are approx. 0.6 mm thick, 75 mm to 130 mm long and approx. 35 mm wide. They lie in the surface layer predominantly in the direction of the longitudinal side of the board and in the middle layer transverse to it. OSB has depending on the direction of the chips different strength properties."@en ;
                        rdfs:label "Oriented Strand Board (OSB)"@en .


###  http://www.semanticweb.org/wood#PHMeter
:PHMeter rdf:type owl:NamedIndividual ,
                  :InSitu ,
                  :InvestigationProcedure ,
                  :NonDestructiveProcesses ,
                  :SlowProcesses ;
         rdfs:comment "Detection of brown rot fungi by measuring the concentration of oxalic acid. During the decomposition of wood substance by brown rot, oxalic acid is produced, reducing the pH of the wood from pH = 5 to pH = 3. In the field, a simple color reaction test provides evidence of active fungal attack. The blue color of the indicator turns to green, yellow, when infestation is present. For chemical analysis in the laboratory, only small amounts of a sample of approx. 2 to 5 g are required."@en ;
         rdfs:label "PH-Meter"@en .


###  http://www.semanticweb.org/wood#PHValue
:PHValue rdf:type owl:NamedIndividual ,
                  :SearchedProperties ;
         :NeedsInvestigationProcedure :IndicatorPaper ,
                                      :PHMeter ;
         rdfs:comment "The PH value is a measure of the acidic or basic character of an aqueous solution."@en ;
         rdfs:label "PH Value"@en .


###  http://www.semanticweb.org/wood#PenetrationResistanceTest
:PenetrationResistanceTest rdf:type owl:NamedIndividual ,
                                    :FastProcesses ,
                                    :InSitu ,
                                    :InvestigationProcedure ,
                                    :LowDestructiveProcesses ;
                           rdfs:comment "In the penetration resistance test, a pointed tool, such as a chisel, is used to pierce the material. The resistance during penetration gives information about the condition of the material."@en ;
                           rdfs:label "Penetration Resistance Test"@en .


###  http://www.semanticweb.org/wood#PhotoDocumentation
:PhotoDocumentation rdf:type owl:NamedIndividual ,
                             :BuildingDocumentation ,
                             :Sources ,
                             :SourcesPresentState ;
                    rdfs:comment "A photo documentation of the area is carried out."@en ;
                    rdfs:label "Photo documentation"@en .


###  http://www.semanticweb.org/wood#Photogrammetry
:Photogrammetry rdf:type owl:NamedIndividual ,
                         :InSitu ,
                         :InvestigationProcedure ,
                         :LowDestructiveProcesses ,
                         :SlowProcesses ;
                rdfs:comment "Photogrammetry is a measuring method or evaluation procedure to indirectly determine the position and shape of an object from photographs by image measurement."@en ;
                rdfs:label "Photogrammetry"@en .


###  http://www.semanticweb.org/wood#Pictures
:Pictures rdf:type owl:NamedIndividual ,
                   :FastProcesses ,
                   :InSitu ,
                   :InvestigationProcedure ,
                   :NonDestructiveProcesses ;
          rdfs:comment "A photograph is an image created by light falling on a photosensitive surface."@en ;
          rdfs:label "Pictures"@en .


###  http://www.semanticweb.org/wood#PineKI
:PineKI rdf:type owl:NamedIndividual ,
                 :HighDimensionalStability ,
                 :LowInsectResistance ,
                 :LowRotResistance ,
                 :MediumDimensionalStability ,
                 :MediumRotResistance ,
                 :Softwood ,
                 :WoodTypes ;
        rdfs:comment """Wood material of pine trees.

Colour:
Light yellowish white/ reddish white, browning after time, late wood darker.


Special properties resistance to fungi:
Sapwood very sensitive to blue stain."""@en ;
        rdfs:label "Pine (KI)"@en .


###  http://www.semanticweb.org/wood#PinePIP
:PinePIP rdf:type owl:NamedIndividual ,
                  :HighDimensionalStability ,
                  :LowInsectResistance ,
                  :LowRotResistance ,
                  :MediumDimensionalStability ,
                  :MediumInsectResistance ,
                  :MediumRotResistance ,
                  :Softwood ,
                  :WoodTypes ;
         rdfs:comment """Wood material of pine trees.

Colour:
Yellowish/ reddish yellow to reddish brown/ late wood is dark.

Special properties resistance to fungi:
Different vulnerabilities for heartwood and sapwood. Sapwood has a low sensitivity; heartwood has a medium sensitivity."""@en ;
         rdfs:label "Pine (PIP)"@en .


###  http://www.semanticweb.org/wood#Planer
:Planer rdf:type owl:NamedIndividual ,
                 :Planing ,
                 :RepairProcedure ,
                 :Separate ;
        rdfs:comment "The planer is a tool where the surface of the wood is machined by removing chips from the material with the plane iron."@en ;
        rdfs:label "Planer"@en .


###  http://www.semanticweb.org/wood#ProfileBoards
:ProfileBoards rdf:type owl:NamedIndividual ,
                        :ConstructionWood ,
                        :SolidWood ;
               rdfs:comment "Planed and profiled lumber is sawn from round timber and then planed and milled."@en ;
               rdfs:label "Profile Boards"@en .


###  http://www.semanticweb.org/wood#Protocols
:Protocols rdf:type owl:NamedIndividual ,
                    :BuildingDocumentation ,
                    :Sources ,
                    :SourcesPresentState ;
           rdfs:comment "A record is a verbatim transcript, or a transcript limited to the essential points, of a meeting, negotiation, or conversation."@en ;
           rdfs:label "Protocols"@en .


###  http://www.semanticweb.org/wood#RadiocarbonMethod
:RadiocarbonMethod rdf:type owl:NamedIndividual ,
                            :InvestigationProcedure ,
                            :Laboratory ,
                            :LowDestructiveProcesses ,
                            :SlowProcesses ;
                   rdfs:comment "Radioactive age determination means the determination of the age of objects based on the radionuclides they contain."@en ;
                   rdfs:label "Radiocarbon Method"@en .


###  http://www.semanticweb.org/wood#Reagents
:Reagents rdf:type owl:NamedIndividual ,
                   :InvestigationProcedure ,
                   :Laboratory ,
                   :LowDestructiveProcesses ,
                   :SlowProcesses ;
          rdfs:comment "Detection reagents are used to detect the increased content of salts and other substances."@en ;
          rdfs:label "Reagents"@en .


###  http://www.semanticweb.org/wood#Records
:Records rdf:type owl:NamedIndividual ,
                  :BuildingDocumentation ,
                  :Sources ,
                  :SourcesPresentState ;
         rdfs:comment "A record is a thing that is evidence of the past, especially a report that is recorded in writing or other permanent form."@en ;
         rdfs:label "Records"@en .


###  http://www.semanticweb.org/wood#ReductionInLoadCapacityDueToWear
:ReductionInLoadCapacityDueToWear rdf:type owl:NamedIndividual ,
                                           :CauseOfDamage ,
                                           :ServiceStresses ,
                                           :mechanicalInfluences ;
                                  :ChangesProperties :EModulus ,
                                                     :GeometricChange ,
                                                     :MaterialSolidity ;
                                  rdfs:comment "Reduction in load capacity due to wear of the component. This can happen if the component has been used incorrectly or if the maximum age of the component has been exceeded."@en ;
                                  rdfs:label "Reduction In Load Capacity Due To Wear"@en .


###  http://www.semanticweb.org/wood#Regulations
:Regulations rdf:type owl:NamedIndividual ,
                      :ExternalResources ,
                      :Sources ,
                      :SourcesTargetState ;
             rdfs:comment "Building regulations come from the laws of the country in which the building project is located. The building codes are regulations that dictate the building process."@en ;
             rdfs:label "Regulations"@en .


###  http://www.semanticweb.org/wood#Report
:Report rdf:type owl:NamedIndividual ,
                 :Report .


###  http://www.semanticweb.org/wood#RobiniaROB
:RobiniaROB rdf:type owl:NamedIndividual ,
                     :Hardwood ,
                     :HighInsectResistance ,
                     :MediumDimensionalStability ,
                     :VeryHighRotResistance ,
                     :WoodTypes ;
            rdfs:comment """Wood material of Robinia trees.

Colour: 
Light yellow to greenish yellow to olive green. Later shiny golden brown."""@en ;
            rdfs:label "Robinia (ROB)"@en .


###  http://www.semanticweb.org/wood#RotContamination
:RotContamination rdf:type owl:NamedIndividual ,
                           :SearchedProperties ;
                  :NeedsInvestigationProcedure :ChangeOfColour ,
                                               :Chromatography ,
                                               :DNAAnalysis ,
                                               :DamagePattern ,
                                               :DrillingResistanceMeasurement ,
                                               :DrillingTest ,
                                               :IndicatorPaper ,
                                               :MeasuringMagnifier ,
                                               :PHMeter ,
                                               :PenetrationResistanceTest ,
                                               :Pictures .


###  http://www.semanticweb.org/wood#RotInfestation
:RotInfestation rdf:type owl:NamedIndividual ,
                         :BiologicalProcesses ,
                         :GK2 ,
                         :GK4 ,
                         :GK5 ,
                         :Gk3point1 ,
                         :Gk3point2 ,
                         :WoodDamage ;
                :CreatedByCause :BeamLeafling ,
                                :BlueStainFungi ,
                                :BrownCellarSponge ,
                                :ButterflySpore ,
                                :DryRot ,
                                :FenceLeaflet ,
                                :FirLeafBlossom ,
                                :MoisturePenetration ,
                                :Molds ,
                                :MusselCrempling ,
                                :OakWhorling ,
                                :ScalySawfly ,
                                :WhiteSporeSponge ;
                :NeedsRepairMethod :Axe ,
                                   :BandSaw ,
                                   :Chainsaw ,
                                   :Chisel ,
                                   :CircularSaw ,
                                   :DrillingMachine ,
                                   :File ,
                                   :FrameSaw ,
                                   :Fumigant ,
                                   :GrindingMachine ,
                                   :Handsaw ,
                                   :Sandpaper ,
                                   :Scraper ,
                                   :WoodPreservatives ;
                rdfs:comment "An infestation of the wood substance by rot."@en ;
                rdfs:label "Rot Infestation"@en .


###  http://www.semanticweb.org/wood#Roundwood
:Roundwood rdf:type owl:NamedIndividual ,
                    :ConstructionWood ,
                    :SolidWood ;
           rdfs:comment "Roundwood consists of logs or log sections."@en ;
           rdfs:label "Roundwood"@en .


###  http://www.semanticweb.org/wood#Salinity
:Salinity rdf:type owl:NamedIndividual ,
                   :SearchedProperties ;
          :NeedsInvestigationProcedure :Reagents ;
          rdfs:comment "Salinity refers to the salt content of a component."@en ;
          rdfs:label "Salinity"@en .


###  http://www.semanticweb.org/wood#Salts
:Salts rdf:type owl:NamedIndividual ,
                :CauseOfDamage ,
                :ChemicalInfluences ;
       :ChangesProperties :ChemicalReaction ,
                          :EModulus ,
                          :MaterialSolidity ,
                          :PHValue ,
                          :Salinity ;
       rdfs:comment "In case of overdosage of salt-containing wood preservatives on wooden components, maceration is likely to occur. The salt can also be washed out of clay bricks or lime mortar."@en ;
       rdfs:label "Salts"@en .


###  http://www.semanticweb.org/wood#Sandpaper
:Sandpaper rdf:type owl:NamedIndividual ,
                    :Grinding ,
                    :RepairProcedure ,
                    :Separate ;
           rdfs:comment "Sandpaper is used to smooth rough surfaces or to break edges. It is also suitable for larger material removal."@en ;
           rdfs:label "Sandpaper"@en .


###  http://www.semanticweb.org/wood#ScalySawfly
:ScalySawfly rdf:type owl:NamedIndividual ,
                      :BiologicalInfluences ,
                      :BrownRot ,
                      :CauseOfDamage ,
                      :Leaflet ,
                      :Rot ;
             :ChangesProperties :MaterialSolidity ,
                                :PHValue ,
                                :RotContamination ,
                                :WoodMoisture ;
             rdfs:comment """Preferred wood species:
Hardwood.

Optimal living conditions of wood moisture content in M-%:
30% to 40%

Optimal living conditions of the temperature range in °C:
26°C to 35°C

Additional notes:
Mycelium dies after prolonged dehydration."""@en ;
             rdfs:label "Lentinus lepideus"@la ,
                        "Scaly Sawfly"@en .


###  http://www.semanticweb.org/wood#Scraper
:Scraper rdf:type owl:NamedIndividual ,
                  :RepairProcedure ,
                  :Scraping ,
                  :Separate ;
         rdfs:comment "A scraper is a tool provided with at least one cutting edge for scraping."@en ;
         rdfs:label "Scraper"@en .


###  http://www.semanticweb.org/wood#Screws
:Screws rdf:type owl:NamedIndividual ,
                 :ForceFit ,
                 :Join ,
                 :RepairProcedure ,
                 :Solvable ;
        rdfs:comment "A screw is a connecting element that has a thread."@en ;
        rdfs:label "Screws"@en .


###  http://www.semanticweb.org/wood#Shocks
:Shocks rdf:type owl:NamedIndividual ,
                 :CauseOfDamage ,
                 :DynamicOverstress ,
                 :mechanicalInfluences ;
        :ChangesProperties :MaterialSolidity ;
        rdfs:comment "Shocks can occur due to construction work or even traffic."@en ;
        rdfs:label "Shocks"@en .


###  http://www.semanticweb.org/wood#SolidStructuralTimber
:SolidStructuralTimber rdf:type owl:NamedIndividual ,
                                :ConstructionWood ,
                                :SolidWood ;
                       rdfs:comment "Is made from higher quality building timber products regarding dimensional accuracy, dimensional stability, reduced cracking and surface quality."@en ;
                       rdfs:label "Solid Structural Timber"@en .


###  http://www.semanticweb.org/wood#SoundTest
:SoundTest rdf:type owl:NamedIndividual ,
                    :FastProcesses ,
                    :InSitu ,
                    :InvestigationProcedure ,
                    :NonDestructiveProcesses ;
           rdfs:comment "By tapping the suspect area, conclusions can be drawn about the condition of the material or cavities."@en ;
           rdfs:label "Sound Test"@en .


###  http://www.semanticweb.org/wood#SpruceFI
:SpruceFI rdf:type owl:NamedIndividual ,
                   :HighDimensionalStability ,
                   :LowInsectResistance ,
                   :LowRotResistance ,
                   :Softwood ,
                   :WoodTypes ;
          rdfs:comment """Wood material of spruce trees.

Colour:
Early wood yellowish white, late wood reddish yellow, sapwood and heartwood are not distinguished.

Special properties resistance to fungi:
Sensitive to blue stain."""@en ;
          rdfs:label "Spruce (FI)"@en .


###  http://www.semanticweb.org/wood#Stain
:Stain rdf:type owl:NamedIndividual ,
                :Coat ,
                :ColourEmphasized ,
                :GrainRemainsVisible ,
                :RepairProcedure ;
       rdfs:comment "Staining is the treatment of the surface with a chemical solution known as stain. The wood grain remains visible."@en ;
       rdfs:label "Stain"@en .


###  http://www.semanticweb.org/wood#SteelBrush
:SteelBrush rdf:type owl:NamedIndividual ,
                     :BrushMachining ,
                     :RepairProcedure ,
                     :Separate ;
            rdfs:comment "A brush consists of a base body and a brush trim. It belongs to the method of machining without a geometrically defined cutting edge."@en ;
            rdfs:label "Steel Brush"@en .


###  http://www.semanticweb.org/wood#Stethoscope
:Stethoscope rdf:type owl:NamedIndividual ,
                      :InSitu ,
                      :InvestigationProcedure ,
                      :NonDestructiveProcesses ,
                      :SlowProcesses ;
             rdfs:comment "The stethoscope can be used to detect sewing noises from active insect infestations."@en ;
             rdfs:label "Stethoscope"@en .


###  http://www.semanticweb.org/wood#SurfacePlaner
:SurfacePlaner rdf:type owl:NamedIndividual ,
                        :Planing ,
                        :RepairProcedure ,
                        :Separate ;
               rdfs:comment "The jointer is a tool for smoothing and planing wood or wood materials."@en ;
               rdfs:label "Surface Planer"@en .


###  http://www.semanticweb.org/wood#TeakTEK
:TeakTEK rdf:type owl:NamedIndividual ,
                  :Hardwood ,
                  :VeryHighDimensionalStability ,
                  :VeryHighInsectResistance ,
                  :VeryHighRotResistance ,
                  :WoodTypes ;
         rdfs:comment """Wood material of teak trees.

Colour:
Grey/ golden yellow, later medium/ to dark brown. Often narrow black veins. Shiny surface.

Special properties resistance to insects:
Termite-proof."""@en ;
         rdfs:label "Teak (TEK)"@en .


###  http://www.semanticweb.org/wood#TechnicalLiterature
:TechnicalLiterature rdf:type owl:NamedIndividual ,
                              :ExternalResources ,
                              :Sources ,
                              :SourcesTargetState ;
                     rdfs:comment "Technical literature is a subset of literature. It is for a specialized audience that is mostly focused on professional application or acquiring new scientific knowledge."@en ;
                     rdfs:label "Technical Literature"@en .


###  http://www.semanticweb.org/wood#TechnicalPlans
:TechnicalPlans rdf:type owl:NamedIndividual ,
                         :BuildingDocumentation ,
                         :Sources ,
                         :SourcesPresentState ;
                rdfs:comment "A technical drawing is a graphic document used to represent in graphic and sometimes also in written form information about components."@en ;
                rdfs:label "Technical Plans"@en .


###  http://www.semanticweb.org/wood#Tenon
:Tenon rdf:type owl:NamedIndividual ,
                :FormFitting ,
                :Join ,
                :RepairProcedure ,
                :Solvable ;
       rdfs:comment "A mortise joint is a wood joint in carpentry. It consists of a tenon and the mortise."@en ;
       rdfs:label "Tenon"@en .


###  http://www.semanticweb.org/wood#Theodolite
:Theodolite rdf:type owl:NamedIndividual ,
                     :InSitu ,
                     :InvestigationProcedure ,
                     :NonDestructiveProcesses ,
                     :SlowProcesses ;
            rdfs:comment "A theodolite is an angle measuring instrument used to measure horizontal directions and zenith or vertical angles."@en ;
            rdfs:label "Theodolite"@en .


###  http://www.semanticweb.org/wood#ThermalInsulation
:ThermalInsulation rdf:type owl:NamedIndividual ,
                            :SearchedProperties ;
                   :NeedsInvestigationProcedure :BlowerDoorTest ,
                                                :Thermography ;
                   rdfs:comment "Thermal insulation is the reduction of heat transfer between objects in thermal contact or in radiation influence to each other."@en ;
                   rdfs:label "Thermal Insulation"@en .


###  http://www.semanticweb.org/wood#Thermography
:Thermography rdf:type owl:NamedIndividual ,
                       :InSitu ,
                       :InvestigationProcedure ,
                       :NonDestructiveProcesses ,
                       :SlowProcesses ;
              rdfs:comment "Thermography can be used to record the thermal radiation of an object. This allows conclusions to be drawn about thermal bridges and causes of moisture."@en ;
              rdfs:label "Thermography"@en .


###  http://www.semanticweb.org/wood#ThicknessPlaner
:ThicknessPlaner rdf:type owl:NamedIndividual ,
                          :Planing ,
                          :RepairProcedure ,
                          :Separate ;
                 rdfs:comment "A thickness planer planes a workpiece to a desired thickness."@en ;
                 rdfs:label "Thickness Planer"@en .


###  http://www.semanticweb.org/wood#ThreeFiveLayerBoards
:ThreeFiveLayerBoards rdf:type owl:NamedIndividual ,
                               :ConstructionWood ,
                               :WoodBasedMaterials ;
                      rdfs:comment "The boards consist of three or five layers of boards, which are crossed at right angles, laid on top of each other and glued together. The strength properties have a very wide range. They can be controlled by the quality of the wood used and the thickness ratios of the individual layers."@en ;
                      rdfs:label "Three/Five Layer Boards"@en .


###  http://www.semanticweb.org/wood#TooHighLoadsFromDeposition
:TooHighLoadsFromDeposition rdf:type owl:NamedIndividual ,
                                     :CauseOfDamage ,
                                     :StaticOverstress ,
                                     :mechanicalInfluences ;
                            :ChangesProperties :GeometricChange ;
                            rdfs:comment "Overstresses on the component that result from created deposition. This could occur for example in a salt deposit."@en ;
                            rdfs:label "Too High Loads From Deposition"@en .


###  http://www.semanticweb.org/wood#TooHighSnowLoads
:TooHighSnowLoads rdf:type owl:NamedIndividual ,
                           :CauseOfDamage ,
                           :StaticOverstress ,
                           :mechanicalInfluences ;
                  :ChangesProperties :GeometricChange ;
                  rdfs:comment "Overstresses on the component that result from not calculated snow loads."@en ;
                  rdfs:label "Too High Snow Loads"@en .


###  http://www.semanticweb.org/wood#UltrasonicEchoMethod
:UltrasonicEchoMethod rdf:type owl:NamedIndividual ,
                               :InSitu ,
                               :InvestigationProcedure ,
                               :NonDestructiveProcesses ,
                               :SlowProcesses ;
                      rdfs:comment "An ultrasonic pulse is emitted, and the speed is determined. To calculate the E-modulus, the bulk density is also required."@en ;
                      rdfs:label "Ultrasonic Echo Method"@en .


###  http://www.semanticweb.org/wood#Vibrations
:Vibrations rdf:type owl:NamedIndividual ,
                     :CauseOfDamage ,
                     :DynamicOverstress ,
                     :mechanicalInfluences ;
            :ChangesProperties :GeometricChange ;
            rdfs:comment "Vibrations from usage or natural disasters can cause cracks, delocalization, and fastener failures."@en ;
            rdfs:label "Vibrations"@en .


###  http://www.semanticweb.org/wood#WashoutStresses
:WashoutStresses rdf:type owl:NamedIndividual ,
                          :ChemicalProcesses ,
                          :GK4 ,
                          :GK5 ,
                          :Gk3point1 ,
                          :Gk3point2 ,
                          :WoodDamage ;
                 :CreatedByCause :MoisturePenetration ;
                 :NeedsRepairMethod :Axe ,
                                    :BandSaw ,
                                    :Chainsaw ,
                                    :Chisel ,
                                    :CircularSaw ,
                                    :DrillingMachine ,
                                    :FrameSaw ,
                                    :Glaze ,
                                    :Handsaw ,
                                    :Laminate ,
                                    :Scraper ;
                 rdfs:comment "In the case of wooden components with direct rainfall, the wood's natural adhesive, lignin, is gradually washed out of the pores. This weakens the wood, and it is more susceptible to damage from UV radiation and insects that can penetrate the interior of the wood."@en ;
                 rdfs:label "Washout Stresses"@en .


###  http://www.semanticweb.org/wood#Wax
:Wax rdf:type owl:NamedIndividual ,
              :Coat ,
              :ColourEmphasized ,
              :GrainEmphasized ,
              :RepairProcedure ;
     rdfs:comment "Waxing is the treatment of the surface with wax. The wood grain and color are emphasized."@en ;
     rdfs:label "Wax"@en .


###  http://www.semanticweb.org/wood#WesternHemlockHEM
:WesternHemlockHEM rdf:type owl:NamedIndividual ,
                            :HighDimensionalStability ,
                            :LowInsectResistance ,
                            :LowRotResistance ,
                            :MediumRotResistance ,
                            :Softwood ,
                            :WoodTypes ;
                   rdfs:comment """Wood material of western hemlock trees.

Colour:
Early wood light brownish grey, occasionally lighter stripes, late wood darkens with time, sapwood and heartwood is not distinguished."""@en ;
                   rdfs:label "Western Hemlock (HEM)"@en .


###  http://www.semanticweb.org/wood#WesternRedcedarRCW
:WesternRedcedarRCW rdf:type owl:NamedIndividual ,
                             :Softwood ,
                             :VeryHighDimensionalStability ,
                             :VeryHighInsectResistance ,
                             :VeryHighRotResistance ,
                             :WoodTypes ;
                    rdfs:comment """Wood material of western redcedar trees.

Colour:
White/ reddish brown, darkens with time, late wood darker."""@en ;
                    rdfs:label "Western Redcedar (RCW)"@en .


###  http://www.semanticweb.org/wood#WhiteSporeSponge
:WhiteSporeSponge rdf:type owl:NamedIndividual ,
                           :BiologicalInfluences ,
                           :CauseOfDamage ,
                           :Rot ,
                           :WetRotFungi ,
                           :WhiteRot ;
                  :ChangesProperties :MaterialSolidity ,
                                     :PHValue ,
                                     :RotContamination ,
                                     :WoodMoisture ;
                  rdfs:comment """Preferred wood species:
Softwood and hardwood.

Optimal living conditions of wood moisture content in M-%:
35% to 50%

Optimal living conditions of the temperature range in °C:
25°C to 31°C

Additional notes:
Long dry rigidity possible."""@en ;
                  rdfs:label "Poria vaillantii"@la ,
                             "White Spore Sponge"@en .


###  http://www.semanticweb.org/wood#WindLoads
:WindLoads rdf:type owl:NamedIndividual ,
                    :CauseOfDamage ,
                    :DynamicOverstress ,
                    :mechanicalInfluences ;
           :ChangesProperties :GeometricChange ;
           rdfs:comment "Extreme wind conditions that were not planned for and lead to failure of the component."@en ;
           rdfs:label "Wind Loads"@en .


###  http://www.semanticweb.org/wood#WoodAge
:WoodAge rdf:type owl:NamedIndividual ,
                  :SearchedProperties ;
         :NeedsInvestigationProcedure :ChangeOfColour ,
                                      :DamagePattern ,
                                      :Dendrochronology ,
                                      :DrillCoreTest ,
                                      :DrillingTest ,
                                      :MeasuringMagnifier ,
                                      :Microscopy ,
                                      :Pictures ,
                                      :RadiocarbonMethod .


###  http://www.semanticweb.org/wood#WoodComponent
:WoodComponent rdf:type owl:NamedIndividual ,
                        :WoodComponent .


###  http://www.semanticweb.org/wood#WoodFiberBoards
:WoodFiberBoards rdf:type owl:NamedIndividual ,
                          :ConstructionWood ,
                          :WoodBasedMaterials ;
                 rdfs:comment "Wood fiberboards are produced using the dry process with binders or in the wet process without binders by strong pressing. The bonding is based on the felting of the fibers and their own bonding ability."@en ;
                 rdfs:label "Wood Fiber Boards"@en .


###  http://www.semanticweb.org/wood#WoodFiberInsulationBoards
:WoodFiberInsulationBoards rdf:type owl:NamedIndividual ,
                                    :ConstructionWood ,
                                    :WoodBasedMaterials ;
                           rdfs:comment "Wood fiber insulation boards are made in a wet process from wood fibers. They have a higher insulation factor than regular wood fiber boards. The bond is based on the felting of the fibers as well as their own bonding ability. The gross density is max. 400 kg/m."@en ;
                           rdfs:label "Wood Fiber Insulation Boards"@en .


###  http://www.semanticweb.org/wood#WoodMoisture
:WoodMoisture rdf:type owl:NamedIndividual ,
                       :SearchedProperties ;
              :NeedsInvestigationProcedure :DrillCoreTest ,
                                           :DrillingTest ,
                                           :ElectricalResistance ,
                                           :GravimetricMethod ,
                                           :SoundTest ;
              rdfs:comment "Wood moisture indicates the degree of presence of water in or on a wooden component."@en ;
              rdfs:label "Wood Moisture"@en .


###  http://www.semanticweb.org/wood#WoodPreservatives
:WoodPreservatives rdf:type owl:NamedIndividual ,
                            :PropertiesChange ,
                            :RepairProcedure ;
                   rdfs:comment "Wood preservatives are intended to prevent infestation of wood or wood-based materials by wood-destroying organisms or to combat such infestation."@en ;
                   rdfs:label "Wood Preservatives"@en .


###  http://www.semanticweb.org/wood#WoodSpecies
:WoodSpecies rdf:type owl:NamedIndividual ,
                      :SearchedProperties ;
             :NeedsInvestigationProcedure :ChangeOfColour ,
                                          :DamagePattern ,
                                          :Dendrochronology ,
                                          :DrillCoreTest ,
                                          :DrillingTest ,
                                          :MeasuringMagnifier ,
                                          :Microscopy ,
                                          :Pictures ;
             rdfs:comment "Wood species are subcategories of wood that have characteristic distinctions."@en ;
             rdfs:label "Wood Species"@en .


###  http://www.semanticweb.org/wood#WoodWoolLightweightPanels
:WoodWoolLightweightPanels rdf:type owl:NamedIndividual ,
                                    :ConstructionWood ,
                                    :WoodBasedMaterials ;
                           rdfs:comment "Wood wool lightweight panels are made from wood wool and mineral binders such as cement."@en ;
                           rdfs:label "Wood Wool Lightweight Panels"@en .


###  http://www.semanticweb.org/wood#XRays
:XRays rdf:type owl:NamedIndividual ,
                :InSitu ,
                :InvestigationProcedure ,
                :NonDestructiveProcesses ,
                :SlowProcesses ;
       rdfs:comment "The X-ray method can be used to obtain images of the internal wood structure and joints. An in-situ application is possible with appropriate equipment."@en ;
       rdfs:label "X-Rays"@en .


###  http://www.semanticweb.org/wood#3DLaserScanning
<http://www.semanticweb.org/wood#3DLaserScanning> rdf:type owl:NamedIndividual ,
                                                           :InSitu ,
                                                           :InvestigationProcedure ,
                                                           :NonDestructiveProcesses ,
                                                           :SlowProcesses ;
                                                  rdfs:comment "Laser scanning refers to the line or grid-like sweeping of a body with a laser beam in order to measure it or to generate an 3D image."@en ;
                                                  rdfs:label "3D Laser Scanning"@en .


#################################################################
#    Annotations
#################################################################

:ChemicalReaction rdfs:comment "A chemical reaction is a process in which one or usually multiple chemical compounds are converted into others and energy is released or absorbed."@en ;
                  rdfs:label "Chemical Reaction"@en .


:Client rdfs:comment "A person who conducts a transaction with a counterparty."@en ;
        rdfs:label "Client"@en .


:ConcealedComponents rdfs:comment "Concealed components are components that are not directly visible to the viewer."@en ;
                     rdfs:label "Concealed Components"@en .


:Contracts rdfs:comment "A contract is a legal agreement between two or more partners."@en ;
           rdfs:label "Contracts"@en .


:GeometricChange rdfs:comment "Geometric deformation of a body is the change of its shape due to the action of an external force."@en ;
                 rdfs:label "Geometric Change"@en .


:InsectContamination rdfs:comment "Insect contamination is the condition of infestation of the component caused by insects."@en ;
                     rdfs:label "Insect Contamination"@en .


:MetalComponents rdfs:comment "Metal components that are inside or on the surface of the component."@en ;
                 rdfs:label "Metal Components"@en .


:Report rdfs:comment "A report is a document that is commissioned by an expert for a court or by a private person, it is to be prepared objectively and impartially. It is presented in a way that is understandable for a layperson and fully comprehensible for an expert. A report is a reasoned presentation of empirical principles and the derivation of conclusions for the actual assessment of an occurrence."@en ;
        rdfs:label "Report"@en .


:RotContamination rdfs:comment "Rot contamination is the condition of infestation on the component caused by Rot."@en ;
                  rdfs:label "Rot Contamination"@en .


:WoodAge rdfs:comment "Age of the wood determined by appropriate examination procedures."@en ;
         rdfs:label "Wood Age"@en .


:WoodComponent rdfs:comment "List of essential properties of wooden components."@en ;
               rdfs:label "Wood component"@en .


#################################################################
#    General axioms
#################################################################

[ rdf:type owl:AllDisjointClasses ;
  owl:members ( :BrushMachining
                :Carving
                :Drilling
                :Filing
                :Grinding
                :Milling
                :Planing
                :Sawing
                :Scraping
                :Splitting
                :Turning
              )
] .


[ rdf:type owl:AllDisjointClasses ;
  owl:members ( :BuildingOwner
                :Client
                :Worker
              )
] .


[ rdf:type owl:AllDisjointClasses ;
  owl:members ( :Cause
                :Costs
                :Evaluation
                :LocalFindings
                :Restoration
                :UsedMethods
              )
] .


[ rdf:type owl:AllDisjointClasses ;
  owl:members ( :DestructiveProcesses
                :LowDestructiveProcesses
                :NonDestructiveProcesses
              )
] .


[ rdf:type owl:AllDisjointClasses ;
  owl:members ( :ForceFit
                :FormFitting
                :MeltLocking
              )
] .


[ rdf:type owl:AllDisjointClasses ;
  owl:members ( :GrainConcealed
                :GrainEmphasized
                :GrainRemainsVisible
              )
] .


#################################################################
#    Rules
#################################################################

:a rdf:type <http://www.w3.org/2003/11/swrl#Variable> .

:b rdf:type <http://www.w3.org/2003/11/swrl#Variable> .

:c rdf:type <http://www.w3.org/2003/11/swrl#Variable> .

[ <http://swrl.stanford.edu/ontologies/3.3/swrla.owl#isRuleEnabled> "true"^^xsd:boolean ;
   rdfs:label "MaterialSolidityInactive" ;
   rdf:type <http://www.w3.org/2003/11/swrl#Imp> ;
   <http://www.w3.org/2003/11/swrl#body> [ rdf:type <http://www.w3.org/2003/11/swrl#AtomList> ;
                                           rdf:first [ rdf:type <http://www.w3.org/2003/11/swrl#ClassAtom> ;
                                                       <http://www.w3.org/2003/11/swrl#classPredicate> :SearchedProperties ;
                                                       <http://www.w3.org/2003/11/swrl#argument1> :a
                                                     ] ;
                                           rdf:rest [ rdf:type <http://www.w3.org/2003/11/swrl#AtomList> ;
                                                      rdf:first [ rdf:type <http://www.w3.org/2003/11/swrl#DatavaluedPropertyAtom> ;
                                                                  <http://www.w3.org/2003/11/swrl#propertyPredicate> :NormalMaterialSolidity ;
                                                                  <http://www.w3.org/2003/11/swrl#argument1> :a ;
                                                                  <http://www.w3.org/2003/11/swrl#argument2> :b
                                                                ] ;
                                                      rdf:rest [ rdf:type <http://www.w3.org/2003/11/swrl#AtomList> ;
                                                                 rdf:first [ rdf:type <http://www.w3.org/2003/11/swrl#DatavaluedPropertyAtom> ;
                                                                             <http://www.w3.org/2003/11/swrl#propertyPredicate> :ChangedMaterialSolidity ;
                                                                             <http://www.w3.org/2003/11/swrl#argument1> :a ;
                                                                             <http://www.w3.org/2003/11/swrl#argument2> :c
                                                                           ] ;
                                                                 rdf:rest [ rdf:type <http://www.w3.org/2003/11/swrl#AtomList> ;
                                                                            rdf:first [ rdf:type <http://www.w3.org/2003/11/swrl#SameIndividualAtom> ;
                                                                                        <http://www.w3.org/2003/11/swrl#argument1> :b ;
                                                                                        <http://www.w3.org/2003/11/swrl#argument2> :c
                                                                                      ] ;
                                                                            rdf:rest rdf:nil
                                                                          ]
                                                               ]
                                                    ]
                                         ] ;
   <http://www.w3.org/2003/11/swrl#head> [ rdf:type <http://www.w3.org/2003/11/swrl#AtomList> ;
                                           rdf:first [ rdf:type <http://www.w3.org/2003/11/swrl#ClassAtom> ;
                                                       <http://www.w3.org/2003/11/swrl#classPredicate> :CauseInactive ;
                                                       <http://www.w3.org/2003/11/swrl#argument1> :a
                                                     ] ;
                                           rdf:rest rdf:nil
                                         ]
 ] .

[ <http://swrl.stanford.edu/ontologies/3.3/swrla.owl#isRuleEnabled> "true"^^xsd:boolean ;
   rdfs:label "MaterialSolidityActive" ;
   rdf:type <http://www.w3.org/2003/11/swrl#Imp> ;
   <http://www.w3.org/2003/11/swrl#body> [ rdf:type <http://www.w3.org/2003/11/swrl#AtomList> ;
                                           rdf:first [ rdf:type <http://www.w3.org/2003/11/swrl#ClassAtom> ;
                                                       <http://www.w3.org/2003/11/swrl#classPredicate> :SearchedProperties ;
                                                       <http://www.w3.org/2003/11/swrl#argument1> :a
                                                     ] ;
                                           rdf:rest [ rdf:type <http://www.w3.org/2003/11/swrl#AtomList> ;
                                                      rdf:first [ rdf:type <http://www.w3.org/2003/11/swrl#DatavaluedPropertyAtom> ;
                                                                  <http://www.w3.org/2003/11/swrl#propertyPredicate> :NormalMaterialSolidity ;
                                                                  <http://www.w3.org/2003/11/swrl#argument1> :a ;
                                                                  <http://www.w3.org/2003/11/swrl#argument2> :b
                                                                ] ;
                                                      rdf:rest [ rdf:type <http://www.w3.org/2003/11/swrl#AtomList> ;
                                                                 rdf:first [ rdf:type <http://www.w3.org/2003/11/swrl#DatavaluedPropertyAtom> ;
                                                                             <http://www.w3.org/2003/11/swrl#propertyPredicate> :ChangedMaterialSolidity ;
                                                                             <http://www.w3.org/2003/11/swrl#argument1> :a ;
                                                                             <http://www.w3.org/2003/11/swrl#argument2> :c
                                                                           ] ;
                                                                 rdf:rest [ rdf:type <http://www.w3.org/2003/11/swrl#AtomList> ;
                                                                            rdf:first [ rdf:type <http://www.w3.org/2003/11/swrl#DifferentIndividualsAtom> ;
                                                                                        <http://www.w3.org/2003/11/swrl#argument1> :b ;
                                                                                        <http://www.w3.org/2003/11/swrl#argument2> :c
                                                                                      ] ;
                                                                            rdf:rest rdf:nil
                                                                          ]
                                                               ]
                                                    ]
                                         ] ;
   <http://www.w3.org/2003/11/swrl#head> [ rdf:type <http://www.w3.org/2003/11/swrl#AtomList> ;
                                           rdf:first [ rdf:type <http://www.w3.org/2003/11/swrl#ClassAtom> ;
                                                       <http://www.w3.org/2003/11/swrl#classPredicate> :CauseActive ;
                                                       <http://www.w3.org/2003/11/swrl#argument1> :a
                                                     ] ;
                                           rdf:rest rdf:nil
                                         ]
 ] .

[ <http://swrl.stanford.edu/ontologies/3.3/swrla.owl#isRuleEnabled> "true"^^xsd:boolean ;
   rdfs:label "PHValueInactive" ;
   rdf:type <http://www.w3.org/2003/11/swrl#Imp> ;
   <http://www.w3.org/2003/11/swrl#body> [ rdf:type <http://www.w3.org/2003/11/swrl#AtomList> ;
                                           rdf:first [ rdf:type <http://www.w3.org/2003/11/swrl#ClassAtom> ;
                                                       <http://www.w3.org/2003/11/swrl#classPredicate> :SearchedProperties ;
                                                       <http://www.w3.org/2003/11/swrl#argument1> :a
                                                     ] ;
                                           rdf:rest [ rdf:type <http://www.w3.org/2003/11/swrl#AtomList> ;
                                                      rdf:first [ rdf:type <http://www.w3.org/2003/11/swrl#DatavaluedPropertyAtom> ;
                                                                  <http://www.w3.org/2003/11/swrl#propertyPredicate> :NormalPHValue ;
                                                                  <http://www.w3.org/2003/11/swrl#argument1> :a ;
                                                                  <http://www.w3.org/2003/11/swrl#argument2> :b
                                                                ] ;
                                                      rdf:rest [ rdf:type <http://www.w3.org/2003/11/swrl#AtomList> ;
                                                                 rdf:first [ rdf:type <http://www.w3.org/2003/11/swrl#DatavaluedPropertyAtom> ;
                                                                             <http://www.w3.org/2003/11/swrl#propertyPredicate> :ChangedPHValue ;
                                                                             <http://www.w3.org/2003/11/swrl#argument1> :a ;
                                                                             <http://www.w3.org/2003/11/swrl#argument2> :c
                                                                           ] ;
                                                                 rdf:rest [ rdf:type <http://www.w3.org/2003/11/swrl#AtomList> ;
                                                                            rdf:first [ rdf:type <http://www.w3.org/2003/11/swrl#SameIndividualAtom> ;
                                                                                        <http://www.w3.org/2003/11/swrl#argument1> :b ;
                                                                                        <http://www.w3.org/2003/11/swrl#argument2> :c
                                                                                      ] ;
                                                                            rdf:rest rdf:nil
                                                                          ]
                                                               ]
                                                    ]
                                         ] ;
   <http://www.w3.org/2003/11/swrl#head> [ rdf:type <http://www.w3.org/2003/11/swrl#AtomList> ;
                                           rdf:first [ rdf:type <http://www.w3.org/2003/11/swrl#ClassAtom> ;
                                                       <http://www.w3.org/2003/11/swrl#classPredicate> :CauseInactive ;
                                                       <http://www.w3.org/2003/11/swrl#argument1> :a
                                                     ] ;
                                           rdf:rest rdf:nil
                                         ]
 ] .

[ <http://swrl.stanford.edu/ontologies/3.3/swrla.owl#isRuleEnabled> "true"^^xsd:boolean ;
   rdfs:label "PHValueActive" ;
   rdf:type <http://www.w3.org/2003/11/swrl#Imp> ;
   <http://www.w3.org/2003/11/swrl#body> [ rdf:type <http://www.w3.org/2003/11/swrl#AtomList> ;
                                           rdf:first [ rdf:type <http://www.w3.org/2003/11/swrl#ClassAtom> ;
                                                       <http://www.w3.org/2003/11/swrl#classPredicate> :SearchedProperties ;
                                                       <http://www.w3.org/2003/11/swrl#argument1> :a
                                                     ] ;
                                           rdf:rest [ rdf:type <http://www.w3.org/2003/11/swrl#AtomList> ;
                                                      rdf:first [ rdf:type <http://www.w3.org/2003/11/swrl#DatavaluedPropertyAtom> ;
                                                                  <http://www.w3.org/2003/11/swrl#propertyPredicate> :NormalPHValue ;
                                                                  <http://www.w3.org/2003/11/swrl#argument1> :a ;
                                                                  <http://www.w3.org/2003/11/swrl#argument2> :b
                                                                ] ;
                                                      rdf:rest [ rdf:type <http://www.w3.org/2003/11/swrl#AtomList> ;
                                                                 rdf:first [ rdf:type <http://www.w3.org/2003/11/swrl#DatavaluedPropertyAtom> ;
                                                                             <http://www.w3.org/2003/11/swrl#propertyPredicate> :ChangedPHValue ;
                                                                             <http://www.w3.org/2003/11/swrl#argument1> :a ;
                                                                             <http://www.w3.org/2003/11/swrl#argument2> :c
                                                                           ] ;
                                                                 rdf:rest [ rdf:type <http://www.w3.org/2003/11/swrl#AtomList> ;
                                                                            rdf:first [ rdf:type <http://www.w3.org/2003/11/swrl#DifferentIndividualsAtom> ;
                                                                                        <http://www.w3.org/2003/11/swrl#argument1> :b ;
                                                                                        <http://www.w3.org/2003/11/swrl#argument2> :c
                                                                                      ] ;
                                                                            rdf:rest rdf:nil
                                                                          ]
                                                               ]
                                                    ]
                                         ] ;
   <http://www.w3.org/2003/11/swrl#head> [ rdf:type <http://www.w3.org/2003/11/swrl#AtomList> ;
                                           rdf:first [ rdf:type <http://www.w3.org/2003/11/swrl#ClassAtom> ;
                                                       <http://www.w3.org/2003/11/swrl#classPredicate> :CauseActive ;
                                                       <http://www.w3.org/2003/11/swrl#argument1> :a
                                                     ] ;
                                           rdf:rest rdf:nil
                                         ]
 ] .

[ <http://swrl.stanford.edu/ontologies/3.3/swrla.owl#isRuleEnabled> "true"^^xsd:boolean ;
   rdfs:label "SalinityInactive" ;
   rdf:type <http://www.w3.org/2003/11/swrl#Imp> ;
   <http://www.w3.org/2003/11/swrl#body> [ rdf:type <http://www.w3.org/2003/11/swrl#AtomList> ;
                                           rdf:first [ rdf:type <http://www.w3.org/2003/11/swrl#ClassAtom> ;
                                                       <http://www.w3.org/2003/11/swrl#classPredicate> :SearchedProperties ;
                                                       <http://www.w3.org/2003/11/swrl#argument1> :a
                                                     ] ;
                                           rdf:rest [ rdf:type <http://www.w3.org/2003/11/swrl#AtomList> ;
                                                      rdf:first [ rdf:type <http://www.w3.org/2003/11/swrl#DatavaluedPropertyAtom> ;
                                                                  <http://www.w3.org/2003/11/swrl#propertyPredicate> :NormalSalinity ;
                                                                  <http://www.w3.org/2003/11/swrl#argument1> :a ;
                                                                  <http://www.w3.org/2003/11/swrl#argument2> :b
                                                                ] ;
                                                      rdf:rest [ rdf:type <http://www.w3.org/2003/11/swrl#AtomList> ;
                                                                 rdf:first [ rdf:type <http://www.w3.org/2003/11/swrl#DatavaluedPropertyAtom> ;
                                                                             <http://www.w3.org/2003/11/swrl#propertyPredicate> :ChangedSalinity ;
                                                                             <http://www.w3.org/2003/11/swrl#argument1> :a ;
                                                                             <http://www.w3.org/2003/11/swrl#argument2> :c
                                                                           ] ;
                                                                 rdf:rest [ rdf:type <http://www.w3.org/2003/11/swrl#AtomList> ;
                                                                            rdf:first [ rdf:type <http://www.w3.org/2003/11/swrl#SameIndividualAtom> ;
                                                                                        <http://www.w3.org/2003/11/swrl#argument1> :b ;
                                                                                        <http://www.w3.org/2003/11/swrl#argument2> :c
                                                                                      ] ;
                                                                            rdf:rest rdf:nil
                                                                          ]
                                                               ]
                                                    ]
                                         ] ;
   <http://www.w3.org/2003/11/swrl#head> [ rdf:type <http://www.w3.org/2003/11/swrl#AtomList> ;
                                           rdf:first [ rdf:type <http://www.w3.org/2003/11/swrl#ClassAtom> ;
                                                       <http://www.w3.org/2003/11/swrl#classPredicate> :CauseInactive ;
                                                       <http://www.w3.org/2003/11/swrl#argument1> :a
                                                     ] ;
                                           rdf:rest rdf:nil
                                         ]
 ] .

[ <http://swrl.stanford.edu/ontologies/3.3/swrla.owl#isRuleEnabled> "true"^^xsd:boolean ;
   rdfs:label "SalinityActive" ;
   rdf:type <http://www.w3.org/2003/11/swrl#Imp> ;
   <http://www.w3.org/2003/11/swrl#body> [ rdf:type <http://www.w3.org/2003/11/swrl#AtomList> ;
                                           rdf:first [ rdf:type <http://www.w3.org/2003/11/swrl#ClassAtom> ;
                                                       <http://www.w3.org/2003/11/swrl#classPredicate> :SearchedProperties ;
                                                       <http://www.w3.org/2003/11/swrl#argument1> :a
                                                     ] ;
                                           rdf:rest [ rdf:type <http://www.w3.org/2003/11/swrl#AtomList> ;
                                                      rdf:first [ rdf:type <http://www.w3.org/2003/11/swrl#DatavaluedPropertyAtom> ;
                                                                  <http://www.w3.org/2003/11/swrl#propertyPredicate> :NormalSalinity ;
                                                                  <http://www.w3.org/2003/11/swrl#argument1> :a ;
                                                                  <http://www.w3.org/2003/11/swrl#argument2> :b
                                                                ] ;
                                                      rdf:rest [ rdf:type <http://www.w3.org/2003/11/swrl#AtomList> ;
                                                                 rdf:first [ rdf:type <http://www.w3.org/2003/11/swrl#DatavaluedPropertyAtom> ;
                                                                             <http://www.w3.org/2003/11/swrl#propertyPredicate> :ChangedSalinity ;
                                                                             <http://www.w3.org/2003/11/swrl#argument1> :a ;
                                                                             <http://www.w3.org/2003/11/swrl#argument2> :c
                                                                           ] ;
                                                                 rdf:rest [ rdf:type <http://www.w3.org/2003/11/swrl#AtomList> ;
                                                                            rdf:first [ rdf:type <http://www.w3.org/2003/11/swrl#DifferentIndividualsAtom> ;
                                                                                        <http://www.w3.org/2003/11/swrl#argument1> :b ;
                                                                                        <http://www.w3.org/2003/11/swrl#argument2> :c
                                                                                      ] ;
                                                                            rdf:rest rdf:nil
                                                                          ]
                                                               ]
                                                    ]
                                         ] ;
   <http://www.w3.org/2003/11/swrl#head> [ rdf:type <http://www.w3.org/2003/11/swrl#AtomList> ;
                                           rdf:first [ rdf:type <http://www.w3.org/2003/11/swrl#ClassAtom> ;
                                                       <http://www.w3.org/2003/11/swrl#classPredicate> :CauseActive ;
                                                       <http://www.w3.org/2003/11/swrl#argument1> :a
                                                     ] ;
                                           rdf:rest rdf:nil
                                         ]
 ] .

[ <http://swrl.stanford.edu/ontologies/3.3/swrla.owl#isRuleEnabled> "true"^^xsd:boolean ;
   rdfs:label "ThermalInsulationInactive" ;
   rdf:type <http://www.w3.org/2003/11/swrl#Imp> ;
   <http://www.w3.org/2003/11/swrl#body> [ rdf:type <http://www.w3.org/2003/11/swrl#AtomList> ;
                                           rdf:first [ rdf:type <http://www.w3.org/2003/11/swrl#ClassAtom> ;
                                                       <http://www.w3.org/2003/11/swrl#classPredicate> :SearchedProperties ;
                                                       <http://www.w3.org/2003/11/swrl#argument1> :a
                                                     ] ;
                                           rdf:rest [ rdf:type <http://www.w3.org/2003/11/swrl#AtomList> ;
                                                      rdf:first [ rdf:type <http://www.w3.org/2003/11/swrl#DatavaluedPropertyAtom> ;
                                                                  <http://www.w3.org/2003/11/swrl#propertyPredicate> :NormalThermalInsulation ;
                                                                  <http://www.w3.org/2003/11/swrl#argument1> :a ;
                                                                  <http://www.w3.org/2003/11/swrl#argument2> :b
                                                                ] ;
                                                      rdf:rest [ rdf:type <http://www.w3.org/2003/11/swrl#AtomList> ;
                                                                 rdf:first [ rdf:type <http://www.w3.org/2003/11/swrl#DatavaluedPropertyAtom> ;
                                                                             <http://www.w3.org/2003/11/swrl#propertyPredicate> :ChangedThermalInsulation ;
                                                                             <http://www.w3.org/2003/11/swrl#argument1> :a ;
                                                                             <http://www.w3.org/2003/11/swrl#argument2> :c
                                                                           ] ;
                                                                 rdf:rest [ rdf:type <http://www.w3.org/2003/11/swrl#AtomList> ;
                                                                            rdf:first [ rdf:type <http://www.w3.org/2003/11/swrl#SameIndividualAtom> ;
                                                                                        <http://www.w3.org/2003/11/swrl#argument1> :b ;
                                                                                        <http://www.w3.org/2003/11/swrl#argument2> :c
                                                                                      ] ;
                                                                            rdf:rest rdf:nil
                                                                          ]
                                                               ]
                                                    ]
                                         ] ;
   <http://www.w3.org/2003/11/swrl#head> [ rdf:type <http://www.w3.org/2003/11/swrl#AtomList> ;
                                           rdf:first [ rdf:type <http://www.w3.org/2003/11/swrl#ClassAtom> ;
                                                       <http://www.w3.org/2003/11/swrl#classPredicate> :CauseInactive ;
                                                       <http://www.w3.org/2003/11/swrl#argument1> :a
                                                     ] ;
                                           rdf:rest rdf:nil
                                         ]
 ] .

[ <http://swrl.stanford.edu/ontologies/3.3/swrla.owl#isRuleEnabled> "true"^^xsd:boolean ;
   rdfs:label "ThermalInsulationActive" ;
   rdf:type <http://www.w3.org/2003/11/swrl#Imp> ;
   <http://www.w3.org/2003/11/swrl#body> [ rdf:type <http://www.w3.org/2003/11/swrl#AtomList> ;
                                           rdf:first [ rdf:type <http://www.w3.org/2003/11/swrl#ClassAtom> ;
                                                       <http://www.w3.org/2003/11/swrl#classPredicate> :SearchedProperties ;
                                                       <http://www.w3.org/2003/11/swrl#argument1> :a
                                                     ] ;
                                           rdf:rest [ rdf:type <http://www.w3.org/2003/11/swrl#AtomList> ;
                                                      rdf:first [ rdf:type <http://www.w3.org/2003/11/swrl#DatavaluedPropertyAtom> ;
                                                                  <http://www.w3.org/2003/11/swrl#propertyPredicate> :NormalThermalInsulation ;
                                                                  <http://www.w3.org/2003/11/swrl#argument1> :a ;
                                                                  <http://www.w3.org/2003/11/swrl#argument2> :b
                                                                ] ;
                                                      rdf:rest [ rdf:type <http://www.w3.org/2003/11/swrl#AtomList> ;
                                                                 rdf:first [ rdf:type <http://www.w3.org/2003/11/swrl#DatavaluedPropertyAtom> ;
                                                                             <http://www.w3.org/2003/11/swrl#propertyPredicate> :ChangedThermalInsulation ;
                                                                             <http://www.w3.org/2003/11/swrl#argument1> :a ;
                                                                             <http://www.w3.org/2003/11/swrl#argument2> :c
                                                                           ] ;
                                                                 rdf:rest [ rdf:type <http://www.w3.org/2003/11/swrl#AtomList> ;
                                                                            rdf:first [ rdf:type <http://www.w3.org/2003/11/swrl#DifferentIndividualsAtom> ;
                                                                                        <http://www.w3.org/2003/11/swrl#argument1> :b ;
                                                                                        <http://www.w3.org/2003/11/swrl#argument2> :c
                                                                                      ] ;
                                                                            rdf:rest rdf:nil
                                                                          ]
                                                               ]
                                                    ]
                                         ] ;
   <http://www.w3.org/2003/11/swrl#head> [ rdf:type <http://www.w3.org/2003/11/swrl#AtomList> ;
                                           rdf:first [ rdf:type <http://www.w3.org/2003/11/swrl#ClassAtom> ;
                                                       <http://www.w3.org/2003/11/swrl#classPredicate> :CauseActive ;
                                                       <http://www.w3.org/2003/11/swrl#argument1> :a
                                                     ] ;
                                           rdf:rest rdf:nil
                                         ]
 ] .

[ <http://swrl.stanford.edu/ontologies/3.3/swrla.owl#isRuleEnabled> "true"^^xsd:boolean ;
   rdfs:label "WoodMoistureInactive" ;
   rdf:type <http://www.w3.org/2003/11/swrl#Imp> ;
   <http://www.w3.org/2003/11/swrl#body> [ rdf:type <http://www.w3.org/2003/11/swrl#AtomList> ;
                                           rdf:first [ rdf:type <http://www.w3.org/2003/11/swrl#ClassAtom> ;
                                                       <http://www.w3.org/2003/11/swrl#classPredicate> :SearchedProperties ;
                                                       <http://www.w3.org/2003/11/swrl#argument1> :a
                                                     ] ;
                                           rdf:rest [ rdf:type <http://www.w3.org/2003/11/swrl#AtomList> ;
                                                      rdf:first [ rdf:type <http://www.w3.org/2003/11/swrl#DatavaluedPropertyAtom> ;
                                                                  <http://www.w3.org/2003/11/swrl#propertyPredicate> :NormalWoodMoisture ;
                                                                  <http://www.w3.org/2003/11/swrl#argument1> :a ;
                                                                  <http://www.w3.org/2003/11/swrl#argument2> :b
                                                                ] ;
                                                      rdf:rest [ rdf:type <http://www.w3.org/2003/11/swrl#AtomList> ;
                                                                 rdf:first [ rdf:type <http://www.w3.org/2003/11/swrl#DatavaluedPropertyAtom> ;
                                                                             <http://www.w3.org/2003/11/swrl#propertyPredicate> :ChangedWoodMoisture ;
                                                                             <http://www.w3.org/2003/11/swrl#argument1> :a ;
                                                                             <http://www.w3.org/2003/11/swrl#argument2> :c
                                                                           ] ;
                                                                 rdf:rest [ rdf:type <http://www.w3.org/2003/11/swrl#AtomList> ;
                                                                            rdf:first [ rdf:type <http://www.w3.org/2003/11/swrl#SameIndividualAtom> ;
                                                                                        <http://www.w3.org/2003/11/swrl#argument1> :b ;
                                                                                        <http://www.w3.org/2003/11/swrl#argument2> :c
                                                                                      ] ;
                                                                            rdf:rest rdf:nil
                                                                          ]
                                                               ]
                                                    ]
                                         ] ;
   <http://www.w3.org/2003/11/swrl#head> [ rdf:type <http://www.w3.org/2003/11/swrl#AtomList> ;
                                           rdf:first [ rdf:type <http://www.w3.org/2003/11/swrl#ClassAtom> ;
                                                       <http://www.w3.org/2003/11/swrl#classPredicate> :CauseInactive ;
                                                       <http://www.w3.org/2003/11/swrl#argument1> :a
                                                     ] ;
                                           rdf:rest rdf:nil
                                         ]
 ] .

[ <http://swrl.stanford.edu/ontologies/3.3/swrla.owl#isRuleEnabled> "true"^^xsd:boolean ;
   rdfs:label "WoodMoistureActive" ;
   rdf:type <http://www.w3.org/2003/11/swrl#Imp> ;
   <http://www.w3.org/2003/11/swrl#body> [ rdf:type <http://www.w3.org/2003/11/swrl#AtomList> ;
                                           rdf:first [ rdf:type <http://www.w3.org/2003/11/swrl#ClassAtom> ;
                                                       <http://www.w3.org/2003/11/swrl#classPredicate> :SearchedProperties ;
                                                       <http://www.w3.org/2003/11/swrl#argument1> :a
                                                     ] ;
                                           rdf:rest [ rdf:type <http://www.w3.org/2003/11/swrl#AtomList> ;
                                                      rdf:first [ rdf:type <http://www.w3.org/2003/11/swrl#DatavaluedPropertyAtom> ;
                                                                  <http://www.w3.org/2003/11/swrl#propertyPredicate> :NormalWoodMoisture ;
                                                                  <http://www.w3.org/2003/11/swrl#argument1> :a ;
                                                                  <http://www.w3.org/2003/11/swrl#argument2> :b
                                                                ] ;
                                                      rdf:rest [ rdf:type <http://www.w3.org/2003/11/swrl#AtomList> ;
                                                                 rdf:first [ rdf:type <http://www.w3.org/2003/11/swrl#DatavaluedPropertyAtom> ;
                                                                             <http://www.w3.org/2003/11/swrl#propertyPredicate> :ChangedWoodMoisture ;
                                                                             <http://www.w3.org/2003/11/swrl#argument1> :a ;
                                                                             <http://www.w3.org/2003/11/swrl#argument2> :c
                                                                           ] ;
                                                                 rdf:rest [ rdf:type <http://www.w3.org/2003/11/swrl#AtomList> ;
                                                                            rdf:first [ rdf:type <http://www.w3.org/2003/11/swrl#DifferentIndividualsAtom> ;
                                                                                        <http://www.w3.org/2003/11/swrl#argument1> :b ;
                                                                                        <http://www.w3.org/2003/11/swrl#argument2> :c
                                                                                      ] ;
                                                                            rdf:rest rdf:nil
                                                                          ]
                                                               ]
                                                    ]
                                         ] ;
   <http://www.w3.org/2003/11/swrl#head> [ rdf:type <http://www.w3.org/2003/11/swrl#AtomList> ;
                                           rdf:first [ rdf:type <http://www.w3.org/2003/11/swrl#ClassAtom> ;
                                                       <http://www.w3.org/2003/11/swrl#classPredicate> :CauseActive ;
                                                       <http://www.w3.org/2003/11/swrl#argument1> :a
                                                     ] ;
                                           rdf:rest rdf:nil
                                         ]
 ] .

[ <http://swrl.stanford.edu/ontologies/3.3/swrla.owl#isRuleEnabled> "true"^^xsd:boolean ;
   rdfs:label "ChemicalReactionInactive" ;
   rdf:type <http://www.w3.org/2003/11/swrl#Imp> ;
   <http://www.w3.org/2003/11/swrl#body> [ rdf:type <http://www.w3.org/2003/11/swrl#AtomList> ;
                                           rdf:first [ rdf:type <http://www.w3.org/2003/11/swrl#ClassAtom> ;
                                                       <http://www.w3.org/2003/11/swrl#classPredicate> :SearchedProperties ;
                                                       <http://www.w3.org/2003/11/swrl#argument1> :a
                                                     ] ;
                                           rdf:rest [ rdf:type <http://www.w3.org/2003/11/swrl#AtomList> ;
                                                      rdf:first [ rdf:type <http://www.w3.org/2003/11/swrl#DatavaluedPropertyAtom> ;
                                                                  <http://www.w3.org/2003/11/swrl#propertyPredicate> :ChemicalReaction ;
                                                                  <http://www.w3.org/2003/11/swrl#argument1> :a ;
                                                                  <http://www.w3.org/2003/11/swrl#argument2> "false"^^xsd:boolean
                                                                ] ;
                                                      rdf:rest rdf:nil
                                                    ]
                                         ] ;
   <http://www.w3.org/2003/11/swrl#head> [ rdf:type <http://www.w3.org/2003/11/swrl#AtomList> ;
                                           rdf:first [ rdf:type <http://www.w3.org/2003/11/swrl#ClassAtom> ;
                                                       <http://www.w3.org/2003/11/swrl#classPredicate> :CauseInactive ;
                                                       <http://www.w3.org/2003/11/swrl#argument1> :a
                                                     ] ;
                                           rdf:rest rdf:nil
                                         ]
 ] .

[ <http://swrl.stanford.edu/ontologies/3.3/swrla.owl#isRuleEnabled> "true"^^xsd:boolean ;
   rdfs:label "ConcealedComponentsInactive" ;
   rdf:type <http://www.w3.org/2003/11/swrl#Imp> ;
   <http://www.w3.org/2003/11/swrl#body> [ rdf:type <http://www.w3.org/2003/11/swrl#AtomList> ;
                                           rdf:first [ rdf:type <http://www.w3.org/2003/11/swrl#ClassAtom> ;
                                                       <http://www.w3.org/2003/11/swrl#classPredicate> :SearchedProperties ;
                                                       <http://www.w3.org/2003/11/swrl#argument1> :a
                                                     ] ;
                                           rdf:rest [ rdf:type <http://www.w3.org/2003/11/swrl#AtomList> ;
                                                      rdf:first [ rdf:type <http://www.w3.org/2003/11/swrl#DatavaluedPropertyAtom> ;
                                                                  <http://www.w3.org/2003/11/swrl#propertyPredicate> :ConcealedComponents ;
                                                                  <http://www.w3.org/2003/11/swrl#argument1> :a ;
                                                                  <http://www.w3.org/2003/11/swrl#argument2> "false"^^xsd:boolean
                                                                ] ;
                                                      rdf:rest rdf:nil
                                                    ]
                                         ] ;
   <http://www.w3.org/2003/11/swrl#head> [ rdf:type <http://www.w3.org/2003/11/swrl#AtomList> ;
                                           rdf:first [ rdf:type <http://www.w3.org/2003/11/swrl#ClassAtom> ;
                                                       <http://www.w3.org/2003/11/swrl#classPredicate> :CauseInactive ;
                                                       <http://www.w3.org/2003/11/swrl#argument1> :a
                                                     ] ;
                                           rdf:rest rdf:nil
                                         ]
 ] .

[ <http://swrl.stanford.edu/ontologies/3.3/swrla.owl#isRuleEnabled> "true"^^xsd:boolean ;
   rdfs:label "GeometricChangeInactive" ;
   rdf:type <http://www.w3.org/2003/11/swrl#Imp> ;
   <http://www.w3.org/2003/11/swrl#body> [ rdf:type <http://www.w3.org/2003/11/swrl#AtomList> ;
                                           rdf:first [ rdf:type <http://www.w3.org/2003/11/swrl#ClassAtom> ;
                                                       <http://www.w3.org/2003/11/swrl#classPredicate> :SearchedProperties ;
                                                       <http://www.w3.org/2003/11/swrl#argument1> :a
                                                     ] ;
                                           rdf:rest [ rdf:type <http://www.w3.org/2003/11/swrl#AtomList> ;
                                                      rdf:first [ rdf:type <http://www.w3.org/2003/11/swrl#DatavaluedPropertyAtom> ;
                                                                  <http://www.w3.org/2003/11/swrl#propertyPredicate> :GeometricChange ;
                                                                  <http://www.w3.org/2003/11/swrl#argument1> :a ;
                                                                  <http://www.w3.org/2003/11/swrl#argument2> "false"^^xsd:boolean
                                                                ] ;
                                                      rdf:rest rdf:nil
                                                    ]
                                         ] ;
   <http://www.w3.org/2003/11/swrl#head> [ rdf:type <http://www.w3.org/2003/11/swrl#AtomList> ;
                                           rdf:first [ rdf:type <http://www.w3.org/2003/11/swrl#ClassAtom> ;
                                                       <http://www.w3.org/2003/11/swrl#classPredicate> :CauseInactive ;
                                                       <http://www.w3.org/2003/11/swrl#argument1> :a
                                                     ] ;
                                           rdf:rest rdf:nil
                                         ]
 ] .

[ <http://swrl.stanford.edu/ontologies/3.3/swrla.owl#isRuleEnabled> "true"^^xsd:boolean ;
   rdfs:label "InsectContaminationInactive" ;
   rdf:type <http://www.w3.org/2003/11/swrl#Imp> ;
   <http://www.w3.org/2003/11/swrl#body> [ rdf:type <http://www.w3.org/2003/11/swrl#AtomList> ;
                                           rdf:first [ rdf:type <http://www.w3.org/2003/11/swrl#ClassAtom> ;
                                                       <http://www.w3.org/2003/11/swrl#classPredicate> :SearchedProperties ;
                                                       <http://www.w3.org/2003/11/swrl#argument1> :a
                                                     ] ;
                                           rdf:rest [ rdf:type <http://www.w3.org/2003/11/swrl#AtomList> ;
                                                      rdf:first [ rdf:type <http://www.w3.org/2003/11/swrl#DatavaluedPropertyAtom> ;
                                                                  <http://www.w3.org/2003/11/swrl#propertyPredicate> :InsectContamination ;
                                                                  <http://www.w3.org/2003/11/swrl#argument1> :a ;
                                                                  <http://www.w3.org/2003/11/swrl#argument2> "false"^^xsd:boolean
                                                                ] ;
                                                      rdf:rest rdf:nil
                                                    ]
                                         ] ;
   <http://www.w3.org/2003/11/swrl#head> [ rdf:type <http://www.w3.org/2003/11/swrl#AtomList> ;
                                           rdf:first [ rdf:type <http://www.w3.org/2003/11/swrl#ClassAtom> ;
                                                       <http://www.w3.org/2003/11/swrl#classPredicate> :CauseInactive ;
                                                       <http://www.w3.org/2003/11/swrl#argument1> :a
                                                     ] ;
                                           rdf:rest rdf:nil
                                         ]
 ] .

[ <http://swrl.stanford.edu/ontologies/3.3/swrla.owl#isRuleEnabled> "true"^^xsd:boolean ;
   rdfs:label "MetalComponentsInactive" ;
   rdf:type <http://www.w3.org/2003/11/swrl#Imp> ;
   <http://www.w3.org/2003/11/swrl#body> [ rdf:type <http://www.w3.org/2003/11/swrl#AtomList> ;
                                           rdf:first [ rdf:type <http://www.w3.org/2003/11/swrl#ClassAtom> ;
                                                       <http://www.w3.org/2003/11/swrl#classPredicate> :SearchedProperties ;
                                                       <http://www.w3.org/2003/11/swrl#argument1> :a
                                                     ] ;
                                           rdf:rest [ rdf:type <http://www.w3.org/2003/11/swrl#AtomList> ;
                                                      rdf:first [ rdf:type <http://www.w3.org/2003/11/swrl#DatavaluedPropertyAtom> ;
                                                                  <http://www.w3.org/2003/11/swrl#propertyPredicate> :MetalComponents ;
                                                                  <http://www.w3.org/2003/11/swrl#argument1> :a ;
                                                                  <http://www.w3.org/2003/11/swrl#argument2> "false"^^xsd:boolean
                                                                ] ;
                                                      rdf:rest rdf:nil
                                                    ]
                                         ] ;
   <http://www.w3.org/2003/11/swrl#head> [ rdf:type <http://www.w3.org/2003/11/swrl#AtomList> ;
                                           rdf:first [ rdf:type <http://www.w3.org/2003/11/swrl#ClassAtom> ;
                                                       <http://www.w3.org/2003/11/swrl#classPredicate> :CauseInactive ;
                                                       <http://www.w3.org/2003/11/swrl#argument1> :a
                                                     ] ;
                                           rdf:rest rdf:nil
                                         ]
 ] .

[ <http://swrl.stanford.edu/ontologies/3.3/swrla.owl#isRuleEnabled> "true"^^xsd:boolean ;
   rdfs:label "RotContaminationInactive" ;
   rdf:type <http://www.w3.org/2003/11/swrl#Imp> ;
   <http://www.w3.org/2003/11/swrl#body> [ rdf:type <http://www.w3.org/2003/11/swrl#AtomList> ;
                                           rdf:first [ rdf:type <http://www.w3.org/2003/11/swrl#ClassAtom> ;
                                                       <http://www.w3.org/2003/11/swrl#classPredicate> :SearchedProperties ;
                                                       <http://www.w3.org/2003/11/swrl#argument1> :a
                                                     ] ;
                                           rdf:rest [ rdf:type <http://www.w3.org/2003/11/swrl#AtomList> ;
                                                      rdf:first [ rdf:type <http://www.w3.org/2003/11/swrl#DatavaluedPropertyAtom> ;
                                                                  <http://www.w3.org/2003/11/swrl#propertyPredicate> :RotContamination ;
                                                                  <http://www.w3.org/2003/11/swrl#argument1> :a ;
                                                                  <http://www.w3.org/2003/11/swrl#argument2> "false"^^xsd:boolean
                                                                ] ;
                                                      rdf:rest rdf:nil
                                                    ]
                                         ] ;
   <http://www.w3.org/2003/11/swrl#head> [ rdf:type <http://www.w3.org/2003/11/swrl#AtomList> ;
                                           rdf:first [ rdf:type <http://www.w3.org/2003/11/swrl#ClassAtom> ;
                                                       <http://www.w3.org/2003/11/swrl#classPredicate> :CauseInactive ;
                                                       <http://www.w3.org/2003/11/swrl#argument1> :a
                                                     ] ;
                                           rdf:rest rdf:nil
                                         ]
 ] .

[ <http://swrl.stanford.edu/ontologies/3.3/swrla.owl#isRuleEnabled> "true"^^xsd:boolean ;
   rdfs:label "ChemicalReactionActive" ;
   rdf:type <http://www.w3.org/2003/11/swrl#Imp> ;
   <http://www.w3.org/2003/11/swrl#body> [ rdf:type <http://www.w3.org/2003/11/swrl#AtomList> ;
                                           rdf:first [ rdf:type <http://www.w3.org/2003/11/swrl#ClassAtom> ;
                                                       <http://www.w3.org/2003/11/swrl#classPredicate> :SearchedProperties ;
                                                       <http://www.w3.org/2003/11/swrl#argument1> :a
                                                     ] ;
                                           rdf:rest [ rdf:type <http://www.w3.org/2003/11/swrl#AtomList> ;
                                                      rdf:first [ rdf:type <http://www.w3.org/2003/11/swrl#DatavaluedPropertyAtom> ;
                                                                  <http://www.w3.org/2003/11/swrl#propertyPredicate> :ChemicalReaction ;
                                                                  <http://www.w3.org/2003/11/swrl#argument1> :a ;
                                                                  <http://www.w3.org/2003/11/swrl#argument2> "true"^^xsd:boolean
                                                                ] ;
                                                      rdf:rest rdf:nil
                                                    ]
                                         ] ;
   <http://www.w3.org/2003/11/swrl#head> [ rdf:type <http://www.w3.org/2003/11/swrl#AtomList> ;
                                           rdf:first [ rdf:type <http://www.w3.org/2003/11/swrl#ClassAtom> ;
                                                       <http://www.w3.org/2003/11/swrl#classPredicate> :CauseActive ;
                                                       <http://www.w3.org/2003/11/swrl#argument1> :a
                                                     ] ;
                                           rdf:rest rdf:nil
                                         ]
 ] .

[ <http://swrl.stanford.edu/ontologies/3.3/swrla.owl#isRuleEnabled> "true"^^xsd:boolean ;
   rdfs:label "ConcealedComponentsActive" ;
   rdf:type <http://www.w3.org/2003/11/swrl#Imp> ;
   <http://www.w3.org/2003/11/swrl#body> [ rdf:type <http://www.w3.org/2003/11/swrl#AtomList> ;
                                           rdf:first [ rdf:type <http://www.w3.org/2003/11/swrl#ClassAtom> ;
                                                       <http://www.w3.org/2003/11/swrl#classPredicate> :SearchedProperties ;
                                                       <http://www.w3.org/2003/11/swrl#argument1> :a
                                                     ] ;
                                           rdf:rest [ rdf:type <http://www.w3.org/2003/11/swrl#AtomList> ;
                                                      rdf:first [ rdf:type <http://www.w3.org/2003/11/swrl#DatavaluedPropertyAtom> ;
                                                                  <http://www.w3.org/2003/11/swrl#propertyPredicate> :ConcealedComponents ;
                                                                  <http://www.w3.org/2003/11/swrl#argument1> :a ;
                                                                  <http://www.w3.org/2003/11/swrl#argument2> "true"^^xsd:boolean
                                                                ] ;
                                                      rdf:rest rdf:nil
                                                    ]
                                         ] ;
   <http://www.w3.org/2003/11/swrl#head> [ rdf:type <http://www.w3.org/2003/11/swrl#AtomList> ;
                                           rdf:first [ rdf:type <http://www.w3.org/2003/11/swrl#ClassAtom> ;
                                                       <http://www.w3.org/2003/11/swrl#classPredicate> :CauseActive ;
                                                       <http://www.w3.org/2003/11/swrl#argument1> :a
                                                     ] ;
                                           rdf:rest rdf:nil
                                         ]
 ] .

[ <http://swrl.stanford.edu/ontologies/3.3/swrla.owl#isRuleEnabled> "true"^^xsd:boolean ;
   rdfs:label "GeometricChangeActive" ;
   rdf:type <http://www.w3.org/2003/11/swrl#Imp> ;
   <http://www.w3.org/2003/11/swrl#body> [ rdf:type <http://www.w3.org/2003/11/swrl#AtomList> ;
                                           rdf:first [ rdf:type <http://www.w3.org/2003/11/swrl#ClassAtom> ;
                                                       <http://www.w3.org/2003/11/swrl#classPredicate> :SearchedProperties ;
                                                       <http://www.w3.org/2003/11/swrl#argument1> :a
                                                     ] ;
                                           rdf:rest [ rdf:type <http://www.w3.org/2003/11/swrl#AtomList> ;
                                                      rdf:first [ rdf:type <http://www.w3.org/2003/11/swrl#DatavaluedPropertyAtom> ;
                                                                  <http://www.w3.org/2003/11/swrl#propertyPredicate> :GeometricChange ;
                                                                  <http://www.w3.org/2003/11/swrl#argument1> :a ;
                                                                  <http://www.w3.org/2003/11/swrl#argument2> "true"^^xsd:boolean
                                                                ] ;
                                                      rdf:rest rdf:nil
                                                    ]
                                         ] ;
   <http://www.w3.org/2003/11/swrl#head> [ rdf:type <http://www.w3.org/2003/11/swrl#AtomList> ;
                                           rdf:first [ rdf:type <http://www.w3.org/2003/11/swrl#ClassAtom> ;
                                                       <http://www.w3.org/2003/11/swrl#classPredicate> :CauseActive ;
                                                       <http://www.w3.org/2003/11/swrl#argument1> :a
                                                     ] ;
                                           rdf:rest rdf:nil
                                         ]
 ] .

[ <http://swrl.stanford.edu/ontologies/3.3/swrla.owl#isRuleEnabled> "true"^^xsd:boolean ;
   rdfs:label "InsectContaminationActive" ;
   rdf:type <http://www.w3.org/2003/11/swrl#Imp> ;
   <http://www.w3.org/2003/11/swrl#body> [ rdf:type <http://www.w3.org/2003/11/swrl#AtomList> ;
                                           rdf:first [ rdf:type <http://www.w3.org/2003/11/swrl#ClassAtom> ;
                                                       <http://www.w3.org/2003/11/swrl#classPredicate> :SearchedProperties ;
                                                       <http://www.w3.org/2003/11/swrl#argument1> :a
                                                     ] ;
                                           rdf:rest [ rdf:type <http://www.w3.org/2003/11/swrl#AtomList> ;
                                                      rdf:first [ rdf:type <http://www.w3.org/2003/11/swrl#DatavaluedPropertyAtom> ;
                                                                  <http://www.w3.org/2003/11/swrl#propertyPredicate> :InsectContamination ;
                                                                  <http://www.w3.org/2003/11/swrl#argument1> :a ;
                                                                  <http://www.w3.org/2003/11/swrl#argument2> "true"^^xsd:boolean
                                                                ] ;
                                                      rdf:rest rdf:nil
                                                    ]
                                         ] ;
   <http://www.w3.org/2003/11/swrl#head> [ rdf:type <http://www.w3.org/2003/11/swrl#AtomList> ;
                                           rdf:first [ rdf:type <http://www.w3.org/2003/11/swrl#ClassAtom> ;
                                                       <http://www.w3.org/2003/11/swrl#classPredicate> :CauseActive ;
                                                       <http://www.w3.org/2003/11/swrl#argument1> :a
                                                     ] ;
                                           rdf:rest rdf:nil
                                         ]
 ] .

[ <http://swrl.stanford.edu/ontologies/3.3/swrla.owl#isRuleEnabled> "true"^^xsd:boolean ;
   rdfs:label "MetalComponentsActive" ;
   rdf:type <http://www.w3.org/2003/11/swrl#Imp> ;
   <http://www.w3.org/2003/11/swrl#body> [ rdf:type <http://www.w3.org/2003/11/swrl#AtomList> ;
                                           rdf:first [ rdf:type <http://www.w3.org/2003/11/swrl#ClassAtom> ;
                                                       <http://www.w3.org/2003/11/swrl#classPredicate> :SearchedProperties ;
                                                       <http://www.w3.org/2003/11/swrl#argument1> :a
                                                     ] ;
                                           rdf:rest [ rdf:type <http://www.w3.org/2003/11/swrl#AtomList> ;
                                                      rdf:first [ rdf:type <http://www.w3.org/2003/11/swrl#DatavaluedPropertyAtom> ;
                                                                  <http://www.w3.org/2003/11/swrl#propertyPredicate> :MetalComponents ;
                                                                  <http://www.w3.org/2003/11/swrl#argument1> :a ;
                                                                  <http://www.w3.org/2003/11/swrl#argument2> "true"^^xsd:boolean
                                                                ] ;
                                                      rdf:rest rdf:nil
                                                    ]
                                         ] ;
   <http://www.w3.org/2003/11/swrl#head> [ rdf:type <http://www.w3.org/2003/11/swrl#AtomList> ;
                                           rdf:first [ rdf:type <http://www.w3.org/2003/11/swrl#ClassAtom> ;
                                                       <http://www.w3.org/2003/11/swrl#classPredicate> :CauseActive ;
                                                       <http://www.w3.org/2003/11/swrl#argument1> :a
                                                     ] ;
                                           rdf:rest rdf:nil
                                         ]
 ] .

[ <http://swrl.stanford.edu/ontologies/3.3/swrla.owl#isRuleEnabled> "true"^^xsd:boolean ;
   rdfs:label "RotContaminationActive" ;
   rdf:type <http://www.w3.org/2003/11/swrl#Imp> ;
   <http://www.w3.org/2003/11/swrl#body> [ rdf:type <http://www.w3.org/2003/11/swrl#AtomList> ;
                                           rdf:first [ rdf:type <http://www.w3.org/2003/11/swrl#ClassAtom> ;
                                                       <http://www.w3.org/2003/11/swrl#classPredicate> :SearchedProperties ;
                                                       <http://www.w3.org/2003/11/swrl#argument1> :a
                                                     ] ;
                                           rdf:rest [ rdf:type <http://www.w3.org/2003/11/swrl#AtomList> ;
                                                      rdf:first [ rdf:type <http://www.w3.org/2003/11/swrl#DatavaluedPropertyAtom> ;
                                                                  <http://www.w3.org/2003/11/swrl#propertyPredicate> :RotContamination ;
                                                                  <http://www.w3.org/2003/11/swrl#argument1> :a ;
                                                                  <http://www.w3.org/2003/11/swrl#argument2> "true"^^xsd:boolean
                                                                ] ;
                                                      rdf:rest rdf:nil
                                                    ]
                                         ] ;
   <http://www.w3.org/2003/11/swrl#head> [ rdf:type <http://www.w3.org/2003/11/swrl#AtomList> ;
                                           rdf:first [ rdf:type <http://www.w3.org/2003/11/swrl#ClassAtom> ;
                                                       <http://www.w3.org/2003/11/swrl#classPredicate> :CauseActive ;
                                                       <http://www.w3.org/2003/11/swrl#argument1> :a
                                                     ] ;
                                           rdf:rest rdf:nil
                                         ]
 ] .

[ <http://swrl.stanford.edu/ontologies/3.3/swrla.owl#isRuleEnabled> "true"^^xsd:boolean ;
   rdfs:label "AirHumidityInactive" ;
   rdf:type <http://www.w3.org/2003/11/swrl#Imp> ;
   <http://www.w3.org/2003/11/swrl#body> [ rdf:type <http://www.w3.org/2003/11/swrl#AtomList> ;
                                           rdf:first [ rdf:type <http://www.w3.org/2003/11/swrl#ClassAtom> ;
                                                       <http://www.w3.org/2003/11/swrl#classPredicate> :SearchedProperties ;
                                                       <http://www.w3.org/2003/11/swrl#argument1> :a
                                                     ] ;
                                           rdf:rest [ rdf:type <http://www.w3.org/2003/11/swrl#AtomList> ;
                                                      rdf:first [ rdf:type <http://www.w3.org/2003/11/swrl#DatavaluedPropertyAtom> ;
                                                                  <http://www.w3.org/2003/11/swrl#propertyPredicate> :NormalAirHumidity ;
                                                                  <http://www.w3.org/2003/11/swrl#argument1> :a ;
                                                                  <http://www.w3.org/2003/11/swrl#argument2> :b
                                                                ] ;
                                                      rdf:rest [ rdf:type <http://www.w3.org/2003/11/swrl#AtomList> ;
                                                                 rdf:first [ rdf:type <http://www.w3.org/2003/11/swrl#DatavaluedPropertyAtom> ;
                                                                             <http://www.w3.org/2003/11/swrl#propertyPredicate> :ChangedAirHumidity ;
                                                                             <http://www.w3.org/2003/11/swrl#argument1> :a ;
                                                                             <http://www.w3.org/2003/11/swrl#argument2> :c
                                                                           ] ;
                                                                 rdf:rest [ rdf:type <http://www.w3.org/2003/11/swrl#AtomList> ;
                                                                            rdf:first [ rdf:type <http://www.w3.org/2003/11/swrl#SameIndividualAtom> ;
                                                                                        <http://www.w3.org/2003/11/swrl#argument1> :b ;
                                                                                        <http://www.w3.org/2003/11/swrl#argument2> :c
                                                                                      ] ;
                                                                            rdf:rest rdf:nil
                                                                          ]
                                                               ]
                                                    ]
                                         ] ;
   <http://www.w3.org/2003/11/swrl#head> [ rdf:type <http://www.w3.org/2003/11/swrl#AtomList> ;
                                           rdf:first [ rdf:type <http://www.w3.org/2003/11/swrl#ClassAtom> ;
                                                       <http://www.w3.org/2003/11/swrl#classPredicate> :CauseInactive ;
                                                       <http://www.w3.org/2003/11/swrl#argument1> :a
                                                     ] ;
                                           rdf:rest rdf:nil
                                         ]
 ] .

[ <http://swrl.stanford.edu/ontologies/3.3/swrla.owl#isRuleEnabled> "true"^^xsd:boolean ;
   rdfs:label "AirHumidityActive" ;
   rdf:type <http://www.w3.org/2003/11/swrl#Imp> ;
   <http://www.w3.org/2003/11/swrl#body> [ rdf:type <http://www.w3.org/2003/11/swrl#AtomList> ;
                                           rdf:first [ rdf:type <http://www.w3.org/2003/11/swrl#ClassAtom> ;
                                                       <http://www.w3.org/2003/11/swrl#classPredicate> :SearchedProperties ;
                                                       <http://www.w3.org/2003/11/swrl#argument1> :a
                                                     ] ;
                                           rdf:rest [ rdf:type <http://www.w3.org/2003/11/swrl#AtomList> ;
                                                      rdf:first [ rdf:type <http://www.w3.org/2003/11/swrl#DatavaluedPropertyAtom> ;
                                                                  <http://www.w3.org/2003/11/swrl#propertyPredicate> :NormalAirHumidity ;
                                                                  <http://www.w3.org/2003/11/swrl#argument1> :a ;
                                                                  <http://www.w3.org/2003/11/swrl#argument2> :b
                                                                ] ;
                                                      rdf:rest [ rdf:type <http://www.w3.org/2003/11/swrl#AtomList> ;
                                                                 rdf:first [ rdf:type <http://www.w3.org/2003/11/swrl#DatavaluedPropertyAtom> ;
                                                                             <http://www.w3.org/2003/11/swrl#propertyPredicate> :ChangedAirHumidity ;
                                                                             <http://www.w3.org/2003/11/swrl#argument1> :a ;
                                                                             <http://www.w3.org/2003/11/swrl#argument2> :c
                                                                           ] ;
                                                                 rdf:rest [ rdf:type <http://www.w3.org/2003/11/swrl#AtomList> ;
                                                                            rdf:first [ rdf:type <http://www.w3.org/2003/11/swrl#DifferentIndividualsAtom> ;
                                                                                        <http://www.w3.org/2003/11/swrl#argument1> :b ;
                                                                                        <http://www.w3.org/2003/11/swrl#argument2> :c
                                                                                      ] ;
                                                                            rdf:rest rdf:nil
                                                                          ]
                                                               ]
                                                    ]
                                         ] ;
   <http://www.w3.org/2003/11/swrl#head> [ rdf:type <http://www.w3.org/2003/11/swrl#AtomList> ;
                                           rdf:first [ rdf:type <http://www.w3.org/2003/11/swrl#ClassAtom> ;
                                                       <http://www.w3.org/2003/11/swrl#classPredicate> :CauseActive ;
                                                       <http://www.w3.org/2003/11/swrl#argument1> :a
                                                     ] ;
                                           rdf:rest rdf:nil
                                         ]
 ] .

[ <http://swrl.stanford.edu/ontologies/3.3/swrla.owl#isRuleEnabled> "true"^^xsd:boolean ;
   rdfs:label "BulkDensityInactive" ;
   rdf:type <http://www.w3.org/2003/11/swrl#Imp> ;
   <http://www.w3.org/2003/11/swrl#body> [ rdf:type <http://www.w3.org/2003/11/swrl#AtomList> ;
                                           rdf:first [ rdf:type <http://www.w3.org/2003/11/swrl#ClassAtom> ;
                                                       <http://www.w3.org/2003/11/swrl#classPredicate> :SearchedProperties ;
                                                       <http://www.w3.org/2003/11/swrl#argument1> :a
                                                     ] ;
                                           rdf:rest [ rdf:type <http://www.w3.org/2003/11/swrl#AtomList> ;
                                                      rdf:first [ rdf:type <http://www.w3.org/2003/11/swrl#DatavaluedPropertyAtom> ;
                                                                  <http://www.w3.org/2003/11/swrl#propertyPredicate> :NormalBulkDensity ;
                                                                  <http://www.w3.org/2003/11/swrl#argument1> :a ;
                                                                  <http://www.w3.org/2003/11/swrl#argument2> :b
                                                                ] ;
                                                      rdf:rest [ rdf:type <http://www.w3.org/2003/11/swrl#AtomList> ;
                                                                 rdf:first [ rdf:type <http://www.w3.org/2003/11/swrl#DatavaluedPropertyAtom> ;
                                                                             <http://www.w3.org/2003/11/swrl#propertyPredicate> :ChangedBulkDensity ;
                                                                             <http://www.w3.org/2003/11/swrl#argument1> :a ;
                                                                             <http://www.w3.org/2003/11/swrl#argument2> :c
                                                                           ] ;
                                                                 rdf:rest [ rdf:type <http://www.w3.org/2003/11/swrl#AtomList> ;
                                                                            rdf:first [ rdf:type <http://www.w3.org/2003/11/swrl#SameIndividualAtom> ;
                                                                                        <http://www.w3.org/2003/11/swrl#argument1> :b ;
                                                                                        <http://www.w3.org/2003/11/swrl#argument2> :c
                                                                                      ] ;
                                                                            rdf:rest rdf:nil
                                                                          ]
                                                               ]
                                                    ]
                                         ] ;
   <http://www.w3.org/2003/11/swrl#head> [ rdf:type <http://www.w3.org/2003/11/swrl#AtomList> ;
                                           rdf:first [ rdf:type <http://www.w3.org/2003/11/swrl#ClassAtom> ;
                                                       <http://www.w3.org/2003/11/swrl#classPredicate> :CauseInactive ;
                                                       <http://www.w3.org/2003/11/swrl#argument1> :a
                                                     ] ;
                                           rdf:rest rdf:nil
                                         ]
 ] .

[ <http://swrl.stanford.edu/ontologies/3.3/swrla.owl#isRuleEnabled> "true"^^xsd:boolean ;
   rdfs:label "BulkDensityActive" ;
   rdf:type <http://www.w3.org/2003/11/swrl#Imp> ;
   <http://www.w3.org/2003/11/swrl#body> [ rdf:type <http://www.w3.org/2003/11/swrl#AtomList> ;
                                           rdf:first [ rdf:type <http://www.w3.org/2003/11/swrl#ClassAtom> ;
                                                       <http://www.w3.org/2003/11/swrl#classPredicate> :SearchedProperties ;
                                                       <http://www.w3.org/2003/11/swrl#argument1> :a
                                                     ] ;
                                           rdf:rest [ rdf:type <http://www.w3.org/2003/11/swrl#AtomList> ;
                                                      rdf:first [ rdf:type <http://www.w3.org/2003/11/swrl#DatavaluedPropertyAtom> ;
                                                                  <http://www.w3.org/2003/11/swrl#propertyPredicate> :NormalBulkDensity ;
                                                                  <http://www.w3.org/2003/11/swrl#argument1> :a ;
                                                                  <http://www.w3.org/2003/11/swrl#argument2> :b
                                                                ] ;
                                                      rdf:rest [ rdf:type <http://www.w3.org/2003/11/swrl#AtomList> ;
                                                                 rdf:first [ rdf:type <http://www.w3.org/2003/11/swrl#DatavaluedPropertyAtom> ;
                                                                             <http://www.w3.org/2003/11/swrl#propertyPredicate> :ChangedBulkDensity ;
                                                                             <http://www.w3.org/2003/11/swrl#argument1> :a ;
                                                                             <http://www.w3.org/2003/11/swrl#argument2> :c
                                                                           ] ;
                                                                 rdf:rest [ rdf:type <http://www.w3.org/2003/11/swrl#AtomList> ;
                                                                            rdf:first [ rdf:type <http://www.w3.org/2003/11/swrl#DifferentIndividualsAtom> ;
                                                                                        <http://www.w3.org/2003/11/swrl#argument1> :b ;
                                                                                        <http://www.w3.org/2003/11/swrl#argument2> :c
                                                                                      ] ;
                                                                            rdf:rest rdf:nil
                                                                          ]
                                                               ]
                                                    ]
                                         ] ;
   <http://www.w3.org/2003/11/swrl#head> [ rdf:type <http://www.w3.org/2003/11/swrl#AtomList> ;
                                           rdf:first [ rdf:type <http://www.w3.org/2003/11/swrl#ClassAtom> ;
                                                       <http://www.w3.org/2003/11/swrl#classPredicate> :CauseActive ;
                                                       <http://www.w3.org/2003/11/swrl#argument1> :a
                                                     ] ;
                                           rdf:rest rdf:nil
                                         ]
 ] .

[ <http://swrl.stanford.edu/ontologies/3.3/swrla.owl#isRuleEnabled> "true"^^xsd:boolean ;
   rdfs:label "EmodulusInactive" ;
   rdf:type <http://www.w3.org/2003/11/swrl#Imp> ;
   <http://www.w3.org/2003/11/swrl#body> [ rdf:type <http://www.w3.org/2003/11/swrl#AtomList> ;
                                           rdf:first [ rdf:type <http://www.w3.org/2003/11/swrl#ClassAtom> ;
                                                       <http://www.w3.org/2003/11/swrl#classPredicate> :SearchedProperties ;
                                                       <http://www.w3.org/2003/11/swrl#argument1> :a
                                                     ] ;
                                           rdf:rest [ rdf:type <http://www.w3.org/2003/11/swrl#AtomList> ;
                                                      rdf:first [ rdf:type <http://www.w3.org/2003/11/swrl#DatavaluedPropertyAtom> ;
                                                                  <http://www.w3.org/2003/11/swrl#propertyPredicate> :NormalEmodulus ;
                                                                  <http://www.w3.org/2003/11/swrl#argument1> :a ;
                                                                  <http://www.w3.org/2003/11/swrl#argument2> :b
                                                                ] ;
                                                      rdf:rest [ rdf:type <http://www.w3.org/2003/11/swrl#AtomList> ;
                                                                 rdf:first [ rdf:type <http://www.w3.org/2003/11/swrl#DatavaluedPropertyAtom> ;
                                                                             <http://www.w3.org/2003/11/swrl#propertyPredicate> :ChangedEmodulus ;
                                                                             <http://www.w3.org/2003/11/swrl#argument1> :a ;
                                                                             <http://www.w3.org/2003/11/swrl#argument2> :c
                                                                           ] ;
                                                                 rdf:rest [ rdf:type <http://www.w3.org/2003/11/swrl#AtomList> ;
                                                                            rdf:first [ rdf:type <http://www.w3.org/2003/11/swrl#SameIndividualAtom> ;
                                                                                        <http://www.w3.org/2003/11/swrl#argument1> :b ;
                                                                                        <http://www.w3.org/2003/11/swrl#argument2> :c
                                                                                      ] ;
                                                                            rdf:rest rdf:nil
                                                                          ]
                                                               ]
                                                    ]
                                         ] ;
   <http://www.w3.org/2003/11/swrl#head> [ rdf:type <http://www.w3.org/2003/11/swrl#AtomList> ;
                                           rdf:first [ rdf:type <http://www.w3.org/2003/11/swrl#ClassAtom> ;
                                                       <http://www.w3.org/2003/11/swrl#classPredicate> :CauseInactive ;
                                                       <http://www.w3.org/2003/11/swrl#argument1> :a
                                                     ] ;
                                           rdf:rest rdf:nil
                                         ]
 ] .

[ <http://swrl.stanford.edu/ontologies/3.3/swrla.owl#isRuleEnabled> "true"^^xsd:boolean ;
   rdfs:label "EmodulusActive" ;
   rdf:type <http://www.w3.org/2003/11/swrl#Imp> ;
   <http://www.w3.org/2003/11/swrl#body> [ rdf:type <http://www.w3.org/2003/11/swrl#AtomList> ;
                                           rdf:first [ rdf:type <http://www.w3.org/2003/11/swrl#ClassAtom> ;
                                                       <http://www.w3.org/2003/11/swrl#classPredicate> :SearchedProperties ;
                                                       <http://www.w3.org/2003/11/swrl#argument1> :a
                                                     ] ;
                                           rdf:rest [ rdf:type <http://www.w3.org/2003/11/swrl#AtomList> ;
                                                      rdf:first [ rdf:type <http://www.w3.org/2003/11/swrl#DatavaluedPropertyAtom> ;
                                                                  <http://www.w3.org/2003/11/swrl#propertyPredicate> :NormalEmodulus ;
                                                                  <http://www.w3.org/2003/11/swrl#argument1> :a ;
                                                                  <http://www.w3.org/2003/11/swrl#argument2> :b
                                                                ] ;
                                                      rdf:rest [ rdf:type <http://www.w3.org/2003/11/swrl#AtomList> ;
                                                                 rdf:first [ rdf:type <http://www.w3.org/2003/11/swrl#DatavaluedPropertyAtom> ;
                                                                             <http://www.w3.org/2003/11/swrl#propertyPredicate> :ChangedEmodulus ;
                                                                             <http://www.w3.org/2003/11/swrl#argument1> :a ;
                                                                             <http://www.w3.org/2003/11/swrl#argument2> :c
                                                                           ] ;
                                                                 rdf:rest [ rdf:type <http://www.w3.org/2003/11/swrl#AtomList> ;
                                                                            rdf:first [ rdf:type <http://www.w3.org/2003/11/swrl#DifferentIndividualsAtom> ;
                                                                                        <http://www.w3.org/2003/11/swrl#argument1> :b ;
                                                                                        <http://www.w3.org/2003/11/swrl#argument2> :c
                                                                                      ] ;
                                                                            rdf:rest rdf:nil
                                                                          ]
                                                               ]
                                                    ]
                                         ] ;
   <http://www.w3.org/2003/11/swrl#head> [ rdf:type <http://www.w3.org/2003/11/swrl#AtomList> ;
                                           rdf:first [ rdf:type <http://www.w3.org/2003/11/swrl#ClassAtom> ;
                                                       <http://www.w3.org/2003/11/swrl#classPredicate> :CauseActive ;
                                                       <http://www.w3.org/2003/11/swrl#argument1> :a
                                                     ] ;
                                           rdf:rest rdf:nil
                                         ]
 ] .

###  Generated by the OWL API (version 5.1.18) https://github.com/owlcs/owlapi/
